@prefix : <http://purl.imsglobal.org/caliper/> .
@prefix owl: <http://www.w3.org/2002/07/owl#> .
@prefix rdf: <http://www.w3.org/1999/02/22-rdf-syntax-ns#> .
@prefix xml: <http://www.w3.org/XML/1998/namespace> .
@prefix xsd: <http://www.w3.org/2001/XMLSchema#> .
@prefix rdfs: <http://www.w3.org/2000/01/rdf-schema#> .
@base <http://purl.imsglobal.org/caliper/> .

<http://purl.imsglobal.org/caliper/> rdf:type owl:Ontology ;
                                      <http://purl.org/dc/terms/license> """Recipients of this document are requested to submit, with their comments, notification of any relevant patent claims or other intellectual property rights of which they may be aware that might be infringed by any implementation of the specification set forth in this document, and to provide supporting documentation.

IMS takes no position regarding the validity or scope of any intellectual property or other rights that might be claimed to pertain to the implementation or use of the technology described in this document or the extent to which any license under such rights might or might not be available; neither does it represent that it has made any effort to identify any such rights. Information on IMS’s procedures with respect to rights in IMS specifications can be found at the IMS Intellectual Property Rights web page: http://www.imsglobal.org/ipr/imsipr_policyFinal.pdf.

Copyright © 2018 IMS Global Learning Consortium. All Rights Reserved.

Use of this ontology to develop products or services is governed by the license with IMS found on the IMS website: http://www.imsglobal.org/speclicense.html.

Permission is granted to all parties to use excerpts from this document as needed in producing requests for proposals.

The limited permissions granted above are perpetual and will not be revoked by IMS or its successors or assigns.

THIS ONTOLOGY IS BEING OFFERED WITHOUT ANY WARRANTY WHATSOEVER, AND IN PARTICULAR, ANY WARRANTY OF NON INFRINGEMENT IS EXPRESSLY DISCLAIMED. ANY USE OF THIS ONTOLOGY SHALL BE MADE ENTIRELY AT THE IMPLEMENTER'S OWN RISK, AND NEITHER THE CONSORTIUM, NOR ANY OF ITS MEMBERS OR SUBMITTERS, SHALL HAVE ANY LIABILITY WHATSOEVER TO ANY IMPLEMENTER OR THIRD PARTY FOR ANY DAMAGES OF ANY NATURE WHATSOEVER, DIRECTLY OR INDIRECTLY, ARISING FROM THE USE OF THIS ONTOLOGY."""@en ;
                                      <http://purl.org/dc/terms/title> "Caliper Analytics® Ontology"@en ;
                                      rdfs:comment """The Caliper Analytics Specification provides a structured approach to describing, collecting and exchanging learning activity data at scale.  Establishing a common vocabulary for describing learning interactions is a central objective.  Promoting data interoperability, data sharing and data-informed decision making are also important goals.

Caliper also defines an application programming interface (the Sensor API) for marshalling and transmitting event data from instrumented applications to target endpoints for storage, analysis and use.

The Caliper ontology provides a machine-readable document that defines the concepts, relationships and constraints that together comprise the Caliper information model."""@en ;
                                      rdfs:label "Caliper Analytics® Ontology"@en ;
                                      rdfs:seeAlso "http://www.imsglobal.org/caliper"^^xsd:string .

#################################################################
#    Annotation properties
#################################################################

###  http://purl.org/dc/terms/isReplacedBy
<http://purl.org/dc/terms/isReplacedBy> rdf:type owl:AnnotationProperty .


###  http://purl.org/dc/terms/license
<http://purl.org/dc/terms/license> rdf:type owl:AnnotationProperty .


###  http://purl.org/dc/terms/title
<http://purl.org/dc/terms/title> rdf:type owl:AnnotationProperty .


###  http://www.w3.org/2002/07/owl#equivalentClass
owl:equivalentClass rdf:type owl:AnnotationProperty .


###  http://www.w3.org/2002/07/owl#equivalentProperty
owl:equivalentProperty rdf:type owl:AnnotationProperty .


#################################################################
#    Datatypes
#################################################################

###  http://www.w3.org/2001/XMLSchema#duration
xsd:duration rdf:type rdfs:Datatype .


#################################################################
#    Object Properties
#################################################################

###  http://purl.imsglobal.org/caliper/action
:action rdf:type owl:ObjectProperty ,
                 owl:FunctionalProperty ;
        rdfs:domain :Event ;
        rdfs:range :Action ;
        rdfs:comment "The action or predicate that binds the Event actor or subject to the Event object."@en ;
        rdfs:isDefinedBy "http://purl.imsglobal.org/caliper"^^xsd:string ;
        rdfs:label "action"@en .


###  http://purl.imsglobal.org/caliper/actor
:actor rdf:type owl:ObjectProperty ,
                owl:FunctionalProperty ;
       rdfs:domain :Event ;
       rdfs:range :Agent ;
       rdfs:comment "The Agent who initiated the Event, typically a Person, Organization or SoftwareApplication."@en ;
       rdfs:isDefinedBy "http://purl.imsglobal.org/caliper"^^xsd:string ;
       rdfs:label "actor"@en .


###  http://purl.imsglobal.org/caliper/alignedLearningObjective
:alignedLearningObjective rdf:type owl:ObjectProperty ;
                          rdfs:domain :DigitalResource ;
                          rdfs:range :LearningObjective ;
                          <http://purl.org/dc/terms/isReplacedBy> :learningObjectives ;
                          rdfs:comment "An ordered collection of one or more LearningObjective entities that describe what a learner is expected to comprehend or accomplish after engaging with the resource.  Deprecated.  Use learningObjectives."@en ;
                          rdfs:isDefinedBy "http://purl.imsglobal.org/caliper"^^xsd:string ;
                          rdfs:label "alignedLearningObjective"@en ;
                          owl:deprecated "true"^^xsd:boolean .


###  http://purl.imsglobal.org/caliper/annotated
:annotated rdf:type owl:ObjectProperty ,
                    owl:FunctionalProperty ;
           rdfs:domain :Annotation ;
           rdfs:range :DigitalResource ;
           rdfs:comment "The DigitalResource that was annotated by the annotator."@en ;
           rdfs:isDefinedBy "http://purl.imsglobal.org/caliper"^^xsd:string ;
           rdfs:label "annotated"@en .


###  http://purl.imsglobal.org/caliper/annotator
:annotator rdf:type owl:ObjectProperty ,
                    owl:FunctionalProperty ;
           rdfs:domain :Annotation ;
           rdfs:range :Agent ;
           rdfs:comment "The Person who created the Annotation."@en ;
           rdfs:isDefinedBy "http://purl.imsglobal.org/caliper"^^xsd:string ;
           rdfs:label "annotator"@en .


###  http://purl.imsglobal.org/caliper/assignable
:assignable rdf:type owl:ObjectProperty ,
                     owl:FunctionalProperty ;
            rdfs:domain :Attempt ;
            rdfs:range :DigitalResource ;
            rdfs:comment "The DigitalResource that constitutes the object of the assignment."@en ;
            rdfs:isDefinedBy "http://purl.imsglobal.org/caliper"^^xsd:string ;
            rdfs:label "assignable"@en .


###  http://purl.imsglobal.org/caliper/assignee
:assignee rdf:type owl:ObjectProperty ,
                   owl:FunctionalProperty ;
          rdfs:domain :Attempt ;
          rdfs:range :Agent ;
          rdfs:comment "The Person who initiated the Attempt of an assigned DigitalResource."@en ;
          rdfs:isDefinedBy "http://purl.imsglobal.org/caliper"^^xsd:string ;
          rdfs:label "assignee"@en .


###  http://purl.imsglobal.org/caliper/attachments
:attachments rdf:type owl:ObjectProperty ;
             rdfs:domain :Message ;
             rdfs:range :DigitalResource ;
             rdfs:comment "An ordered collection of one or more DigitalResource entities attached to a Message."@en ;
             rdfs:isDefinedBy "http://purl.imsglobal.org/caliper"^^xsd:string ;
             rdfs:label "attachments"@en .


###  http://purl.imsglobal.org/caliper/attempt
:attempt rdf:type owl:ObjectProperty ,
                  owl:FunctionalProperty ;
         rdfs:domain [ rdf:type owl:Class ;
                       owl:unionOf ( :Response
                                     :Result
                                     :Score
                                   )
                     ] ;
         rdfs:range :Attempt ;
         rdfs:comment "The associated Attempt."@en ;
         rdfs:isDefinedBy "http://purl.imsglobal.org/caliper"^^xsd:string ;
         rdfs:label "attempt"@en .


###  http://purl.imsglobal.org/caliper/commentedOn
:commentedOn rdf:type owl:ObjectProperty ,
                      owl:FunctionalProperty ;
             rdfs:domain :Comment ;
             rdfs:range :Entity ;
             rdfs:comment "The Entity which received the comment."@en ;
             rdfs:isDefinedBy "https://purl.imsglobal.org/caliper"@en ;
             rdfs:label "commentedOn"@en .


###  http://purl.imsglobal.org/caliper/commenter
:commenter rdf:type owl:ObjectProperty ,
                    owl:FunctionalProperty ;
           rdfs:domain :Comment ;
           rdfs:range :Person ;
           rdfs:comment "The Person who provided the comment."@en ;
           rdfs:isDefinedBy "https://purl.imsglobal.org/caliper"^^xsd:string .


###  http://purl.imsglobal.org/caliper/creator
:creator rdf:type owl:ObjectProperty ,
                  owl:FunctionalProperty ;
         rdfs:domain :Query ;
         rdfs:range :Person ;
         rdfs:comment "The Person who authored, devised or otherwise brought into being a resource."@en ;
         rdfs:isDefinedBy "http://purl.imsglobal.org/caliper"^^xsd:string ;
         rdfs:label "creator"@en .


###  http://purl.imsglobal.org/caliper/creators
:creators rdf:type owl:ObjectProperty ;
          rdfs:domain :DigitalResource ;
          rdfs:range :Agent ;
          rdfs:comment "An ordered collection of Agent entities, typically of type Person, that are responsible for bringing resource into being"@en ;
          rdfs:isDefinedBy "http://purl.imsglobal.org/caliper"^^xsd:string ;
          rdfs:label "creators"@en .


###  http://purl.imsglobal.org/caliper/data
:data rdf:type owl:ObjectProperty ;
      rdfs:domain :Envelope ;
      rdfs:range [ rdf:type owl:Class ;
                   owl:unionOf ( :Entity
                                 :Event
                               )
                 ] ;
      rdfs:comment "Envelope data array."@en ;
      rdfs:isDefinedBy "http://purl.imsglobal.org/caliper"^^xsd:string ;
      rdfs:label "data"@en .


###  http://purl.imsglobal.org/caliper/edApp
:edApp rdf:type owl:ObjectProperty ,
                owl:FunctionalProperty ;
       rdfs:domain :Event ;
       rdfs:range :SoftwareApplication ;
       rdfs:comment "A SoftwareApplication that represents the application context within which an Event occurs."@en ;
       rdfs:isDefinedBy "http://purl.imsglobal.org/caliper"^^xsd:string ;
       rdfs:label "edApp"@en .


###  http://purl.imsglobal.org/caliper/extensions
:extensions rdf:type owl:ObjectProperty ;
            rdfs:domain [ rdf:type owl:Class ;
                          owl:unionOf ( :Entity
                                        :Event
                                      )
                        ] ;
            rdfs:comment "An ordered collection of objects not defined by the Caliper Information Model."@en ;
            rdfs:isDefinedBy "http://purl.imsglobal.org/caliper"^^xsd:string ;
            rdfs:label "extensions"@en .


###  http://purl.imsglobal.org/caliper/federatedSession
:federatedSession rdf:type owl:ObjectProperty ,
                           owl:FunctionalProperty ;
                  rdfs:domain :Event ;
                  rdfs:range :LtiSession ;
                  rdfs:comment "If an Event occurs within the context of an LTI tool launch, the federatedSession constitutes the tool consumer's LtiSession."@en ;
                  rdfs:isDefinedBy "http://purl.imsglobal.org/caliper"^^xsd:string ;
                  rdfs:label "federatedSession"@en .


###  http://purl.imsglobal.org/caliper/generated
:generated rdf:type owl:ObjectProperty ,
                    owl:FunctionalProperty ;
           rdfs:domain :Event ;
           rdfs:range :Entity ;
           rdfs:comment "An Entity created or generated as a result of an interaction between an actor and an object."@en ;
           rdfs:isDefinedBy "http://purl.imsglobal.org/caliper"^^xsd:string ;
           rdfs:label "generated"@en .


###  http://purl.imsglobal.org/caliper/group
:group rdf:type owl:ObjectProperty ,
                owl:FunctionalProperty ;
       rdfs:domain :Event ;
       rdfs:range :Organization ;
       rdfs:comment "An Organization that represents the group or organizational context within which an Event occurs."@en ;
       rdfs:isDefinedBy "http://purl.imsglobal.org/caliper"^^xsd:string ;
       rdfs:label "group"@en .


###  http://purl.imsglobal.org/caliper/isPartOf
:isPartOf rdf:type owl:ObjectProperty ,
                   owl:FunctionalProperty ;
          rdfs:domain :Entity ;
          rdfs:range :Entity ;
          rdfs:comment "A related Entity that includes or incorporates the resource as a part of its whole."@en ;
          rdfs:isDefinedBy "http://purl.imsglobal.org/caliper"^^xsd:string ;
          rdfs:label "isPartOf"@en .


###  http://purl.imsglobal.org/caliper/itemLabels
:itemLabels rdf:type owl:ObjectProperty ;
            rdfs:domain [ rdf:type owl:Class ;
                          owl:unionOf ( :LikertScale
                                        :MultiSelectScale
                                      )
                        ] ;
            rdfs:comment "The ordered list of labels for each point on the Likert scale."@en ;
            rdfs:isDefinedBy "https://purl.imsglobal.org/caliper"^^xsd:string ;
            rdfs:label "itemLabels"@en .


###  http://purl.imsglobal.org/caliper/itemValues
:itemValues rdf:type owl:ObjectProperty ;
            rdfs:domain [ rdf:type owl:Class ;
                          owl:unionOf ( :LikertScale
                                        :MultiSelectScale
                                      )
                        ] ;
            rdfs:comment "The ordered list of values for each point on the Likert scale."@en ;
            rdfs:isDefinedBy "https://purl.imsglobal.org/caliper"^^xsd:string ;
            rdfs:label "itemValues"@en .


###  http://purl.imsglobal.org/caliper/items
:items rdf:type owl:ObjectProperty ;
       rdfs:domain :Collection ;
       rdfs:range :Entity ;
       rdfs:comment "An ordered collection of resources that comprise the collection."@en ;
       rdfs:isDefinedBy "http://purl.imsglobal.org/caliper"^^xsd:string ;
       rdfs:label "items"@en .


###  http://purl.imsglobal.org/caliper/learningObjectives
:learningObjectives rdf:type owl:ObjectProperty ;
                    rdfs:domain :DigitalResource ;
                    rdfs:range :LearningObjective ;
                    rdfs:comment "An ordered collection of one or more LearningObjective entities that describe what a learner is expected to comprehend or accomplish after engaging with the resource."@en ;
                    rdfs:isDefinedBy "http://purl.imsglobal.org/caliper"^^xsd:string ;
                    rdfs:label "learningObjectives"@en .


###  http://purl.imsglobal.org/caliper/member
:member rdf:type owl:ObjectProperty ,
                 owl:FunctionalProperty ;
        rdfs:domain :Membership ;
        rdfs:range :Agent ;
        rdfs:comment "The Person associated with a Membership."@en ;
        rdfs:isDefinedBy "http://purl.imsglobal.org/caliper"^^xsd:string ;
        rdfs:label "member"@en .


###  http://purl.imsglobal.org/caliper/members
:members rdf:type owl:ObjectProperty ;
         rdfs:domain :Organization ;
         rdfs:range :Agent ;
         rdfs:comment "An ordered collection of entities of type Agent that belong to a particular group."@en ;
         rdfs:isDefinedBy "http://purl.imsglobal.org/caliper"^^xsd:string ;
         rdfs:label "members"@en .


###  http://purl.imsglobal.org/caliper/membership
:membership rdf:type owl:ObjectProperty ,
                     owl:FunctionalProperty ;
            rdfs:domain :Event ;
            rdfs:range :Membership ;
            rdfs:comment "The relationship between the actor and the group in terms of roles assigned and current status."@en ;
            rdfs:isDefinedBy "http://purl.imsglobal.org/caliper"^^xsd:string ;
            rdfs:label "membership"@en .


###  http://purl.imsglobal.org/caliper/messageParameters
:messageParameters rdf:type owl:ObjectProperty ;
                   rdfs:domain :LtiSession ;
                   rdfs:comment "A map of LTI-specified message parameters that provide Tool Consumer-related contextual information MAY be specified.  LTI message parameters of whatever type (i.e., required, recommended, optional, custom and extension) MAY be referenced."@en ;
                   rdfs:isDefinedBy "http://purl.imsglobal.org/caliper"^^xsd:string ;
                   rdfs:label "messageParameters"@en .


###  http://purl.imsglobal.org/caliper/messageType
:messageType rdf:type owl:ObjectProperty ,
                      owl:FunctionalProperty ;
             rdfs:domain :LtiLink ;
             rdfs:range :LtiMessageType .


###  http://purl.imsglobal.org/caliper/navigatedFrom
:navigatedFrom rdf:type owl:ObjectProperty ,
                        owl:FunctionalProperty ;
               rdfs:domain :NavigationEvent ;
               rdfs:range :Entity ;
               <http://purl.org/dc/terms/isReplacedBy> :referrer ;
               rdfs:comment "The DigitalResource or SoftwareApplication that constitutes the referring context of a Navigation Event.  Deprecated."@en ;
               rdfs:isDefinedBy "http://purl.imsglobal.org/caliper"^^xsd:string ;
               rdfs:label "navigatedFrom"@en ;
               owl:deprecated "true"^^xsd:boolean .


###  http://purl.imsglobal.org/caliper/object
:object rdf:type owl:ObjectProperty ,
                 owl:FunctionalProperty ;
        rdfs:domain :Event ;
        rdfs:range :Entity ;
        rdfs:comment "An Entity that an Event actor interacts with as described by the Event action."@en ;
        rdfs:isDefinedBy "http://purl.imsglobal.org/caliper"^^xsd:string ;
        rdfs:label "object"@en .


###  http://purl.imsglobal.org/caliper/organization
:organization rdf:type owl:ObjectProperty ,
                       owl:FunctionalProperty ;
              rdfs:domain :Membership ;
              rdfs:range :Organization ;
              rdfs:comment "The Organization associated with a Membership."@en ;
              rdfs:isDefinedBy "http://purl.imsglobal.org/caliper"^^xsd:string ;
              rdfs:label "organization"@en .


###  http://purl.imsglobal.org/caliper/query
:query rdf:type owl:ObjectProperty ,
                owl:FunctionalProperty ;
       rdfs:domain :SearchResponse ;
       rdfs:range :Query ;
       rdfs:comment "The Query submitted by an actor."@en ;
       rdfs:isDefinedBy "http://purl.imsglobal.org/caliper"^^xsd:string ;
       rdfs:label "query"@en .


###  http://purl.imsglobal.org/caliper/rated
:rated rdf:type owl:ObjectProperty ,
                owl:FunctionalProperty ;
       rdfs:domain :Rating ;
       rdfs:range :Entity ;
       rdfs:comment "The Entity which received the rating."@en ;
       rdfs:isDefinedBy "https://purl.imsglobal.org/caliper"^^xsd:string ;
       rdfs:label "rated"@en .


###  http://purl.imsglobal.org/caliper/rater
:rater rdf:type owl:ObjectProperty ,
                owl:FunctionalProperty ;
       rdfs:domain :Rating ;
       rdfs:range :Person ;
       rdfs:comment "The Person who provided the Rating."@en ;
       rdfs:isDefinedBy "https://purl.imsglobal.org/caliper"^^xsd:string ;
       rdfs:label "rater"@en .


###  http://purl.imsglobal.org/caliper/ratingComment
:ratingComment rdf:type owl:ObjectProperty ,
                        owl:FunctionalProperty ;
               rdfs:domain :Rating ;
               rdfs:range :Comment ;
               rdfs:comment "The Comment left with the Rating."@en ;
               rdfs:isDefinedBy "http://purl.imsglobal.org/caliper"^^xsd:string ;
               rdfs:label "ratingComment"@en .


###  http://purl.imsglobal.org/caliper/referrer
:referrer rdf:type owl:ObjectProperty ,
                   owl:FunctionalProperty ;
          rdfs:domain :Event ;
          rdfs:range :Entity ;
          rdfs:comment "An Entity that represents the referring context within which an Event occurs.  A SoftwareApplication or DigitalResource will typically constitute the referring context."@en ;
          rdfs:isDefinedBy "http://purl.imsglobal.org/caliper"^^xsd:string ;
          rdfs:label "referrer"@en .


###  http://purl.imsglobal.org/caliper/replyTo
:replyTo rdf:type owl:ObjectProperty ,
                  owl:FunctionalProperty ,
                  owl:IrreflexiveProperty ;
         rdfs:domain :Message ;
         rdfs:range :Message ;
         rdfs:comment "A prior Message that represents the post to which a Message is directed in reply."@en ;
         rdfs:isDefinedBy "http://purl.imsglobal.org/caliper"^^xsd:string ;
         rdfs:label "replyTo"@en .


###  http://purl.imsglobal.org/caliper/roles
:roles rdf:type owl:ObjectProperty ;
       rdfs:domain :Membership ;
       rdfs:range :Role ;
       rdfs:comment "An ordered collection of organizational roles assigned to a member."@en ;
       rdfs:isDefinedBy "http://purl.imsglobal.org/caliper"^^xsd:string ;
       rdfs:label "roles"@en .


###  http://purl.imsglobal.org/caliper/scale
:scale rdf:type owl:ObjectProperty ,
                owl:FunctionalProperty ;
       rdfs:domain :Rating ;
       rdfs:range :Scale ;
       rdfs:comment "The Scale used for the Rating."@en ;
       rdfs:isDefinedBy "https://purl.imsglobal.org/caliper"^^xsd:string ;
       rdfs:label "scale"@en .


###  http://purl.imsglobal.org/caliper/scoredBy
:scoredBy rdf:type owl:ObjectProperty ,
                   owl:FunctionalProperty ;
          rdfs:domain [ rdf:type owl:Class ;
                        owl:unionOf ( :Result
                                      :Score
                                    )
                      ] ;
          rdfs:range :Agent ;
          rdfs:comment "The Agent who scored or graded an Attempt."@en ;
          rdfs:isDefinedBy "http://purl.imsglobal.org/caliper"^^xsd:string ;
          rdfs:label "scoredBy"@en .


###  http://purl.imsglobal.org/caliper/searchProvider
:searchProvider rdf:type owl:ObjectProperty ,
                         owl:FunctionalProperty ;
                rdfs:domain :SearchResponse ;
                rdfs:range :SoftwareApplication ;
                rdfs:comment "The SoftwareApplication that is the provider of a SearchResponse."@en ;
                rdfs:isDefinedBy "http://purl.imsglobal.org/caliper"^^xsd:string ;
                rdfs:label "searchProvider"@en .


###  http://purl.imsglobal.org/caliper/searchResults
:searchResults rdf:type owl:ObjectProperty ,
                        owl:FunctionalProperty ;
               rdfs:domain :SearchResponse ;
               rdfs:range :Entity ;
               rdfs:comment "An ordered collection of entities, typically of type DigitalResource that constitute the results of the search."@en ;
               rdfs:isDefinedBy "http://purl.imsglobal.org/caliper"^^xsd:string ;
               rdfs:label "searchResults"@en .


###  http://purl.imsglobal.org/caliper/searchTarget
:searchTarget rdf:type owl:ObjectProperty ,
                       owl:FunctionalProperty ;
              rdfs:domain [ rdf:type owl:Class ;
                            owl:unionOf ( :Query
                                          :SearchResponse
                                        )
                          ] ;
              rdfs:range :Entity ;
              rdfs:comment "The Entity, typically a DigitalResource or  SoftwareApplication, that is the target of the search."@en ;
              rdfs:isDefinedBy "http://purl.imsglobal.org/caliper"^^xsd:string ;
              rdfs:label "searchTarget"@en .


###  http://purl.imsglobal.org/caliper/selection
:selection rdf:type owl:ObjectProperty ,
                    owl:FunctionalProperty ;
           rdfs:domain :HighlightAnnotation ;
           rdfs:range :TextPositionSelector ;
           rdfs:comment "A Selector that describes a fragment or segment of a resource."@en ;
           rdfs:isDefinedBy "http://purl.imsglobal.org/caliper"^^xsd:string ;
           rdfs:label "selection"@en .


###  http://purl.imsglobal.org/caliper/selections
:selections rdf:type owl:ObjectProperty ;
            rdfs:comment "An array of the values representing the rater's selected response."@en ;
            rdfs:isDefinedBy "https://purl.imsglobal.org/caliper"^^xsd:string ;
            rdfs:label "selections"@en .


###  http://purl.imsglobal.org/caliper/session
:session rdf:type owl:ObjectProperty ,
                  owl:FunctionalProperty ;
         rdfs:domain :Event ;
         rdfs:range :Session ;
         rdfs:comment "The current user Session."@en ;
         rdfs:isDefinedBy "http://purl.imsglobal.org/caliper"^^xsd:string ;
         rdfs:label "session"@en .


###  http://purl.imsglobal.org/caliper/status
:status rdf:type owl:ObjectProperty ,
                 owl:FunctionalProperty ;
        rdfs:domain :Membership ;
        rdfs:range :Status ;
        rdfs:comment "The current standing of a member."@en ;
        rdfs:isDefinedBy "http://purl.imsglobal.org/caliper"^^xsd:string ;
        rdfs:label "status"@en .


###  http://purl.imsglobal.org/caliper/subOrganizationOf
:subOrganizationOf rdf:type owl:ObjectProperty ,
                            owl:FunctionalProperty ,
                            owl:IrreflexiveProperty ;
                   rdfs:domain :Organization ;
                   rdfs:range :Organization ;
                   rdfs:comment "The parent Organization of an Organization."@en ;
                   rdfs:isDefinedBy "http://purl.imsglobal.org/caliper"^^xsd:string ;
                   rdfs:label "subOrganizationOf"@en .


###  http://purl.imsglobal.org/caliper/target
:target rdf:type owl:ObjectProperty ,
                 owl:FunctionalProperty ;
        rdfs:domain :Event ;
        rdfs:range :Entity ;
        rdfs:comment "An Entity that represents a particular segment or location within an Event object."@en ;
        rdfs:isDefinedBy "http://purl.imsglobal.org/caliper"^^xsd:string ;
        rdfs:label "target"@en .


###  http://purl.imsglobal.org/caliper/user
:user rdf:type owl:ObjectProperty ,
               owl:FunctionalProperty ;
      rdfs:domain :Session ;
      rdfs:range :Agent ;
      rdfs:comment "The Person who initiated a Session."@en ;
      rdfs:isDefinedBy "http://purl.imsglobal.org/caliper"^^xsd:string ;
      rdfs:label "user"@en .


###  http://purl.imsglobal.org/caliper/withAgents
:withAgents rdf:type owl:ObjectProperty ;
            rdfs:domain :SharedAnnotation ;
            rdfs:range :Agent ;
            rdfs:comment "An ordered collection of one or more Agent entities, typically of type Person, with whom the annotated DigitalResource has been shared."@en ;
            rdfs:isDefinedBy "http://purl.imsglobal.org/caliper"^^xsd:string ;
            rdfs:label "withAgents"@en .


#################################################################
#    Data properties
#################################################################

###  http://purl.imsglobal.org/caliper/academicSession
:academicSession rdf:type owl:DatatypeProperty ,
                          owl:FunctionalProperty ;
                 rdfs:domain :CourseOffering ;
                 rdfs:range xsd:string ;
                 rdfs:comment "A human-readable identifier of the designated period in which a CourseOffering occurs."@en ;
                 rdfs:isDefinedBy "http://purl.imsglobal.org/caliper"^^xsd:string ;
                 rdfs:label "academicSession"@en .


###  http://purl.imsglobal.org/caliper/body
:body rdf:type owl:DatatypeProperty ,
               owl:FunctionalProperty ;
      rdfs:domain :Message ;
      rdfs:range xsd:string ;
      rdfs:comment "A plain-text rendering of the body content of a Message."@en ;
      rdfs:isDefinedBy "http://purl.imsglobal.org/caliper"^^xsd:string ;
      rdfs:label "body"@en .


###  http://purl.imsglobal.org/caliper/bookmarkNotes
:bookmarkNotes rdf:type owl:DatatypeProperty ,
                        owl:FunctionalProperty ;
               rdfs:domain :BookmarkAnnotation ;
               rdfs:range xsd:string ;
               rdfs:comment "A plain text rendering of the note associated with a BookmarkAnnotation."@en ;
               rdfs:isDefinedBy "http://purl.imsglobal.org/caliper"^^xsd:string ;
               rdfs:label "bookmarkNotes"@en .


###  http://purl.imsglobal.org/caliper/category
:category rdf:type owl:DatatypeProperty ,
                   owl:FunctionalProperty ;
          rdfs:domain :CourseSection ;
          rdfs:range xsd:string ;
          rdfs:comment "A plain-text descriptor that characterizes the purpose of the CourseSection such as \"lecture\", \"lab\" or \"seminar\"."@en ;
          rdfs:isDefinedBy "http://purl.imsglobal.org/caliper"^^xsd:string ;
          rdfs:label "category"@en .


###  http://purl.imsglobal.org/caliper/comment
:comment rdf:type owl:DatatypeProperty ,
                  owl:FunctionalProperty ;
         rdfs:domain :Result ;
         rdfs:range xsd:string ;
         rdfs:comment "Plain text feedback provided by the scorer of a Result."@en ;
         rdfs:isDefinedBy "http://purl.imsglobal.org/caliper"^^xsd:string ;
         rdfs:label "comment"@en .


###  http://purl.imsglobal.org/caliper/count
:count rdf:type owl:DatatypeProperty ,
                owl:FunctionalProperty ;
       rdfs:domain :Attempt ;
       rdfs:range xsd:nonNegativeInteger ;
       rdfs:comment "The total number of attempts inclusive of the current Attempt that have been registered by the learner against the assigned resource."@en ;
       rdfs:isDefinedBy "http://purl.imsglobal.org/caliper"^^xsd:string ;
       rdfs:label "count"@en .


###  http://purl.imsglobal.org/caliper/courseNumber
:courseNumber rdf:type owl:DatatypeProperty ,
                       owl:FunctionalProperty ;
              rdfs:domain :CourseOffering ;
              rdfs:range xsd:string ;
              rdfs:comment "A human-readable identifier of the CourseOffering or CourseSection."@en ;
              rdfs:isDefinedBy "http://purl.imsglobal.org/caliper"^^xsd:string ;
              rdfs:label "courseNumber"@en .


###  http://purl.imsglobal.org/caliper/currentTime
:currentTime rdf:type owl:DatatypeProperty ,
                      owl:FunctionalProperty ;
             rdfs:domain :MediaLocation ;
             rdfs:range xsd:duration ;
             rdfs:comment "A time interval or duration that represents the current playback position measured from the beginning of a MediaObject."@en ;
             rdfs:isDefinedBy "http://purl.imsglobal.org/caliper"^^xsd:string ;
             rdfs:label "currentTime"@en .


###  http://purl.imsglobal.org/caliper/curveFactor
:curveFactor rdf:type owl:DatatypeProperty ,
                      owl:FunctionalProperty ;
             rdfs:domain :Result ;
             rdfs:range xsd:decimal ;
             rdfs:comment "A scale factor to be used in adjusting the totalScore."@en ;
             rdfs:isDefinedBy "http://purl.imsglobal.org/caliper"^^xsd:string ;
             rdfs:label "curveFactor"@en ;
             owl:deprecated "true"^^xsd:boolean .


###  http://purl.imsglobal.org/caliper/curvedTotalScore
:curvedTotalScore rdf:type owl:DatatypeProperty ,
                           owl:FunctionalProperty ;
                  rdfs:domain :Result ;
                  rdfs:range xsd:decimal ;
                  rdfs:comment "The total score earned by the learner after applying a curveFactor to a method for computing a scaled score; e.g., adjusting the score equal to the sum of 100 - curvedFactor(100 - totalScore)."@en ;
                  rdfs:isDefinedBy "http://purl.imsglobal.org/caliper"^^xsd:string ;
                  rdfs:label "curvedTotalScore"@en ;
                  owl:deprecated "true"^^xsd:boolean .


###  http://purl.imsglobal.org/caliper/dataVersion
:dataVersion rdf:type owl:DatatypeProperty ,
                      owl:FunctionalProperty ;
             rdfs:domain :Envelope ;
             rdfs:range xsd:string ;
             rdfs:comment "Envelope data payload Caliper version."@en ;
             rdfs:isDefinedBy "http://purl.imsglobal.org/caliper"^^xsd:string ;
             rdfs:label "dataVersion"@en .


###  http://purl.imsglobal.org/caliper/dateCreated
:dateCreated rdf:type owl:DatatypeProperty ,
                      owl:FunctionalProperty ;
             rdfs:domain :Entity ;
             rdfs:range xsd:dateTime ;
             owl:propertyDisjointWith :dateModified ;
             rdfs:comment "A date and time value expressed with millisecond precision that describes when an Entity was created."@en ;
             rdfs:isDefinedBy "http://purl.imsglobal.org/caliper"^^xsd:string ;
             rdfs:label "dateCreated"@en .


###  http://purl.imsglobal.org/caliper/dateModified
:dateModified rdf:type owl:DatatypeProperty ,
                       owl:FunctionalProperty ;
              rdfs:domain :Entity ;
              rdfs:range xsd:dateTime ;
              rdfs:comment "A date and time value expressed with millisecond precision that describes when an Entity was last changed or modified."@en ;
              rdfs:isDefinedBy "http://purl.imsglobal.org/caliper"^^xsd:string ;
              rdfs:label "dateModified"@en .


###  http://purl.imsglobal.org/caliper/datePublished
:datePublished rdf:type owl:DatatypeProperty ,
                        owl:FunctionalProperty ;
               rdfs:domain :DigitalResource ;
               rdfs:range xsd:dateTime ;
               rdfs:comment "A date and time value expressed with millisecond precision that provides the publication date of a resource."@en ;
               rdfs:isDefinedBy "http://purl.imsglobal.org/caliper"^^xsd:string ;
               rdfs:label "datePublished"@en .


###  http://purl.imsglobal.org/caliper/dateToActivate
:dateToActivate rdf:type owl:DatatypeProperty ,
                         owl:FunctionalProperty ;
                rdfs:domain :DigitalResource ;
                rdfs:range xsd:dateTime ;
                rdfs:comment "A date and time value expressed with millisecond precision that describes when a resource was activated."@en ;
                rdfs:isDefinedBy "http://purl.imsglobal.org/caliper"^^xsd:string ;
                rdfs:label "dateToActivate"@en .


###  http://purl.imsglobal.org/caliper/dateToShow
:dateToShow rdf:type owl:DatatypeProperty ,
                     owl:FunctionalProperty ;
            rdfs:domain :DigitalResource ;
            rdfs:range xsd:dateTime ;
            rdfs:comment "A date and time value expressed with millisecond precision that describes when a resource should be shown or made available."@en ;
            rdfs:isDefinedBy "http://purl.imsglobal.org/caliper"^^xsd:string ;
            rdfs:label "dateToShow"@en .


###  http://purl.imsglobal.org/caliper/dateToStartOn
:dateToStartOn rdf:type owl:DatatypeProperty ,
                        owl:FunctionalProperty ;
               rdfs:domain :DigitalResource ;
               rdfs:range xsd:dateTime ;
               rdfs:comment "A date and time value expressed with millisecond precision that describes when the resource can be started."@en ;
               rdfs:isDefinedBy "http://purl.imsglobal.org/caliper"^^xsd:string ;
               rdfs:label "dateToStartOn"@en .


###  http://purl.imsglobal.org/caliper/dateToSubmit
:dateToSubmit rdf:type owl:DatatypeProperty ,
                       owl:FunctionalProperty ;
              rdfs:domain :DigitalResource ;
              rdfs:range xsd:dateTime ;
              rdfs:comment "A date and time value expressed with millisecond precision that describes when the resource is to be submitted for evaluation."@en ;
              rdfs:isDefinedBy "http://purl.imsglobal.org/caliper"^^xsd:string ;
              rdfs:label "dateToSubmit"@en .


###  http://purl.imsglobal.org/caliper/description
:description rdf:type owl:DatatypeProperty ,
                      owl:FunctionalProperty ;
             rdfs:domain :Entity ;
             rdfs:range xsd:string ;
             rdfs:comment "A brief, plain-text representation of the resource."@en ;
             rdfs:isDefinedBy "http://purl.imsglobal.org/caliper"^^xsd:string ;
             rdfs:label "description"@en .


###  http://purl.imsglobal.org/caliper/duration
:duration rdf:type owl:DatatypeProperty ,
                   owl:FunctionalProperty ;
          rdfs:domain [ rdf:type owl:Class ;
                        owl:unionOf ( :Attempt
                                      :MediaObject
                                      :Response
                                      :Session
                                    )
                      ] ;
          rdfs:range xsd:duration ;
          rdfs:comment "A time interval that represents the total time required to complete an activity."@en ;
          rdfs:isDefinedBy "http://purl.imsglobal.org/caliper"^^xsd:string ;
          rdfs:label "duration"@en .


###  http://purl.imsglobal.org/caliper/end
:end rdf:type owl:DatatypeProperty ,
              owl:FunctionalProperty ;
     rdfs:domain :TextPositionSelector ;
     rdfs:range xsd:nonNegativeInteger ;
     owl:propertyDisjointWith :start ;
     rdfs:comment "The end position of a segment of text. The first character in the full text is position 0. The character that represents the end position is NOT included within the selected segment."@en ;
     rdfs:isDefinedBy "http://purl.imsglobal.org/caliper"^^xsd:string ;
     rdfs:label "end"@en .


###  http://purl.imsglobal.org/caliper/endedAtTime
:endedAtTime rdf:type owl:DatatypeProperty ,
                      owl:FunctionalProperty ;
             rdfs:domain [ rdf:type owl:Class ;
                           owl:unionOf ( :AggregateMeasure
                                         :Attempt
                                         :Response
                                         :Session
                                       )
                         ] ;
             rdfs:range xsd:dateTime ;
             owl:propertyDisjointWith :startedAtTime ;
             rdfs:comment "A date and time value expressed with millisecond precision that describes when the activity was completed or terminated."@en ;
             rdfs:isDefinedBy "http://purl.imsglobal.org/caliper"^^xsd:string ;
             rdfs:label "endedAtTime"@en .


###  http://purl.imsglobal.org/caliper/eventTime
:eventTime rdf:type owl:DatatypeProperty ,
                    owl:FunctionalProperty ;
           rdfs:domain :Event ;
           rdfs:range xsd:dateTime ;
           rdfs:comment "A date and time value expressed with millisecond precision that indicates when an Event occurred."@en ;
           rdfs:isDefinedBy "http://purl.imsglobal.org/caliper"^^xsd:string ;
           rdfs:label "eventTime"@en .


###  http://purl.imsglobal.org/caliper/extraCreditScore
:extraCreditScore rdf:type owl:DatatypeProperty ,
                           owl:FunctionalProperty ;
                  rdfs:domain :Result ;
                  rdfs:range xsd:decimal ;
                  rdfs:comment "The number of extra credit points earned by the learner."@en ;
                  rdfs:isDefinedBy "http://purl.imsglobal.org/caliper"^^xsd:string ;
                  rdfs:label "extraCreditScore"@en ;
                  owl:deprecated "true"^^xsd:boolean .


###  http://purl.imsglobal.org/caliper/id
:id rdf:type owl:DatatypeProperty ,
             owl:FunctionalProperty ;
    rdfs:domain [ rdf:type owl:Class ;
                  owl:unionOf ( :Entity
                                :Event
                              )
                ] ;
    rdfs:range xsd:string ;
    rdfs:comment "The Event or Entity identifier.  For an Event, the id MUST be a UUID expressed as a URN using the form urn:uuid:<UUID> per RFC 4122.  For Entities a valid IRI MUST be specified. The IRI MUST be unique and persistent. The IRI SHOULD also be dereferenceable, i.e., capable of returning a representation of the resource.  An Entity MAY be provisioned with a URI employing the URN scheme in cases where a Linked Data friendly HTTP URI is either unavailable or inappropriate."@en ;
    rdfs:isDefinedBy "http://purl.imsglobal.org/caliper"^^xsd:string ;
    rdfs:label "id"@en .


###  http://purl.imsglobal.org/caliper/index
:index rdf:type owl:DatatypeProperty ,
                owl:FunctionalProperty ;
       rdfs:domain :Frame ;
       rdfs:range xsd:long ;
       rdfs:comment "A non-negative integer that represents the position of the Frame."@en ;
       rdfs:isDefinedBy "http://purl.imsglobal.org/caliper"^^xsd:string ;
       rdfs:label "index"@en .


###  http://purl.imsglobal.org/caliper/isTimeDependent
:isTimeDependent rdf:type owl:DatatypeProperty ,
                          owl:FunctionalProperty ;
                 rdfs:domain :AssessmentItem ;
                 rdfs:range xsd:boolean ;
                 rdfs:comment "A boolean value indicating whether or not interacting with the item is time dependent."@en ;
                 rdfs:isDefinedBy "http://purl.imsglobal.org/caliper"^^xsd:string ;
                 rdfs:label "isTimeDependent"@en .


###  http://purl.imsglobal.org/caliper/keywords
:keywords rdf:type owl:DatatypeProperty ;
          rdfs:domain :DigitalResource ;
          rdfs:range xsd:string ;
          rdfs:comment "An ordered collection of one or more string values that represent tags or labels used to identify the resource."@en ;
          rdfs:isDefinedBy "http://purl.imsglobal.org/caliper"^^xsd:string ;
          rdfs:label "keywords"@en .


###  http://purl.imsglobal.org/caliper/maxAttempts
:maxAttempts rdf:type owl:DatatypeProperty ,
                      owl:FunctionalProperty ;
             rdfs:domain :DigitalResource ;
             rdfs:range xsd:nonNegativeInteger ;
             rdfs:comment "A non-negative integer indicating the number of permitted attempts."@en ;
             rdfs:isDefinedBy "http://purl.imsglobal.org/caliper"^^xsd:string ;
             rdfs:label "maxAttempts"@en .


###  http://purl.imsglobal.org/caliper/maxLabel
:maxLabel rdf:type owl:DatatypeProperty ,
                   owl:FunctionalProperty ;
          rdfs:domain :NumericScale ;
          rdfs:range xsd:string ;
          owl:propertyDisjointWith :minLabel ;
          rdfs:comment "The label for the maximum value."@en ;
          rdfs:isDefinedBy "https://purl.imsglobal.org/caliper"^^xsd:string ;
          rdfs:label "maxLabel"@en .


###  http://purl.imsglobal.org/caliper/maxMetricValue
:maxMetricValue rdf:type owl:DatatypeProperty ;
                rdfs:domain :AggregateMeasure ;
                rdfs:range xsd:decimal ;
                rdfs:comment "An integer value representing the total possible curricular progress the actor can make in the context of the application."@en ;
                rdfs:isDefinedBy "http://purl.imsglobal.org/caliper"^^xsd:string ;
                rdfs:label "maxMetricValue"@en .


###  http://purl.imsglobal.org/caliper/maxResultScore
:maxResultScore rdf:type owl:DatatypeProperty ,
                         owl:FunctionalProperty ;
                rdfs:domain :Result ;
                rdfs:range xsd:decimal ;
                rdfs:comment "The maximum score permitted for a Result."@en ;
                rdfs:isDefinedBy "http://purl.imsglobal.org/caliper"^^xsd:string ;
                rdfs:label "maxResultScore"@en .


###  http://purl.imsglobal.org/caliper/maxScore
:maxScore rdf:type owl:DatatypeProperty ,
                   owl:FunctionalProperty ;
          rdfs:domain [ rdf:type owl:Class ;
                        owl:unionOf ( :DigitalResource
                                      :Score
                                    )
                      ] ;
          rdfs:range xsd:decimal ;
          rdfs:comment "A non-negative integer indicating the maximum score permitted."@en ;
          rdfs:isDefinedBy "http://purl.imsglobal.org/caliper"^^xsd:string ;
          rdfs:label "maxScore"@en .


###  http://purl.imsglobal.org/caliper/maxSelections
:maxSelections rdf:type owl:DatatypeProperty ,
                        owl:FunctionalProperty ;
               rdfs:domain :MultiSelectScale ;
               rdfs:range xsd:integer ;
               owl:propertyDisjointWith :minSelections ;
               rdfs:comment "Indicates the maximum number of selections that can be chosen."@en ;
               rdfs:isDefinedBy "https://purl.imsglobal.org/caliper"^^xsd:string ;
               rdfs:label "maxSelections"@en .


###  http://purl.imsglobal.org/caliper/maxSubmits
:maxSubmits rdf:type owl:DatatypeProperty ,
                     owl:FunctionalProperty ;
            rdfs:domain :DigitalResource ;
            rdfs:range xsd:nonNegativeInteger ;
            rdfs:comment "A non-negative integer indicating the number of permitted submissions."@en ;
            rdfs:isDefinedBy "http://purl.imsglobal.org/caliper"^^xsd:string ;
            rdfs:label "maxSubmits"@en .


###  http://purl.imsglobal.org/caliper/maxValue
:maxValue rdf:type owl:DatatypeProperty ,
                   owl:FunctionalProperty ;
          rdfs:domain :NumericScale ;
          rdfs:range xsd:decimal ;
          owl:propertyDisjointWith :minValue ;
          rdfs:comment "A decimal value used to determine the maximum value of the  NumericScale."@en ;
          rdfs:isDefinedBy "https://purl.imsglobal.org/caliper"^^xsd:string ;
          rdfs:label "maxValue"@en .


###  http://purl.imsglobal.org/caliper/mediaType
:mediaType rdf:type owl:DatatypeProperty ,
                    owl:FunctionalProperty ;
           rdfs:domain :DigitalResource ;
           rdfs:range xsd:string ;
           rdfs:comment "A string value drawn from the list of IANA approved media types and subtypes that identifies the file format of a resource."@en ;
           rdfs:isDefinedBy "http://purl.imsglobal.org/caliper"^^xsd:string ;
           rdfs:label "mediaType"@en .


###  http://purl.imsglobal.org/caliper/metric
:metric rdf:type owl:DatatypeProperty ;
        rdfs:subPropertyOf owl:topDataProperty ;
        rdfs:domain :AggregateMeasure ;
        rdfs:comment "The standard of measurement associated with the progress value."@en ;
        rdfs:isDefinedBy "http://purl.imsglobal.org/caliper"^^xsd:string ;
        rdfs:label "metric"@en .


###  http://purl.imsglobal.org/caliper/metricValue
:metricValue rdf:type owl:DatatypeProperty ,
                      owl:FunctionalProperty ;
             rdfs:domain :AggregateMeasure ;
             rdfs:range xsd:decimal ;
             rdfs:comment "An integer value representing the total curricular progress the actor has made in the context of the application."@en ;
             rdfs:isDefinedBy "http://purl.imsglobal.org/caliper"^^xsd:string ;
             rdfs:label "metricValue"@en .


###  http://purl.imsglobal.org/caliper/minLabel
:minLabel rdf:type owl:DatatypeProperty ,
                   owl:FunctionalProperty ;
          rdfs:domain :NumericScale ;
          rdfs:range xsd:string ;
          rdfs:comment "The label for the minimum value."@en ;
          rdfs:isDefinedBy "https://purl.imsglobal.org/caliper"^^xsd:string ;
          rdfs:label "minLabel"@en .


###  http://purl.imsglobal.org/caliper/minSelections
:minSelections rdf:type owl:DatatypeProperty ,
                        owl:FunctionalProperty ;
               rdfs:domain :MultiSelectScale ;
               rdfs:range xsd:integer ;
               rdfs:comment "Indicates the minimum number of selections that can be chosen."@en ;
               rdfs:isDefinedBy "https://purl.imsglobal.org/caliper"^^xsd:string ;
               rdfs:label "minSelections"@en .


###  http://purl.imsglobal.org/caliper/minValue
:minValue rdf:type owl:DatatypeProperty ,
                   owl:FunctionalProperty ;
          rdfs:domain :NumericScale ;
          rdfs:range xsd:decimal ;
          rdfs:comment "A decimal value used to determine the minimum value of the  NumericScale."@en ;
          rdfs:isDefinedBy "https://purl.imsglobal.org/caliper"^^xsd:string ;
          rdfs:label "minValue"@en .


###  http://purl.imsglobal.org/caliper/muted
:muted rdf:type owl:DatatypeProperty ,
                owl:FunctionalProperty ;
       rdfs:domain :AudioObject ;
       rdfs:range xsd:boolean ;
       rdfs:comment "An optional boolean value indicating whether or not the MediaObject has been muted ."@en ;
       rdfs:isDefinedBy "http://purl.imsglobal.org/caliper"^^xsd:string ;
       rdfs:label "muted"@en .


###  http://purl.imsglobal.org/caliper/name
:name rdf:type owl:DatatypeProperty ,
               owl:FunctionalProperty ;
      rdfs:domain :Entity ;
      rdfs:range xsd:string ;
      rdfs:comment "A string value comprising a word or phrase by which the resource is known."@en ;
      rdfs:isDefinedBy "http://purl.imsglobal.org/caliper"^^xsd:string ;
      rdfs:label "name"@en .


###  http://purl.imsglobal.org/caliper/normalScore
:normalScore rdf:type owl:DatatypeProperty ,
                      owl:FunctionalProperty ;
             rdfs:domain :Result ;
             rdfs:range xsd:decimal ;
             rdfs:comment "The score earned by the learner before adding the extraCreditScore, subtracting the penaltyScore or applying the curveFactor, if any."@en ;
             rdfs:isDefinedBy "http://purl.imsglobal.org/caliper"^^xsd:string ;
             rdfs:label "normalScore"@en ;
             owl:deprecated "true"^^xsd:boolean .


###  http://purl.imsglobal.org/caliper/objectType
:objectType rdf:type owl:DatatypeProperty ,
                     owl:FunctionalProperty ;
            rdfs:domain :DigitalResource ;
            rdfs:comment "A string value that designates the resource type."@en ;
            rdfs:isDefinedBy "http://purl.imsglobal.org/caliper"^^xsd:string ;
            rdfs:label "objectType"@en ;
            owl:deprecated "true"^^xsd:boolean .


###  http://purl.imsglobal.org/caliper/orderedSelection
:orderedSelection rdf:type owl:DatatypeProperty ,
                           owl:FunctionalProperty ;
                  rdfs:domain :MultiSelectScale ;
                  rdfs:range xsd:boolean ;
                  rdfs:comment "Indicates whether the order of the selected items is important."@en ;
                  rdfs:isDefinedBy "https://purl.imsglobal.org/caliper"^^xsd:string ;
                  rdfs:label "isOrderedSelection"@en .


###  http://purl.imsglobal.org/caliper/penaltyScore
:penaltyScore rdf:type owl:DatatypeProperty ,
                       owl:FunctionalProperty ;
              rdfs:domain :Result ;
              rdfs:range xsd:decimal ;
              rdfs:comment "The number of points deducted from the normalScore due to an infraction such as submitting an Attempt after the due date."@en ;
              rdfs:isDefinedBy "http://purl.imsglobal.org/caliper"^^xsd:string ;
              rdfs:label "penaltyScore"@en ;
              owl:deprecated "true"^^xsd:boolean .


###  http://purl.imsglobal.org/caliper/points
:points rdf:type owl:DatatypeProperty ,
                 owl:FunctionalProperty ;
        rdfs:domain [ rdf:type owl:Class ;
                      owl:unionOf ( :LikertScale
                                    :MultiSelectScale
                                  )
                    ] ;
        rdfs:range xsd:integer ;
        rdfs:comment "A integer value used to determine the amount of points on the LikertScale."@en ;
        rdfs:isDefinedBy "https://purl.imsglobal.org/caliper"^^xsd:string ;
        rdfs:label "scalePoints"@en .


###  http://purl.imsglobal.org/caliper/question
:question rdf:type owl:DatatypeProperty ,
                   owl:FunctionalProperty ;
          rdfs:domain :Scale ;
          rdfs:range xsd:string ;
          rdfs:comment "A string value comprising the question posed to be scaled."@en ;
          rdfs:isDefinedBy "https://purl.imsglobal.org/caliper"@en ;
          rdfs:label "question"@en .


###  http://purl.imsglobal.org/caliper/resultScore
:resultScore rdf:type owl:DatatypeProperty ,
                      owl:FunctionalProperty ;
             rdfs:domain :Result ;
             rdfs:range xsd:decimal ;
             rdfs:comment "The result score awarded to the learner.  A result score can be updated."@en ;
             rdfs:isDefinedBy "http://purl.imsglobal.org/caliper"^^xsd:string ;
             rdfs:label "resultScore"@en .


###  http://purl.imsglobal.org/caliper/scoreGiven
:scoreGiven rdf:type owl:DatatypeProperty ,
                     owl:FunctionalProperty ;
            rdfs:domain :Score ;
            rdfs:range xsd:decimal ;
            rdfs:comment "The score value."@en ;
            rdfs:isDefinedBy "http://purl.imsglobal.org/caliper"^^xsd:string ;
            rdfs:label "scoreGiven"@en .


###  http://purl.imsglobal.org/caliper/searchResultsItemCount
:searchResultsItemCount rdf:type owl:DatatypeProperty ,
                                 owl:FunctionalProperty ;
                        rdfs:domain :SearchResponse ;
                        rdfs:range xsd:nonNegativeInteger ;
                        rdfs:comment "A total count of searchResults returned. If the Query submitted returned no results the count equal to zero (0)."@en ;
                        rdfs:isDefinedBy "http://purl.imsglobal.org/caliper"^^xsd:string ;
                        rdfs:label "searchResultsItemCount"@en .


###  http://purl.imsglobal.org/caliper/searchTerms
:searchTerms rdf:type owl:DatatypeProperty ,
                      owl:FunctionalProperty ;
             rdfs:domain :Query ;
             rdfs:range xsd:string ;
             rdfs:comment "The search terms employed by the creator of a Query."@en ;
             rdfs:isDefinedBy "http://purl.imsglobal.org/caliper"^^xsd:string ;
             rdfs:label "searchTerms"@en .


###  http://purl.imsglobal.org/caliper/selectionText
:selectionText rdf:type owl:DatatypeProperty ,
                        owl:FunctionalProperty ;
               rdfs:domain :HighlightAnnotation ;
               rdfs:range xsd:string ;
               rdfs:comment "A string value representing a plain-text rendering of the selected segment of the annotated resource."@en ;
               rdfs:isDefinedBy "http://purl.imsglobal.org/caliper"^^xsd:string ;
               rdfs:label "selectionText"@en .


###  http://purl.imsglobal.org/caliper/sendTime
:sendTime rdf:type owl:DatatypeProperty ,
                   owl:FunctionalProperty ;
          rdfs:domain :Envelope ;
          rdfs:range xsd:dateTime ;
          rdfs:comment "Envelope send time."@en ;
          rdfs:isDefinedBy "http://purl.imsglobal.org/caliper"^^xsd:string ;
          rdfs:label "sendTime"@en .


###  http://purl.imsglobal.org/caliper/sensor
:sensor rdf:type owl:DatatypeProperty ,
                 owl:FunctionalProperty ;
        rdfs:domain :Envelope ;
        rdfs:range xsd:string ;
        rdfs:comment "Sensor identifier."@en ;
        rdfs:isDefinedBy "http://purl.imsglobal.org/caliper"^^xsd:string ;
        rdfs:label "sensor"@en .


###  http://purl.imsglobal.org/caliper/start
:start rdf:type owl:DatatypeProperty ,
                owl:FunctionalProperty ;
       rdfs:domain :TextPositionSelector ;
       rdfs:range xsd:nonNegativeInteger ;
       rdfs:comment "The starting position of a segment of text. The first character in the full text is position 0. The character that represents the start position is included within the selected segment."@en ;
       rdfs:isDefinedBy "http://purl.imsglobal.org/caliper"^^xsd:string ;
       rdfs:label "start"@en .


###  http://purl.imsglobal.org/caliper/startedAtTime
:startedAtTime rdf:type owl:DatatypeProperty ,
                        owl:FunctionalProperty ;
               rdfs:domain [ rdf:type owl:Class ;
                             owl:unionOf ( :AggregateMeasure
                                           :Attempt
                                           :Response
                                           :Session
                                         )
                           ] ;
               rdfs:range xsd:dateTime ;
               rdfs:comment "A date and time value expressed with millisecond precision that describes when the activity commenced."@en ;
               rdfs:isDefinedBy "http://purl.imsglobal.org/caliper"^^xsd:string ;
               rdfs:label "startedAtTime"@en .


###  http://purl.imsglobal.org/caliper/step
:step rdf:type owl:DatatypeProperty ,
               owl:FunctionalProperty ;
      rdfs:domain :NumericScale ;
      rdfs:range xsd:decimal ;
      rdfs:comment "Indicates the decimal step used for determining the options between the minimum and maximum values."@en ;
      rdfs:isDefinedBy "https://purl.imsglobal.org/caliper"^^xsd:string ;
      rdfs:label "step"@en .


###  http://purl.imsglobal.org/caliper/storageName
:storageName rdf:type owl:DatatypeProperty ,
                      owl:FunctionalProperty ;
             rdfs:domain :DigitalResource ;
             rdfs:range xsd:string ;
             rdfs:comment "The name of resource when stored in a file system."@en ;
             rdfs:isDefinedBy "http://purl.imsglobal.org/caliper"^^xsd:string ;
             rdfs:label "storageName"@en .


###  http://purl.imsglobal.org/caliper/tags
:tags rdf:type owl:DatatypeProperty ,
               owl:FunctionalProperty ;
      rdfs:domain :TagAnnotation ;
      rdfs:range xsd:string ;
      rdfs:comment "An ordered collection of one or more string values that represent labels or tags associated with the annotated DigitalResource."@en ;
      rdfs:isDefinedBy "http://purl.imsglobal.org/caliper"^^xsd:string ;
      rdfs:label "tags"@en .


###  http://purl.imsglobal.org/caliper/totalScore
:totalScore rdf:type owl:DatatypeProperty ,
                     owl:FunctionalProperty ;
            rdfs:domain :Result ;
            rdfs:range xsd:decimal ;
            rdfs:comment "A score earned by the learner equal to the sum of normalScore + extraCreditScore - penaltyScore. This value does not take into account the effects of curving."@en ;
            rdfs:isDefinedBy "http://purl.imsglobal.org/caliper"^^xsd:string ;
            rdfs:label "totalScore"@en ;
            owl:deprecated "true"^^xsd:boolean .


###  http://purl.imsglobal.org/caliper/type
:type rdf:type owl:DatatypeProperty ,
               owl:FunctionalProperty ;
      rdfs:domain [ rdf:type owl:Class ;
                    owl:unionOf ( :Entity
                                  :Event
                                )
                  ] ;
      rdfs:range xsd:string ;
      rdfs:comment "A string value corresponding to the Class name or label of an Event or Entity."@en ;
      rdfs:isDefinedBy "http://purl.imsglobal.org/caliper"^^xsd:string ;
      rdfs:label "type"@en .


###  http://purl.imsglobal.org/caliper/value
:value rdf:type owl:DatatypeProperty ,
                owl:FunctionalProperty ;
       rdfs:domain [ rdf:type owl:Class ;
                     owl:unionOf ( :MultipleChoiceResponse
                                   :TrueFalseResponse
                                 )
                   ] ;
       rdfs:range xsd:string ;
       rdfs:comment "A string value that represents the options selected."@en ;
       rdfs:isDefinedBy "http://purl.imsglobal.org/caliper"^^xsd:string ;
       rdfs:label "value"@en .


###  http://purl.imsglobal.org/caliper/values
:values rdf:type owl:DatatypeProperty ;
        rdfs:domain [ rdf:type owl:Class ;
                      owl:unionOf ( :FillinBlankResponse
                                    :MultipleResponseResponse
                                    :SelectTextResponse
                                  )
                    ] ;
        rdfs:range xsd:string ;
        rdfs:comment "An ordered collection of one or more selected options."@en ;
        rdfs:isDefinedBy "http://purl.imsglobal.org/caliper"^^xsd:string ;
        rdfs:label "values"@en .


###  http://purl.imsglobal.org/caliper/version
:version rdf:type owl:DatatypeProperty ,
                  owl:FunctionalProperty ;
         rdfs:domain [ rdf:type owl:Class ;
                       owl:unionOf ( :DigitalResource
                                     :SoftwareApplication
                                   )
                     ] ;
         rdfs:range xsd:string ;
         rdfs:comment "A string value that designates the current form or version of the resource."@en ;
         rdfs:isDefinedBy "http://purl.imsglobal.org/caliper"^^xsd:string ;
         rdfs:label "version"@en .


###  http://purl.imsglobal.org/caliper/volumeLevel
:volumeLevel rdf:type owl:DatatypeProperty ,
                      owl:FunctionalProperty ;
             rdfs:domain :AudioObject ;
             rdfs:range xsd:string ;
             rdfs:comment "The current volume level."@en ;
             rdfs:isDefinedBy "http://purl.imsglobal.org/caliper"^^xsd:string ;
             rdfs:label "volumeLevel"@en .


###  http://purl.imsglobal.org/caliper/volumeMax
:volumeMax rdf:type owl:DatatypeProperty ,
                    owl:FunctionalProperty ;
           rdfs:domain :AudioObject ;
           rdfs:range xsd:string ;
           owl:propertyDisjointWith :volumeMin ;
           rdfs:comment "A string value indicating the maximum volume level permitted."@en ;
           rdfs:isDefinedBy "http://purl.imsglobal.org/caliper"^^xsd:string ;
           rdfs:label "volumeMax"@en .


###  http://purl.imsglobal.org/caliper/volumeMin
:volumeMin rdf:type owl:DatatypeProperty ,
                    owl:FunctionalProperty ;
           rdfs:domain :AudioObject ;
           rdfs:range xsd:string ;
           rdfs:comment "A string value indicating the minimum volume level permitted."@en ;
           rdfs:isDefinedBy "http://purl.imsglobal.org/caliper"^^xsd:string ;
           rdfs:label "volumeMin"@en .


#################################################################
#    Classes
#################################################################

###  http://purl.imsglobal.org/caliper/Action
:Action rdf:type owl:Class ;
        rdfs:comment "Caliper includes a vocabulary of actions for describing learning interactions. Each action is based on the past-tense form of an English (en-US) verb. An action can also indicate a change in a particular characteristic of the object (e.g., resolution, size, speed, volume).  Each action is also linked to a brief definition (\"gloss\") derived in whole or in part from Princeton University's WordNet® project in order to eliminate ambiguity and aid natural language processing."@en ;
        rdfs:isDefinedBy "http://purl.imsglobal.org/caliper"^^xsd:string ;
        rdfs:label "Action"@en .


###  http://purl.imsglobal.org/caliper/Agent
:Agent rdf:type owl:Class ;
       rdfs:subClassOf :Entity ;
       rdfs:comment "A Caliper Agent is a generic type that represents an Entity that can initiate or perform an action.  Utilize Agent only if no suitable subtype exists to represent the actor being described."@en ;
       rdfs:isDefinedBy "http://purl.imsglobal.org/caliper"^^xsd:string ;
       rdfs:label "Agent"@en .


###  http://purl.imsglobal.org/caliper/AggregateMeasure
:AggregateMeasure rdf:type owl:Class ;
                  rdfs:subClassOf :Entity ;
                  rdfs:comment "A Caliper AggregateMeasure represents an aggregated measure of a learner's use of a learning tool. For example, an AggregateMeasure may represent the total time on task a learner has spent on a learning tool over a period of time."@en ;
                  rdfs:isDefinedBy "http://purl.imsglobal.org/caliper"^^xsd:string ;
                  rdfs:label "AggregateMeasure"@en .


###  http://purl.imsglobal.org/caliper/AggregateMeasureCollection
:AggregateMeasureCollection rdf:type owl:Class ;
                            rdfs:subClassOf :Collection ,
                                            [ owl:intersectionOf ( [ rdf:type owl:Restriction ;
                                                                     owl:onProperty :items ;
                                                                     owl:someValuesFrom :Entity
                                                                   ]
                                                                   [ rdf:type owl:Restriction ;
                                                                     owl:onProperty :items ;
                                                                     owl:allValuesFrom :AggregateMeasure
                                                                   ]
                                                                 ) ;
                                              rdf:type owl:Class
                                            ] ;
                            rdfs:comment "A Caliper AggregateMeasureCollection represents an unordered collection of AggregateMeasure entities."@en ;
                            rdfs:isDefinedBy "http://purl.imsglobal.org/caliper"^^xsd:string ;
                            rdfs:label "AggregateMeasureCollection"@en .


###  http://purl.imsglobal.org/caliper/Annotation
:Annotation rdf:type owl:Class ;
            rdfs:subClassOf :Entity ,
                            [ owl:intersectionOf ( [ rdf:type owl:Restriction ;
                                                     owl:onProperty :annotated ;
                                                     owl:someValuesFrom :Entity
                                                   ]
                                                   [ rdf:type owl:Restriction ;
                                                     owl:onProperty :annotated ;
                                                     owl:allValuesFrom :DigitalResource
                                                   ]
                                                 ) ;
                              rdf:type owl:Class
                            ] ,
                            [ owl:intersectionOf ( [ rdf:type owl:Restriction ;
                                                     owl:onProperty :annotator ;
                                                     owl:someValuesFrom :Agent
                                                   ]
                                                   [ rdf:type owl:Restriction ;
                                                     owl:onProperty :annotator ;
                                                     owl:allValuesFrom :Person
                                                   ]
                                                 ) ;
                              rdf:type owl:Class
                            ] ;
            rdfs:comment "A Caliper Annotation is a generic type that represents a comment, explanation, highlight, mark, note, question or tag linked to a DigitalResource."@en ;
            rdfs:isDefinedBy "http://purl.imsglobal.org/caliper"^^xsd:string ;
            rdfs:label "Annotation"@en .


###  http://purl.imsglobal.org/caliper/AnnotationEvent
:AnnotationEvent rdf:type owl:Class ;
                 rdfs:subClassOf :Event ,
                                 [ owl:intersectionOf ( [ rdf:type owl:Restriction ;
                                                          owl:onProperty :action ;
                                                          owl:someValuesFrom :Action
                                                        ]
                                                        [ rdf:type owl:Restriction ;
                                                          owl:onProperty :action ;
                                                          owl:someValuesFrom [ rdf:type owl:Class ;
                                                                               owl:oneOf ( <http://purl.imsglobal.org/caliper/actions/Bookmarked>
                                                                                           <http://purl.imsglobal.org/caliper/actions/Highlighted>
                                                                                           <http://purl.imsglobal.org/caliper/actions/Shared>
                                                                                           <http://purl.imsglobal.org/caliper/actions/Tagged>
                                                                                         )
                                                                             ]
                                                        ]
                                                      ) ;
                                   rdf:type owl:Class
                                 ] ,
                                 [ owl:intersectionOf ( [ rdf:type owl:Restriction ;
                                                          owl:onProperty :actor ;
                                                          owl:someValuesFrom :Agent
                                                        ]
                                                        [ rdf:type owl:Restriction ;
                                                          owl:onProperty :actor ;
                                                          owl:allValuesFrom :Person
                                                        ]
                                                      ) ;
                                   rdf:type owl:Class
                                 ] ,
                                 [ owl:intersectionOf ( [ rdf:type owl:Restriction ;
                                                          owl:onProperty :object ;
                                                          owl:someValuesFrom :Entity
                                                        ]
                                                        [ rdf:type owl:Restriction ;
                                                          owl:onProperty :object ;
                                                          owl:allValuesFrom :DigitalResource
                                                        ]
                                                      ) ;
                                   rdf:type owl:Class
                                 ] ,
                                 [ rdf:type owl:Restriction ;
                                   owl:onProperty :generated ;
                                   owl:someValuesFrom :Annotation
                                 ] ,
                                 [ rdf:type owl:Restriction ;
                                   owl:onProperty :target ;
                                   owl:someValuesFrom :Frame
                                 ] ;
                 rdfs:comment "A Caliper AnnotationEvent models the annotating of digital content. The resulting Annotation is also described and is subtyped for greater type specificity."@en ;
                 rdfs:isDefinedBy "http://purl.imsglobal.org/caliper"^^xsd:string ;
                 rdfs:label "AnnotationEvent"@en .


###  http://purl.imsglobal.org/caliper/Assessment
:Assessment rdf:type owl:Class ;
            rdfs:subClassOf [ owl:intersectionOf ( :AssignableDigitalResource
                                                   :DigitalResourceCollection
                                                 ) ;
                              rdf:type owl:Class
                            ] ,
                            [ owl:intersectionOf ( [ rdf:type owl:Restriction ;
                                                     owl:onProperty :items ;
                                                     owl:someValuesFrom :AssignableDigitalResource
                                                   ]
                                                   [ rdf:type owl:Restriction ;
                                                     owl:onProperty :items ;
                                                     owl:allValuesFrom :AssessmentItem
                                                   ]
                                                 ) ;
                              rdf:type owl:Class
                            ] ;
            rdfs:comment "A Caliper Assessment represents an assessment instrument such as a test or quiz."@en ;
            rdfs:isDefinedBy "http://purl.imsglobal.org/caliper"^^xsd:string ;
            rdfs:label "Assessment"@en .


###  http://purl.imsglobal.org/caliper/AssessmentEvent
:AssessmentEvent rdf:type owl:Class ;
                 rdfs:subClassOf :Event ,
                                 [ owl:intersectionOf ( [ rdf:type owl:Restriction ;
                                                          owl:onProperty :action ;
                                                          owl:someValuesFrom :Action
                                                        ]
                                                        [ rdf:type owl:Restriction ;
                                                          owl:onProperty :action ;
                                                          owl:someValuesFrom [ rdf:type owl:Class ;
                                                                               owl:oneOf ( <http://purl.imsglobal.org/caliper/actions/Paused>
                                                                                           <http://purl.imsglobal.org/caliper/actions/Reset>
                                                                                           <http://purl.imsglobal.org/caliper/actions/Restarted>
                                                                                           <http://purl.imsglobal.org/caliper/actions/Resumed>
                                                                                           <http://purl.imsglobal.org/caliper/actions/Started>
                                                                                           <http://purl.imsglobal.org/caliper/actions/Submitted>
                                                                                         )
                                                                             ]
                                                        ]
                                                      ) ;
                                   rdf:type owl:Class
                                 ] ,
                                 [ owl:intersectionOf ( [ rdf:type owl:Restriction ;
                                                          owl:onProperty :actor ;
                                                          owl:someValuesFrom :Agent
                                                        ]
                                                        [ rdf:type owl:Restriction ;
                                                          owl:onProperty :actor ;
                                                          owl:allValuesFrom :Person
                                                        ]
                                                      ) ;
                                   rdf:type owl:Class
                                 ] ,
                                 [ owl:intersectionOf ( [ rdf:type owl:Restriction ;
                                                          owl:onProperty :object ;
                                                          owl:someValuesFrom :AssignableDigitalResource
                                                        ]
                                                        [ rdf:type owl:Restriction ;
                                                          owl:onProperty :object ;
                                                          owl:allValuesFrom :Assessment
                                                        ]
                                                      ) ;
                                   rdf:type owl:Class
                                 ] ,
                                 [ rdf:type owl:Restriction ;
                                   owl:onProperty :generated ;
                                   owl:someValuesFrom :Attempt
                                 ] ;
                 rdfs:comment "A Caliper AssessmentEvent models learner interactions with assessments instruments such as online tests or quizzes."@en ;
                 rdfs:isDefinedBy "http://purl.imsglobal.org/caliper"^^xsd:string ;
                 rdfs:label "AssessmentEvent"@en .


###  http://purl.imsglobal.org/caliper/AssessmentItem
:AssessmentItem rdf:type owl:Class ;
                rdfs:subClassOf :AssignableDigitalResource ,
                                [ owl:intersectionOf ( [ rdf:type owl:Restriction ;
                                                         owl:onProperty :isPartOf ;
                                                         owl:someValuesFrom :AssignableDigitalResource
                                                       ]
                                                       [ rdf:type owl:Restriction ;
                                                         owl:onProperty :isPartOf ;
                                                         owl:allValuesFrom :Assessment
                                                       ]
                                                     ) ;
                                  rdf:type owl:Class
                                ] ;
                rdfs:comment "A Caliper AssessmentItem represents a single test question."@en ;
                rdfs:isDefinedBy "http://purl.imsglobal.org/caliper"^^xsd:string ;
                rdfs:label "AssessmentItem"@en .


###  http://purl.imsglobal.org/caliper/AssessmentItemEvent
:AssessmentItemEvent rdf:type owl:Class ;
                     rdfs:subClassOf :Event ,
                                     [ owl:intersectionOf ( [ rdf:type owl:Restriction ;
                                                              owl:onProperty :action ;
                                                              owl:someValuesFrom :Action
                                                            ]
                                                            [ rdf:type owl:Restriction ;
                                                              owl:onProperty :action ;
                                                              owl:someValuesFrom [ rdf:type owl:Class ;
                                                                                   owl:oneOf ( <http://purl.imsglobal.org/caliper/actions/Completed>
                                                                                               <http://purl.imsglobal.org/caliper/actions/Skipped>
                                                                                               <http://purl.imsglobal.org/caliper/actions/Started>
                                                                                             )
                                                                                 ]
                                                            ]
                                                          ) ;
                                       rdf:type owl:Class
                                     ] ,
                                     [ owl:intersectionOf ( [ rdf:type owl:Restriction ;
                                                              owl:onProperty :actor ;
                                                              owl:someValuesFrom :Agent
                                                            ]
                                                            [ rdf:type owl:Restriction ;
                                                              owl:onProperty :actor ;
                                                              owl:allValuesFrom :Person
                                                            ]
                                                          ) ;
                                       rdf:type owl:Class
                                     ] ,
                                     [ owl:intersectionOf ( [ rdf:type owl:Restriction ;
                                                              owl:onProperty :object ;
                                                              owl:someValuesFrom :AssignableDigitalResource
                                                            ]
                                                            [ rdf:type owl:Restriction ;
                                                              owl:onProperty :object ;
                                                              owl:allValuesFrom :AssessmentItem
                                                            ]
                                                          ) ;
                                       rdf:type owl:Class
                                     ] ,
                                     [ owl:intersectionOf ( [ rdf:type owl:Restriction ;
                                                              owl:onProperty :referrer ;
                                                              owl:someValuesFrom :AssignableDigitalResource
                                                            ]
                                                            [ rdf:type owl:Restriction ;
                                                              owl:onProperty :referrer ;
                                                              owl:allValuesFrom :AssessmentItem
                                                            ]
                                                          ) ;
                                       rdf:type owl:Class
                                     ] ,
                                     [ rdf:type owl:Restriction ;
                                       owl:onProperty :generated ;
                                       owl:someValuesFrom :Response
                                     ] ;
                     rdfs:comment "A Caliper AssessmentItemEvent models a learner's interaction with an individual AssessmentItem."@en ;
                     rdfs:isDefinedBy "http://purl.imsglobal.org/caliper"^^xsd:string ;
                     rdfs:label "AssessmentItemEvent"@en .


###  http://purl.imsglobal.org/caliper/AssignableDigitalResource
:AssignableDigitalResource rdf:type owl:Class ;
                           rdfs:subClassOf :DigitalResource ;
                           <http://purl.org/dc/terms/isReplacedBy> :DigitalResource ;
                           rdfs:comment "A Caliper AssignableDigitalResource is a generic type that represents digital content associated with a graded or ungraded assignment.  Utilize AssignableDigitalResource only if no suitable subtype exists to represent the resource being described."@en ;
                           rdfs:isDefinedBy "http://purl.imsglobal.org/caliper"^^xsd:string ;
                           rdfs:label "AssignableDigitalResource"@en .


###  http://purl.imsglobal.org/caliper/AssignableEvent
:AssignableEvent rdf:type owl:Class ;
                 rdfs:subClassOf :Event ,
                                 [ owl:intersectionOf ( [ rdf:type owl:Restriction ;
                                                          owl:onProperty :action ;
                                                          owl:someValuesFrom :Action
                                                        ]
                                                        [ rdf:type owl:Restriction ;
                                                          owl:onProperty :action ;
                                                          owl:someValuesFrom [ rdf:type owl:Class ;
                                                                               owl:oneOf ( <http://purl.imsglobal.org/caliper/actions/Activated>
                                                                                           <http://purl.imsglobal.org/caliper/actions/Completed>
                                                                                           <http://purl.imsglobal.org/caliper/actions/Deactivated>
                                                                                           <http://purl.imsglobal.org/caliper/actions/Reviewed>
                                                                                           <http://purl.imsglobal.org/caliper/actions/Started>
                                                                                           <http://purl.imsglobal.org/caliper/actions/Submitted>
                                                                                         )
                                                                             ]
                                                        ]
                                                      ) ;
                                   rdf:type owl:Class
                                 ] ,
                                 [ owl:intersectionOf ( [ rdf:type owl:Restriction ;
                                                          owl:onProperty :actor ;
                                                          owl:someValuesFrom :Agent
                                                        ]
                                                        [ rdf:type owl:Restriction ;
                                                          owl:onProperty :actor ;
                                                          owl:allValuesFrom :Person
                                                        ]
                                                      ) ;
                                   rdf:type owl:Class
                                 ] ,
                                 [ owl:intersectionOf ( [ rdf:type owl:Restriction ;
                                                          owl:onProperty :object ;
                                                          owl:someValuesFrom :DigitalResource
                                                        ]
                                                        [ rdf:type owl:Restriction ;
                                                          owl:onProperty :object ;
                                                          owl:allValuesFrom :AssignableDigitalResource
                                                        ]
                                                      ) ;
                                   rdf:type owl:Class
                                 ] ,
                                 [ rdf:type owl:Restriction ;
                                   owl:onProperty :generated ;
                                   owl:someValuesFrom :Attempt
                                 ] ,
                                 [ rdf:type owl:Restriction ;
                                   owl:onProperty :target ;
                                   owl:someValuesFrom :Frame
                                 ] ;
                 rdfs:comment "A Caliper AssignableEvent models activities associated with the assignment of digital content assigned to a learner for completion."@en ;
                 rdfs:isDefinedBy "http://purl.imsglobal.org/caliper"^^xsd:string ;
                 rdfs:label "AssignableEvent"@en .


###  http://purl.imsglobal.org/caliper/Attempt
:Attempt rdf:type owl:Class ;
         rdfs:subClassOf :Entity ,
                         [ owl:intersectionOf ( [ rdf:type owl:Restriction ;
                                                  owl:onProperty :assignable ;
                                                  owl:someValuesFrom :Entity
                                                ]
                                                [ rdf:type owl:Restriction ;
                                                  owl:onProperty :assignable ;
                                                  owl:allValuesFrom :DigitalResource
                                                ]
                                              ) ;
                           rdf:type owl:Class
                         ] ,
                         [ owl:intersectionOf ( [ rdf:type owl:Restriction ;
                                                  owl:onProperty :assignee ;
                                                  owl:someValuesFrom :Agent
                                                ]
                                                [ rdf:type owl:Restriction ;
                                                  owl:onProperty :assignee ;
                                                  owl:allValuesFrom :Person
                                                ]
                                              ) ;
                           rdf:type owl:Class
                         ] ,
                         [ rdf:type owl:Restriction ;
                           owl:onProperty :isPartOf ;
                           owl:someValuesFrom :Attempt
                         ] ;
         rdfs:comment "A Caliper Attempt provides a count of the number of times an actor has interacted with an AssignableDigitalResource along with start time, end time and duration information. An Attempt is generated as the result of an action such as starting an Assessment."@en ;
         rdfs:isDefinedBy "http://purl.imsglobal.org/caliper"^^xsd:string ;
         rdfs:label "Attempt"@en .


###  http://purl.imsglobal.org/caliper/AudioObject
:AudioObject rdf:type owl:Class ;
             rdfs:subClassOf :MediaObject ;
             rdfs:comment "A Caliper AudioObject represents an audio or sound file."@en ;
             rdfs:isDefinedBy "http://purl.imsglobal.org/caliper"^^xsd:string ;
             rdfs:label "AudioObject"@en .


###  http://purl.imsglobal.org/caliper/BookmarkAnnotation
:BookmarkAnnotation rdf:type owl:Class ;
                    rdfs:subClassOf :Annotation ;
                    rdfs:comment "A Caliper BookmarkAnnotation represents the act of marking a DigitalResource at a particular location."@en ;
                    rdfs:isDefinedBy "http://purl.imsglobal.org/caliper"^^xsd:string ;
                    rdfs:label "BookmarkAnnotation"@en .


###  http://purl.imsglobal.org/caliper/Chapter
:Chapter rdf:type owl:Class ;
         rdfs:subClassOf :DigitalResource ;
         rdfs:comment "A Caliper Chapter represents a major sub-division of a piece of digital content."@en ;
         rdfs:isDefinedBy "http://purl.imsglobal.org/caliper"^^xsd:string ;
         rdfs:label "Chapter"@en .


###  http://purl.imsglobal.org/caliper/Collection
:Collection rdf:type owl:Class ;
            rdfs:subClassOf :Entity ;
            rdfs:comment "A Caliper Collection represents an unordered collection of entities."@en ;
            rdfs:isDefinedBy "http://purl.imsglobal.org/caliper"^^xsd:string ;
            rdfs:label "Collection"@en .


###  http://purl.imsglobal.org/caliper/Comment
:Comment rdf:type owl:Class ;
         rdfs:subClassOf :Entity ,
                         [ owl:intersectionOf ( [ rdf:type owl:Restriction ;
                                                  owl:onProperty :commenter ;
                                                  owl:someValuesFrom :Agent
                                                ]
                                                [ rdf:type owl:Restriction ;
                                                  owl:onProperty :commenter ;
                                                  owl:allValuesFrom :Person
                                                ]
                                              ) ;
                           rdf:type owl:Class
                         ] ,
                         [ rdf:type owl:Restriction ;
                           owl:onProperty :commentedOn ;
                           owl:someValuesFrom :Entity
                         ] ;
         rdfs:comment "A Caliper Comment models a person's qualitative reactions to a Entity."@en ;
         rdfs:isDefinedBy "https://purl.imsglobal.org/caliper"^^xsd:string ;
         rdfs:label "Comment"@en .


###  http://purl.imsglobal.org/caliper/CourseOffering
:CourseOffering rdf:type owl:Class ;
                rdfs:subClassOf :Organization ;
                owl:disjointWith :Group ;
                rdfs:comment "A Caliper CourseOffering represents the occurrence of a course or a type during a specified time period."@en ;
                rdfs:isDefinedBy "http://purl.imsglobal.org/caliper"^^xsd:string ;
                rdfs:label "CourseOffering"@en .


###  http://purl.imsglobal.org/caliper/CourseSection
:CourseSection rdf:type owl:Class ;
               rdfs:subClassOf :CourseOffering ;
               rdfs:comment "A Caliper CourseSection represents a specific instance of a CourseOffering occurring during a specific semester, term or period."@en ;
               rdfs:isDefinedBy "http://purl.imsglobal.org/caliper"^^xsd:string ;
               rdfs:label "CourseSection"@en .


###  http://purl.imsglobal.org/caliper/DigitalResource
:DigitalResource rdf:type owl:Class ;
                 rdfs:subClassOf :Entity ;
                 rdfs:comment "A Caliper DigitalResource is a generic type that represents digital content.  Utilize DigitalResource only if no suitable subtype exists to represent the resource being described."@en ;
                 rdfs:isDefinedBy "http://purl.imsglobal.org/caliper"^^xsd:string ;
                 rdfs:label "DigitalResource"@en .


###  http://purl.imsglobal.org/caliper/DigitalResourceCollection
:DigitalResourceCollection rdf:type owl:Class ;
                           rdfs:subClassOf :Collection ,
                                           :DigitalResource ,
                                           [ owl:intersectionOf ( [ rdf:type owl:Restriction ;
                                                                    owl:onProperty :items ;
                                                                    owl:someValuesFrom :Entity
                                                                  ]
                                                                  [ rdf:type owl:Restriction ;
                                                                    owl:onProperty :items ;
                                                                    owl:allValuesFrom :DigitalResource
                                                                  ]
                                                                ) ;
                                             rdf:type owl:Class
                                           ] ;
                           rdfs:comment "A Caliper DigitalResourceCollection represents an ordered collection of DigitalResource entities."@en ;
                           rdfs:isDefinedBy "http://purl.imsglobal.org/caliper"^^xsd:string ;
                           rdfs:label "DigitalResourceCollection"@en .


###  http://purl.imsglobal.org/caliper/Document
:Document rdf:type owl:Class ;
          rdfs:subClassOf :DigitalResource ;
          rdfs:comment "A Caliper Document represents paginated textual content."@en ;
          rdfs:isDefinedBy "http://purl.imsglobal.org/caliper"^^xsd:string ;
          rdfs:label "Document"@en .


###  http://purl.imsglobal.org/caliper/Entity
:Entity rdf:type owl:Class ;
        rdfs:comment "A Caliper Entity is a generic type that represents objects or things that participate in learning-related activities. Entity is subtyped for enhanced type specificity in order to better describe people, groups, digital content, courses, assignments, assessments, forums, messages, software applications and other entities that constitute the \"stuff\" of a Caliper Event.  Utilize Entity only if no suitable subtype exists to represent the thing being described."@en ;
        rdfs:isDefinedBy "http://purl.imsglobal.org/caliper"^^xsd:string ;
        rdfs:label "Entity"@en .


###  http://purl.imsglobal.org/caliper/Envelope
:Envelope rdf:type owl:Class ;
          rdfs:comment "A Caliper Envelope is a container that is used to transmit one or more Caliper Events and/or Caliper Entity describes."@en ;
          rdfs:isDefinedBy "http://purl.imsglobal.org/caliper"^^xsd:string ;
          rdfs:label "Envelope"@en .


###  http://purl.imsglobal.org/caliper/Event
:Event rdf:type owl:Class ;
       rdfs:comment "A Caliper Event is a generic type that describes a relationship established between an actor and an object, formed as a result of a purposeful action undertaken by the actor in connection to the object at a particular moment in time."@en ;
       rdfs:isDefinedBy "http://purl.imsglobal.org/caliper"^^xsd:string ;
       rdfs:label "Event"@en .


###  http://purl.imsglobal.org/caliper/FeedbackEvent
:FeedbackEvent rdf:type owl:Class ;
               rdfs:subClassOf :Event ,
                               [ owl:intersectionOf ( [ rdf:type owl:Restriction ;
                                                        owl:onProperty :action ;
                                                        owl:someValuesFrom :Action
                                                      ]
                                                      [ rdf:type owl:Restriction ;
                                                        owl:onProperty :action ;
                                                        owl:someValuesFrom [ rdf:type owl:Class ;
                                                                             owl:oneOf ( <http://purl.imsglobal.org/caliper/actions/Commented>
                                                                                         <http://purl.imsglobal.org/caliper/actions/Ranked>
                                                                                       )
                                                                           ]
                                                      ]
                                                    ) ;
                                 rdf:type owl:Class
                               ] ,
                               [ owl:intersectionOf ( [ rdf:type owl:Restriction ;
                                                        owl:onProperty :actor ;
                                                        owl:someValuesFrom :Agent
                                                      ]
                                                      [ rdf:type owl:Restriction ;
                                                        owl:onProperty :actor ;
                                                        owl:allValuesFrom :Person
                                                      ]
                                                    ) ;
                                 rdf:type owl:Class
                               ] ,
                               [ owl:intersectionOf ( [ rdf:type owl:Restriction ;
                                                        owl:onProperty :generated ;
                                                        owl:someValuesFrom :Entity
                                                      ]
                                                      [ rdf:type owl:Restriction ;
                                                        owl:onProperty :generated ;
                                                        owl:allValuesFrom [ rdf:type owl:Class ;
                                                                            owl:unionOf ( :Comment
                                                                                          :Rating
                                                                                        )
                                                                          ]
                                                      ]
                                                    ) ;
                                 rdf:type owl:Class
                               ] ,
                               [ owl:intersectionOf ( [ rdf:type owl:Restriction ;
                                                        owl:onProperty :target ;
                                                        owl:someValuesFrom :DigitalResource
                                                      ]
                                                      [ rdf:type owl:Restriction ;
                                                        owl:onProperty :target ;
                                                        owl:allValuesFrom :Frame
                                                      ]
                                                    ) ;
                                 rdf:type owl:Class
                               ] ,
                               [ rdf:type owl:Restriction ;
                                 owl:onProperty :object ;
                                 owl:someValuesFrom :Entity
                               ] ;
               rdfs:comment "A Caliper FeedbackEvent models a Person providing informal feedback on an Entity, typically a DigitalResource or another Person."@en ;
               rdfs:isDefinedBy "http://purl.imsglobal.org/caliper"^^xsd:string ;
               rdfs:label "FeedbackEvent"@en .


###  http://purl.imsglobal.org/caliper/FillinBlankResponse
:FillinBlankResponse rdf:type owl:Class ;
                     rdfs:subClassOf :Response ;
                     rdfs:comment "A Caliper FillinBlankResponse represents a type of Response in which a respondent is asked to provide one or more words, expressions or short phrases that correctly completes a statement."@en ;
                     rdfs:isDefinedBy "http://purl.imsglobal.org/caliper"^^xsd:string ;
                     rdfs:label "FillinBlankResponse"@en .


###  http://purl.imsglobal.org/caliper/Forum
:Forum rdf:type owl:Class ;
       rdfs:subClassOf :DigitalResourceCollection ,
                       [ owl:intersectionOf ( [ rdf:type owl:Restriction ;
                                                owl:onProperty :items ;
                                                owl:someValuesFrom :Entity
                                              ]
                                              [ rdf:type owl:Restriction ;
                                                owl:onProperty :items ;
                                                owl:allValuesFrom :Thread
                                              ]
                                            ) ;
                         rdf:type owl:Class
                       ] ;
       owl:disjointWith :Thread ;
       rdfs:comment "A Caliper Forum represents a channel or virtual space in which group discussions take place.  A Forum typically comprises one or more threaded conversations to which members can subscribe, post messages and reply to other messages."@en ;
       rdfs:isDefinedBy "http://purl.imsglobal.org/caliper"^^xsd:string ;
       rdfs:label "Forum"@en .


###  http://purl.imsglobal.org/caliper/ForumEvent
:ForumEvent rdf:type owl:Class ;
            rdfs:subClassOf :Event ,
                            [ owl:intersectionOf ( [ rdf:type owl:Restriction ;
                                                     owl:onProperty :action ;
                                                     owl:someValuesFrom :Action
                                                   ]
                                                   [ rdf:type owl:Restriction ;
                                                     owl:onProperty :action ;
                                                     owl:someValuesFrom [ rdf:type owl:Class ;
                                                                          owl:oneOf ( <http://purl.imsglobal.org/caliper/actions/Subscribed>
                                                                                      <http://purl.imsglobal.org/caliper/actions/Unsubscribed>
                                                                                    )
                                                                        ]
                                                   ]
                                                 ) ;
                              rdf:type owl:Class
                            ] ,
                            [ owl:intersectionOf ( [ rdf:type owl:Restriction ;
                                                     owl:onProperty :actor ;
                                                     owl:someValuesFrom :Agent
                                                   ]
                                                   [ rdf:type owl:Restriction ;
                                                     owl:onProperty :actor ;
                                                     owl:allValuesFrom :Person
                                                   ]
                                                 ) ;
                              rdf:type owl:Class
                            ] ,
                            [ owl:intersectionOf ( [ rdf:type owl:Restriction ;
                                                     owl:onProperty :object ;
                                                     owl:someValuesFrom :DigitalResource
                                                   ]
                                                   [ rdf:type owl:Restriction ;
                                                     owl:onProperty :object ;
                                                     owl:allValuesFrom :Forum
                                                   ]
                                                 ) ;
                              rdf:type owl:Class
                            ] ;
            rdfs:comment "A Caliper ForumEvent models learners and others participating in online forum communities. Forums typically encompass one or more threads or topics to which members can subscribe, post messages and reply to other messages if a threaded discussion is permitted."@en ;
            rdfs:isDefinedBy "http://purl.imsglobal.org/caliper"^^xsd:string ;
            rdfs:label "ForumEvent"@en .


###  http://purl.imsglobal.org/caliper/Frame
:Frame rdf:type owl:Class ;
       rdfs:subClassOf :DigitalResource ;
       rdfs:comment "A Caliper Frame represents a part, portion or segment of a DigitalResource."@en ;
       rdfs:isDefinedBy "http://purl.imsglobal.org/caliper"^^xsd:string ;
       rdfs:label "Frame"@en .


###  http://purl.imsglobal.org/caliper/GradeEvent
:GradeEvent rdf:type owl:Class ;
            rdfs:subClassOf :Event ,
                            [ owl:intersectionOf ( [ rdf:type owl:Restriction ;
                                                     owl:onProperty :action ;
                                                     owl:someValuesFrom :Action
                                                   ]
                                                   [ rdf:type owl:Restriction ;
                                                     owl:onProperty :action ;
                                                     owl:hasValue <http://purl.imsglobal.org/caliper/actions/Graded>
                                                   ]
                                                 ) ;
                              rdf:type owl:Class
                            ] ,
                            [ owl:intersectionOf ( [ rdf:type owl:Restriction ;
                                                     owl:onProperty :actor ;
                                                     owl:someValuesFrom :Agent
                                                   ]
                                                   [ rdf:type owl:Restriction ;
                                                     owl:onProperty :actor ;
                                                     owl:allValuesFrom [ rdf:type owl:Class ;
                                                                         owl:unionOf ( :Person
                                                                                       :SoftwareApplication
                                                                                     )
                                                                       ]
                                                   ]
                                                 ) ;
                              rdf:type owl:Class
                            ] ,
                            [ owl:intersectionOf ( [ rdf:type owl:Restriction ;
                                                     owl:onProperty :object ;
                                                     owl:someValuesFrom :Entity
                                                   ]
                                                   [ rdf:type owl:Restriction ;
                                                     owl:onProperty :object ;
                                                     owl:allValuesFrom :Attempt
                                                   ]
                                                 ) ;
                              rdf:type owl:Class
                            ] ,
                            [ rdf:type owl:Restriction ;
                              owl:onProperty :generated ;
                              owl:someValuesFrom :Score
                            ] ;
            rdfs:comment "A Caliper GradeEvent models grading activities performed by an Agent, typically a Person or a SoftwareApplication."@en ;
            rdfs:isDefinedBy "http://purl.imsglobal.org/caliper"^^xsd:string ;
            rdfs:label "GradeEvent"@en .


###  http://purl.imsglobal.org/caliper/Group
:Group rdf:type owl:Class ;
       rdfs:subClassOf :Organization ;
       rdfs:comment "A Caliper Group represents an ad-hoc, informal or short-lived collection of people organized for some common educational or social purpose.  A Group can act as an Agent. It can be linked both to a parent Organization and to its members."@en ;
       rdfs:isDefinedBy "http://purl.imsglobal.org/caliper"^^xsd:string ;
       rdfs:label "Group"@en .


###  http://purl.imsglobal.org/caliper/HighlightAnnotation
:HighlightAnnotation rdf:type owl:Class ;
                     rdfs:subClassOf :Annotation ;
                     rdfs:comment "A Caliper HighlightAnnotation represents the act of marking a particular segment of a DigitalResource between two known coordinates."@en ;
                     rdfs:isDefinedBy "http://purl.imsglobal.org/caliper"^^xsd:string ;
                     rdfs:label "HighlightAnnotation"@en .


###  http://purl.imsglobal.org/caliper/ImageObject
:ImageObject rdf:type owl:Class ;
             rdfs:subClassOf :MediaObject ;
             rdfs:comment "A Caliper ImageObject represents an image file."@en ;
             rdfs:isDefinedBy "http://purl.imsglobal.org/caliper"^^xsd:string ;
             rdfs:label "ImageObject"@en .


###  http://purl.imsglobal.org/caliper/LearningObjective
:LearningObjective rdf:type owl:Class ;
                   rdfs:subClassOf :Entity ;
                   rdfs:comment "A Caliper LearningObjective represents a brief statement of what a learner should know or be able to perform after completing a unit of instruction or a period of learning."@en ;
                   rdfs:isDefinedBy "http://purl.imsglobal.org/caliper"^^xsd:string ;
                   rdfs:label "LearningObjective"@en .


###  http://purl.imsglobal.org/caliper/LikertScale
:LikertScale rdf:type owl:Class ;
             rdfs:subClassOf :Scale ;
             rdfs:comment "A Caliper LikertScale models a Likert scale employed for scaling responses."@en ;
             rdfs:isDefinedBy "https://purl.imsglobal.org/caliper"^^xsd:string ;
             rdfs:label "LikertScale"@en .


###  http://purl.imsglobal.org/caliper/Link
:Link rdf:type owl:Class ;
      rdfs:subClassOf :Entity ;
      rdfs:comment "The Link entity represents a URL that might be a UI workflow or service endpoint (transient or otherwise), and not necessarily a proper Digital Resource (such as a WebPage or LtiLink."@en ;
      rdfs:isDefinedBy "http://purl.imsglobal.org/caliper"^^xsd:string ;
      rdfs:label "Link"@en .


###  http://purl.imsglobal.org/caliper/LtiLink
:LtiLink rdf:type owl:Class ;
         rdfs:subClassOf :DigitalResource ;
         rdfs:comment "The LtiLink entity represents a digital resource that must be retrieved from an external tool application via an LTI request message. It is, effectively, a Digital Resource that must use LTI for access."@en ;
         rdfs:isDefinedBy "http://purl.imsglobal.org/caliper"^^xsd:string ;
         rdfs:label "LtiLink"@en .


###  http://purl.imsglobal.org/caliper/LtiMessageType
:LtiMessageType rdf:type owl:Class ;
                rdfs:comment "The LTI specification defines a number of message types that are exchanged between platforms and tools.  Each LTI message type describes or asserts a set of required and optional sender claims that are communicated to a receiver at particular moments in the workflow."@en ;
                rdfs:isDefinedBy "http://purl.imsglobal.org/caliper"^^xsd:string ;
                rdfs:label "LtiMessageType"@en .


###  http://purl.imsglobal.org/caliper/LtiSession
:LtiSession rdf:type owl:Class ;
            rdfs:subClassOf :Session ;
            rdfs:comment "A Caliper LtiSession represents an LTI Tool Consumer user session."@en ;
            rdfs:label "LtiSession"@en .


###  http://purl.imsglobal.org/caliper/MediaEvent
:MediaEvent rdf:type owl:Class ;
            rdfs:subClassOf :Event ,
                            [ owl:intersectionOf ( [ rdf:type owl:Restriction ;
                                                     owl:onProperty :action ;
                                                     owl:someValuesFrom :Action
                                                   ]
                                                   [ rdf:type owl:Restriction ;
                                                     owl:onProperty :action ;
                                                     owl:someValuesFrom [ rdf:type owl:Class ;
                                                                          owl:oneOf ( <http://purl.imsglobal.org/caliper/actions/ChangedResolution>
                                                                                      <http://purl.imsglobal.org/caliper/actions/ChangedSize>
                                                                                      <http://purl.imsglobal.org/caliper/actions/ChangedSpeed>
                                                                                      <http://purl.imsglobal.org/caliper/actions/ChangedVolume>
                                                                                      <http://purl.imsglobal.org/caliper/actions/ClosedPopout>
                                                                                      <http://purl.imsglobal.org/caliper/actions/DisabledClosedCaptioning>
                                                                                      <http://purl.imsglobal.org/caliper/actions/EnabledClosedCaptioning>
                                                                                      <http://purl.imsglobal.org/caliper/actions/Ended>
                                                                                      <http://purl.imsglobal.org/caliper/actions/EnteredFullScreen>
                                                                                      <http://purl.imsglobal.org/caliper/actions/ExitedFullScreen>
                                                                                      <http://purl.imsglobal.org/caliper/actions/ForwardedTo>
                                                                                      <http://purl.imsglobal.org/caliper/actions/JumpedTo>
                                                                                      <http://purl.imsglobal.org/caliper/actions/Muted>
                                                                                      <http://purl.imsglobal.org/caliper/actions/OpenedPopout>
                                                                                      <http://purl.imsglobal.org/caliper/actions/Paused>
                                                                                      <http://purl.imsglobal.org/caliper/actions/Restarted>
                                                                                      <http://purl.imsglobal.org/caliper/actions/Resumed>
                                                                                      <http://purl.imsglobal.org/caliper/actions/Started>
                                                                                      <http://purl.imsglobal.org/caliper/actions/Unmuted>
                                                                                    )
                                                                        ]
                                                   ]
                                                 ) ;
                              rdf:type owl:Class
                            ] ,
                            [ owl:intersectionOf ( [ rdf:type owl:Restriction ;
                                                     owl:onProperty :actor ;
                                                     owl:someValuesFrom :Agent
                                                   ]
                                                   [ rdf:type owl:Restriction ;
                                                     owl:onProperty :actor ;
                                                     owl:allValuesFrom :Person
                                                   ]
                                                 ) ;
                              rdf:type owl:Class
                            ] ,
                            [ owl:intersectionOf ( [ rdf:type owl:Restriction ;
                                                     owl:onProperty :object ;
                                                     owl:someValuesFrom :DigitalResource
                                                   ]
                                                   [ rdf:type owl:Restriction ;
                                                     owl:onProperty :object ;
                                                     owl:allValuesFrom :MediaObject
                                                   ]
                                                 ) ;
                              rdf:type owl:Class
                            ] ,
                            [ rdf:type owl:Restriction ;
                              owl:onProperty :target ;
                              owl:someValuesFrom :MediaLocation
                            ] ;
            rdfs:comment "A Caliper MediaEvent models interactions between learners and rich content such as audio, images and video."@en ;
            rdfs:isDefinedBy "http://purl.imsglobal.org/caliper"^^xsd:string ;
            rdfs:label "MediaEvent"@en .


###  http://purl.imsglobal.org/caliper/MediaLocation
:MediaLocation rdf:type owl:Class ;
               rdfs:subClassOf :DigitalResource ;
               rdfs:comment "A Caliper MediaLocation provides the current playback position in a MediaObject such as an AudioObject or VideoObject."@en ;
               rdfs:isDefinedBy "http://purl.imsglobal.org/caliper"^^xsd:string ;
               rdfs:label "MediaLocation"@en .


###  http://purl.imsglobal.org/caliper/MediaObject
:MediaObject rdf:type owl:Class ;
             rdfs:subClassOf :DigitalResource ;
             rdfs:comment "A Caliper MediaObject represents a generic piece of media content.  Utilize MediaObject only if no suitable subtype exists to represent the resource being described."@en ;
             rdfs:isDefinedBy "http://purl.imsglobal.org/caliper"^^xsd:string ;
             rdfs:label "MediaObject"@en .


###  http://purl.imsglobal.org/caliper/Membership
:Membership rdf:type owl:Class ;
            rdfs:subClassOf :Entity ,
                            [ owl:intersectionOf ( [ rdf:type owl:Restriction ;
                                                     owl:onProperty :member ;
                                                     owl:someValuesFrom :Agent
                                                   ]
                                                   [ rdf:type owl:Restriction ;
                                                     owl:onProperty :member ;
                                                     owl:allValuesFrom :Person
                                                   ]
                                                 ) ;
                              rdf:type owl:Class
                            ] ,
                            [ owl:intersectionOf ( [ rdf:type owl:Restriction ;
                                                     owl:onProperty :organization ;
                                                     owl:someValuesFrom :Agent
                                                   ]
                                                   [ rdf:type owl:Restriction ;
                                                     owl:onProperty :organization ;
                                                     owl:allValuesFrom :Organization
                                                   ]
                                                 ) ;
                              rdf:type owl:Class
                            ] ;
            rdfs:comment "A Caliper Membership describes the relationship between an Organization and a Person (i.e., a member) in terms of the roles assigned and current status."@en ;
            rdfs:isDefinedBy "http://purl.imsglobal.org/caliper"^^xsd:string ;
            rdfs:label "Membership"@en .


###  http://purl.imsglobal.org/caliper/Message
:Message rdf:type owl:Class ;
         rdfs:subClassOf :DigitalResource ,
                         [ owl:intersectionOf ( [ rdf:type owl:Restriction ;
                                                  owl:onProperty :isPartOf ;
                                                  owl:someValuesFrom :Entity
                                                ]
                                                [ rdf:type owl:Restriction ;
                                                  owl:onProperty :isPartOf ;
                                                  owl:allValuesFrom :Thread
                                                ]
                                              ) ;
                           rdf:type owl:Class
                         ] ;
         rdfs:comment "A Caliper Message is a digital form of written communication sent to a recipient. A series of messages may constitute a Thread if they share a common subject and are connected by a reply or by date relationships."@en ;
         rdfs:isDefinedBy "http://purl.imsglobal.org/caliper"^^xsd:string ;
         rdfs:label "Message"@en .


###  http://purl.imsglobal.org/caliper/MessageEvent
:MessageEvent rdf:type owl:Class ;
              rdfs:subClassOf :Event ,
                              [ owl:intersectionOf ( [ rdf:type owl:Restriction ;
                                                       owl:onProperty :action ;
                                                       owl:someValuesFrom :Action
                                                     ]
                                                     [ rdf:type owl:Restriction ;
                                                       owl:onProperty :action ;
                                                       owl:someValuesFrom [ rdf:type owl:Class ;
                                                                            owl:oneOf ( <http://purl.imsglobal.org/caliper/actions/MarkedAsRead>
                                                                                        <http://purl.imsglobal.org/caliper/actions/MarkedAsUnread>
                                                                                        <http://purl.imsglobal.org/caliper/actions/Posted>
                                                                                      )
                                                                          ]
                                                     ]
                                                   ) ;
                                rdf:type owl:Class
                              ] ,
                              [ owl:intersectionOf ( [ rdf:type owl:Restriction ;
                                                       owl:onProperty :actor ;
                                                       owl:someValuesFrom :Agent
                                                     ]
                                                     [ rdf:type owl:Restriction ;
                                                       owl:onProperty :actor ;
                                                       owl:allValuesFrom :Person
                                                     ]
                                                   ) ;
                                rdf:type owl:Class
                              ] ,
                              [ owl:intersectionOf ( [ rdf:type owl:Restriction ;
                                                       owl:onProperty :object ;
                                                       owl:someValuesFrom :DigitalResource
                                                     ]
                                                     [ rdf:type owl:Restriction ;
                                                       owl:onProperty :object ;
                                                       owl:allValuesFrom :Message
                                                     ]
                                                   ) ;
                                rdf:type owl:Class
                              ] ;
              rdfs:comment "A Caliper MessageEvent describes a Person posting a Message or marking a post as either read or unread."@en ;
              rdfs:isDefinedBy "http://purl.imsglobal.org/caliper"^^xsd:string ;
              rdfs:label "MessageEvent"@en .


###  http://purl.imsglobal.org/caliper/Metric
:Metric rdf:type owl:Class ;
        rdfs:comment "The AggregateMeasure entity includes a required metric property for denoting the metric related to the ToolUseEvent."@en ;
        rdfs:isDefinedBy "http://purl.imsglobal.org/caliper"^^xsd:string ;
        rdfs:label "Metric"@en .


###  http://purl.imsglobal.org/caliper/MultiSelectScale
:MultiSelectScale rdf:type owl:Class ;
                  rdfs:subClassOf :Scale ;
                  rdfs:comment "A Caliper MultiselectScale models a scale used to capture one or more rating options."@en ;
                  rdfs:isDefinedBy "https://purl.imsglobal.org/caliper"^^xsd:string ;
                  rdfs:label "MultiSelectScale"@en .


###  http://purl.imsglobal.org/caliper/MultipleChoiceResponse
:MultipleChoiceResponse rdf:type owl:Class ;
                        rdfs:subClassOf :Response ;
                        rdfs:comment "A Caliper MultipleChoiceResponse represents a type of Response in which a respondent is asked to provide the best possible answer from a list of choices."@en ;
                        rdfs:isDefinedBy "http://purl.imsglobal.org/caliper"^^xsd:string ;
                        rdfs:label "MultipleChoiceResponse"@en .


###  http://purl.imsglobal.org/caliper/MultipleResponseResponse
:MultipleResponseResponse rdf:type owl:Class ;
                          rdfs:subClassOf :Response ;
                          rdfs:comment "A Caliper MultipleResponseResponse represents a form of response in which a respondent is asked to select more than one correct answer from a list of choices."@en ;
                          rdfs:isDefinedBy "http://purl.imsglobal.org/caliper"^^xsd:string ;
                          rdfs:label "MultipleResponseResponse"@en .


###  http://purl.imsglobal.org/caliper/NavigationEvent
:NavigationEvent rdf:type owl:Class ;
                 rdfs:subClassOf :Event ,
                                 [ owl:intersectionOf ( [ rdf:type owl:Restriction ;
                                                          owl:onProperty :action ;
                                                          owl:someValuesFrom :Action
                                                        ]
                                                        [ rdf:type owl:Restriction ;
                                                          owl:onProperty :action ;
                                                          owl:hasValue <http://purl.imsglobal.org/caliper/actions/NavigatedTo>
                                                        ]
                                                      ) ;
                                   rdf:type owl:Class
                                 ] ,
                                 [ owl:intersectionOf ( [ rdf:type owl:Restriction ;
                                                          owl:onProperty :actor ;
                                                          owl:someValuesFrom :Agent
                                                        ]
                                                        [ rdf:type owl:Restriction ;
                                                          owl:onProperty :actor ;
                                                          owl:allValuesFrom :Person
                                                        ]
                                                      ) ;
                                   rdf:type owl:Class
                                 ] ,
                                 [ owl:intersectionOf ( [ rdf:type owl:Restriction ;
                                                          owl:onProperty :object ;
                                                          owl:someValuesFrom :Entity
                                                        ]
                                                        [ rdf:type owl:Restriction ;
                                                          owl:onProperty :object ;
                                                          owl:allValuesFrom [ rdf:type owl:Class ;
                                                                              owl:unionOf ( :DigitalResource
                                                                                            :SoftwareApplication
                                                                                          )
                                                                            ]
                                                        ]
                                                      ) ;
                                   rdf:type owl:Class
                                 ] ,
                                 [ owl:intersectionOf ( [ rdf:type owl:Restriction ;
                                                          owl:onProperty :referrer ;
                                                          owl:someValuesFrom :Entity
                                                        ]
                                                        [ rdf:type owl:Restriction ;
                                                          owl:onProperty :referrer ;
                                                          owl:allValuesFrom [ rdf:type owl:Class ;
                                                                              owl:unionOf ( :DigitalResource
                                                                                            :SoftwareApplication
                                                                                          )
                                                                            ]
                                                        ]
                                                      ) ;
                                   rdf:type owl:Class
                                 ] ,
                                 [ rdf:type owl:Restriction ;
                                   owl:onProperty :target ;
                                   owl:someValuesFrom :Frame
                                 ] ;
                 rdfs:comment "A Caliper NavigationEvent models an actor traversing a network of digital resources."@en ;
                 rdfs:isDefinedBy "http://purl.imsglobal.org/caliper"^^xsd:string ;
                 rdfs:label "NavigationEvent"@en .


###  http://purl.imsglobal.org/caliper/NumericScale
:NumericScale rdf:type owl:Class ;
              rdfs:subClassOf :Scale ;
              rdfs:comment "A Caliper NumericScale models a numeric scale used to capture some rating."@en ;
              rdfs:isDefinedBy "https://purl.imsglobal.org/caliper"^^xsd:string ;
              rdfs:label "NumericScale"@en .


###  http://purl.imsglobal.org/caliper/Organization
:Organization rdf:type owl:Class ;
              rdfs:subClassOf :Agent ;
              rdfs:comment "A Caliper Organization represents a formal collection of people organized for some common educational, social or administrative purpose. An Organization can act as an Agent. It can be linked both to a parent Organization and to its members."@en ;
              rdfs:isDefinedBy "http://purl.imsglobal.org/caliper"^^xsd:string ;
              rdfs:label "Organization"@en .


###  http://purl.imsglobal.org/caliper/OutcomeEvent
:OutcomeEvent rdf:type owl:Class ;
              rdfs:subClassOf :Event ,
                              [ owl:intersectionOf ( [ rdf:type owl:Restriction ;
                                                       owl:onProperty :action ;
                                                       owl:someValuesFrom :Action
                                                     ]
                                                     [ rdf:type owl:Restriction ;
                                                       owl:onProperty :action ;
                                                       owl:hasValue <http://purl.imsglobal.org/caliper/actions/Graded>
                                                     ]
                                                   ) ;
                                rdf:type owl:Class
                              ] ,
                              [ owl:intersectionOf ( [ rdf:type owl:Restriction ;
                                                       owl:onProperty :actor ;
                                                       owl:someValuesFrom :Agent
                                                     ]
                                                     [ rdf:type owl:Restriction ;
                                                       owl:onProperty :actor ;
                                                       owl:allValuesFrom [ rdf:type owl:Class ;
                                                                           owl:unionOf ( :Person
                                                                                         :SoftwareApplication
                                                                                       )
                                                                         ]
                                                     ]
                                                   ) ;
                                rdf:type owl:Class
                              ] ,
                              [ owl:intersectionOf ( [ rdf:type owl:Restriction ;
                                                       owl:onProperty :generated ;
                                                       owl:someValuesFrom :Entity
                                                     ]
                                                     [ rdf:type owl:Restriction ;
                                                       owl:onProperty :generated ;
                                                       owl:allValuesFrom :Result
                                                     ]
                                                   ) ;
                                rdf:type owl:Class
                              ] ,
                              [ owl:intersectionOf ( [ rdf:type owl:Restriction ;
                                                       owl:onProperty :object ;
                                                       owl:someValuesFrom :Entity
                                                     ]
                                                     [ rdf:type owl:Restriction ;
                                                       owl:onProperty :object ;
                                                       owl:allValuesFrom :Attempt
                                                     ]
                                                   ) ;
                                rdf:type owl:Class
                              ] ;
              <http://purl.org/dc/terms/isReplacedBy> :GradeEvent ;
              rdfs:comment "A Caliper OutcomeEvent models grading activities performed by an Agent, typically a Person or a SoftwareApplication.  OutcomeEvent is DEPRECATED and will be removed in a future version of the specification. Use GradeEvent instead."@en ;
              rdfs:isDefinedBy "http://purl.imsglobal.org/caliper"^^xsd:string ;
              rdfs:label "OutcomeEvent"@en ;
              owl:deprecated "true"^^xsd:boolean .


###  http://purl.imsglobal.org/caliper/Page
:Page rdf:type owl:Class ;
      rdfs:subClassOf :DigitalResource ;
      rdfs:comment "A Caliper Page represents an item of paginated content."@en ;
      rdfs:isDefinedBy "http://purl.imsglobal.org/caliper"^^xsd:string ;
      rdfs:label "Page"@en .


###  http://purl.imsglobal.org/caliper/Person
:Person rdf:type owl:Class ;
        rdfs:subClassOf :Agent ;
        rdfs:comment "A Caliper Person represents a human being, alive or deceased, real or imaginary."@en ;
        rdfs:isDefinedBy "http://purl.imsglobal.org/caliper"^^xsd:string ;
        rdfs:label "Person"@en .


###  http://purl.imsglobal.org/caliper/Query
:Query rdf:type owl:Class ;
       rdfs:subClassOf :Entity ;
       rdfs:comment "A Caliper Query models search criteria created by an actor that targets a searchable resource."@en ;
       rdfs:isDefinedBy "http://purl.imsglobal.org/caliper"^^xsd:string ;
       rdfs:label "Query"@en .


###  http://purl.imsglobal.org/caliper/Rating
:Rating rdf:type owl:Class ;
        rdfs:subClassOf :Entity ,
                        [ owl:intersectionOf ( [ rdf:type owl:Restriction ;
                                                 owl:onProperty :rater ;
                                                 owl:someValuesFrom :Agent
                                               ]
                                               [ rdf:type owl:Restriction ;
                                                 owl:onProperty :rater ;
                                                 owl:allValuesFrom :Person
                                               ]
                                             ) ;
                          rdf:type owl:Class
                        ] ,
                        [ rdf:type owl:Restriction ;
                          owl:onProperty :rated ;
                          owl:someValuesFrom :Entity
                        ] ;
        rdfs:comment "A Caliper Rating models quantitative reactions to an Entity."@en ;
        rdfs:isDefinedBy "https://purl.imsglobal.org/caliper"^^xsd:string ;
        rdfs:label "Rating"@en .


###  http://purl.imsglobal.org/caliper/Reading
:Reading rdf:type owl:Class ;
         rdfs:subClassOf :DigitalResource ;
         <http://purl.org/dc/terms/isReplacedBy> :Document ;
         rdfs:comment "A Caliper Reading represents paginated content. Reading is a DEPRECATED entity superseded by Document that will be removed in a future version of the specification. It SHOULD NOT be referenced."@en ;
         rdfs:isDefinedBy "http://purl.imsglobal.org/caliper"^^xsd:string ;
         rdfs:label "Reading"@en ;
         owl:deprecated "true"^^xsd:boolean .


###  http://purl.imsglobal.org/caliper/ReadingEvent
:ReadingEvent rdf:type owl:Class ;
              rdfs:subClassOf :Event ,
                              [ owl:intersectionOf ( [ rdf:type owl:Restriction ;
                                                       owl:onProperty :action ;
                                                       owl:someValuesFrom :Action
                                                     ]
                                                     [ rdf:type owl:Restriction ;
                                                       owl:onProperty :action ;
                                                       owl:someValuesFrom [ rdf:type owl:Class ;
                                                                            owl:oneOf ( <http://purl.imsglobal.org/caliper/actions/NavigatedTo>
                                                                                        <http://purl.imsglobal.org/caliper/actions/Searched>
                                                                                        <http://purl.imsglobal.org/caliper/actions/Viewed>
                                                                                      )
                                                                          ]
                                                     ]
                                                   ) ;
                                rdf:type owl:Class
                              ] ,
                              [ owl:intersectionOf ( [ rdf:type owl:Restriction ;
                                                       owl:onProperty :actor ;
                                                       owl:someValuesFrom :Agent
                                                     ]
                                                     [ rdf:type owl:Restriction ;
                                                       owl:onProperty :actor ;
                                                       owl:allValuesFrom :Person
                                                     ]
                                                   ) ;
                                rdf:type owl:Class
                              ] ,
                              [ owl:intersectionOf ( [ rdf:type owl:Restriction ;
                                                       owl:onProperty :object ;
                                                       owl:someValuesFrom :Entity
                                                     ]
                                                     [ rdf:type owl:Restriction ;
                                                       owl:onProperty :object ;
                                                       owl:allValuesFrom :DigitalResource
                                                     ]
                                                   ) ;
                                rdf:type owl:Class
                              ] ,
                              [ rdf:type owl:Restriction ;
                                owl:onProperty :target ;
                                owl:someValuesFrom :Frame
                              ] ;
              rdfs:comment "A Caliper ReadingEvent models an actor reading textural content.  ReadingEvent is DEPRECATED and will be removed in a future version of the specification.  It SHOULD NOT be referenced."@en ;
              rdfs:isDefinedBy "http://purl.imsglobal.org/caliper"^^xsd:string ;
              rdfs:label "ReadingEvent"@en ;
              owl:deprecated "true"^^xsd:boolean .


###  http://purl.imsglobal.org/caliper/ResourceManagementEvent
:ResourceManagementEvent rdf:type owl:Class ;
                         rdfs:subClassOf :Event ,
                                         [ owl:intersectionOf ( [ rdf:type owl:Restriction ;
                                                                  owl:onProperty :action ;
                                                                  owl:someValuesFrom :Action
                                                                ]
                                                                [ rdf:type owl:Restriction ;
                                                                  owl:onProperty :action ;
                                                                  owl:someValuesFrom [ rdf:type owl:Class ;
                                                                                       owl:oneOf ( <http://purl.imsglobal.org/actions/Archived>
                                                                                                   <http://purl.imsglobal.org/actions/Copied>
                                                                                                   <http://purl.imsglobal.org/actions/Published>
                                                                                                   <http://purl.imsglobal.org/actions/Restored>
                                                                                                   <http://purl.imsglobal.org/actions/Unpublished>
                                                                                                   <http://purl.imsglobal.org/caliper/actions/Created>
                                                                                                   <http://purl.imsglobal.org/caliper/actions/Deleted>
                                                                                                   <http://purl.imsglobal.org/caliper/actions/Described>
                                                                                                   <http://purl.imsglobal.org/caliper/actions/Modified>
                                                                                                   <http://purl.imsglobal.org/caliper/actions/Retrieved>
                                                                                                 )
                                                                                     ]
                                                                ]
                                                              ) ;
                                           rdf:type owl:Class
                                         ] ,
                                         [ owl:intersectionOf ( [ rdf:type owl:Restriction ;
                                                                  owl:onProperty :actor ;
                                                                  owl:someValuesFrom :Agent
                                                                ]
                                                                [ rdf:type owl:Restriction ;
                                                                  owl:onProperty :actor ;
                                                                  owl:allValuesFrom :Person
                                                                ]
                                                              ) ;
                                           rdf:type owl:Class
                                         ] ,
                                         [ owl:intersectionOf ( [ rdf:type owl:Restriction ;
                                                                  owl:onProperty :object ;
                                                                  owl:someValuesFrom :Entity
                                                                ]
                                                                [ rdf:type owl:Restriction ;
                                                                  owl:onProperty :object ;
                                                                  owl:allValuesFrom :DigitalResource
                                                                ]
                                                              ) ;
                                           rdf:type owl:Class
                                         ] ,
                                         [ rdf:type owl:Restriction ;
                                           owl:onProperty :generated ;
                                           owl:someValuesFrom :Entity
                                         ] ;
                         rdfs:comment "A Caliper ResourceManagementEvent models a Person managing an Entity."@en ;
                         rdfs:isDefinedBy "http://purl.imsglobal.org/caliper"^^xsd:string ;
                         rdfs:label "ResourceManagementEvent"@en .


###  http://purl.imsglobal.org/caliper/Response
:Response rdf:type owl:Class ;
          rdfs:subClassOf :Entity ;
          rdfs:comment "A Caliper Response is a generic type that represents the selected option generated by a Person interacting with an AssessmentItem.  Utilize Response only if no suitable subtype exists to represent the response being described."@en ;
          rdfs:isDefinedBy "http://purl.imsglobal.org/caliper"^^xsd:string ;
          rdfs:label "Response"@en .


###  http://purl.imsglobal.org/caliper/Result
:Result rdf:type owl:Class ;
        rdfs:subClassOf :Entity ;
        rdfs:comment "A Caliper Result represents a grade applied to an assignment submission."@en ;
        rdfs:isDefinedBy "http://purl.imsglobal.org/caliper"^^xsd:string ;
        rdfs:label "Result"@en .


###  http://purl.imsglobal.org/caliper/Role
:Role rdf:type owl:Class ;
      rdfs:comment "A member can have multiple roles in a Membership.  These different roles would be reflected in separate instances of the Role."@en ;
      rdfs:isDefinedBy "http://www.imsglobal.org/lis/"^^xsd:string ;
      rdfs:label "Role"@en .


###  http://purl.imsglobal.org/caliper/Scale
:Scale rdf:type owl:Class ;
       rdfs:subClassOf :Entity ;
       rdfs:comment "A Caliper Scale models a scale employed in order to capture some rating."@en ;
       rdfs:isDefinedBy "https://purl.imsglobal.org/caliper"@en ;
       rdfs:label "Scale"@en .


###  http://purl.imsglobal.org/caliper/Score
:Score rdf:type owl:Class ;
       rdfs:subClassOf :Entity ;
       rdfs:comment "A Caliper Score represents a grade.  The Score value is considered immutable."@en ;
       rdfs:isDefinedBy "http://purl.imsglobal.org/caliper"^^xsd:string ;
       rdfs:label "Score"@en .


###  http://purl.imsglobal.org/caliper/SearchEvent
:SearchEvent rdf:type owl:Class ;
             rdfs:subClassOf :Event ,
                             [ owl:intersectionOf ( [ rdf:type owl:Restriction ;
                                                      owl:onProperty :action ;
                                                      owl:someValuesFrom :Action
                                                    ]
                                                    [ rdf:type owl:Restriction ;
                                                      owl:onProperty :action ;
                                                      owl:hasValue <http://purl.imsglobal.org/caliper/actions/Searched>
                                                    ]
                                                  ) ;
                               rdf:type owl:Class
                             ] ,
                             [ owl:intersectionOf ( [ rdf:type owl:Restriction ;
                                                      owl:onProperty :actor ;
                                                      owl:someValuesFrom :Agent
                                                    ]
                                                    [ rdf:type owl:Restriction ;
                                                      owl:onProperty :actor ;
                                                      owl:allValuesFrom :Person
                                                    ]
                                                  ) ;
                               rdf:type owl:Class
                             ] ,
                             [ rdf:type owl:Restriction ;
                               owl:onProperty :generated ;
                               owl:someValuesFrom :SearchResponse
                             ] ;
             rdfs:comment "A Caliper SearchEvent models a Person querying a resource for information, typically a DigitalResource or SoftwareApplication. A SearchResponse may be referenced using the generated property."@en ;
             rdfs:isDefinedBy "http://purl.imsglobal.org/caliper"^^xsd:string ;
             rdfs:label "SearchEvent"@en .


###  http://purl.imsglobal.org/caliper/SearchResponse
:SearchResponse rdf:type owl:Class ;
                rdfs:subClassOf :Entity ;
                rdfs:comment "A Caliper SearchResponse models a search engine response to an actor querying a searchable resource."@en ;
                rdfs:isDefinedBy "http://purl.imsglobal.org/caliper"@en ;
                rdfs:label "SearchResponse"@en .


###  http://purl.imsglobal.org/caliper/SelectTextResponse
:SelectTextResponse rdf:type owl:Class ;
                    rdfs:subClassOf :Response ;
                    rdfs:comment "A Caliper SelectTextResponse represents a type of Response that identifies text or a mapping from a presented paragraph or list."@en ;
                    rdfs:isDefinedBy "http://purl.imsglobal.org/caliper"^^xsd:string ;
                    rdfs:label "SelectTextResponse"@en .


###  http://purl.imsglobal.org/caliper/Selector
:Selector rdf:type owl:Class ;
          rdfs:comment "A Caliper Selector is a generic class that describes a fragment or segment of a resource.  Utilize Selector only if no suitable subtype exists to represent the selection being described."@en ;
          rdfs:isDefinedBy "http://purl.imsglobal.org/caliper"^^xsd:string ;
          rdfs:label "Selector"@en .


###  http://purl.imsglobal.org/caliper/Session
:Session rdf:type owl:Class ;
         rdfs:subClassOf :Entity ,
                         [ owl:intersectionOf ( [ rdf:type owl:Restriction ;
                                                  owl:onProperty :user ;
                                                  owl:someValuesFrom :Agent
                                                ]
                                                [ rdf:type owl:Restriction ;
                                                  owl:onProperty :user ;
                                                  owl:allValuesFrom :Person
                                                ]
                                              ) ;
                           rdf:type owl:Class
                         ] ;
         rdfs:comment "A Caliper Session represents a web application user session."@en ;
         rdfs:isDefinedBy "http://purl.imsglobal.org/caliper"^^xsd:string ;
         rdfs:label "Session"@en .


###  http://purl.imsglobal.org/caliper/SessionEvent
:SessionEvent rdf:type owl:Class ;
              rdfs:subClassOf :Event ,
                              [ owl:intersectionOf ( [ rdf:type owl:Restriction ;
                                                       owl:onProperty :action ;
                                                       owl:someValuesFrom :Action
                                                     ]
                                                     [ rdf:type owl:Restriction ;
                                                       owl:onProperty :action ;
                                                       owl:someValuesFrom [ rdf:type owl:Class ;
                                                                            owl:oneOf ( <http://purl.imsglobal.org/caliper/actions/LoggedIn>
                                                                                        <http://purl.imsglobal.org/caliper/actions/LoggedOut>
                                                                                        <http://purl.imsglobal.org/caliper/actions/TimedOut>
                                                                                      )
                                                                          ]
                                                     ]
                                                   ) ;
                                rdf:type owl:Class
                              ] ,
                              [ owl:intersectionOf ( [ rdf:type owl:Restriction ;
                                                       owl:onProperty :actor ;
                                                       owl:someValuesFrom :Agent
                                                     ]
                                                     [ rdf:type owl:Restriction ;
                                                       owl:onProperty :actor ;
                                                       owl:allValuesFrom [ rdf:type owl:Class ;
                                                                           owl:unionOf ( :Person
                                                                                         :SoftwareApplication
                                                                                       )
                                                                         ]
                                                     ]
                                                   ) ;
                                rdf:type owl:Class
                              ] ,
                              [ owl:intersectionOf ( [ rdf:type owl:Restriction ;
                                                       owl:onProperty :object ;
                                                       owl:someValuesFrom :Entity
                                                     ]
                                                     [ rdf:type owl:Restriction ;
                                                       owl:onProperty :object ;
                                                       owl:allValuesFrom [ rdf:type owl:Class ;
                                                                           owl:unionOf ( :Session
                                                                                         :SoftwareApplication
                                                                                       )
                                                                         ]
                                                     ]
                                                   ) ;
                                rdf:type owl:Class
                              ] ,
                              [ owl:intersectionOf ( [ rdf:type owl:Restriction ;
                                                       owl:onProperty :referrer ;
                                                       owl:someValuesFrom :Entity
                                                     ]
                                                     [ rdf:type owl:Restriction ;
                                                       owl:onProperty :referrer ;
                                                       owl:allValuesFrom [ rdf:type owl:Class ;
                                                                           owl:unionOf ( :DigitalResource
                                                                                         :SoftwareApplication
                                                                                       )
                                                                         ]
                                                     ]
                                                   ) ;
                                rdf:type owl:Class
                              ] ,
                              [ rdf:type owl:Restriction ;
                                owl:onProperty :target ;
                                owl:someValuesFrom :DigitalResource
                              ] ;
              rdfs:comment "A Caliper SessionEvent models the creation and subsequent termination of a user session established by a Person interacting with a SoftwareApplication."@en ;
              rdfs:isDefinedBy "http://purl.imsglobal.org/caliper"^^xsd:string ;
              rdfs:label "SessionEvent"@en .


###  http://purl.imsglobal.org/caliper/SharedAnnotation
:SharedAnnotation rdf:type owl:Class ;
                  rdfs:subClassOf :Annotation ;
                  rdfs:comment "A Caliper SharedAnnotation represents the act of sharing a reference to a DigitalResource with other agents."@en ;
                  rdfs:isDefinedBy "http://purl.imsglobal.org/caliper"^^xsd:string ;
                  rdfs:label "SharedAnnotation"@en .


###  http://purl.imsglobal.org/caliper/SoftwareApplication
:SoftwareApplication rdf:type owl:Class ;
                     rdfs:subClassOf :Agent ;
                     rdfs:comment "A Caliper SoftwareApplication represents a computer program, application, module, platform or system."@en ;
                     rdfs:isDefinedBy "http://purl.imsglobal.org/caliper"^^xsd:string ;
                     rdfs:label "SoftwareApplication"@en .


###  http://purl.imsglobal.org/caliper/Status
:Status rdf:type owl:Class ;
        rdfs:comment "Indicates if a member is active or inactive in the collection. This allows the source system to specifically tell the target system that a member is now active or inactive.  Another view is that the absence of a Membership object when membership data is passed implies inactivity and the existence of an object implies active membership.  This will logically work for a ‘snap-shot’ interface where all members are passed every time objects are sent from one system to another but it will not support an interface where individual Membership objects are passed."@en ;
        rdfs:isDefinedBy "http://www.imsglobal.org/lis/"^^xsd:string ;
        rdfs:label "Status"@en .


###  http://purl.imsglobal.org/caliper/TagAnnotation
:TagAnnotation rdf:type owl:Class ;
               rdfs:subClassOf :Annotation ;
               rdfs:comment "A Caliper TagAnnotation represents the act of tagging a DigitalResource with tags or labels."@en ;
               rdfs:isDefinedBy "http://purl.imsglobal.org/caliper"^^xsd:string ;
               rdfs:label "TagAnnotation"@en .


###  http://purl.imsglobal.org/caliper/TextPositionSelector
:TextPositionSelector rdf:type owl:Class ;
                      rdfs:subClassOf :Selector ;
                      rdfs:comment "A Caliper TextPositionSelector represents a fragment or selection of textual content, the starting and ending positions of which are determined by the distance in characters from the initial character (position 0) of the enclosing full text."@en ;
                      rdfs:isDefinedBy "http://purl.imsglobal.org/caliper"^^xsd:string ;
                      rdfs:label "TextPositionSelector"@en .


###  http://purl.imsglobal.org/caliper/Thread
:Thread rdf:type owl:Class ;
        rdfs:subClassOf :DigitalResourceCollection ,
                        [ owl:intersectionOf ( [ rdf:type owl:Restriction ;
                                                 owl:onProperty :isPartOf ;
                                                 owl:someValuesFrom :Entity
                                               ]
                                               [ rdf:type owl:Restriction ;
                                                 owl:onProperty :isPartOf ;
                                                 owl:allValuesFrom :Forum
                                               ]
                                             ) ;
                          rdf:type owl:Class
                        ] ,
                        [ owl:intersectionOf ( [ rdf:type owl:Restriction ;
                                                 owl:onProperty :items ;
                                                 owl:someValuesFrom :Entity
                                               ]
                                               [ rdf:type owl:Restriction ;
                                                 owl:onProperty :items ;
                                                 owl:allValuesFrom :Message
                                               ]
                                             ) ;
                          rdf:type owl:Class
                        ] ;
        rdfs:comment "A Caliper Thread represents a series of one or more messages that share a common subject and are connected by a reply or by date relationships."@en ;
        rdfs:isDefinedBy "http://purl.imsglobal.org/caliper"^^xsd:string ;
        rdfs:label "Thread"@en .


###  http://purl.imsglobal.org/caliper/ThreadEvent
:ThreadEvent rdf:type owl:Class ;
             rdfs:subClassOf :Event ,
                             [ owl:intersectionOf ( [ rdf:type owl:Restriction ;
                                                      owl:onProperty :action ;
                                                      owl:someValuesFrom :Action
                                                    ]
                                                    [ rdf:type owl:Restriction ;
                                                      owl:onProperty :action ;
                                                      owl:someValuesFrom [ rdf:type owl:Class ;
                                                                           owl:oneOf ( <http://purl.imsglobal.org/caliper/actions/MarkedAsRead>
                                                                                       <http://purl.imsglobal.org/caliper/actions/MarkedAsUnread>
                                                                                     )
                                                                         ]
                                                    ]
                                                  ) ;
                               rdf:type owl:Class
                             ] ,
                             [ owl:intersectionOf ( [ rdf:type owl:Restriction ;
                                                      owl:onProperty :actor ;
                                                      owl:someValuesFrom :Agent
                                                    ]
                                                    [ rdf:type owl:Restriction ;
                                                      owl:onProperty :actor ;
                                                      owl:allValuesFrom :Person
                                                    ]
                                                  ) ;
                               rdf:type owl:Class
                             ] ,
                             [ owl:intersectionOf ( [ rdf:type owl:Restriction ;
                                                      owl:onProperty :object ;
                                                      owl:someValuesFrom :DigitalResource
                                                    ]
                                                    [ rdf:type owl:Restriction ;
                                                      owl:onProperty :object ;
                                                      owl:allValuesFrom :Thread
                                                    ]
                                                  ) ;
                               rdf:type owl:Class
                             ] ;
             rdfs:comment "A Caliper ThreadEvent models an actor interacting with a Forum thread or topic."@en ;
             rdfs:isDefinedBy "http://purl.imsglobal.org/caliper"^^xsd:string ;
             rdfs:label "ThreadEvent"@en .


###  http://purl.imsglobal.org/caliper/ToolLaunchEvent
:ToolLaunchEvent rdf:type owl:Class ;
                 rdfs:subClassOf :Event ,
                                 [ owl:intersectionOf ( [ rdf:type owl:Restriction ;
                                                          owl:onProperty :action ;
                                                          owl:someValuesFrom :Action
                                                        ]
                                                        [ rdf:type owl:Restriction ;
                                                          owl:onProperty :action ;
                                                          owl:someValuesFrom [ rdf:type owl:Class ;
                                                                               owl:oneOf ( <http://purl.imsglobal.org/actions/Launched>
                                                                                           <http://purl.imsglobal.org/actions/Returned>
                                                                                         )
                                                                             ]
                                                        ]
                                                      ) ;
                                   rdf:type owl:Class
                                 ] ,
                                 [ owl:intersectionOf ( [ rdf:type owl:Restriction ;
                                                          owl:onProperty :actor ;
                                                          owl:someValuesFrom :Agent
                                                        ]
                                                        [ rdf:type owl:Restriction ;
                                                          owl:onProperty :actor ;
                                                          owl:allValuesFrom :Person
                                                        ]
                                                      ) ;
                                   rdf:type owl:Class
                                 ] ,
                                 [ owl:intersectionOf ( [ rdf:type owl:Restriction ;
                                                          owl:onProperty :object ;
                                                          owl:someValuesFrom :Agent
                                                        ]
                                                        [ rdf:type owl:Restriction ;
                                                          owl:onProperty :object ;
                                                          owl:allValuesFrom :SoftwareApplication
                                                        ]
                                                      ) ;
                                   rdf:type owl:Class
                                 ] ,
                                 [ owl:intersectionOf ( [ rdf:type owl:Restriction ;
                                                          owl:onProperty :target ;
                                                          owl:someValuesFrom :Entity
                                                        ]
                                                        [ rdf:type owl:Restriction ;
                                                          owl:onProperty :target ;
                                                          owl:allValuesFrom [ rdf:type owl:Class ;
                                                                              owl:unionOf ( :Link
                                                                                            :LtiLink
                                                                                          )
                                                                            ]
                                                        ]
                                                      ) ;
                                   rdf:type owl:Class
                                 ] ,
                                 [ rdf:type owl:Restriction ;
                                   owl:onProperty :generated ;
                                   owl:someValuesFrom :DigitalResource
                                 ] ,
                                 [ rdf:type owl:Restriction ;
                                   owl:onProperty :federatedSession ;
                                   owl:allValuesFrom :LtiSession
                                 ] ;
                 rdfs:comment "The ToolLaunchEvent models an interaction between a Person and a SoftwareApplication), at a given time and in a given context at a given time and in a given context."@en ;
                 rdfs:isDefinedBy "http://purl.imsglobal.org/caliper"@en ;
                 rdfs:label "ToolLaunchEvent"@en .


###  http://purl.imsglobal.org/caliper/ToolUseEvent
:ToolUseEvent rdf:type owl:Class ;
              rdfs:subClassOf :Event ,
                              [ owl:intersectionOf ( [ rdf:type owl:Restriction ;
                                                       owl:onProperty :action ;
                                                       owl:someValuesFrom :Action
                                                     ]
                                                     [ rdf:type owl:Restriction ;
                                                       owl:onProperty :action ;
                                                       owl:hasValue <http://purl.imsglobal.org/caliper/actions/Used>
                                                     ]
                                                   ) ;
                                rdf:type owl:Class
                              ] ,
                              [ owl:intersectionOf ( [ rdf:type owl:Restriction ;
                                                       owl:onProperty :actor ;
                                                       owl:someValuesFrom :Agent
                                                     ]
                                                     [ rdf:type owl:Restriction ;
                                                       owl:onProperty :actor ;
                                                       owl:allValuesFrom :Person
                                                     ]
                                                   ) ;
                                rdf:type owl:Class
                              ] ,
                              [ owl:intersectionOf ( [ rdf:type owl:Restriction ;
                                                       owl:onProperty :object ;
                                                       owl:someValuesFrom :Agent
                                                     ]
                                                     [ rdf:type owl:Restriction ;
                                                       owl:onProperty :object ;
                                                       owl:allValuesFrom :SoftwareApplication
                                                     ]
                                                   ) ;
                                rdf:type owl:Class
                              ] ,
                              [ rdf:type owl:Restriction ;
                                owl:onProperty :target ;
                                owl:someValuesFrom :SoftwareApplication
                              ] ;
              rdfs:comment "A Caliper ToolUseEvent models a Person using a learning tool in a way that the tool's creators have determined is an indication of a learning interaction."@en ;
              rdfs:isDefinedBy "http://purl.imsglobal.org/caliper"^^xsd:string ;
              rdfs:label "ToolUseEvent"@en .


###  http://purl.imsglobal.org/caliper/TrueFalseResponse
:TrueFalseResponse rdf:type owl:Class ;
                   rdfs:subClassOf :Response ;
                   rdfs:comment "A Caliper TrueFalseResponse represents a type of Response to an AssessmentItem in which only two possible options are provided (e.g., true/false, yes/no)."@en ;
                   rdfs:isDefinedBy "http://purl.imsglobal.org/caliper"^^xsd:string ;
                   rdfs:label "TrueFalseResponse"@en .


###  http://purl.imsglobal.org/caliper/VideoObject
:VideoObject rdf:type owl:Class ;
             rdfs:subClassOf :MediaObject ;
             rdfs:comment "A Caliper VideoObject represents a visual recording stored in digital form."@en ;
             rdfs:isDefinedBy "http://purl.imsglobal.org/caliper"^^xsd:string ;
             rdfs:label "VideoObject"@en .


###  http://purl.imsglobal.org/caliper/ViewEvent
:ViewEvent rdf:type owl:Class ;
           rdfs:subClassOf :Event ,
                           [ owl:intersectionOf ( [ rdf:type owl:Restriction ;
                                                    owl:onProperty :action ;
                                                    owl:someValuesFrom :Action
                                                  ]
                                                  [ rdf:type owl:Restriction ;
                                                    owl:onProperty :action ;
                                                    owl:hasValue <http://purl.imsglobal.org/caliper/actions/Viewed>
                                                  ]
                                                ) ;
                             rdf:type owl:Class
                           ] ,
                           [ owl:intersectionOf ( [ rdf:type owl:Restriction ;
                                                    owl:onProperty :actor ;
                                                    owl:someValuesFrom :Agent
                                                  ]
                                                  [ rdf:type owl:Restriction ;
                                                    owl:onProperty :actor ;
                                                    owl:allValuesFrom :Person
                                                  ]
                                                ) ;
                             rdf:type owl:Class
                           ] ,
                           [ owl:intersectionOf ( [ rdf:type owl:Restriction ;
                                                    owl:onProperty :object ;
                                                    owl:someValuesFrom :Entity
                                                  ]
                                                  [ rdf:type owl:Restriction ;
                                                    owl:onProperty :object ;
                                                    owl:allValuesFrom :DigitalResource
                                                  ]
                                                ) ;
                             rdf:type owl:Class
                           ] ,
                           [ rdf:type owl:Restriction ;
                             owl:onProperty :target ;
                             owl:someValuesFrom :Frame
                           ] ;
           rdfs:comment "A Caliper ViewEvent describes an actor's examination of digital content whenever the activity emphasizes thoughtful observation or study as opposed to the mere retrieval of a resource."@en ;
           rdfs:isDefinedBy "http://purl.imsglobal.org/caliper"^^xsd:string ;
           rdfs:label "ViewEvent"@en .


###  http://purl.imsglobal.org/caliper/WebPage
:WebPage rdf:type owl:Class ;
         rdfs:subClassOf :DigitalResource ;
         rdfs:comment "A Caliper WebPage represents a document containing markup that is suitable for display in a web browser."@en ;
         rdfs:isDefinedBy "http://purl.imsglobal.org/caliper"^^xsd:string ;
         rdfs:label "WebPage"@en .


###  http://purl.imsglobal.org/caliper/epubChapter
:epubChapter rdf:type owl:Class ;
             rdfs:subClassOf :DigitalResource ;
             <http://purl.org/dc/terms/isReplacedBy> :Chapter ;
             rdfs:comment "A Caliper EpubChapter represents a major structural division of a piece of writing. EpubChapter is a DEPRECATED entity that will be removed in a future version of the specification. It SHOULD NOT be referenced."@en ;
             rdfs:isDefinedBy "http://purl.imsglobal.org/caliper"^^xsd:string ;
             rdfs:label "EpubChapter"@en ;
             owl:deprecated "true"^^xsd:boolean .


###  http://purl.imsglobal.org/caliper/epubPart
:epubPart rdf:type owl:Class ;
          rdfs:subClassOf :DigitalResource ;
          rdfs:comment "A Caliper EpubPart represents a major structural division of a piece of writing, typically encapsulating a set of related chapters. EpubPart is a DEPRECATED entity that will be removed in a future version of the specification. It SHOULD NOT be referenced."@en ;
          rdfs:isDefinedBy "http://purl.imsglobal.org/caliper"^^xsd:string ;
          rdfs:label "EpubPart"@en ;
          owl:deprecated "true"^^xsd:boolean .


###  http://purl.imsglobal.org/caliper/epubSubChapter
:epubSubChapter rdf:type owl:Class ;
                rdfs:subClassOf :DigitalResource ,
                                [ owl:intersectionOf ( [ rdf:type owl:Restriction ;
                                                         owl:onProperty :isPartOf ;
                                                         owl:someValuesFrom :Entity
                                                       ]
                                                       [ rdf:type owl:Restriction ;
                                                         owl:onProperty :isPartOf ;
                                                         owl:allValuesFrom :epubChapter
                                                       ]
                                                     ) ;
                                  rdf:type owl:Class
                                ] ;
                rdfs:comment "A Caliper EpubSubChapter represents a major sub-division of an EpubChapter. EpubSubChapter is a DEPRECATED entity that will be removed in a future version of the specification. It SHOULD NOT be referenced."^^xsd:string ;
                rdfs:isDefinedBy "http://purl.imsglobal.org/caliper"^^xsd:string ;
                rdfs:label "EpubSubChapter"@en ;
                owl:deprecated "true"^^xsd:boolean .


###  http://purl.imsglobal.org/caliper/epubVolume
:epubVolume rdf:type owl:Class ;
            rdfs:subClassOf :DigitalResource ;
            <http://purl.org/dc/terms/isReplacedBy> :Document ;
            rdfs:comment "A Caliper EpubVolume represents a component of a collection. EpubVolume inherits all the properties and requirements defined for DigitalResource, its supertype. EpubVolume is a DEPRECATED entity that will be removed in a future version of the specification. It SHOULD NOT be referenced."@en ;
            rdfs:isDefinedBy "http://purl.imsglobal.org/caliper"^^xsd:string ;
            rdfs:label "EpubVolume"@en ;
            owl:deprecated "true"^^xsd:boolean .


###  http://purl.imsglobal.org/vocab/lis/v2/membership#Administrator
<http://purl.imsglobal.org/vocab/lis/v2/membership#Administrator> rdf:type owl:Class ;
                                                                  rdfs:subClassOf :Role ;
                                                                  rdfs:comment "The role of a formal administrator in the Membership."@en ;
                                                                  rdfs:isDefinedBy "http://www.imsglobal.org/lis/"^^xsd:string ;
                                                                  rdfs:label "Administrator"@en .


###  http://purl.imsglobal.org/vocab/lis/v2/membership#ContentDeveloper
<http://purl.imsglobal.org/vocab/lis/v2/membership#ContentDeveloper> rdf:type owl:Class ;
                                                                     rdfs:subClassOf :Role ;
                                                                     rdfs:comment "The role of an author of content for learning material presented through the Membership."@en ;
                                                                     rdfs:isDefinedBy "http://www.imsglobal.org/lis/"^^xsd:string ;
                                                                     rdfs:label "ContentDeveloper"@en .


###  http://purl.imsglobal.org/vocab/lis/v2/membership#Instructor
<http://purl.imsglobal.org/vocab/lis/v2/membership#Instructor> rdf:type owl:Class ;
                                                               rdfs:subClassOf :Role ;
                                                               rdfs:comment "The role of teaching instructor for learning material presented through the Membership."@en ;
                                                               rdfs:isDefinedBy "http://www.imsglobal.org/lis/"^^xsd:string ;
                                                               rdfs:label "Instructor"@en .


###  http://purl.imsglobal.org/vocab/lis/v2/membership#Learner
<http://purl.imsglobal.org/vocab/lis/v2/membership#Learner> rdf:type owl:Class ;
                                                            rdfs:subClassOf :Role ;
                                                            rdfs:comment "The role of someone undergoing some form of formal learning."@en ;
                                                            rdfs:isDefinedBy "http://www.imsglobal.org/lis/"^^xsd:string ;
                                                            rdfs:label "Learner"@en .


###  http://purl.imsglobal.org/vocab/lis/v2/membership#Manager
<http://purl.imsglobal.org/vocab/lis/v2/membership#Manager> rdf:type owl:Class ;
                                                            rdfs:subClassOf :Role ;
                                                            rdfs:comment "The role of manager of the Group for which the Membership is being defined."@en ;
                                                            rdfs:isDefinedBy "http://www.imsglobal.org/lis/"^^xsd:string ;
                                                            rdfs:label "Manager"@en .


###  http://purl.imsglobal.org/vocab/lis/v2/membership#Member
<http://purl.imsglobal.org/vocab/lis/v2/membership#Member> rdf:type owl:Class ;
                                                           rdfs:subClassOf :Role ;
                                                           rdfs:comment "The role of a member of the associated Membership."@en ;
                                                           rdfs:isDefinedBy "http://www.imsglobal.org/lis/"^^xsd:string ;
                                                           rdfs:label "Member"@en .


###  http://purl.imsglobal.org/vocab/lis/v2/membership#Mentor
<http://purl.imsglobal.org/vocab/lis/v2/membership#Mentor> rdf:type owl:Class ;
                                                           rdfs:subClassOf :Role ;
                                                           rdfs:comment "The role of a personal mentor of other individuals in the Membership."@en ;
                                                           rdfs:isDefinedBy "http://www.imsglobal.org/lis/"^^xsd:string ;
                                                           rdfs:label "Mentor"@en .


###  http://purl.imsglobal.org/vocab/lis/v2/membership#Officer
<http://purl.imsglobal.org/vocab/lis/v2/membership#Officer> rdf:type owl:Class ;
                                                            rdfs:subClassOf :Role ;
                                                            rdfs:comment "The role of an officer of organization e.g., Chair, Secretary, etc. in the Membership."@en ;
                                                            rdfs:isDefinedBy "http://www.imsglobal.org/lis/"^^xsd:string ;
                                                            rdfs:label "Officer"@en .


###  http://purl.imsglobal.org/vocab/lis/v2/membership#TeachingAssistant
<http://purl.imsglobal.org/vocab/lis/v2/membership#TeachingAssistant> rdf:type owl:Class ;
                                                                      rdfs:subClassOf :Role ;
                                                                      rdfs:comment "The role of teaching assistant to an Instructor in the Membership."@en ;
                                                                      rdfs:isDefinedBy "http://www.imsglobal.org/lis/"^^xsd:string ;
                                                                      rdfs:label "TeachingAssistant"@en .


#################################################################
#    Individuals
#################################################################

###  http://purl.imsglobal.org/actions/Archived
<http://purl.imsglobal.org/actions/Archived> rdf:type owl:NamedIndividual ,
                                                      :Action ;
                                             rdfs:comment "Put into an archive. The Archived action signals that a resource has been put into long-term storage. Inverse of Restored."@en ;
                                             rdfs:isDefinedBy "http://wordnet-rdf.princeton.edu/wn31/201387292-v"^^xsd:string ;
                                             rdfs:label "Archived"@en .


###  http://purl.imsglobal.org/actions/Copied
<http://purl.imsglobal.org/actions/Copied> rdf:type owl:NamedIndividual ;
                                           rdfs:comment "Make a replica of."@en ;
                                           rdfs:isDefinedBy "http://wordnet-rdf.princeton.edu/wn31/201697776-v"^^xsd:string ;
                                           rdfs:label "Copied"@en .


###  http://purl.imsglobal.org/actions/Launched
<http://purl.imsglobal.org/actions/Launched> rdf:type owl:NamedIndividual ,
                                                      :Action ;
                                             rdfs:comment "Get going; give impetus to."@en ;
                                             rdfs:isDefinedBy "href=\"http://wordnet-rdf.princeton.edu/wn31/01515196-v"^^xsd:string ;
                                             rdfs:label "Launched"@en .


###  http://purl.imsglobal.org/actions/Published
<http://purl.imsglobal.org/actions/Published> rdf:type owl:NamedIndividual ;
                                              rdfs:comment "Prepare and issue for public distribution or sale. Inverse of Unpublished."@en ;
                                              rdfs:isDefinedBy "http://wordnet-rdf.princeton.edu/wn31/200969657-v"^^xsd:string ;
                                              rdfs:label "Published"@en .


###  http://purl.imsglobal.org/actions/Restored
<http://purl.imsglobal.org/actions/Restored> rdf:type owl:NamedIndividual ;
                                             rdfs:comment "Return to its original or usable and functioning condition. Inverse of Archived."@en ;
                                             rdfs:isDefinedBy "http://wordnet-rdf.princeton.edu/wn31/202558146-v"^^xsd:string ;
                                             rdfs:label "Restored"@en .


###  http://purl.imsglobal.org/actions/Returned
<http://purl.imsglobal.org/actions/Returned> rdf:type owl:NamedIndividual ,
                                                      :Action ;
                                             rdfs:comment "Go or come back to place, condition, or activity where one has been before."@en ;
                                             rdfs:isDefinedBy "http://wordnet-rdf.princeton.edu/wn31/01515196-v"^^xsd:string ;
                                             rdfs:label "Returned"@en .


###  http://purl.imsglobal.org/actions/Unpublished
<http://purl.imsglobal.org/actions/Unpublished> rdf:type owl:NamedIndividual ;
                                                rdfs:comment "Remove from public distribution or sale. Inverse of Published."@en ;
                                                rdfs:isDefinedBy "http://wordnet-rdf.princeton.edu/wn31/200969657-v"^^xsd:string ;
                                                rdfs:label "Unpublished"@en .


###  http://purl.imsglobal.org/caliper/actions/Abandoned
<http://purl.imsglobal.org/caliper/actions/Abandoned> rdf:type owl:NamedIndividual ,
                                                               :Action ;
                                                      rdfs:comment "Forsake, leave behind."@en ;
                                                      rdfs:isDefinedBy "http://wordnet-rdf.princeton.edu/wn31/202232813-v"^^xsd:string ;
                                                      rdfs:label "Abandoned"@en .


###  http://purl.imsglobal.org/caliper/actions/Activated
<http://purl.imsglobal.org/caliper/actions/Activated> rdf:type owl:NamedIndividual ,
                                                               :Action ;
                                                      rdfs:comment "Make active or more active. Inverse of Deactivated."@en ;
                                                      rdfs:isDefinedBy "http://wordnet-rdf.princeton.edu/wn31/200191014-v"^^xsd:string ;
                                                      rdfs:label "Activated"@en .


###  http://purl.imsglobal.org/caliper/actions/Added
<http://purl.imsglobal.org/caliper/actions/Added> rdf:type owl:NamedIndividual ,
                                                           :Action ;
                                                  rdfs:comment "Make an addition (to); join or combine or unite with others; increase the quality, quantity, size or scope of. Inverse of Removed."@en ;
                                                  rdfs:isDefinedBy "http://wordnet-rdf.princeton.edu/wn31/200182551-v"^^xsd:string ;
                                                  rdfs:label "Added"@en .


###  http://purl.imsglobal.org/caliper/actions/Attached
<http://purl.imsglobal.org/caliper/actions/Attached> rdf:type owl:NamedIndividual ,
                                                              :Action ;
                                                     rdfs:comment "Cause to be attached."@en ;
                                                     rdfs:isDefinedBy "http://wordnet-rdf.princeton.edu/wn31/201299048-v"^^xsd:string ;
                                                     rdfs:label "Attached"@en .


###  http://purl.imsglobal.org/caliper/actions/Bookmarked
<http://purl.imsglobal.org/caliper/actions/Bookmarked> rdf:type owl:NamedIndividual ,
                                                                :Action ;
                                                       rdfs:comment "A marker that specifies a location of interest in a DigitalResource that is recorded for later retrieval."@en ;
                                                       rdfs:isDefinedBy "http://purl.imsglobal.org/caliper"^^xsd:string ;
                                                       rdfs:label "Bookmarked"@en ;
                                                       rdfs:seeAlso "http://wordnet-rdf.princeton.edu/wn31/102874508-n"^^xsd:string .


###  http://purl.imsglobal.org/caliper/actions/ChangedResolution
<http://purl.imsglobal.org/caliper/actions/ChangedResolution> rdf:type owl:NamedIndividual ,
                                                                       :Action ;
                                                              rdfs:comment "Cause to change; make different; cause a transformation of the number of pixels per square inch on a computer-generated display."@en ;
                                                              rdfs:isDefinedBy "http://wordnet-rdf.princeton.edu/wn31/200126072-v"^^xsd:string ;
                                                              rdfs:label "ChangedResolution"@en ;
                                                              rdfs:seeAlso "http://wordnet-rdf.princeton.edu/wn31/111526370-n"^^xsd:string .


###  http://purl.imsglobal.org/caliper/actions/ChangedSize
<http://purl.imsglobal.org/caliper/actions/ChangedSize> rdf:type owl:NamedIndividual ,
                                                                 :Action ;
                                                        rdfs:comment "Cause to change; make different; cause a transformation of the physical magnitude of something."@en ;
                                                        rdfs:isDefinedBy "http://wordnet-rdf.princeton.edu/wn31/200126072-v"^^xsd:string ;
                                                        rdfs:label "ChangedSize"@en ;
                                                        rdfs:seeAlso "http://wordnet-rdf.princeton.edu/wn31/105106204-n"^^xsd:string .


###  http://purl.imsglobal.org/caliper/actions/ChangedSpeed
<http://purl.imsglobal.org/caliper/actions/ChangedSpeed> rdf:type owl:NamedIndividual ,
                                                                  :Action ;
                                                         rdfs:comment "Cause to change; make different; cause a transformation of the rate at which something happens."@en ;
                                                         rdfs:isDefinedBy "http://wordnet-rdf.princeton.edu/wn31/200126072-v"^^xsd:string ;
                                                         rdfs:label "ChangedSpeed"@en ;
                                                         rdfs:seeAlso "http://wordnet-rdf.princeton.edu/wn31/105065291-n"^^xsd:string .


###  http://purl.imsglobal.org/caliper/actions/ChangedVolume
<http://purl.imsglobal.org/caliper/actions/ChangedVolume> rdf:type owl:NamedIndividual ,
                                                                   :Action ;
                                                          rdfs:comment "Cause to change; make different; cause a transformation of the magnitude of sound (usually in a specified direction)."@en ;
                                                          rdfs:isDefinedBy "http://wordnet-rdf.princeton.edu/wn31/200126072-v"^^xsd:string ;
                                                          rdfs:label "ChangedVolume"@en ;
                                                          rdfs:seeAlso "http://wordnet-rdf.princeton.edu/wn31/104997456-n"^^xsd:string .


###  http://purl.imsglobal.org/caliper/actions/Classified
<http://purl.imsglobal.org/caliper/actions/Classified> rdf:type owl:NamedIndividual ,
                                                                :Action ;
                                                       rdfs:comment "Assign to a class or kind."@en ;
                                                       rdfs:isDefinedBy "http://wordnet-rdf.princeton.edu/wn31/200741667-v"^^xsd:string ;
                                                       rdfs:label "Classified"@en .


###  http://purl.imsglobal.org/caliper/actions/ClosedPopout
<http://purl.imsglobal.org/caliper/actions/ClosedPopout> rdf:type owl:NamedIndividual ,
                                                                  :Action ;
                                                         rdfs:comment "Close or shut a video popout. Inverse of OpenedPopout."@en ;
                                                         rdfs:isDefinedBy "http://wordnet-rdf.princeton.edu/wn31/201349660-v"^^xsd:string ;
                                                         rdfs:label "ClosedPopout"@en .


###  http://purl.imsglobal.org/caliper/actions/Commented
<http://purl.imsglobal.org/caliper/actions/Commented> rdf:type owl:NamedIndividual ,
                                                               :Action ;
                                                      rdfs:comment "Make or write a comment on. The Commented action signals that qualitative feedback in the form of a Comment has been provided."@en ;
                                                      rdfs:isDefinedBy "http://wordnet-rdf.princeton.edu/wn31/201060446-v"^^xsd:string ;
                                                      rdfs:label "Commented"@en .


###  http://purl.imsglobal.org/caliper/actions/Completed
<http://purl.imsglobal.org/caliper/actions/Completed> rdf:type owl:NamedIndividual ,
                                                               :Action ;
                                                      rdfs:comment "Come or bring to a finish or an end."@en ;
                                                      rdfs:isDefinedBy "http://wordnet-rdf.princeton.edu/wn31/200485097-v"^^xsd:string ;
                                                      rdfs:label "Completed"@en .


###  http://purl.imsglobal.org/caliper/actions/Copied
<http://purl.imsglobal.org/caliper/actions/Copied> rdf:type owl:NamedIndividual ,
                                                            :Action ;
                                                   rdfs:comment "Make a replica of. The Copied action signals that a resource has been duplicated."@en ;
                                                   rdfs:isDefinedBy "http://wordnet-rdf.princeton.edu/wn31/201697776-v"^^xsd:string ;
                                                   rdfs:label "Copied"@en .


###  http://purl.imsglobal.org/caliper/actions/Created
<http://purl.imsglobal.org/caliper/actions/Created> rdf:type owl:NamedIndividual ,
                                                             :Action ;
                                                    rdfs:comment "Make or cause to be or to become. The Created action signals that a resource has been brought into existence. Inverse of Deleted."@en ;
                                                    rdfs:isDefinedBy "http://wordnet-rdf.princeton.edu/wn31/201620211-v"^^xsd:string ;
                                                    rdfs:label "Created"@en .


###  http://purl.imsglobal.org/caliper/actions/Deactivated
<http://purl.imsglobal.org/caliper/actions/Deactivated> rdf:type owl:NamedIndividual ,
                                                                 :Action ;
                                                        rdfs:comment "Make inactive. Inverse of Activated."@en ;
                                                        rdfs:isDefinedBy "http://wordnet-rdf.princeton.edu/wn31/200191849-v"^^xsd:string ;
                                                        rdfs:label "Deactivated"@en .


###  http://purl.imsglobal.org/caliper/actions/Deleted
<http://purl.imsglobal.org/caliper/actions/Deleted> rdf:type owl:NamedIndividual ,
                                                             :Action ;
                                                    rdfs:comment "Wipe out digitally. The Deleted action signals that a resource has been removed permanently from a system. Inverse of Created."@en ;
                                                    rdfs:isDefinedBy "http://wordnet-rdf.princeton.edu/wn31/201001860-v"^^xsd:string ;
                                                    rdfs:label "Deleted"@en .


###  http://purl.imsglobal.org/caliper/actions/Described
<http://purl.imsglobal.org/caliper/actions/Described> rdf:type owl:NamedIndividual ,
                                                               :Action ;
                                                      rdfs:comment "Give a description of. The Described action signals that a description of a resource has been provided."@en ;
                                                      rdfs:isDefinedBy "http://wordnet-rdf.princeton.edu/wn31/200989103-v"^^xsd:string ;
                                                      rdfs:label "Described"@en .


###  http://purl.imsglobal.org/caliper/actions/DisabledClosedCaptioning
<http://purl.imsglobal.org/caliper/actions/DisabledClosedCaptioning> rdf:type owl:NamedIndividual ,
                                                                              :Action ;
                                                                     rdfs:comment "Render unable to perform the visual display of a plain text transcription of audio output. Inverse of EnabledClosedCaptioning."@en ;
                                                                     rdfs:isDefinedBy "http://purl.imsglobal.org/caliper"^^xsd:string ;
                                                                     rdfs:label "DisabledClosedCaptioning"@en ;
                                                                     rdfs:seeAlso "http://wordnet-rdf.princeton.edu/wn31/200513267-v"^^xsd:string .


###  http://purl.imsglobal.org/caliper/actions/Disliked
<http://purl.imsglobal.org/caliper/actions/Disliked> rdf:type owl:NamedIndividual ,
                                                              :Action ;
                                                     rdfs:comment "Have or feel a dislike or distaste for. Inverse of Liked."@en ;
                                                     rdfs:isDefinedBy "http://wordnet-rdf.princeton.edu/wn31/201780648-v"^^xsd:string ;
                                                     rdfs:label "Disliked"@en .


###  http://purl.imsglobal.org/caliper/actions/Downloaded
<http://purl.imsglobal.org/caliper/actions/Downloaded> rdf:type owl:NamedIndividual ,
                                                                :Action ;
                                                       rdfs:comment "Transfer a file or program from a central computer to a smaller computer or to a computer at a remote location. The Downloaded action signals that a copy of the resource has been transferred from a central or primary system to a remote or secondary system. Inverse of Uploaded."@en ;
                                                       rdfs:isDefinedBy "http://wordnet-rdf.princeton.edu/wn31/02233704-v"^^xsd:string ;
                                                       rdfs:label "Downloaded"@en .


###  http://purl.imsglobal.org/caliper/actions/EnabledClosedCaptioning
<http://purl.imsglobal.org/caliper/actions/EnabledClosedCaptioning> rdf:type owl:NamedIndividual ,
                                                                             :Action ;
                                                                    rdfs:comment "Render capable or able the visual display of a plain text transcription of audio output. Inverse of DisabledClosedCaptioning."@en ;
                                                                    rdfs:isDefinedBy "http://purl.imsglobal.org/caliper"^^xsd:string ;
                                                                    rdfs:label "EnabledClosedCaptioning"@en ;
                                                                    rdfs:seeAlso "http://wordnet-rdf.princeton.edu/wn31/200513958-v"^^xsd:string .


###  http://purl.imsglobal.org/caliper/actions/Ended
<http://purl.imsglobal.org/caliper/actions/Ended> rdf:type owl:NamedIndividual ,
                                                           :Action ;
                                                  rdfs:comment "Bring to an end or halt. Inverse of Started."@en ;
                                                  rdfs:isDefinedBy "http://wordnet-rdf.princeton.edu/wn31/200353480-v"^^xsd:string ;
                                                  rdfs:label "Ended"@en .


###  http://purl.imsglobal.org/caliper/actions/EnteredFullScreen
<http://purl.imsglobal.org/caliper/actions/EnteredFullScreen> rdf:type owl:NamedIndividual ,
                                                                       :Action ;
                                                              rdfs:comment "To come or go into a view mode that utilizes all the available display surface of a screen. Inverse of ExitedFullScreen."@en ;
                                                              rdfs:isDefinedBy "http://purl.imsglobal.org/caliper"^^xsd:string ;
                                                              rdfs:label "EnteredFullScreen"@en ;
                                                              rdfs:seeAlso "http://wordnet-rdf.princeton.edu/wn31/202020375-v"^^xsd:string .


###  http://purl.imsglobal.org/caliper/actions/ExitedFullScreen
<http://purl.imsglobal.org/caliper/actions/ExitedFullScreen> rdf:type owl:NamedIndividual ,
                                                                      :Action ;
                                                             rdfs:comment "Move out of or depart from a view mode that utilizes all the available display surface of a screen. Inverse of EnteredFullScreen."@en ;
                                                             rdfs:isDefinedBy "http://purl.imsglobal.org/caliper"^^xsd:string ;
                                                             rdfs:label "ExitedFullScreen"@en ;
                                                             rdfs:seeAlso "http://wordnet-rdf.princeton.edu/wn31/202019450-v"^^xsd:string .


###  http://purl.imsglobal.org/caliper/actions/ForwardedTo
<http://purl.imsglobal.org/caliper/actions/ForwardedTo> rdf:type owl:NamedIndividual ,
                                                                 :Action ;
                                                        rdfs:comment "Send or ship onward."@en ;
                                                        rdfs:isDefinedBy "http://wordnet-rdf.princeton.edu/wn31/201959367-v"^^xsd:string ;
                                                        rdfs:label "ForwardedTo"@en .


###  http://purl.imsglobal.org/caliper/actions/Graded
<http://purl.imsglobal.org/caliper/actions/Graded> rdf:type owl:NamedIndividual ,
                                                            :Action ;
                                                   rdfs:comment "Assign a grade or rank to, according to one's evaluation."@en ;
                                                   rdfs:isDefinedBy "http://wordnet-rdf.princeton.edu/wn31/200659399-v"^^xsd:string ;
                                                   rdfs:label "Graded"@en .


###  http://purl.imsglobal.org/caliper/actions/Hid
<http://purl.imsglobal.org/caliper/actions/Hid> rdf:type owl:NamedIndividual ,
                                                         :Action ;
                                                rdfs:comment "Prevent from being seen or discovered. Inverse of Showed."@en ;
                                                rdfs:isDefinedBy "http://wordnet-rdf.princeton.edu/wn31/202149298-v"^^xsd:string ;
                                                rdfs:label "Hid"@en .


###  http://purl.imsglobal.org/caliper/actions/Highlighted
<http://purl.imsglobal.org/caliper/actions/Highlighted> rdf:type owl:NamedIndividual ,
                                                                 :Action ;
                                                        rdfs:comment "Move into the foreground to make more visible or prominent."@en ;
                                                        rdfs:isDefinedBy "http://wordnet-rdf.princeton.edu/wn31/200515150-v"^^xsd:string ;
                                                        rdfs:label "Highlighted"@en .


###  http://purl.imsglobal.org/caliper/actions/Identified
<http://purl.imsglobal.org/caliper/actions/Identified> rdf:type owl:NamedIndividual ,
                                                                :Action ;
                                                       rdfs:comment "Recognize as being; establish the identity of someone or something."@en ;
                                                       rdfs:isDefinedBy "http://wordnet-rdf.princeton.edu/wn31/200620568-v"^^xsd:string ;
                                                       rdfs:label "Identified"@en .


###  http://purl.imsglobal.org/caliper/actions/JumpedTo
<http://purl.imsglobal.org/caliper/actions/JumpedTo> rdf:type owl:NamedIndividual ,
                                                              :Action ;
                                                     rdfs:comment "Pass abruptly from one state or topic to another."@en ;
                                                     rdfs:isDefinedBy "http://wordnet-rdf.princeton.edu/wn31/200561468-v"^^xsd:string ;
                                                     rdfs:label "JumpedTo"@en .


###  http://purl.imsglobal.org/caliper/actions/Liked
<http://purl.imsglobal.org/caliper/actions/Liked> rdf:type owl:NamedIndividual ,
                                                           :Action ;
                                                  rdfs:comment "Be fond of. Inverse of Disliked."@en ;
                                                  rdfs:isDefinedBy "http://wordnet-rdf.princeton.edu/wn31/201780873-v"^^xsd:string ;
                                                  rdfs:label "Liked"@en .


###  http://purl.imsglobal.org/caliper/actions/Linked
<http://purl.imsglobal.org/caliper/actions/Linked> rdf:type owl:NamedIndividual ,
                                                            :Action ;
                                                   rdfs:comment "Connect, fasten, or put together two or more pieces."@en ;
                                                   rdfs:isDefinedBy "http://wordnet-rdf.princeton.edu/wn31/201357376-v"^^xsd:string ;
                                                   rdfs:label "Linked"@en .


###  http://purl.imsglobal.org/caliper/actions/LoggedIn
<http://purl.imsglobal.org/caliper/actions/LoggedIn> rdf:type owl:NamedIndividual ,
                                                              :Action ;
                                                     rdfs:comment "Enter a computer or software application. Inverse of LoggedOut."@en ;
                                                     rdfs:isDefinedBy "http://wordnet-rdf.princeton.edu/wn31/202253955-v"^^xsd:string ;
                                                     rdfs:label "LoggedIn"@en .


###  http://purl.imsglobal.org/caliper/actions/LoggedOut
<http://purl.imsglobal.org/caliper/actions/LoggedOut> rdf:type owl:NamedIndividual ,
                                                               :Action ;
                                                      rdfs:comment "Exit a computer or software application. Inverse of LoggedIn."@en ;
                                                      rdfs:isDefinedBy "http://wordnet-rdf.princeton.edu/wn31/202254101-v"^^xsd:string ;
                                                      rdfs:label "LoggedOut"@en .


###  http://purl.imsglobal.org/caliper/actions/MarkedAsRead
<http://purl.imsglobal.org/caliper/actions/MarkedAsRead> rdf:type owl:NamedIndividual ,
                                                                  :Action ;
                                                         rdfs:comment "Mark: designate as if by a mark, read: interpret something that is written or printed. Inverse of MarkedAsUnread."@en ;
                                                         rdfs:isDefinedBy "http://wordnet-rdf.princeton.edu/wn31/200923709-v"^^xsd:string ;
                                                         rdfs:label "MarkedAsRead"@en ;
                                                         rdfs:seeAlso "http://wordnet-rdf.princeton.edu/wn31/200626756-v"^^xsd:string .


###  http://purl.imsglobal.org/caliper/actions/MarkedAsUnread
<http://purl.imsglobal.org/caliper/actions/MarkedAsUnread> rdf:type owl:NamedIndividual ,
                                                                    :Action ;
                                                           rdfs:comment "Remove designation as if by a mark.  Inverse of MarkedAsRead."@en ;
                                                           rdfs:isDefinedBy "http://purl.imsglobal.org/caliper"^^xsd:string ;
                                                           rdfs:label "MarkedAsUnread"@en ;
                                                           rdfs:seeAlso "http://wordnet-rdf.princeton.edu/wn31/200923709-v"^^xsd:string .


###  http://purl.imsglobal.org/caliper/actions/Modified
<http://purl.imsglobal.org/caliper/actions/Modified> rdf:type owl:NamedIndividual ,
                                                              :Action ;
                                                     rdfs:comment "Cause to change; make different; cause a transformation. The Modified action signals that a resource has been altered or changed."@en ;
                                                     rdfs:isDefinedBy "http://wordnet-rdf.princeton.edu/wn31/200126072-v"^^xsd:string ;
                                                     rdfs:label "Modified"@en .


###  http://purl.imsglobal.org/caliper/actions/Muted
<http://purl.imsglobal.org/caliper/actions/Muted> rdf:type owl:NamedIndividual ,
                                                           :Action ;
                                                  rdfs:comment "Deaden (a sound or noise). Inverse of Unmuted."@en ;
                                                  rdfs:isDefinedBy "http://wordnet-rdf.princeton.edu/wn31/mute-v"^^xsd:string ;
                                                  rdfs:label "Muted"@en .


###  http://purl.imsglobal.org/caliper/actions/NavigatedTo
<http://purl.imsglobal.org/caliper/actions/NavigatedTo> rdf:type owl:NamedIndividual ,
                                                                 :Action ;
                                                        rdfs:comment "Direct the course; determine the direction of travelling."@en ;
                                                        rdfs:isDefinedBy "http://wordnet-rdf.princeton.edu/wn31/201935739-v"^^xsd:string ;
                                                        rdfs:label "NavigatedTo"@en .


###  http://purl.imsglobal.org/caliper/actions/OpenedPopout
<http://purl.imsglobal.org/caliper/actions/OpenedPopout> rdf:type owl:NamedIndividual ,
                                                                  :Action ;
                                                         rdfs:comment "Start to operate or function or cause to start operating or functioning a video popout. Inverse of ClosedPopout."@en ;
                                                         rdfs:isDefinedBy "http://purl.imsglobal.org/caliper"^^xsd:string ;
                                                         rdfs:label "OpenedPopout"@en ;
                                                         rdfs:seeAlso "http://wordnet-rdf.princeton.edu/wn31/202431018-v"^^xsd:string .


###  http://purl.imsglobal.org/caliper/actions/Paused
<http://purl.imsglobal.org/caliper/actions/Paused> rdf:type owl:NamedIndividual ,
                                                            :Action ;
                                                   rdfs:comment "Cease an action temporarily. Inverse of Resumed."@en ;
                                                   rdfs:isDefinedBy "http://wordnet-rdf.princeton.edu/wn31/200781106-v"^^xsd:string ;
                                                   rdfs:label "Paused"@en .


###  http://purl.imsglobal.org/caliper/actions/Posted
<http://purl.imsglobal.org/caliper/actions/Posted> rdf:type owl:NamedIndividual ,
                                                            :Action ;
                                                   rdfs:comment "To cause to be directed or transmitted to another place."@en ;
                                                   rdfs:isDefinedBy "http://wordnet-rdf.princeton.edu/wn31/201033289-v"^^xsd:string ;
                                                   rdfs:label "Posted"@en .


###  http://purl.imsglobal.org/caliper/actions/Printed
<http://purl.imsglobal.org/caliper/actions/Printed> rdf:type owl:NamedIndividual ,
                                                             :Action ;
                                                    rdfs:comment "Reproduce by printing. The Printed action signals that a mechanical process has been invoked in order to produce a printed representation of a resource."@en ;
                                                    rdfs:isDefinedBy "http://wordnet-rdf.princeton.edu/wn31/01747945-v"^^xsd:string ;
                                                    rdfs:label "Printed"@en .


###  http://purl.imsglobal.org/caliper/actions/Published
<http://purl.imsglobal.org/caliper/actions/Published> rdf:type owl:NamedIndividual ,
                                                               :Action ;
                                                      rdfs:comment "Prepare and issue for public distribution or sale. The Published action signals that a resource is now available for public consumption. Inverse of Unpublished."@en ;
                                                      rdfs:isDefinedBy "http://wordnet-rdf.princeton.edu/wn31/200969657-v"^^xsd:string ;
                                                      rdfs:label "Published"@en .


###  http://purl.imsglobal.org/caliper/actions/Questioned
<http://purl.imsglobal.org/caliper/actions/Questioned> rdf:type owl:NamedIndividual ,
                                                                :Action ;
                                                       rdfs:comment "Pose a question."@en ;
                                                       rdfs:isDefinedBy "http://wordnet-rdf.princeton.edu/wn31/200786670-v"^^xsd:string ;
                                                       rdfs:label "Questioned"@en .


###  http://purl.imsglobal.org/caliper/actions/Ranked
<http://purl.imsglobal.org/caliper/actions/Ranked> rdf:type owl:NamedIndividual ,
                                                            :Action ;
                                                   rdfs:comment "Assign a rank or rating to. The Ranked action signals that quantitative feedback in the form of a Rating has been provided."@en ;
                                                   rdfs:isDefinedBy "http://wordnet-rdf.princeton.edu/wn31/200659723-v"^^xsd:string ;
                                                   rdfs:label "Ranked"@en .


###  http://purl.imsglobal.org/caliper/actions/Recommended
<http://purl.imsglobal.org/caliper/actions/Recommended> rdf:type owl:NamedIndividual ,
                                                                 :Action ;
                                                        rdfs:comment "Express a good opinion of."@en ;
                                                        rdfs:isDefinedBy "http://wordnet-rdf.princeton.edu/wn31/200884469-v"^^xsd:string ;
                                                        rdfs:label "Recommended"@en .


###  http://purl.imsglobal.org/caliper/actions/Removed
<http://purl.imsglobal.org/caliper/actions/Removed> rdf:type owl:NamedIndividual ,
                                                             :Action ;
                                                    rdfs:comment "Remove from sight. Inverse of Added."@en ;
                                                    rdfs:isDefinedBy "http://wordnet-rdf.princeton.edu/wn31/200181704-v"^^xsd:string ;
                                                    rdfs:label "Removed"@en .


###  http://purl.imsglobal.org/caliper/actions/Reset
<http://purl.imsglobal.org/caliper/actions/Reset> rdf:type owl:NamedIndividual ,
                                                           :Action ;
                                                  rdfs:comment "Set anew."@en ;
                                                  rdfs:isDefinedBy "http://wordnet-rdf.princeton.edu/wn31/200949623-v"^^xsd:string ;
                                                  rdfs:label "Reset"@en .


###  http://purl.imsglobal.org/caliper/actions/Restarted
<http://purl.imsglobal.org/caliper/actions/Restarted> rdf:type owl:NamedIndividual ,
                                                               :Action ;
                                                      rdfs:comment "Take up or begin anew, as in to start something, make progress but then stop and return to the beginning in order to start again."@en ;
                                                      rdfs:isDefinedBy "http://purl.imglobal.org/caliper"^^xsd:string ;
                                                      rdfs:label "Restarted"@en ;
                                                      rdfs:seeAlso "http://wordnet-rdf.princeton.edu/wn31/200350758-v"^^xsd:string .


###  http://purl.imsglobal.org/caliper/actions/Restored
<http://purl.imsglobal.org/caliper/actions/Restored> rdf:type owl:NamedIndividual ,
                                                              :Action ;
                                                     rdfs:comment "Return to its original or usable and functioning condition. The Restored action signals that an archived resource has been retrieved from long-term storage. Inverse of Archived."@en ;
                                                     rdfs:isDefinedBy "http://wordnet-rdf.princeton.edu/wn31/202558146-v"^^xsd:string ;
                                                     rdfs:label "Restored"@en .


###  http://purl.imsglobal.org/caliper/actions/Resumed
<http://purl.imsglobal.org/caliper/actions/Resumed> rdf:type owl:NamedIndividual ,
                                                             :Action ;
                                                    rdfs:comment "Take up or begin anew, as in to start something, pause and then begin again at the location where the pause in action occurred. Inverse of Paused."@en ;
                                                    rdfs:isDefinedBy "http://purl.imsglobal.org/caliper"^^xsd:string ;
                                                    rdfs:label "Resumed"@en ;
                                                    rdfs:seeAlso "http://wordnet-rdf.princeton.edu/wn31/200350758-v"^^xsd:string .


###  http://purl.imsglobal.org/caliper/actions/Retrieved
<http://purl.imsglobal.org/caliper/actions/Retrieved> rdf:type owl:NamedIndividual ,
                                                               :Action ;
                                                      rdfs:comment "Obtain or retrieve from a storage device; as of information on a computer. The Retrieved action signals that a resource has been accessed or obtained."@en ;
                                                      rdfs:isDefinedBy "http://wordnet-rdf.princeton.edu/wn31/202253616-v"^^xsd:string ;
                                                      rdfs:label "Retrieved"@en .


###  http://purl.imsglobal.org/caliper/actions/Reviewed
<http://purl.imsglobal.org/caliper/actions/Reviewed> rdf:type owl:NamedIndividual ,
                                                              :Action ;
                                                     rdfs:comment "Appraise critically."@en ;
                                                     rdfs:isDefinedBy "http://wordnet-rdf.princeton.edu/wn31/200857194-v"^^xsd:string ;
                                                     rdfs:label "Reviewed"@en .


###  http://purl.imsglobal.org/caliper/actions/Rewound
<http://purl.imsglobal.org/caliper/actions/Rewound> rdf:type owl:NamedIndividual ,
                                                             :Action ;
                                                    rdfs:comment "Wind up again."@en ;
                                                    rdfs:isDefinedBy "http://wordnet-rdf.princeton.edu/wn31/201524927-v"^^xsd:string ;
                                                    rdfs:label "Rewound"@en .


###  http://purl.imsglobal.org/caliper/actions/Saved
<http://purl.imsglobal.org/caliper/actions/Saved> rdf:type owl:NamedIndividual ,
                                                           :Action ;
                                                  rdfs:comment "Record data on a computer. The Saved action signals that the current state of a resource has been stored for future use."@en ;
                                                  rdfs:isDefinedBy "http://wordnet-rdf.princeton.edu/wn31/00998886-v"^^xsd:string ;
                                                  rdfs:label "Saved"@en .


###  http://purl.imsglobal.org/caliper/actions/Searched
<http://purl.imsglobal.org/caliper/actions/Searched> rdf:type owl:NamedIndividual ,
                                                              :Action ;
                                                     rdfs:comment "Try to locate or discover, or try to establish the existence of."@en ;
                                                     rdfs:isDefinedBy "http://wordnet-rdf.princeton.edu/wn31/201318273-v"^^xsd:string ;
                                                     rdfs:label "Searched"@en .


###  http://purl.imsglobal.org/caliper/actions/Shared
<http://purl.imsglobal.org/caliper/actions/Shared> rdf:type owl:NamedIndividual ,
                                                            :Action ;
                                                   rdfs:comment "Communicate."@en ;
                                                   rdfs:isDefinedBy "http://wordnet-rdf.princeton.edu/wn31/201065952-v"^^xsd:string ;
                                                   rdfs:label "Shared"@en .


###  http://purl.imsglobal.org/caliper/actions/Showed
<http://purl.imsglobal.org/caliper/actions/Showed> rdf:type owl:NamedIndividual ,
                                                            :Action ;
                                                   rdfs:comment "Make visible or noticeable. Inverse of Hid."@en ;
                                                   rdfs:isDefinedBy "http://wordnet-rdf.princeton.edu/wn31/202141597-v"^^xsd:string ;
                                                   rdfs:label "Showed"@en .


###  http://purl.imsglobal.org/caliper/actions/Skipped
<http://purl.imsglobal.org/caliper/actions/Skipped> rdf:type owl:NamedIndividual ,
                                                             :Action ;
                                                    rdfs:comment "Bypass."@en ;
                                                    rdfs:isDefinedBy "http://wordnet-rdf.princeton.edu/wn31/200618188-v"^^xsd:string ;
                                                    rdfs:label "Skipped"@en .


###  http://purl.imsglobal.org/caliper/actions/Started
<http://purl.imsglobal.org/caliper/actions/Started> rdf:type owl:NamedIndividual ,
                                                             :Action ;
                                                    rdfs:comment "Set in motion, cause to start. Inverse of Ended."@en ;
                                                    rdfs:isDefinedBy "http://wordnet-rdf.princeton.edu/wn31/200349400-v"^^xsd:string ;
                                                    rdfs:label "Started"@en .


###  http://purl.imsglobal.org/caliper/actions/Submitted
<http://purl.imsglobal.org/caliper/actions/Submitted> rdf:type owl:NamedIndividual ,
                                                               :Action ;
                                                      rdfs:comment "Hand over formally."@en ;
                                                      rdfs:isDefinedBy "http://wordnet-rdf.princeton.edu/wn31/202267560-v"^^xsd:string ;
                                                      rdfs:label "Submitted"@en .


###  http://purl.imsglobal.org/caliper/actions/Subscribed
<http://purl.imsglobal.org/caliper/actions/Subscribed> rdf:type owl:NamedIndividual ,
                                                                :Action ;
                                                       rdfs:comment "Receive or obtain regularly. Inverse of Unsubscribed."@en ;
                                                       rdfs:isDefinedBy "http://wordnet-rdf.princeton.edu/wn31/202214527-v"^^xsd:string ;
                                                       rdfs:label "Subscribed"@en .


###  http://purl.imsglobal.org/caliper/actions/Tagged
<http://purl.imsglobal.org/caliper/actions/Tagged> rdf:type owl:NamedIndividual ,
                                                            :Action ;
                                                   rdfs:comment "Attach a tag or label to."@en ;
                                                   rdfs:isDefinedBy "http://wordnet-rdf.princeton.edu/wn31/201591414-v"^^xsd:string ;
                                                   rdfs:label "Tagged"@en .


###  http://purl.imsglobal.org/caliper/actions/TimedOut
<http://purl.imsglobal.org/caliper/actions/TimedOut> rdf:type owl:NamedIndividual ,
                                                              :Action ;
                                                     rdfs:comment "Cancellation of a user session after a predetermined time interval has occurred without activity."@en ;
                                                     rdfs:isDefinedBy "http://purl.imsglobal.org/caliper"^^xsd:string ;
                                                     rdfs:label "TimedOut"@en .


###  http://purl.imsglobal.org/caliper/actions/Unmuted
<http://purl.imsglobal.org/caliper/actions/Unmuted> rdf:type owl:NamedIndividual ,
                                                             :Action ;
                                                    rdfs:comment "Inverse of Muted."@en ;
                                                    rdfs:isDefinedBy "http://purl.imsglobal.org/caliper"^^xsd:string ;
                                                    rdfs:label "Unmuted"@en ;
                                                    rdfs:seeAlso "http://wordnet-rdf.princeton.edu/wn31/mute-v"^^xsd:string .


###  http://purl.imsglobal.org/caliper/actions/Unpublished
<http://purl.imsglobal.org/caliper/actions/Unpublished> rdf:type owl:NamedIndividual ,
                                                                 :Action ;
                                                        rdfs:comment "Remove from public distribution or sale. The Unpublished action signals that a published resource has been rendered unavailable for public consumption. Inverse of Published."@en ;
                                                        rdfs:isDefinedBy "http://wordnet-rdf.princeton.edu/wn31/200969657-v"^^xsd:string ;
                                                        rdfs:label "Unpublished"@en .


###  http://purl.imsglobal.org/caliper/actions/Unsubscribed
<http://purl.imsglobal.org/caliper/actions/Unsubscribed> rdf:type owl:NamedIndividual ,
                                                                  :Action ;
                                                         rdfs:comment "Inverse of Subscribed."@en ;
                                                         rdfs:isDefinedBy "http://purl.imsglobal.org/caliper"^^xsd:string ;
                                                         rdfs:label "Unsubscribed"@en ;
                                                         rdfs:seeAlso "http://wordnet-rdf.princeton.edu/wn31/202214527-v"^^xsd:string .


###  http://purl.imsglobal.org/caliper/actions/Uploaded
<http://purl.imsglobal.org/caliper/actions/Uploaded> rdf:type owl:NamedIndividual ,
                                                              :Action ;
                                                     rdfs:comment "Transfer a file or program to a central computer from a smaller computer or a computer at a remote location. The Uploaded action signals that a copy of the resource has been transferred from a remote or secondary system to a central or primary system. Inverse of Downloaded."@en ;
                                                     rdfs:isDefinedBy "http://wordnet-rdf.princeton.edu/wn31/02233898-v"^^xsd:string ;
                                                     rdfs:label "Uploaded"@en .


###  http://purl.imsglobal.org/caliper/actions/Used
<http://purl.imsglobal.org/caliper/actions/Used> rdf:type owl:NamedIndividual ,
                                                          :Action ;
                                                 rdfs:comment "Put into service; make work or employ for a particular purpose or for its inherent or natural purpose."@en ;
                                                 rdfs:isDefinedBy "http://wordnet-rdf.princeton.edu/wn31/201161188-v"^^xsd:string ;
                                                 rdfs:label "Used"@en .


###  http://purl.imsglobal.org/caliper/actions/Viewed
<http://purl.imsglobal.org/caliper/actions/Viewed> rdf:type owl:NamedIndividual ,
                                                            :Action ;
                                                   rdfs:comment "Look at carefully; study mentally."@en ;
                                                   rdfs:isDefinedBy "http://wordnet-rdf.princeton.edu/wn31/202134765-v"^^xsd:string ;
                                                   rdfs:label "Viewed"@en .


###  http://purl.imsglobal.org/caliper/lti/LtiDeepLinkingRequest
<http://purl.imsglobal.org/caliper/lti/LtiDeepLinkingRequest> rdf:type owl:NamedIndividual ,
                                                                       :LtiMessageType ;
                                                              rdfs:comment "An LTI message type."@en ;
                                                              rdfs:isDefinedBy "http://purl.imsglobal.org/caliper"^^xsd:string ;
                                                              rdfs:label "LtiDeepLinkingRequest"@en .


###  http://purl.imsglobal.org/caliper/lti/LtiResourceLinkRequest
<http://purl.imsglobal.org/caliper/lti/LtiResourceLinkRequest> rdf:type owl:NamedIndividual ,
                                                                        :LtiMessageType ;
                                                               rdfs:comment "An LTI message type."@en ;
                                                               rdfs:isDefinedBy "http://purl.imsglobal.org/caliper"^^xsd:string ;
                                                               rdfs:label "LtiResourceLinkRequest"@en .


###  http://purl.imsglobal.org/caliper/metrics/AssessmentsPassed
<http://purl.imsglobal.org/caliper/metrics/AssessmentsPassed> rdf:type owl:NamedIndividual ,
                                                                       :Metric ;
                                                              rdfs:comment "Count of assessments that have been passed by the learner."@en ;
                                                              rdfs:isDefinedBy "http://purl.imsglobal.org/caliper"^^xsd:string ;
                                                              rdfs:label "AssessmentsPassed"@en .


###  http://purl.imsglobal.org/caliper/metrics/AssessmentsSubmitted
<http://purl.imsglobal.org/caliper/metrics/AssessmentsSubmitted> rdf:type owl:NamedIndividual ,
                                                                          :Metric ;
                                                                 rdfs:comment "Count of assessments that have been submitted by the learner."@en ;
                                                                 rdfs:isDefinedBy "http://purl.imsglobal.org/caliper"^^xsd:string ;
                                                                 rdfs:label "AssessmentsSubmitted"@en .


###  http://purl.imsglobal.org/caliper/metrics/MinutesOnTask
<http://purl.imsglobal.org/caliper/metrics/MinutesOnTask> rdf:type owl:NamedIndividual ,
                                                                   :Metric ;
                                                          rdfs:comment "Active time spent by learner utilizing the tool."@en ;
                                                          rdfs:isDefinedBy "http://purl.imsglobal.org/caliper"^^xsd:string ;
                                                          rdfs:label "MinutesOnTask"@en .


###  http://purl.imsglobal.org/caliper/metrics/SkillsMastered
<http://purl.imsglobal.org/caliper/metrics/SkillsMastered> rdf:type owl:NamedIndividual ,
                                                                    :Metric ;
                                                           rdfs:comment "Count of learning skills or targets for which the learner has demonstrated understanding."@en ;
                                                           rdfs:isDefinedBy "http://purl.imsglobal.org/caliper"^^xsd:string ;
                                                           rdfs:label "SkillsMastered"@en .


###  http://purl.imsglobal.org/caliper/metrics/StandardsMastered
<http://purl.imsglobal.org/caliper/metrics/StandardsMastered> rdf:type owl:NamedIndividual ,
                                                                       :Metric ;
                                                              rdfs:comment "Count of learning standards or competencies for which the learner has demonstrated understanding."@en ;
                                                              rdfs:isDefinedBy "http://purl.imsglobal.org/caliper"^^xsd:string ;
                                                              rdfs:label "StandardsMastered"@en .


###  http://purl.imsglobal.org/caliper/metrics/UnitsCompleted
<http://purl.imsglobal.org/caliper/metrics/UnitsCompleted> rdf:type owl:NamedIndividual ,
                                                                    :Metric ;
                                                           rdfs:comment "Count of instructional units completed by the learner."@en ;
                                                           rdfs:isDefinedBy "http://purl.imsglobal.org/caliper"^^xsd:string ;
                                                           rdfs:label "UnitsCompleted"@en .


###  http://purl.imsglobal.org/caliper/metrics/UnitsPassed
<http://purl.imsglobal.org/caliper/metrics/UnitsPassed> rdf:type owl:NamedIndividual ,
                                                                 :Metric ;
                                                        rdfs:comment "Count of instructional units completed by the learner, submitted for evaluation, and scored with a passing mark."@en ;
                                                        rdfs:isDefinedBy "http://purl.imsglobal.org/caliper"^^xsd:string ;
                                                        rdfs:label "UnitsPassed"@en .


###  http://purl.imsglobal.org/caliper/metrics/WordsRead
<http://purl.imsglobal.org/caliper/metrics/WordsRead> rdf:type owl:NamedIndividual ,
                                                               :Metric ;
                                                      rdfs:comment "Count of the number of words read by the learner."@en ;
                                                      rdfs:isDefinedBy "http://purl.imsglobal.org/caliper"^^xsd:string ;
                                                      rdfs:label "WordsRead"@en .


###  http://purl.imsglobal.org/vocab/lis/v2/membership/Administrator#Administrator
<http://purl.imsglobal.org/vocab/lis/v2/membership/Administrator#Administrator> rdf:type owl:NamedIndividual ,
                                                                                         <http://purl.imsglobal.org/vocab/lis/v2/membership#Administrator> ;
                                                                                rdfs:comment "Someone who typically works with a system and all sub-structures (LMS, SIS, etc.)."@en ;
                                                                                rdfs:isDefinedBy "http://www.imsglobal.org/lis/"^^xsd:string ;
                                                                                rdfs:label "Administrator"@en .


###  http://purl.imsglobal.org/vocab/lis/v2/membership/Administrator#Developer
<http://purl.imsglobal.org/vocab/lis/v2/membership/Administrator#Developer> rdf:type owl:NamedIndividual ,
                                                                                     <http://purl.imsglobal.org/vocab/lis/v2/membership#Administrator> ;
                                                                            rdfs:comment "Provides programmatic development for use in a LMS, SIS, or associated tool(s)."@en ;
                                                                            rdfs:isDefinedBy "http://www.imsglobal.org/lis/"^^xsd:string ;
                                                                            rdfs:label "Developer"@en .


###  http://purl.imsglobal.org/vocab/lis/v2/membership/Administrator#ExternalDeveloper
<http://purl.imsglobal.org/vocab/lis/v2/membership/Administrator#ExternalDeveloper> rdf:type owl:NamedIndividual ,
                                                                                             <http://purl.imsglobal.org/vocab/lis/v2/membership#Administrator> ;
                                                                                    rdfs:comment "A user who is not a member of the institution but provides programmatic development for use in a LMS, SIS, or associated tool(s)."@en ;
                                                                                    rdfs:isDefinedBy "http://www.imsglobal.org/lis/"^^xsd:string ;
                                                                                    rdfs:label "ExternalDeveloper"@en .


###  http://purl.imsglobal.org/vocab/lis/v2/membership/Administrator#ExternalSupport
<http://purl.imsglobal.org/vocab/lis/v2/membership/Administrator#ExternalSupport> rdf:type owl:NamedIndividual ,
                                                                                           <http://purl.imsglobal.org/vocab/lis/v2/membership#Administrator> ;
                                                                                  rdfs:comment "A user who is not a member of the institution but provides support for the system; usually has fewer privileges then an administrator."@en ;
                                                                                  rdfs:isDefinedBy "http://www.imsglobal.org/lis/"^^xsd:string ;
                                                                                  rdfs:label "ExternalSupport"@en .


###  http://purl.imsglobal.org/vocab/lis/v2/membership/Administrator#ExternalSystemAdministrator
<http://purl.imsglobal.org/vocab/lis/v2/membership/Administrator#ExternalSystemAdministrator> rdf:type owl:NamedIndividual ,
                                                                                                       <http://purl.imsglobal.org/vocab/lis/v2/membership#Administrator> ;
                                                                                              rdfs:comment "A user who is not a member of the institution that provides support, e.g., vendor support accounts, 3rd party support accounts, etc."@en ;
                                                                                              rdfs:isDefinedBy "http://www.imsglobal.org/lis/"^^xsd:string ;
                                                                                              rdfs:label "ExternalSystemAdministrator"@en .


###  http://purl.imsglobal.org/vocab/lis/v2/membership/Administrator#Support
<http://purl.imsglobal.org/vocab/lis/v2/membership/Administrator#Support> rdf:type owl:NamedIndividual ,
                                                                                   <http://purl.imsglobal.org/vocab/lis/v2/membership#Administrator> ;
                                                                          rdfs:comment "Provides support for the system, usually has fewer privileges then an administrator."@en ;
                                                                          rdfs:isDefinedBy "http://www.imsglobal.org/lis/"^^xsd:string ;
                                                                          rdfs:label "Support"@en .


###  http://purl.imsglobal.org/vocab/lis/v2/membership/Administrator#SystemAdministrator
<http://purl.imsglobal.org/vocab/lis/v2/membership/Administrator#SystemAdministrator> rdf:type owl:NamedIndividual ,
                                                                                               <http://purl.imsglobal.org/vocab/lis/v2/membership#Administrator> ;
                                                                                      rdfs:comment "A person who has greater privileges then an administrator."@en ;
                                                                                      rdfs:isDefinedBy "http://www.imsglobal.org/lis/"^^xsd:string ;
                                                                                      rdfs:label "SystemAdministrator"@en .


###  http://purl.imsglobal.org/vocab/lis/v2/membership/ContentDeveloper#ContentDeveloper
<http://purl.imsglobal.org/vocab/lis/v2/membership/ContentDeveloper#ContentDeveloper> rdf:type owl:NamedIndividual ,
                                                                                               <http://purl.imsglobal.org/vocab/lis/v2/membership#ContentDeveloper> ;
                                                                                      rdfs:comment "Someone who usually develops materials within a specific course structure."@en ;
                                                                                      rdfs:isDefinedBy "http://www.imsglobal.org/lis/"^^xsd:string ;
                                                                                      rdfs:label "ContentDeveloper"@en .


###  http://purl.imsglobal.org/vocab/lis/v2/membership/ContentDeveloper#ContentExpert
<http://purl.imsglobal.org/vocab/lis/v2/membership/ContentDeveloper#ContentExpert> rdf:type owl:NamedIndividual ,
                                                                                            <http://purl.imsglobal.org/vocab/lis/v2/membership#ContentDeveloper> ;
                                                                                   rdfs:comment "An expert that participates in the course because of their knowledge; e.g., guest speaker, artist in residence, etc."@en ;
                                                                                   rdfs:isDefinedBy "http://www.imsglobal.org/lis/"^^xsd:string ;
                                                                                   rdfs:label "ContentExpert"@en .


###  http://purl.imsglobal.org/vocab/lis/v2/membership/ContentDeveloper#ExternalContentExpert
<http://purl.imsglobal.org/vocab/lis/v2/membership/ContentDeveloper#ExternalContentExpert> rdf:type owl:NamedIndividual ,
                                                                                                    <http://purl.imsglobal.org/vocab/lis/v2/membership#ContentDeveloper> ;
                                                                                           rdfs:comment "An expert who is not a member of the institution butparticipates in the course because of their knowledge; e.g., guest speaker, artist in residence, etc."@en ;
                                                                                           rdfs:isDefinedBy "http://www.imsglobal.org/lis/"^^xsd:string ;
                                                                                           rdfs:label "ExternalContentExpert"@en .


###  http://purl.imsglobal.org/vocab/lis/v2/membership/ContentDeveloper#Librarian
<http://purl.imsglobal.org/vocab/lis/v2/membership/ContentDeveloper#Librarian> rdf:type owl:NamedIndividual ,
                                                                                        <http://purl.imsglobal.org/vocab/lis/v2/membership#ContentDeveloper> ;
                                                                               rdfs:comment "A librarian who provides content support."@en ;
                                                                               rdfs:isDefinedBy "http://www.imsglobal.org/lis/"^^xsd:string ;
                                                                               rdfs:label "Librarian"@en .


###  http://purl.imsglobal.org/vocab/lis/v2/membership/Instructor#ExternalInstructor
<http://purl.imsglobal.org/vocab/lis/v2/membership/Instructor#ExternalInstructor> rdf:type owl:NamedIndividual ,
                                                                                           <http://purl.imsglobal.org/vocab/lis/v2/membership#Instructor> ;
                                                                                  rdfs:comment "An instructor who is not a member of the institution."@en ;
                                                                                  rdfs:isDefinedBy "http://www.imsglobal.org/lis/"^^xsd:string ;
                                                                                  rdfs:label "ExternalInstructor"@en .


###  http://purl.imsglobal.org/vocab/lis/v2/membership/Instructor#GuestInstructor
<http://purl.imsglobal.org/vocab/lis/v2/membership/Instructor#GuestInstructor> rdf:type owl:NamedIndividual ,
                                                                                        <http://purl.imsglobal.org/vocab/lis/v2/membership#Instructor> ;
                                                                               rdfs:comment ""@en ,
                                                                                            "An instructor who is teaching this course outside of their normal responsibilities"@en ;
                                                                               rdfs:isDefinedBy "http://www.imsglobal.org/lis/"^^xsd:string ;
                                                                               rdfs:label "GuestInstructor"@en .


###  http://purl.imsglobal.org/vocab/lis/v2/membership/Instructor#Instructor
<http://purl.imsglobal.org/vocab/lis/v2/membership/Instructor#Instructor> rdf:type owl:NamedIndividual ,
                                                                                   <http://purl.imsglobal.org/vocab/lis/v2/membership#Instructor> ;
                                                                          rdfs:comment "Someone who usually teaches within a specific course structure."@en ;
                                                                          rdfs:isDefinedBy "http://www.imsglobal.org/lis/"^^xsd:string ;
                                                                          rdfs:label "Instructor"@en .


###  http://purl.imsglobal.org/vocab/lis/v2/membership/Instructor#Lecturer
<http://purl.imsglobal.org/vocab/lis/v2/membership/Instructor#Lecturer> rdf:type owl:NamedIndividual ,
                                                                                 <http://purl.imsglobal.org/vocab/lis/v2/membership#Instructor> ;
                                                                        rdfs:comment "An instructor that has limited permissions to modify the course."@en ;
                                                                        rdfs:isDefinedBy "http://www.imsglobal.org/lis/"^^xsd:string ;
                                                                        rdfs:label "Lecturer"@en .


###  http://purl.imsglobal.org/vocab/lis/v2/membership/Instructor#PrimaryInstructor
<http://purl.imsglobal.org/vocab/lis/v2/membership/Instructor#PrimaryInstructor> rdf:type owl:NamedIndividual ,
                                                                                          <http://purl.imsglobal.org/vocab/lis/v2/membership#Instructor> ;
                                                                                 rdfs:comment "An instructor who is primarily responsible for the instruction."@en ;
                                                                                 rdfs:isDefinedBy "http://www.imsglobal.org/lis/"^^xsd:string ;
                                                                                 rdfs:label "PrimaryInstructor"@en .


###  http://purl.imsglobal.org/vocab/lis/v2/membership/Instructor#SecondaryInstructor
<http://purl.imsglobal.org/vocab/lis/v2/membership/Instructor#SecondaryInstructor> rdf:type owl:NamedIndividual ,
                                                                                            <http://purl.imsglobal.org/vocab/lis/v2/membership#Instructor> ;
                                                                                   rdfs:comment "An instructor who has secondary responsibility for the instruction."@en ;
                                                                                   rdfs:isDefinedBy "http://www.imsglobal.org/lis/"^^xsd:string ;
                                                                                   rdfs:label "SecondaryInstructor"@en .


###  http://purl.imsglobal.org/vocab/lis/v2/membership/Instructor#TeachingAssistant
<http://purl.imsglobal.org/vocab/lis/v2/membership/Instructor#TeachingAssistant> rdf:type owl:NamedIndividual ,
                                                                                          <http://purl.imsglobal.org/vocab/lis/v2/membership#TeachingAssistant> ;
                                                                                 rdfs:comment "Someone who usually has a subset of instructional responsibilities for some portion of a course structure"@en ,
                                                                                              "The role of a teaching assistant to an Instructor in the Membership."@en ;
                                                                                 rdfs:isDefinedBy "http://www.imsglobal.org/lis/"^^xsd:string ;
                                                                                 rdfs:label "TeachingAssistant"@en .


###  http://purl.imsglobal.org/vocab/lis/v2/membership/Instructor#TeachingAssistantGroup
<http://purl.imsglobal.org/vocab/lis/v2/membership/Instructor#TeachingAssistantGroup> rdf:type owl:NamedIndividual ,
                                                                                               <http://purl.imsglobal.org/vocab/lis/v2/membership#TeachingAssistant> ;
                                                                                      rdfs:comment "A teaching assistant for a Group."@en ;
                                                                                      rdfs:isDefinedBy "http://www.imsglobal.org/lis/"^^xsd:string ;
                                                                                      rdfs:label "TeachingAssistantGroup"@en .


###  http://purl.imsglobal.org/vocab/lis/v2/membership/Instructor#TeachingAssistantOffering
<http://purl.imsglobal.org/vocab/lis/v2/membership/Instructor#TeachingAssistantOffering> rdf:type owl:NamedIndividual ,
                                                                                                  <http://purl.imsglobal.org/vocab/lis/v2/membership#TeachingAssistant> ;
                                                                                         rdfs:comment "A teaching assistant for a CourseOffering."@en ;
                                                                                         rdfs:isDefinedBy "http://www.imsglobal.org/lis/"^^xsd:string ;
                                                                                         rdfs:label "TeachingAssistantOffering"@en .


###  http://purl.imsglobal.org/vocab/lis/v2/membership/Instructor#TeachingAssistantSection
<http://purl.imsglobal.org/vocab/lis/v2/membership/Instructor#TeachingAssistantSection> rdf:type owl:NamedIndividual ,
                                                                                                 <http://purl.imsglobal.org/vocab/lis/v2/membership#TeachingAssistant> ;
                                                                                        rdfs:comment "A teaching assistant for a CourseSection."@en ;
                                                                                        rdfs:isDefinedBy "http://www.imsglobal.org/lis/"^^xsd:string ;
                                                                                        rdfs:label "TeachingAssistantSection"@en .


###  http://purl.imsglobal.org/vocab/lis/v2/membership/Instructor#TeachingAssistantTemplate
<http://purl.imsglobal.org/vocab/lis/v2/membership/Instructor#TeachingAssistantTemplate> rdf:type owl:NamedIndividual ,
                                                                                                  <http://purl.imsglobal.org/vocab/lis/v2/membership#TeachingAssistant> ;
                                                                                         rdfs:comment "A teaching assistant for a template."@en ;
                                                                                         rdfs:isDefinedBy "http://www.imsglobal.org/lis/"^^xsd:string ;
                                                                                         rdfs:label "TeachingAssistantTemplate"@en .


###  http://purl.imsglobal.org/vocab/lis/v2/membership/Learner#ExternalLearner
<http://purl.imsglobal.org/vocab/lis/v2/membership/Learner#ExternalLearner> rdf:type owl:NamedIndividual ,
                                                                                     <http://purl.imsglobal.org/vocab/lis/v2/membership#Learner> ;
                                                                            rdfs:comment "A learner who is not a member of the institution."@en ;
                                                                            rdfs:isDefinedBy "http://www.imsglobal.org/lis/"^^xsd:string ;
                                                                            rdfs:label "ExternalLearner"@en .


###  http://purl.imsglobal.org/vocab/lis/v2/membership/Learner#GuestLearner
<http://purl.imsglobal.org/vocab/lis/v2/membership/Learner#GuestLearner> rdf:type owl:NamedIndividual ,
                                                                                  <http://purl.imsglobal.org/vocab/lis/v2/membership#Learner> ;
                                                                         rdfs:comment "A learner who is not enrolled in the same process as a learner; may or may not receive credit for the course."@en ;
                                                                         rdfs:isDefinedBy "http://www.imsglobal.org/lis/"^^xsd:string ;
                                                                         rdfs:label "GuestLearner"@en .


###  http://purl.imsglobal.org/vocab/lis/v2/membership/Learner#Learner
<http://purl.imsglobal.org/vocab/lis/v2/membership/Learner#Learner> rdf:type owl:NamedIndividual ,
                                                                             <http://purl.imsglobal.org/vocab/lis/v2/membership#Learner> ;
                                                                    rdfs:comment "Someone who usually learns within a specific course structure."@en ;
                                                                    rdfs:isDefinedBy "http://www.imsglobal.org/lis/"^^xsd:string ;
                                                                    rdfs:label "Learner"@en .


###  http://purl.imsglobal.org/vocab/lis/v2/membership/Learner#NonCreditLearner
<http://purl.imsglobal.org/vocab/lis/v2/membership/Learner#NonCreditLearner> rdf:type owl:NamedIndividual ,
                                                                                      <http://purl.imsglobal.org/vocab/lis/v2/membership#Learner> ;
                                                                             rdfs:comment "A learner who is enrolled through the same process as a learner, but is not receiving credit for the course of study."@en ;
                                                                             rdfs:isDefinedBy "http://www.imsglobal.org/lis/"^^xsd:string ;
                                                                             rdfs:label "NonCreditLearner"@en .


###  http://purl.imsglobal.org/vocab/lis/v2/membership/Manager#AreaManager
<http://purl.imsglobal.org/vocab/lis/v2/membership/Manager#AreaManager> rdf:type owl:NamedIndividual ,
                                                                                 <http://purl.imsglobal.org/vocab/lis/v2/membership#Manager> ;
                                                                        rdfs:comment "Someone who provides assistance, administration, and/or support to multiple course structures; e.g., Departmental Staff, Cohort Leader, etc."@en ;
                                                                        rdfs:isDefinedBy "http://www.imsglobal.org/lis/"^^xsd:string ;
                                                                        rdfs:label "AreaManager"@en .


###  http://purl.imsglobal.org/vocab/lis/v2/membership/Manager#CourseCoordinator
<http://purl.imsglobal.org/vocab/lis/v2/membership/Manager#CourseCoordinator> rdf:type owl:NamedIndividual ,
                                                                                       <http://purl.imsglobal.org/vocab/lis/v2/membership#Manager> ;
                                                                              rdfs:comment "Someone who provides assistance to a set of course structures that are related, a lab manager, etc."@en ;
                                                                              rdfs:isDefinedBy "http://www.imsglobal.org/lis/"^^xsd:string ;
                                                                              rdfs:label "CourseCoordinator"@en .


###  http://purl.imsglobal.org/vocab/lis/v2/membership/Manager#ExternalObserver
<http://purl.imsglobal.org/vocab/lis/v2/membership/Manager#ExternalObserver> rdf:type owl:NamedIndividual ,
                                                                                      <http://purl.imsglobal.org/vocab/lis/v2/membership#Manager> ;
                                                                             rdfs:comment "Person that is not a member of the institution but views multiple course structures for non-instructional purposes; e.g., peer review committee, accreditation staff, etc."@en ;
                                                                             rdfs:isDefinedBy "http://www.imsglobal.org/lis/"^^xsd:string ;
                                                                             rdfs:label "ExternalObserver"@en .


###  http://purl.imsglobal.org/vocab/lis/v2/membership/Manager#Manager
<http://purl.imsglobal.org/vocab/lis/v2/membership/Manager#Manager> rdf:type owl:NamedIndividual ,
                                                                             <http://purl.imsglobal.org/vocab/lis/v2/membership#Manager> ;
                                                                    rdfs:comment "Someone who usually interacts with multiple course structures."@en ;
                                                                    rdfs:isDefinedBy "http://www.imsglobal.org/lis/"^^xsd:string ;
                                                                    rdfs:label "Manager"@en .


###  http://purl.imsglobal.org/vocab/lis/v2/membership/Manager#Observer
<http://purl.imsglobal.org/vocab/lis/v2/membership/Manager#Observer> rdf:type owl:NamedIndividual ,
                                                                              <http://purl.imsglobal.org/vocab/lis/v2/membership#Manager> ;
                                                                     rdfs:comment "Views multiple course structures for non-instructional purposes; e.g., peer review committee, accreditation staff, etc."@en ;
                                                                     rdfs:isDefinedBy "http://www.imsglobal.org/lis/"^^xsd:string ;
                                                                     rdfs:label "Observer"@en .


###  http://purl.imsglobal.org/vocab/lis/v2/membership/Member#Member
<http://purl.imsglobal.org/vocab/lis/v2/membership/Member#Member> rdf:type owl:NamedIndividual ,
                                                                           <http://purl.imsglobal.org/vocab/lis/v2/membership#Member> ;
                                                                  rdfs:comment "Someone who is a member of an Organization."@en ;
                                                                  rdfs:isDefinedBy "http://www.imsglobal.org/lis/"^^xsd:string ;
                                                                  rdfs:label "Member"@en .


###  http://purl.imsglobal.org/vocab/lis/v2/membership/Mentor#Advisor
<http://purl.imsglobal.org/vocab/lis/v2/membership/Mentor#Advisor> rdf:type owl:NamedIndividual ,
                                                                            <http://purl.imsglobal.org/vocab/lis/v2/membership#Mentor> ;
                                                                   rdfs:comment "Advises learners."@en ;
                                                                   rdfs:isDefinedBy "http://www.imsglobal.org/lis/"^^xsd:string ;
                                                                   rdfs:label "Advisor"@en .


###  http://purl.imsglobal.org/vocab/lis/v2/membership/Mentor#Auditor
<http://purl.imsglobal.org/vocab/lis/v2/membership/Mentor#Auditor> rdf:type owl:NamedIndividual ,
                                                                            <http://purl.imsglobal.org/vocab/lis/v2/membership#Mentor> ;
                                                                   rdfs:comment "Audits learner activities; e.g., staff that verifies continuing eligibility for a scholarship, etc."@en ;
                                                                   rdfs:isDefinedBy "http://www.imsglobal.org/lis/"^^xsd:string ;
                                                                   rdfs:label "Auditor"@en .


###  http://purl.imsglobal.org/vocab/lis/v2/membership/Mentor#ExternalAdvisor
<http://purl.imsglobal.org/vocab/lis/v2/membership/Mentor#ExternalAdvisor> rdf:type owl:NamedIndividual ,
                                                                                    <http://purl.imsglobal.org/vocab/lis/v2/membership#Mentor> ;
                                                                           rdfs:comment "A user who is not a member of the institution that advises learners."@en ;
                                                                           rdfs:isDefinedBy "http://www.imsglobal.org/lis/"^^xsd:string ;
                                                                           rdfs:label "ExternalAdvisor"@en .


###  http://purl.imsglobal.org/vocab/lis/v2/membership/Mentor#ExternalAuditor
<http://purl.imsglobal.org/vocab/lis/v2/membership/Mentor#ExternalAuditor> rdf:type owl:NamedIndividual ,
                                                                                    <http://purl.imsglobal.org/vocab/lis/v2/membership#Mentor> ;
                                                                           rdfs:comment "A user who is not a member of the institution that audits learner activities; e.g., staff that verifies continuing eligibility for a scholarship, etc."@en ;
                                                                           rdfs:isDefinedBy "http://www.imsglobal.org/lis/"^^xsd:string ;
                                                                           rdfs:label "ExternalAuditor"@en .


###  http://purl.imsglobal.org/vocab/lis/v2/membership/Mentor#ExternalLearningFacilitator
<http://purl.imsglobal.org/vocab/lis/v2/membership/Mentor#ExternalLearningFacilitator> rdf:type owl:NamedIndividual ,
                                                                                                <http://purl.imsglobal.org/vocab/lis/v2/membership#Mentor> ;
                                                                                       rdfs:comment "A user who is not a member of the institution that works with individual learner to access materials; e.g., translator, assistant for persons of differing abilities, etc."@en ;
                                                                                       rdfs:isDefinedBy "http://www.imsglobal.org/lis/"^^xsd:string ;
                                                                                       rdfs:label "ExternalLearningFacilitator"@en .


###  http://purl.imsglobal.org/vocab/lis/v2/membership/Mentor#ExternalMentor
<http://purl.imsglobal.org/vocab/lis/v2/membership/Mentor#ExternalMentor> rdf:type owl:NamedIndividual ,
                                                                                   <http://purl.imsglobal.org/vocab/lis/v2/membership#Mentor> ;
                                                                          rdfs:comment "A user who is not a member of the institution that mentors learners."@en ,
                                                                                       "ExternalMentor"@en ;
                                                                          rdfs:isDefinedBy "http://www.imsglobal.org/lis/"^^xsd:string .


###  http://purl.imsglobal.org/vocab/lis/v2/membership/Mentor#ExternalReviewer
<http://purl.imsglobal.org/vocab/lis/v2/membership/Mentor#ExternalReviewer> rdf:type owl:NamedIndividual ,
                                                                                     <http://purl.imsglobal.org/vocab/lis/v2/membership#Mentor> ;
                                                                            rdfs:comment "A user who is not a member of the institution that reviews work by learners."@en ;
                                                                            rdfs:isDefinedBy "http://www.imsglobal.org/lis/"^^xsd:string ;
                                                                            rdfs:label "ExternalReviewer"@en .


###  http://purl.imsglobal.org/vocab/lis/v2/membership/Mentor#ExternalTutor
<http://purl.imsglobal.org/vocab/lis/v2/membership/Mentor#ExternalTutor> rdf:type owl:NamedIndividual ,
                                                                                  <http://purl.imsglobal.org/vocab/lis/v2/membership#Mentor> ;
                                                                         rdfs:comment "A user who is not a member of the institution that works with individual learners to assist in their instruction."@en ;
                                                                         rdfs:isDefinedBy "http://www.imsglobal.org/lis/"^^xsd:string ;
                                                                         rdfs:label "ExternalTutor"@en .


###  http://purl.imsglobal.org/vocab/lis/v2/membership/Mentor#LearningFacilitator
<http://purl.imsglobal.org/vocab/lis/v2/membership/Mentor#LearningFacilitator> rdf:type owl:NamedIndividual ,
                                                                                        <http://purl.imsglobal.org/vocab/lis/v2/membership#Mentor> ;
                                                                               rdfs:comment "Works with individual learner to access materials; e.g., translator, assistant for persons of differing abilities, etc."@en ;
                                                                               rdfs:isDefinedBy "http://www.imsglobal.org/lis/"^^xsd:string ;
                                                                               rdfs:label "LearningFacilitator"@en .


###  http://purl.imsglobal.org/vocab/lis/v2/membership/Mentor#Mentor
<http://purl.imsglobal.org/vocab/lis/v2/membership/Mentor#Mentor> rdf:type owl:NamedIndividual ,
                                                                           <http://purl.imsglobal.org/vocab/lis/v2/membership#Mentor> ;
                                                                  rdfs:comment "Someone who usually works with a specific course structure with a specific learner."@en ;
                                                                  rdfs:isDefinedBy "http://www.imsglobal.org/lis/"^^xsd:string ;
                                                                  rdfs:label "Mentor"@en .


###  http://purl.imsglobal.org/vocab/lis/v2/membership/Mentor#Reviewer
<http://purl.imsglobal.org/vocab/lis/v2/membership/Mentor#Reviewer> rdf:type owl:NamedIndividual ,
                                                                             <http://purl.imsglobal.org/vocab/lis/v2/membership#Mentor> ;
                                                                    rdfs:comment "Reviews work by learners."@en ;
                                                                    rdfs:isDefinedBy "http://www.imsglobal.org/lis/"^^xsd:string ;
                                                                    rdfs:label "Reviewer"@en .


###  http://purl.imsglobal.org/vocab/lis/v2/membership/Mentor#Tutor
<http://purl.imsglobal.org/vocab/lis/v2/membership/Mentor#Tutor> rdf:type owl:NamedIndividual ,
                                                                          <http://purl.imsglobal.org/vocab/lis/v2/membership#Mentor> ;
                                                                 rdfs:comment "Works with individual learners to assist in their instruction."@en ;
                                                                 rdfs:isDefinedBy "http://www.imsglobal.org/lis/"^^xsd:string ;
                                                                 rdfs:label "Tutor"@en .


###  http://purl.imsglobal.org/vocab/lis/v2/membership/Officer#Chair
<http://purl.imsglobal.org/vocab/lis/v2/membership/Officer#Chair> rdf:type owl:NamedIndividual ,
                                                                           <http://purl.imsglobal.org/vocab/lis/v2/membership#Officer> ;
                                                                  rdfs:comment "Chair of the Group."@en ;
                                                                  rdfs:isDefinedBy "http://www.imsglobal.org/lis/"^^xsd:string ;
                                                                  rdfs:label "Chair"@en .


###  http://purl.imsglobal.org/vocab/lis/v2/membership/Officer#Communications
<http://purl.imsglobal.org/vocab/lis/v2/membership/Officer#Communications> rdf:type owl:NamedIndividual ,
                                                                                    <http://purl.imsglobal.org/vocab/lis/v2/membership#Officer> ;
                                                                           rdfs:comment "Communications officer for the Group."@en ;
                                                                           rdfs:isDefinedBy "http://www.imsglobal.org/lis/"^^xsd:string ;
                                                                           rdfs:label "Communications"@en .


###  http://purl.imsglobal.org/vocab/lis/v2/membership/Officer#Officer
<http://purl.imsglobal.org/vocab/lis/v2/membership/Officer#Officer> rdf:type owl:NamedIndividual ,
                                                                             <http://purl.imsglobal.org/vocab/lis/v2/membership#Officer> ;
                                                                    rdfs:comment "The role of an officer of organization e.g., Chair, Secretary, etc. in the Membership."@en ;
                                                                    rdfs:isDefinedBy "http://www.imsglobal.org/lis/"^^xsd:string ;
                                                                    rdfs:label "Officer"@en .


###  http://purl.imsglobal.org/vocab/lis/v2/membership/Officer#Secretary
<http://purl.imsglobal.org/vocab/lis/v2/membership/Officer#Secretary> rdf:type owl:NamedIndividual ,
                                                                               <http://purl.imsglobal.org/vocab/lis/v2/membership#Officer> ;
                                                                      rdfs:comment "Secretary to the Group."@en ;
                                                                      rdfs:isDefinedBy "http://www.imsglobal.org/lis/"^^xsd:string ;
                                                                      rdfs:label "Secretary"@en .


###  http://purl.imsglobal.org/vocab/lis/v2/membership/Officer#Treasurer
<http://purl.imsglobal.org/vocab/lis/v2/membership/Officer#Treasurer> rdf:type owl:NamedIndividual ,
                                                                               <http://purl.imsglobal.org/vocab/lis/v2/membership#Officer> ;
                                                                      rdfs:comment "Treasurer to the Group."@en ;
                                                                      rdfs:isDefinedBy "http://www.imsglobal.org/lis/"^^xsd:string ;
                                                                      rdfs:label "Treasurer"@en .


###  http://purl.imsglobal.org/vocab/lis/v2/membership/Officer#ViceChair
<http://purl.imsglobal.org/vocab/lis/v2/membership/Officer#ViceChair> rdf:type owl:NamedIndividual ,
                                                                               <http://purl.imsglobal.org/vocab/lis/v2/membership#Officer> ;
                                                                      rdfs:comment "Vice Chair to the Group."@en ;
                                                                      rdfs:isDefinedBy "http://www.imsglobal.org/lis/"^^xsd:string ;
                                                                      rdfs:label "ViceChair"@en .


###  http://purl.imsglobal.org/vocab/lis/v2/membership/TeachingAssistant#Grader
<http://purl.imsglobal.org/vocab/lis/v2/membership/TeachingAssistant#Grader> rdf:type owl:NamedIndividual ,
                                                                                      <http://purl.imsglobal.org/vocab/lis/v2/membership#Instructor> ;
                                                                             rdfs:comment "Primary responsibility is assignment of grades."@en ;
                                                                             rdfs:isDefinedBy "http://www.imsglobal.org/lis/"^^xsd:string ;
                                                                             rdfs:label "Grader"@en .


###  http://purl.imsglobal.org/vocab/lis/v2/membership/TeachingAssistant#TeachingAssistantSectionAssociation
<http://purl.imsglobal.org/vocab/lis/v2/membership/TeachingAssistant#TeachingAssistantSectionAssociation> rdf:type owl:NamedIndividual ,
                                                                                                                   <http://purl.imsglobal.org/vocab/lis/v2/membership#TeachingAssistant> ;
                                                                                                          rdfs:comment "A teaching assistant for a section association."@en ;
                                                                                                          rdfs:isDefinedBy "http://www.imsglobal.org/lis/"^^xsd:string ;
                                                                                                          rdfs:label "TeachingAssistantSectionAssociation"@en .


###  http://purl.imsglobal.org/vocab/lis/v2/status#Active
<http://purl.imsglobal.org/vocab/lis/v2/status#Active> rdf:type owl:NamedIndividual ,
                                                                :Status ;
                                                       rdfs:comment "The member is active in the Membership."@en ;
                                                       rdfs:isDefinedBy "http://www.imsglobal.org/lis/"^^xsd:string ;
                                                       rdfs:label "Active"@en .


###  http://purl.imsglobal.org/vocab/lis/v2/status#Inactive
<http://purl.imsglobal.org/vocab/lis/v2/status#Inactive> rdf:type owl:NamedIndividual ,
                                                                  :Status ;
                                                         rdfs:comment "The member is inactive in the Membership."@en ;
                                                         rdfs:isDefinedBy "http://www.imsglobal.org/lis/"^^xsd:string ;
                                                         rdfs:label "Inactive"@en .


#################################################################
#    General axioms
#################################################################

[ rdf:type owl:AllDisjointClasses ;
  owl:members ( :Action
                :Entity
                :Envelope
                :Event
                :Role
                :Selector
                :Status
              )
] .


[ rdf:type owl:AllDisjointClasses ;
  owl:members ( :Agent
                :AggregateMeasure
                :Annotation
                :Attempt
                :Collection
                :Comment
                :LearningObjective
                :Link
                :Membership
                :Query
                :Rating
                :Response
                :Result
                :Scale
                :Score
                :SearchResponse
                :Session
              )
] .


[ rdf:type owl:AllDisjointClasses ;
  owl:members ( :Agent
                :Annotation
                :Attempt
                :Comment
                :DigitalResource
                :LearningObjective
                :Link
                :Membership
                :Query
                :Rating
                :Response
                :Result
                :Scale
                :Score
                :SearchResponse
                :Session
              )
] .


[ rdf:type owl:AllDisjointClasses ;
  owl:members ( :Agent
                :Annotation
                :Attempt
                :DigitalResource
                :LearningObjective
                :Link
                :Membership
                :Query
                :Response
                :Result
                :Score
                :SearchResponse
                :Session
              )
] .


[ rdf:type owl:AllDisjointClasses ;
  owl:members ( :Agent
                :Annotation
                :Attempt
                :DigitalResource
                :LearningObjective
                :Membership
                :Query
                :Response
                :Result
                :Score
                :SearchResponse
                :Session
              )
] .


[ rdf:type owl:AllDisjointClasses ;
  owl:members ( :AnnotationEvent
                :AssessmentEvent
                :AssessmentItemEvent
                :AssignableEvent
                :FeedbackEvent
                :ForumEvent
                :GradeEvent
                :MediaEvent
                :MessageEvent
                :NavigationEvent
                :OutcomeEvent
                :ReadingEvent
                :ResourceManagementEvent
                :SearchEvent
                :SessionEvent
                :ThreadEvent
                :ToolLaunchEvent
                :ToolUseEvent
                :ViewEvent
              )
] .


[ rdf:type owl:AllDisjointClasses ;
  owl:members ( :AssignableDigitalResource
                :Chapter
                :Document
                :Frame
                :LtiLink
                :MediaLocation
                :MediaObject
                :Message
                :Page
                :WebPage
              )
] .


[ rdf:type owl:AllDisjointClasses ;
  owl:members ( :AudioObject
                :ImageObject
                :VideoObject
              )
] .


[ rdf:type owl:AllDisjointClasses ;
  owl:members ( :BookmarkAnnotation
                :HighlightAnnotation
                :SharedAnnotation
                :TagAnnotation
              )
] .


[ rdf:type owl:AllDisjointClasses ;
  owl:members ( :FillinBlankResponse
                :MultipleChoiceResponse
                :MultipleResponseResponse
                :SelectTextResponse
                :TrueFalseResponse
              )
] .


[ rdf:type owl:AllDisjointClasses ;
  owl:members ( :LikertScale
                :MultiSelectScale
                :NumericScale
              )
] .


[ rdf:type owl:AllDisjointClasses ;
  owl:members ( :Organization
                :Person
                :SoftwareApplication
              )
] .


[ rdf:type owl:AllDisjointClasses ;
  owl:members ( <http://purl.imsglobal.org/vocab/lis/v2/membership#Administrator>
                <http://purl.imsglobal.org/vocab/lis/v2/membership#ContentDeveloper>
                <http://purl.imsglobal.org/vocab/lis/v2/membership#Instructor>
                <http://purl.imsglobal.org/vocab/lis/v2/membership#Learner>
                <http://purl.imsglobal.org/vocab/lis/v2/membership#Manager>
                <http://purl.imsglobal.org/vocab/lis/v2/membership#Member>
                <http://purl.imsglobal.org/vocab/lis/v2/membership#Mentor>
                <http://purl.imsglobal.org/vocab/lis/v2/membership#Officer>
              )
] .


[ rdf:type owl:AllDifferent ;
  owl:distinctMembers ( <http://purl.imsglobal.org/actions/Archived>
                        <http://purl.imsglobal.org/actions/Copied>
                        <http://purl.imsglobal.org/actions/Launched>
                        <http://purl.imsglobal.org/actions/Published>
                        <http://purl.imsglobal.org/actions/Restored>
                        <http://purl.imsglobal.org/actions/Returned>
                        <http://purl.imsglobal.org/actions/Unpublished>
                        <http://purl.imsglobal.org/caliper/actions/Abandoned>
                        <http://purl.imsglobal.org/caliper/actions/Activated>
                        <http://purl.imsglobal.org/caliper/actions/Added>
                        <http://purl.imsglobal.org/caliper/actions/Attached>
                        <http://purl.imsglobal.org/caliper/actions/Bookmarked>
                        <http://purl.imsglobal.org/caliper/actions/ChangedResolution>
                        <http://purl.imsglobal.org/caliper/actions/ChangedSize>
                        <http://purl.imsglobal.org/caliper/actions/ChangedSpeed>
                        <http://purl.imsglobal.org/caliper/actions/ChangedVolume>
                        <http://purl.imsglobal.org/caliper/actions/Classified>
                        <http://purl.imsglobal.org/caliper/actions/ClosedPopout>
                        <http://purl.imsglobal.org/caliper/actions/Commented>
                        <http://purl.imsglobal.org/caliper/actions/Completed>
                        <http://purl.imsglobal.org/caliper/actions/Copied>
                        <http://purl.imsglobal.org/caliper/actions/Created>
                        <http://purl.imsglobal.org/caliper/actions/Deactivated>
                        <http://purl.imsglobal.org/caliper/actions/Deleted>
                        <http://purl.imsglobal.org/caliper/actions/Described>
                        <http://purl.imsglobal.org/caliper/actions/DisabledClosedCaptioning>
                        <http://purl.imsglobal.org/caliper/actions/Disliked>
                        <http://purl.imsglobal.org/caliper/actions/Downloaded>
                        <http://purl.imsglobal.org/caliper/actions/EnabledClosedCaptioning>
                        <http://purl.imsglobal.org/caliper/actions/Ended>
                        <http://purl.imsglobal.org/caliper/actions/EnteredFullScreen>
                        <http://purl.imsglobal.org/caliper/actions/ExitedFullScreen>
                        <http://purl.imsglobal.org/caliper/actions/ForwardedTo>
                        <http://purl.imsglobal.org/caliper/actions/Graded>
                        <http://purl.imsglobal.org/caliper/actions/Hid>
                        <http://purl.imsglobal.org/caliper/actions/Highlighted>
                        <http://purl.imsglobal.org/caliper/actions/Identified>
                        <http://purl.imsglobal.org/caliper/actions/JumpedTo>
                        <http://purl.imsglobal.org/caliper/actions/Liked>
                        <http://purl.imsglobal.org/caliper/actions/Linked>
                        <http://purl.imsglobal.org/caliper/actions/LoggedIn>
                        <http://purl.imsglobal.org/caliper/actions/LoggedOut>
                        <http://purl.imsglobal.org/caliper/actions/MarkedAsRead>
                        <http://purl.imsglobal.org/caliper/actions/MarkedAsUnread>
                        <http://purl.imsglobal.org/caliper/actions/Modified>
                        <http://purl.imsglobal.org/caliper/actions/Muted>
                        <http://purl.imsglobal.org/caliper/actions/NavigatedTo>
                        <http://purl.imsglobal.org/caliper/actions/OpenedPopout>
                        <http://purl.imsglobal.org/caliper/actions/Paused>
                        <http://purl.imsglobal.org/caliper/actions/Posted>
                        <http://purl.imsglobal.org/caliper/actions/Printed>
                        <http://purl.imsglobal.org/caliper/actions/Published>
                        <http://purl.imsglobal.org/caliper/actions/Questioned>
                        <http://purl.imsglobal.org/caliper/actions/Ranked>
                        <http://purl.imsglobal.org/caliper/actions/Recommended>
                        <http://purl.imsglobal.org/caliper/actions/Removed>
                        <http://purl.imsglobal.org/caliper/actions/Reset>
                        <http://purl.imsglobal.org/caliper/actions/Restarted>
                        <http://purl.imsglobal.org/caliper/actions/Restored>
                        <http://purl.imsglobal.org/caliper/actions/Resumed>
                        <http://purl.imsglobal.org/caliper/actions/Retrieved>
                        <http://purl.imsglobal.org/caliper/actions/Reviewed>
                        <http://purl.imsglobal.org/caliper/actions/Rewound>
                        <http://purl.imsglobal.org/caliper/actions/Saved>
                        <http://purl.imsglobal.org/caliper/actions/Searched>
                        <http://purl.imsglobal.org/caliper/actions/Shared>
                        <http://purl.imsglobal.org/caliper/actions/Showed>
                        <http://purl.imsglobal.org/caliper/actions/Skipped>
                        <http://purl.imsglobal.org/caliper/actions/Started>
                        <http://purl.imsglobal.org/caliper/actions/Submitted>
                        <http://purl.imsglobal.org/caliper/actions/Subscribed>
                        <http://purl.imsglobal.org/caliper/actions/Tagged>
                        <http://purl.imsglobal.org/caliper/actions/TimedOut>
                        <http://purl.imsglobal.org/caliper/actions/Unmuted>
                        <http://purl.imsglobal.org/caliper/actions/Unpublished>
                        <http://purl.imsglobal.org/caliper/actions/Unsubscribed>
                        <http://purl.imsglobal.org/caliper/actions/Uploaded>
                        <http://purl.imsglobal.org/caliper/actions/Used>
                        <http://purl.imsglobal.org/caliper/actions/Viewed>
                      )
] .


[ rdf:type owl:AllDifferent ;
  owl:distinctMembers ( <http://purl.imsglobal.org/caliper/lti/LtiDeepLinkingRequest>
                        <http://purl.imsglobal.org/caliper/lti/LtiResourceLinkRequest>
                      )
] .


[ rdf:type owl:AllDifferent ;
  owl:distinctMembers ( <http://purl.imsglobal.org/caliper/metrics/AssessmentsPassed>
                        <http://purl.imsglobal.org/caliper/metrics/AssessmentsSubmitted>
                        <http://purl.imsglobal.org/caliper/metrics/MinutesOnTask>
                        <http://purl.imsglobal.org/caliper/metrics/SkillsMastered>
                        <http://purl.imsglobal.org/caliper/metrics/StandardsMastered>
                        <http://purl.imsglobal.org/caliper/metrics/UnitsCompleted>
                        <http://purl.imsglobal.org/caliper/metrics/UnitsPassed>
                        <http://purl.imsglobal.org/caliper/metrics/WordsRead>
                      )
] .


###  Generated by the OWL API (version 4.5.9.2019-02-01T07:24:44Z) https://github.com/owlcs/owlapi
