<?xml version="1.0"?>
<rdf:RDF xmlns="http://purl.imsglobal.org/caliper/"
     xml:base="http://purl.imsglobal.org/caliper/"
     xmlns:owl="http://www.w3.org/2002/07/owl#"
     xmlns:rdf="http://www.w3.org/1999/02/22-rdf-syntax-ns#"
     xmlns:xml="http://www.w3.org/XML/1998/namespace"
     xmlns:xsd="http://www.w3.org/2001/XMLSchema#"
     xmlns:rdfs="http://www.w3.org/2000/01/rdf-schema#"
     xmlns:terms="http://purl.org/dc/terms/">
    <owl:Ontology rdf:about="http://purl.imsglobal.org/caliper/">
        <terms:license xml:lang="en">Recipients of this document are requested to submit, with their comments, notification of any relevant patent claims or other intellectual property rights of which they may be aware that might be infringed by any implementation of the specification set forth in this document, and to provide supporting documentation.

IMS takes no position regarding the validity or scope of any intellectual property or other rights that might be claimed to pertain to the implementation or use of the technology described in this document or the extent to which any license under such rights might or might not be available; neither does it represent that it has made any effort to identify any such rights. Information on IMS’s procedures with respect to rights in IMS specifications can be found at the IMS Intellectual Property Rights web page: http://www.imsglobal.org/ipr/imsipr_policyFinal.pdf.

Copyright © 2018 IMS Global Learning Consortium. All Rights Reserved.

Use of this ontology to develop products or services is governed by the license with IMS found on the IMS website: http://www.imsglobal.org/speclicense.html.

Permission is granted to all parties to use excerpts from this document as needed in producing requests for proposals.

The limited permissions granted above are perpetual and will not be revoked by IMS or its successors or assigns.

THIS ONTOLOGY IS BEING OFFERED WITHOUT ANY WARRANTY WHATSOEVER, AND IN PARTICULAR, ANY WARRANTY OF NON INFRINGEMENT IS EXPRESSLY DISCLAIMED. ANY USE OF THIS ONTOLOGY SHALL BE MADE ENTIRELY AT THE IMPLEMENTER&apos;S OWN RISK, AND NEITHER THE CONSORTIUM, NOR ANY OF ITS MEMBERS OR SUBMITTERS, SHALL HAVE ANY LIABILITY WHATSOEVER TO ANY IMPLEMENTER OR THIRD PARTY FOR ANY DAMAGES OF ANY NATURE WHATSOEVER, DIRECTLY OR INDIRECTLY, ARISING FROM THE USE OF THIS ONTOLOGY.</terms:license>
        <terms:title xml:lang="en">Caliper Analytics® Ontology</terms:title>
        <rdfs:comment xml:lang="en">The Caliper Analytics Specification provides a structured approach to describing, collecting and exchanging learning activity data at scale.  Establishing a common vocabulary for describing learning interactions is a central objective.  Promoting data interoperability, data sharing and data-informed decision making are also important goals.

Caliper also defines an application programming interface (the Sensor API) for marshalling and transmitting event data from instrumented applications to target endpoints for storage, analysis and use.

The Caliper ontology provides a machine-readable document that defines the concepts, relationships and constraints that together comprise the Caliper information model.</rdfs:comment>
        <rdfs:label xml:lang="en">Caliper Analytics® Ontology</rdfs:label>
        <rdfs:seeAlso rdf:datatype="http://www.w3.org/2001/XMLSchema#string">http://www.imsglobal.org/caliper</rdfs:seeAlso>
    </owl:Ontology>
    


    <!-- 
    ///////////////////////////////////////////////////////////////////////////////////////
    //
    // Annotation properties
    //
    ///////////////////////////////////////////////////////////////////////////////////////
     -->

    


    <!-- http://purl.org/dc/terms/isReplacedBy -->

    <owl:AnnotationProperty rdf:about="http://purl.org/dc/terms/isReplacedBy"/>
    


    <!-- http://purl.org/dc/terms/license -->

    <owl:AnnotationProperty rdf:about="http://purl.org/dc/terms/license"/>
    


    <!-- http://purl.org/dc/terms/title -->

    <owl:AnnotationProperty rdf:about="http://purl.org/dc/terms/title"/>
    


    <!-- http://www.w3.org/2002/07/owl#equivalentClass -->

    <owl:AnnotationProperty rdf:about="http://www.w3.org/2002/07/owl#equivalentClass"/>
    


    <!-- http://www.w3.org/2002/07/owl#equivalentProperty -->

    <owl:AnnotationProperty rdf:about="http://www.w3.org/2002/07/owl#equivalentProperty"/>
    


    <!-- 
    ///////////////////////////////////////////////////////////////////////////////////////
    //
    // Datatypes
    //
    ///////////////////////////////////////////////////////////////////////////////////////
     -->

    


    <!-- http://www.w3.org/2001/XMLSchema#duration -->

    <rdfs:Datatype rdf:about="http://www.w3.org/2001/XMLSchema#duration"/>
    


    <!-- 
    ///////////////////////////////////////////////////////////////////////////////////////
    //
    // Object Properties
    //
    ///////////////////////////////////////////////////////////////////////////////////////
     -->

    


    <!-- http://purl.imsglobal.org/caliper/action -->

    <owl:ObjectProperty rdf:about="http://purl.imsglobal.org/caliper/action">
        <rdf:type rdf:resource="http://www.w3.org/2002/07/owl#FunctionalProperty"/>
        <rdfs:domain rdf:resource="http://purl.imsglobal.org/caliper/Event"/>
        <rdfs:range rdf:resource="http://purl.imsglobal.org/caliper/Action"/>
        <rdfs:comment xml:lang="en">The action or predicate that binds the Event actor or subject to the Event object.</rdfs:comment>
        <rdfs:isDefinedBy rdf:datatype="http://www.w3.org/2001/XMLSchema#string">http://purl.imsglobal.org/caliper</rdfs:isDefinedBy>
        <rdfs:label xml:lang="en">action</rdfs:label>
    </owl:ObjectProperty>
    


    <!-- http://purl.imsglobal.org/caliper/actor -->

    <owl:ObjectProperty rdf:about="http://purl.imsglobal.org/caliper/actor">
        <rdf:type rdf:resource="http://www.w3.org/2002/07/owl#FunctionalProperty"/>
        <rdfs:domain rdf:resource="http://purl.imsglobal.org/caliper/Event"/>
        <rdfs:range rdf:resource="http://purl.imsglobal.org/caliper/Agent"/>
        <rdfs:comment xml:lang="en">The Agent who initiated the Event, typically a Person, Organization or SoftwareApplication.</rdfs:comment>
        <rdfs:isDefinedBy rdf:datatype="http://www.w3.org/2001/XMLSchema#string">http://purl.imsglobal.org/caliper</rdfs:isDefinedBy>
        <rdfs:label xml:lang="en">actor</rdfs:label>
    </owl:ObjectProperty>
    


    <!-- http://purl.imsglobal.org/caliper/alignedLearningObjective -->

    <owl:ObjectProperty rdf:about="http://purl.imsglobal.org/caliper/alignedLearningObjective">
        <rdfs:domain rdf:resource="http://purl.imsglobal.org/caliper/DigitalResource"/>
        <rdfs:range rdf:resource="http://purl.imsglobal.org/caliper/LearningObjective"/>
        <terms:isReplacedBy rdf:resource="http://purl.imsglobal.org/caliper/learningObjectives"/>
        <rdfs:comment xml:lang="en">An ordered collection of one or more LearningObjective entities that describe what a learner is expected to comprehend or accomplish after engaging with the resource.  Deprecated.  Use learningObjectives.</rdfs:comment>
        <rdfs:isDefinedBy rdf:datatype="http://www.w3.org/2001/XMLSchema#string">http://purl.imsglobal.org/caliper</rdfs:isDefinedBy>
        <rdfs:label xml:lang="en">alignedLearningObjective</rdfs:label>
        <owl:deprecated rdf:datatype="http://www.w3.org/2001/XMLSchema#boolean">true</owl:deprecated>
    </owl:ObjectProperty>
    


    <!-- http://purl.imsglobal.org/caliper/annotated -->

    <owl:ObjectProperty rdf:about="http://purl.imsglobal.org/caliper/annotated">
        <rdf:type rdf:resource="http://www.w3.org/2002/07/owl#FunctionalProperty"/>
        <rdfs:domain rdf:resource="http://purl.imsglobal.org/caliper/Annotation"/>
        <rdfs:range rdf:resource="http://purl.imsglobal.org/caliper/DigitalResource"/>
        <rdfs:comment xml:lang="en">The DigitalResource that was annotated by the annotator.</rdfs:comment>
        <rdfs:isDefinedBy rdf:datatype="http://www.w3.org/2001/XMLSchema#string">http://purl.imsglobal.org/caliper</rdfs:isDefinedBy>
        <rdfs:label xml:lang="en">annotated</rdfs:label>
    </owl:ObjectProperty>
    


    <!-- http://purl.imsglobal.org/caliper/annotator -->

    <owl:ObjectProperty rdf:about="http://purl.imsglobal.org/caliper/annotator">
        <rdf:type rdf:resource="http://www.w3.org/2002/07/owl#FunctionalProperty"/>
        <rdfs:domain rdf:resource="http://purl.imsglobal.org/caliper/Annotation"/>
        <rdfs:range rdf:resource="http://purl.imsglobal.org/caliper/Agent"/>
        <rdfs:comment xml:lang="en">The Person who created the Annotation.</rdfs:comment>
        <rdfs:isDefinedBy rdf:datatype="http://www.w3.org/2001/XMLSchema#string">http://purl.imsglobal.org/caliper</rdfs:isDefinedBy>
        <rdfs:label xml:lang="en">annotator</rdfs:label>
    </owl:ObjectProperty>
    


    <!-- http://purl.imsglobal.org/caliper/assignable -->

    <owl:ObjectProperty rdf:about="http://purl.imsglobal.org/caliper/assignable">
        <rdf:type rdf:resource="http://www.w3.org/2002/07/owl#FunctionalProperty"/>
        <rdfs:domain rdf:resource="http://purl.imsglobal.org/caliper/Attempt"/>
        <rdfs:range rdf:resource="http://purl.imsglobal.org/caliper/DigitalResource"/>
        <rdfs:comment xml:lang="en">The DigitalResource that constitutes the object of the assignment.</rdfs:comment>
        <rdfs:isDefinedBy rdf:datatype="http://www.w3.org/2001/XMLSchema#string">http://purl.imsglobal.org/caliper</rdfs:isDefinedBy>
        <rdfs:label xml:lang="en">assignable</rdfs:label>
    </owl:ObjectProperty>
    


    <!-- http://purl.imsglobal.org/caliper/assignee -->

    <owl:ObjectProperty rdf:about="http://purl.imsglobal.org/caliper/assignee">
        <rdf:type rdf:resource="http://www.w3.org/2002/07/owl#FunctionalProperty"/>
        <rdfs:domain rdf:resource="http://purl.imsglobal.org/caliper/Attempt"/>
        <rdfs:range rdf:resource="http://purl.imsglobal.org/caliper/Agent"/>
        <rdfs:comment xml:lang="en">The Person who initiated the Attempt of an assigned DigitalResource.</rdfs:comment>
        <rdfs:isDefinedBy rdf:datatype="http://www.w3.org/2001/XMLSchema#string">http://purl.imsglobal.org/caliper</rdfs:isDefinedBy>
        <rdfs:label xml:lang="en">assignee</rdfs:label>
    </owl:ObjectProperty>
    


    <!-- http://purl.imsglobal.org/caliper/attachments -->

    <owl:ObjectProperty rdf:about="http://purl.imsglobal.org/caliper/attachments">
        <rdfs:domain rdf:resource="http://purl.imsglobal.org/caliper/Message"/>
        <rdfs:range rdf:resource="http://purl.imsglobal.org/caliper/DigitalResource"/>
        <rdfs:comment xml:lang="en">An ordered collection of one or more DigitalResource entities attached to a Message.</rdfs:comment>
        <rdfs:isDefinedBy rdf:datatype="http://www.w3.org/2001/XMLSchema#string">http://purl.imsglobal.org/caliper</rdfs:isDefinedBy>
        <rdfs:label xml:lang="en">attachments</rdfs:label>
    </owl:ObjectProperty>
    


    <!-- http://purl.imsglobal.org/caliper/attempt -->

    <owl:ObjectProperty rdf:about="http://purl.imsglobal.org/caliper/attempt">
        <rdf:type rdf:resource="http://www.w3.org/2002/07/owl#FunctionalProperty"/>
        <rdfs:domain>
            <owl:Class>
                <owl:unionOf rdf:parseType="Collection">
                    <rdf:Description rdf:about="http://purl.imsglobal.org/caliper/Response"/>
                    <rdf:Description rdf:about="http://purl.imsglobal.org/caliper/Result"/>
                    <rdf:Description rdf:about="http://purl.imsglobal.org/caliper/Score"/>
                </owl:unionOf>
            </owl:Class>
        </rdfs:domain>
        <rdfs:range rdf:resource="http://purl.imsglobal.org/caliper/Attempt"/>
        <rdfs:comment xml:lang="en">The associated Attempt.</rdfs:comment>
        <rdfs:isDefinedBy rdf:datatype="http://www.w3.org/2001/XMLSchema#string">http://purl.imsglobal.org/caliper</rdfs:isDefinedBy>
        <rdfs:label xml:lang="en">attempt</rdfs:label>
    </owl:ObjectProperty>
    


    <!-- http://purl.imsglobal.org/caliper/commentedOn -->

    <owl:ObjectProperty rdf:about="http://purl.imsglobal.org/caliper/commentedOn">
        <rdf:type rdf:resource="http://www.w3.org/2002/07/owl#FunctionalProperty"/>
        <rdfs:domain rdf:resource="http://purl.imsglobal.org/caliper/Comment"/>
        <rdfs:range rdf:resource="http://purl.imsglobal.org/caliper/Entity"/>
        <rdfs:comment xml:lang="en">The Entity which received the comment.</rdfs:comment>
        <rdfs:isDefinedBy xml:lang="en">https://purl.imsglobal.org/caliper</rdfs:isDefinedBy>
        <rdfs:label xml:lang="en">commentedOn</rdfs:label>
    </owl:ObjectProperty>
    


    <!-- http://purl.imsglobal.org/caliper/commenter -->

    <owl:ObjectProperty rdf:about="http://purl.imsglobal.org/caliper/commenter">
        <rdf:type rdf:resource="http://www.w3.org/2002/07/owl#FunctionalProperty"/>
        <rdfs:domain rdf:resource="http://purl.imsglobal.org/caliper/Comment"/>
        <rdfs:range rdf:resource="http://purl.imsglobal.org/caliper/Person"/>
        <rdfs:comment xml:lang="en">The Person who provided the comment.</rdfs:comment>
        <rdfs:isDefinedBy rdf:datatype="http://www.w3.org/2001/XMLSchema#string">https://purl.imsglobal.org/caliper</rdfs:isDefinedBy>
    </owl:ObjectProperty>
    


    <!-- http://purl.imsglobal.org/caliper/creator -->

    <owl:ObjectProperty rdf:about="http://purl.imsglobal.org/caliper/creator">
        <rdf:type rdf:resource="http://www.w3.org/2002/07/owl#FunctionalProperty"/>
        <rdfs:domain rdf:resource="http://purl.imsglobal.org/caliper/Query"/>
        <rdfs:range rdf:resource="http://purl.imsglobal.org/caliper/Person"/>
        <rdfs:comment xml:lang="en">The Person who authored, devised or otherwise brought into being a resource.</rdfs:comment>
        <rdfs:isDefinedBy rdf:datatype="http://www.w3.org/2001/XMLSchema#string">http://purl.imsglobal.org/caliper</rdfs:isDefinedBy>
        <rdfs:label xml:lang="en">creator</rdfs:label>
    </owl:ObjectProperty>
    


    <!-- http://purl.imsglobal.org/caliper/creators -->

    <owl:ObjectProperty rdf:about="http://purl.imsglobal.org/caliper/creators">
        <rdfs:domain rdf:resource="http://purl.imsglobal.org/caliper/DigitalResource"/>
        <rdfs:range rdf:resource="http://purl.imsglobal.org/caliper/Agent"/>
        <rdfs:comment xml:lang="en">An ordered collection of Agent entities, typically of type Person, that are responsible for bringing resource into being</rdfs:comment>
        <rdfs:isDefinedBy rdf:datatype="http://www.w3.org/2001/XMLSchema#string">http://purl.imsglobal.org/caliper</rdfs:isDefinedBy>
        <rdfs:label xml:lang="en">creators</rdfs:label>
    </owl:ObjectProperty>
    


    <!-- http://purl.imsglobal.org/caliper/data -->

    <owl:ObjectProperty rdf:about="http://purl.imsglobal.org/caliper/data">
        <rdfs:domain rdf:resource="http://purl.imsglobal.org/caliper/Envelope"/>
        <rdfs:range>
            <owl:Class>
                <owl:unionOf rdf:parseType="Collection">
                    <rdf:Description rdf:about="http://purl.imsglobal.org/caliper/Entity"/>
                    <rdf:Description rdf:about="http://purl.imsglobal.org/caliper/Event"/>
                </owl:unionOf>
            </owl:Class>
        </rdfs:range>
        <rdfs:comment xml:lang="en">Envelope data array.</rdfs:comment>
        <rdfs:isDefinedBy rdf:datatype="http://www.w3.org/2001/XMLSchema#string">http://purl.imsglobal.org/caliper</rdfs:isDefinedBy>
        <rdfs:label xml:lang="en">data</rdfs:label>
    </owl:ObjectProperty>
    


    <!-- http://purl.imsglobal.org/caliper/edApp -->

    <owl:ObjectProperty rdf:about="http://purl.imsglobal.org/caliper/edApp">
        <rdf:type rdf:resource="http://www.w3.org/2002/07/owl#FunctionalProperty"/>
        <rdfs:domain rdf:resource="http://purl.imsglobal.org/caliper/Event"/>
        <rdfs:range rdf:resource="http://purl.imsglobal.org/caliper/SoftwareApplication"/>
        <rdfs:comment xml:lang="en">A SoftwareApplication that represents the application context within which an Event occurs.</rdfs:comment>
        <rdfs:isDefinedBy rdf:datatype="http://www.w3.org/2001/XMLSchema#string">http://purl.imsglobal.org/caliper</rdfs:isDefinedBy>
        <rdfs:label xml:lang="en">edApp</rdfs:label>
    </owl:ObjectProperty>
    


    <!-- http://purl.imsglobal.org/caliper/extensions -->

    <owl:ObjectProperty rdf:about="http://purl.imsglobal.org/caliper/extensions">
        <rdfs:domain>
            <owl:Class>
                <owl:unionOf rdf:parseType="Collection">
                    <rdf:Description rdf:about="http://purl.imsglobal.org/caliper/Entity"/>
                    <rdf:Description rdf:about="http://purl.imsglobal.org/caliper/Event"/>
                </owl:unionOf>
            </owl:Class>
        </rdfs:domain>
        <rdfs:comment xml:lang="en">An ordered collection of objects not defined by the Caliper Information Model.</rdfs:comment>
        <rdfs:isDefinedBy rdf:datatype="http://www.w3.org/2001/XMLSchema#string">http://purl.imsglobal.org/caliper</rdfs:isDefinedBy>
        <rdfs:label xml:lang="en">extensions</rdfs:label>
    </owl:ObjectProperty>
    


    <!-- http://purl.imsglobal.org/caliper/federatedSession -->

    <owl:ObjectProperty rdf:about="http://purl.imsglobal.org/caliper/federatedSession">
        <rdf:type rdf:resource="http://www.w3.org/2002/07/owl#FunctionalProperty"/>
        <rdfs:domain rdf:resource="http://purl.imsglobal.org/caliper/Event"/>
        <rdfs:range rdf:resource="http://purl.imsglobal.org/caliper/LtiSession"/>
        <rdfs:comment xml:lang="en">If an Event occurs within the context of an LTI tool launch, the federatedSession constitutes the tool consumer&apos;s LtiSession.</rdfs:comment>
        <rdfs:isDefinedBy rdf:datatype="http://www.w3.org/2001/XMLSchema#string">http://purl.imsglobal.org/caliper</rdfs:isDefinedBy>
        <rdfs:label xml:lang="en">federatedSession</rdfs:label>
    </owl:ObjectProperty>
    


    <!-- http://purl.imsglobal.org/caliper/generated -->

    <owl:ObjectProperty rdf:about="http://purl.imsglobal.org/caliper/generated">
        <rdf:type rdf:resource="http://www.w3.org/2002/07/owl#FunctionalProperty"/>
        <rdfs:domain rdf:resource="http://purl.imsglobal.org/caliper/Event"/>
        <rdfs:range rdf:resource="http://purl.imsglobal.org/caliper/Entity"/>
        <rdfs:comment xml:lang="en">An Entity created or generated as a result of an interaction between an actor and an object.</rdfs:comment>
        <rdfs:isDefinedBy rdf:datatype="http://www.w3.org/2001/XMLSchema#string">http://purl.imsglobal.org/caliper</rdfs:isDefinedBy>
        <rdfs:label xml:lang="en">generated</rdfs:label>
    </owl:ObjectProperty>
    


    <!-- http://purl.imsglobal.org/caliper/group -->

    <owl:ObjectProperty rdf:about="http://purl.imsglobal.org/caliper/group">
        <rdf:type rdf:resource="http://www.w3.org/2002/07/owl#FunctionalProperty"/>
        <rdfs:domain rdf:resource="http://purl.imsglobal.org/caliper/Event"/>
        <rdfs:range rdf:resource="http://purl.imsglobal.org/caliper/Organization"/>
        <rdfs:comment xml:lang="en">An Organization that represents the group or organizational context within which an Event occurs.</rdfs:comment>
        <rdfs:isDefinedBy rdf:datatype="http://www.w3.org/2001/XMLSchema#string">http://purl.imsglobal.org/caliper</rdfs:isDefinedBy>
        <rdfs:label xml:lang="en">group</rdfs:label>
    </owl:ObjectProperty>
    


    <!-- http://purl.imsglobal.org/caliper/isPartOf -->

    <owl:ObjectProperty rdf:about="http://purl.imsglobal.org/caliper/isPartOf">
        <rdf:type rdf:resource="http://www.w3.org/2002/07/owl#FunctionalProperty"/>
        <rdfs:domain rdf:resource="http://purl.imsglobal.org/caliper/Entity"/>
        <rdfs:range rdf:resource="http://purl.imsglobal.org/caliper/Entity"/>
        <rdfs:comment xml:lang="en">A related Entity that includes or incorporates the resource as a part of its whole.</rdfs:comment>
        <rdfs:isDefinedBy rdf:datatype="http://www.w3.org/2001/XMLSchema#string">http://purl.imsglobal.org/caliper</rdfs:isDefinedBy>
        <rdfs:label xml:lang="en">isPartOf</rdfs:label>
    </owl:ObjectProperty>
    


    <!-- http://purl.imsglobal.org/caliper/itemLabels -->

    <owl:ObjectProperty rdf:about="http://purl.imsglobal.org/caliper/itemLabels">
        <rdfs:domain>
            <owl:Class>
                <owl:unionOf rdf:parseType="Collection">
                    <rdf:Description rdf:about="http://purl.imsglobal.org/caliper/LikertScale"/>
                    <rdf:Description rdf:about="http://purl.imsglobal.org/caliper/MultiSelectScale"/>
                </owl:unionOf>
            </owl:Class>
        </rdfs:domain>
        <rdfs:comment xml:lang="en">The ordered list of labels for each point on the Likert scale.</rdfs:comment>
        <rdfs:isDefinedBy rdf:datatype="http://www.w3.org/2001/XMLSchema#string">https://purl.imsglobal.org/caliper</rdfs:isDefinedBy>
        <rdfs:label xml:lang="en">itemLabels</rdfs:label>
    </owl:ObjectProperty>
    


    <!-- http://purl.imsglobal.org/caliper/itemValues -->

    <owl:ObjectProperty rdf:about="http://purl.imsglobal.org/caliper/itemValues">
        <rdfs:domain>
            <owl:Class>
                <owl:unionOf rdf:parseType="Collection">
                    <rdf:Description rdf:about="http://purl.imsglobal.org/caliper/LikertScale"/>
                    <rdf:Description rdf:about="http://purl.imsglobal.org/caliper/MultiSelectScale"/>
                </owl:unionOf>
            </owl:Class>
        </rdfs:domain>
        <rdfs:comment xml:lang="en">The ordered list of values for each point on the Likert scale.</rdfs:comment>
        <rdfs:isDefinedBy rdf:datatype="http://www.w3.org/2001/XMLSchema#string">https://purl.imsglobal.org/caliper</rdfs:isDefinedBy>
        <rdfs:label xml:lang="en">itemValues</rdfs:label>
    </owl:ObjectProperty>
    


    <!-- http://purl.imsglobal.org/caliper/items -->

    <owl:ObjectProperty rdf:about="http://purl.imsglobal.org/caliper/items">
        <rdfs:domain rdf:resource="http://purl.imsglobal.org/caliper/Collection"/>
        <rdfs:range rdf:resource="http://purl.imsglobal.org/caliper/Entity"/>
        <rdfs:comment xml:lang="en">An ordered collection of resources that comprise the collection.</rdfs:comment>
        <rdfs:isDefinedBy rdf:datatype="http://www.w3.org/2001/XMLSchema#string">http://purl.imsglobal.org/caliper</rdfs:isDefinedBy>
        <rdfs:label xml:lang="en">items</rdfs:label>
    </owl:ObjectProperty>
    


    <!-- http://purl.imsglobal.org/caliper/learningObjectives -->

    <owl:ObjectProperty rdf:about="http://purl.imsglobal.org/caliper/learningObjectives">
        <rdfs:domain rdf:resource="http://purl.imsglobal.org/caliper/DigitalResource"/>
        <rdfs:range rdf:resource="http://purl.imsglobal.org/caliper/LearningObjective"/>
        <rdfs:comment xml:lang="en">An ordered collection of one or more LearningObjective entities that describe what a learner is expected to comprehend or accomplish after engaging with the resource.</rdfs:comment>
        <rdfs:isDefinedBy rdf:datatype="http://www.w3.org/2001/XMLSchema#string">http://purl.imsglobal.org/caliper</rdfs:isDefinedBy>
        <rdfs:label xml:lang="en">learningObjectives</rdfs:label>
    </owl:ObjectProperty>
    


    <!-- http://purl.imsglobal.org/caliper/member -->

    <owl:ObjectProperty rdf:about="http://purl.imsglobal.org/caliper/member">
        <rdf:type rdf:resource="http://www.w3.org/2002/07/owl#FunctionalProperty"/>
        <rdfs:domain rdf:resource="http://purl.imsglobal.org/caliper/Membership"/>
        <rdfs:range rdf:resource="http://purl.imsglobal.org/caliper/Agent"/>
        <rdfs:comment xml:lang="en">The Person associated with a Membership.</rdfs:comment>
        <rdfs:isDefinedBy rdf:datatype="http://www.w3.org/2001/XMLSchema#string">http://purl.imsglobal.org/caliper</rdfs:isDefinedBy>
        <rdfs:label xml:lang="en">member</rdfs:label>
    </owl:ObjectProperty>
    


    <!-- http://purl.imsglobal.org/caliper/members -->

    <owl:ObjectProperty rdf:about="http://purl.imsglobal.org/caliper/members">
        <rdfs:domain rdf:resource="http://purl.imsglobal.org/caliper/Organization"/>
        <rdfs:range rdf:resource="http://purl.imsglobal.org/caliper/Agent"/>
        <rdfs:comment xml:lang="en">An ordered collection of entities of type Agent that belong to a particular group.</rdfs:comment>
        <rdfs:isDefinedBy rdf:datatype="http://www.w3.org/2001/XMLSchema#string">http://purl.imsglobal.org/caliper</rdfs:isDefinedBy>
        <rdfs:label xml:lang="en">members</rdfs:label>
    </owl:ObjectProperty>
    


    <!-- http://purl.imsglobal.org/caliper/membership -->

    <owl:ObjectProperty rdf:about="http://purl.imsglobal.org/caliper/membership">
        <rdf:type rdf:resource="http://www.w3.org/2002/07/owl#FunctionalProperty"/>
        <rdfs:domain rdf:resource="http://purl.imsglobal.org/caliper/Event"/>
        <rdfs:range rdf:resource="http://purl.imsglobal.org/caliper/Membership"/>
        <rdfs:comment xml:lang="en">The relationship between the actor and the group in terms of roles assigned and current status.</rdfs:comment>
        <rdfs:isDefinedBy rdf:datatype="http://www.w3.org/2001/XMLSchema#string">http://purl.imsglobal.org/caliper</rdfs:isDefinedBy>
        <rdfs:label xml:lang="en">membership</rdfs:label>
    </owl:ObjectProperty>
    


    <!-- http://purl.imsglobal.org/caliper/messageParameters -->

    <owl:ObjectProperty rdf:about="http://purl.imsglobal.org/caliper/messageParameters">
        <rdfs:domain rdf:resource="http://purl.imsglobal.org/caliper/LtiSession"/>
        <rdfs:comment xml:lang="en">A map of LTI-specified message parameters that provide Tool Consumer-related contextual information MAY be specified.  LTI message parameters of whatever type (i.e., required, recommended, optional, custom and extension) MAY be referenced.</rdfs:comment>
        <rdfs:isDefinedBy rdf:datatype="http://www.w3.org/2001/XMLSchema#string">http://purl.imsglobal.org/caliper</rdfs:isDefinedBy>
        <rdfs:label xml:lang="en">messageParameters</rdfs:label>
    </owl:ObjectProperty>
    


    <!-- http://purl.imsglobal.org/caliper/messageType -->

    <owl:ObjectProperty rdf:about="http://purl.imsglobal.org/caliper/messageType">
        <rdf:type rdf:resource="http://www.w3.org/2002/07/owl#FunctionalProperty"/>
        <rdfs:domain rdf:resource="http://purl.imsglobal.org/caliper/LtiLink"/>
        <rdfs:range rdf:resource="http://purl.imsglobal.org/caliper/LtiMessageType"/>
    </owl:ObjectProperty>
    


    <!-- http://purl.imsglobal.org/caliper/navigatedFrom -->

    <owl:ObjectProperty rdf:about="http://purl.imsglobal.org/caliper/navigatedFrom">
        <rdf:type rdf:resource="http://www.w3.org/2002/07/owl#FunctionalProperty"/>
        <rdfs:domain rdf:resource="http://purl.imsglobal.org/caliper/NavigationEvent"/>
        <rdfs:range rdf:resource="http://purl.imsglobal.org/caliper/Entity"/>
        <terms:isReplacedBy rdf:resource="http://purl.imsglobal.org/caliper/referrer"/>
        <rdfs:comment xml:lang="en">The DigitalResource or SoftwareApplication that constitutes the referring context of a Navigation Event.  Deprecated.</rdfs:comment>
        <rdfs:isDefinedBy rdf:datatype="http://www.w3.org/2001/XMLSchema#string">http://purl.imsglobal.org/caliper</rdfs:isDefinedBy>
        <rdfs:label xml:lang="en">navigatedFrom</rdfs:label>
        <owl:deprecated rdf:datatype="http://www.w3.org/2001/XMLSchema#boolean">true</owl:deprecated>
    </owl:ObjectProperty>
    


    <!-- http://purl.imsglobal.org/caliper/object -->

    <owl:ObjectProperty rdf:about="http://purl.imsglobal.org/caliper/object">
        <rdf:type rdf:resource="http://www.w3.org/2002/07/owl#FunctionalProperty"/>
        <rdfs:domain rdf:resource="http://purl.imsglobal.org/caliper/Event"/>
        <rdfs:range rdf:resource="http://purl.imsglobal.org/caliper/Entity"/>
        <rdfs:comment xml:lang="en">An Entity that an Event actor interacts with as described by the Event action.</rdfs:comment>
        <rdfs:isDefinedBy rdf:datatype="http://www.w3.org/2001/XMLSchema#string">http://purl.imsglobal.org/caliper</rdfs:isDefinedBy>
        <rdfs:label xml:lang="en">object</rdfs:label>
    </owl:ObjectProperty>
    


    <!-- http://purl.imsglobal.org/caliper/organization -->

    <owl:ObjectProperty rdf:about="http://purl.imsglobal.org/caliper/organization">
        <rdf:type rdf:resource="http://www.w3.org/2002/07/owl#FunctionalProperty"/>
        <rdfs:domain rdf:resource="http://purl.imsglobal.org/caliper/Membership"/>
        <rdfs:range rdf:resource="http://purl.imsglobal.org/caliper/Organization"/>
        <rdfs:comment xml:lang="en">The Organization associated with a Membership.</rdfs:comment>
        <rdfs:isDefinedBy rdf:datatype="http://www.w3.org/2001/XMLSchema#string">http://purl.imsglobal.org/caliper</rdfs:isDefinedBy>
        <rdfs:label xml:lang="en">organization</rdfs:label>
    </owl:ObjectProperty>
    


    <!-- http://purl.imsglobal.org/caliper/query -->

    <owl:ObjectProperty rdf:about="http://purl.imsglobal.org/caliper/query">
        <rdf:type rdf:resource="http://www.w3.org/2002/07/owl#FunctionalProperty"/>
        <rdfs:domain rdf:resource="http://purl.imsglobal.org/caliper/SearchResponse"/>
        <rdfs:range rdf:resource="http://purl.imsglobal.org/caliper/Query"/>
        <rdfs:comment xml:lang="en">The Query submitted by an actor.</rdfs:comment>
        <rdfs:isDefinedBy rdf:datatype="http://www.w3.org/2001/XMLSchema#string">http://purl.imsglobal.org/caliper</rdfs:isDefinedBy>
        <rdfs:label xml:lang="en">query</rdfs:label>
    </owl:ObjectProperty>
    


    <!-- http://purl.imsglobal.org/caliper/rated -->

    <owl:ObjectProperty rdf:about="http://purl.imsglobal.org/caliper/rated">
        <rdf:type rdf:resource="http://www.w3.org/2002/07/owl#FunctionalProperty"/>
        <rdfs:domain rdf:resource="http://purl.imsglobal.org/caliper/Rating"/>
        <rdfs:range rdf:resource="http://purl.imsglobal.org/caliper/Entity"/>
        <rdfs:comment xml:lang="en">The Entity which received the rating.</rdfs:comment>
        <rdfs:isDefinedBy rdf:datatype="http://www.w3.org/2001/XMLSchema#string">https://purl.imsglobal.org/caliper</rdfs:isDefinedBy>
        <rdfs:label xml:lang="en">rated</rdfs:label>
    </owl:ObjectProperty>
    


    <!-- http://purl.imsglobal.org/caliper/rater -->

    <owl:ObjectProperty rdf:about="http://purl.imsglobal.org/caliper/rater">
        <rdf:type rdf:resource="http://www.w3.org/2002/07/owl#FunctionalProperty"/>
        <rdfs:domain rdf:resource="http://purl.imsglobal.org/caliper/Rating"/>
        <rdfs:range rdf:resource="http://purl.imsglobal.org/caliper/Person"/>
        <rdfs:comment xml:lang="en">The Person who provided the Rating.</rdfs:comment>
        <rdfs:isDefinedBy rdf:datatype="http://www.w3.org/2001/XMLSchema#string">https://purl.imsglobal.org/caliper</rdfs:isDefinedBy>
        <rdfs:label xml:lang="en">rater</rdfs:label>
    </owl:ObjectProperty>
    


    <!-- http://purl.imsglobal.org/caliper/ratingComment -->

    <owl:ObjectProperty rdf:about="http://purl.imsglobal.org/caliper/ratingComment">
        <rdf:type rdf:resource="http://www.w3.org/2002/07/owl#FunctionalProperty"/>
        <rdfs:domain rdf:resource="http://purl.imsglobal.org/caliper/Rating"/>
        <rdfs:range rdf:resource="http://purl.imsglobal.org/caliper/Comment"/>
        <rdfs:comment xml:lang="en">The Comment left with the Rating.</rdfs:comment>
        <rdfs:isDefinedBy rdf:datatype="http://www.w3.org/2001/XMLSchema#string">http://purl.imsglobal.org/caliper</rdfs:isDefinedBy>
        <rdfs:label xml:lang="en">ratingComment</rdfs:label>
    </owl:ObjectProperty>
    


    <!-- http://purl.imsglobal.org/caliper/referrer -->

    <owl:ObjectProperty rdf:about="http://purl.imsglobal.org/caliper/referrer">
        <rdf:type rdf:resource="http://www.w3.org/2002/07/owl#FunctionalProperty"/>
        <rdfs:domain rdf:resource="http://purl.imsglobal.org/caliper/Event"/>
        <rdfs:range rdf:resource="http://purl.imsglobal.org/caliper/Entity"/>
        <rdfs:comment xml:lang="en">An Entity that represents the referring context within which an Event occurs.  A SoftwareApplication or DigitalResource will typically constitute the referring context.</rdfs:comment>
        <rdfs:isDefinedBy rdf:datatype="http://www.w3.org/2001/XMLSchema#string">http://purl.imsglobal.org/caliper</rdfs:isDefinedBy>
        <rdfs:label xml:lang="en">referrer</rdfs:label>
    </owl:ObjectProperty>
    


    <!-- http://purl.imsglobal.org/caliper/replyTo -->

    <owl:ObjectProperty rdf:about="http://purl.imsglobal.org/caliper/replyTo">
        <rdf:type rdf:resource="http://www.w3.org/2002/07/owl#FunctionalProperty"/>
        <rdf:type rdf:resource="http://www.w3.org/2002/07/owl#IrreflexiveProperty"/>
        <rdfs:domain rdf:resource="http://purl.imsglobal.org/caliper/Message"/>
        <rdfs:range rdf:resource="http://purl.imsglobal.org/caliper/Message"/>
        <rdfs:comment xml:lang="en">A prior Message that represents the post to which a Message is directed in reply.</rdfs:comment>
        <rdfs:isDefinedBy rdf:datatype="http://www.w3.org/2001/XMLSchema#string">http://purl.imsglobal.org/caliper</rdfs:isDefinedBy>
        <rdfs:label xml:lang="en">replyTo</rdfs:label>
    </owl:ObjectProperty>
    


    <!-- http://purl.imsglobal.org/caliper/roles -->

    <owl:ObjectProperty rdf:about="http://purl.imsglobal.org/caliper/roles">
        <rdfs:domain rdf:resource="http://purl.imsglobal.org/caliper/Membership"/>
        <rdfs:range rdf:resource="http://purl.imsglobal.org/caliper/Role"/>
        <rdfs:comment xml:lang="en">An ordered collection of organizational roles assigned to a member.</rdfs:comment>
        <rdfs:isDefinedBy rdf:datatype="http://www.w3.org/2001/XMLSchema#string">http://purl.imsglobal.org/caliper</rdfs:isDefinedBy>
        <rdfs:label xml:lang="en">roles</rdfs:label>
    </owl:ObjectProperty>
    


    <!-- http://purl.imsglobal.org/caliper/scale -->

    <owl:ObjectProperty rdf:about="http://purl.imsglobal.org/caliper/scale">
        <rdf:type rdf:resource="http://www.w3.org/2002/07/owl#FunctionalProperty"/>
        <rdfs:domain rdf:resource="http://purl.imsglobal.org/caliper/Rating"/>
        <rdfs:range rdf:resource="http://purl.imsglobal.org/caliper/Scale"/>
        <rdfs:comment xml:lang="en">The Scale used for the Rating.</rdfs:comment>
        <rdfs:isDefinedBy rdf:datatype="http://www.w3.org/2001/XMLSchema#string">https://purl.imsglobal.org/caliper</rdfs:isDefinedBy>
        <rdfs:label xml:lang="en">scale</rdfs:label>
    </owl:ObjectProperty>
    


    <!-- http://purl.imsglobal.org/caliper/scoredBy -->

    <owl:ObjectProperty rdf:about="http://purl.imsglobal.org/caliper/scoredBy">
        <rdf:type rdf:resource="http://www.w3.org/2002/07/owl#FunctionalProperty"/>
        <rdfs:domain>
            <owl:Class>
                <owl:unionOf rdf:parseType="Collection">
                    <rdf:Description rdf:about="http://purl.imsglobal.org/caliper/Result"/>
                    <rdf:Description rdf:about="http://purl.imsglobal.org/caliper/Score"/>
                </owl:unionOf>
            </owl:Class>
        </rdfs:domain>
        <rdfs:range rdf:resource="http://purl.imsglobal.org/caliper/Agent"/>
        <rdfs:comment xml:lang="en">The Agent who scored or graded an Attempt.</rdfs:comment>
        <rdfs:isDefinedBy rdf:datatype="http://www.w3.org/2001/XMLSchema#string">http://purl.imsglobal.org/caliper</rdfs:isDefinedBy>
        <rdfs:label xml:lang="en">scoredBy</rdfs:label>
    </owl:ObjectProperty>
    


    <!-- http://purl.imsglobal.org/caliper/searchProvider -->

    <owl:ObjectProperty rdf:about="http://purl.imsglobal.org/caliper/searchProvider">
        <rdf:type rdf:resource="http://www.w3.org/2002/07/owl#FunctionalProperty"/>
        <rdfs:domain rdf:resource="http://purl.imsglobal.org/caliper/SearchResponse"/>
        <rdfs:range rdf:resource="http://purl.imsglobal.org/caliper/SoftwareApplication"/>
        <rdfs:comment xml:lang="en">The SoftwareApplication that is the provider of a SearchResponse.</rdfs:comment>
        <rdfs:isDefinedBy rdf:datatype="http://www.w3.org/2001/XMLSchema#string">http://purl.imsglobal.org/caliper</rdfs:isDefinedBy>
        <rdfs:label xml:lang="en">searchProvider</rdfs:label>
    </owl:ObjectProperty>
    


    <!-- http://purl.imsglobal.org/caliper/searchResults -->

    <owl:ObjectProperty rdf:about="http://purl.imsglobal.org/caliper/searchResults">
        <rdf:type rdf:resource="http://www.w3.org/2002/07/owl#FunctionalProperty"/>
        <rdfs:domain rdf:resource="http://purl.imsglobal.org/caliper/SearchResponse"/>
        <rdfs:range rdf:resource="http://purl.imsglobal.org/caliper/Entity"/>
        <rdfs:comment xml:lang="en">An ordered collection of entities, typically of type DigitalResource that constitute the results of the search.</rdfs:comment>
        <rdfs:isDefinedBy rdf:datatype="http://www.w3.org/2001/XMLSchema#string">http://purl.imsglobal.org/caliper</rdfs:isDefinedBy>
        <rdfs:label xml:lang="en">searchResults</rdfs:label>
    </owl:ObjectProperty>
    


    <!-- http://purl.imsglobal.org/caliper/searchTarget -->

    <owl:ObjectProperty rdf:about="http://purl.imsglobal.org/caliper/searchTarget">
        <rdf:type rdf:resource="http://www.w3.org/2002/07/owl#FunctionalProperty"/>
        <rdfs:domain>
            <owl:Class>
                <owl:unionOf rdf:parseType="Collection">
                    <rdf:Description rdf:about="http://purl.imsglobal.org/caliper/Query"/>
                    <rdf:Description rdf:about="http://purl.imsglobal.org/caliper/SearchResponse"/>
                </owl:unionOf>
            </owl:Class>
        </rdfs:domain>
        <rdfs:range rdf:resource="http://purl.imsglobal.org/caliper/Entity"/>
        <rdfs:comment xml:lang="en">The Entity, typically a DigitalResource or  SoftwareApplication, that is the target of the search.</rdfs:comment>
        <rdfs:isDefinedBy rdf:datatype="http://www.w3.org/2001/XMLSchema#string">http://purl.imsglobal.org/caliper</rdfs:isDefinedBy>
        <rdfs:label xml:lang="en">searchTarget</rdfs:label>
    </owl:ObjectProperty>
    


    <!-- http://purl.imsglobal.org/caliper/selection -->

    <owl:ObjectProperty rdf:about="http://purl.imsglobal.org/caliper/selection">
        <rdf:type rdf:resource="http://www.w3.org/2002/07/owl#FunctionalProperty"/>
        <rdfs:domain rdf:resource="http://purl.imsglobal.org/caliper/HighlightAnnotation"/>
        <rdfs:range rdf:resource="http://purl.imsglobal.org/caliper/TextPositionSelector"/>
        <rdfs:comment xml:lang="en">A Selector that describes a fragment or segment of a resource.</rdfs:comment>
        <rdfs:isDefinedBy rdf:datatype="http://www.w3.org/2001/XMLSchema#string">http://purl.imsglobal.org/caliper</rdfs:isDefinedBy>
        <rdfs:label xml:lang="en">selection</rdfs:label>
    </owl:ObjectProperty>
    


    <!-- http://purl.imsglobal.org/caliper/selections -->

    <owl:ObjectProperty rdf:about="http://purl.imsglobal.org/caliper/selections">
        <rdfs:comment xml:lang="en">An array of the values representing the rater&apos;s selected response.</rdfs:comment>
        <rdfs:isDefinedBy rdf:datatype="http://www.w3.org/2001/XMLSchema#string">https://purl.imsglobal.org/caliper</rdfs:isDefinedBy>
        <rdfs:label xml:lang="en">selections</rdfs:label>
    </owl:ObjectProperty>
    


    <!-- http://purl.imsglobal.org/caliper/session -->

    <owl:ObjectProperty rdf:about="http://purl.imsglobal.org/caliper/session">
        <rdf:type rdf:resource="http://www.w3.org/2002/07/owl#FunctionalProperty"/>
        <rdfs:domain rdf:resource="http://purl.imsglobal.org/caliper/Event"/>
        <rdfs:range rdf:resource="http://purl.imsglobal.org/caliper/Session"/>
        <rdfs:comment xml:lang="en">The current user Session.</rdfs:comment>
        <rdfs:isDefinedBy rdf:datatype="http://www.w3.org/2001/XMLSchema#string">http://purl.imsglobal.org/caliper</rdfs:isDefinedBy>
        <rdfs:label xml:lang="en">session</rdfs:label>
    </owl:ObjectProperty>
    


    <!-- http://purl.imsglobal.org/caliper/status -->

    <owl:ObjectProperty rdf:about="http://purl.imsglobal.org/caliper/status">
        <rdf:type rdf:resource="http://www.w3.org/2002/07/owl#FunctionalProperty"/>
        <rdfs:domain rdf:resource="http://purl.imsglobal.org/caliper/Membership"/>
        <rdfs:range rdf:resource="http://purl.imsglobal.org/caliper/Status"/>
        <rdfs:comment xml:lang="en">The current standing of a member.</rdfs:comment>
        <rdfs:isDefinedBy rdf:datatype="http://www.w3.org/2001/XMLSchema#string">http://purl.imsglobal.org/caliper</rdfs:isDefinedBy>
        <rdfs:label xml:lang="en">status</rdfs:label>
    </owl:ObjectProperty>
    


    <!-- http://purl.imsglobal.org/caliper/subOrganizationOf -->

    <owl:ObjectProperty rdf:about="http://purl.imsglobal.org/caliper/subOrganizationOf">
        <rdf:type rdf:resource="http://www.w3.org/2002/07/owl#FunctionalProperty"/>
        <rdf:type rdf:resource="http://www.w3.org/2002/07/owl#IrreflexiveProperty"/>
        <rdfs:domain rdf:resource="http://purl.imsglobal.org/caliper/Organization"/>
        <rdfs:range rdf:resource="http://purl.imsglobal.org/caliper/Organization"/>
        <rdfs:comment xml:lang="en">The parent Organization of an Organization.</rdfs:comment>
        <rdfs:isDefinedBy rdf:datatype="http://www.w3.org/2001/XMLSchema#string">http://purl.imsglobal.org/caliper</rdfs:isDefinedBy>
        <rdfs:label xml:lang="en">subOrganizationOf</rdfs:label>
    </owl:ObjectProperty>
    


    <!-- http://purl.imsglobal.org/caliper/target -->

    <owl:ObjectProperty rdf:about="http://purl.imsglobal.org/caliper/target">
        <rdf:type rdf:resource="http://www.w3.org/2002/07/owl#FunctionalProperty"/>
        <rdfs:domain rdf:resource="http://purl.imsglobal.org/caliper/Event"/>
        <rdfs:range rdf:resource="http://purl.imsglobal.org/caliper/Entity"/>
        <rdfs:comment xml:lang="en">An Entity that represents a particular segment or location within an Event object.</rdfs:comment>
        <rdfs:isDefinedBy rdf:datatype="http://www.w3.org/2001/XMLSchema#string">http://purl.imsglobal.org/caliper</rdfs:isDefinedBy>
        <rdfs:label xml:lang="en">target</rdfs:label>
    </owl:ObjectProperty>
    


    <!-- http://purl.imsglobal.org/caliper/user -->

    <owl:ObjectProperty rdf:about="http://purl.imsglobal.org/caliper/user">
        <rdf:type rdf:resource="http://www.w3.org/2002/07/owl#FunctionalProperty"/>
        <rdfs:domain rdf:resource="http://purl.imsglobal.org/caliper/Session"/>
        <rdfs:range rdf:resource="http://purl.imsglobal.org/caliper/Agent"/>
        <rdfs:comment xml:lang="en">The Person who initiated a Session.</rdfs:comment>
        <rdfs:isDefinedBy rdf:datatype="http://www.w3.org/2001/XMLSchema#string">http://purl.imsglobal.org/caliper</rdfs:isDefinedBy>
        <rdfs:label xml:lang="en">user</rdfs:label>
    </owl:ObjectProperty>
    


    <!-- http://purl.imsglobal.org/caliper/withAgents -->

    <owl:ObjectProperty rdf:about="http://purl.imsglobal.org/caliper/withAgents">
        <rdfs:domain rdf:resource="http://purl.imsglobal.org/caliper/SharedAnnotation"/>
        <rdfs:range rdf:resource="http://purl.imsglobal.org/caliper/Agent"/>
        <rdfs:comment xml:lang="en">An ordered collection of one or more Agent entities, typically of type Person, with whom the annotated DigitalResource has been shared.</rdfs:comment>
        <rdfs:isDefinedBy rdf:datatype="http://www.w3.org/2001/XMLSchema#string">http://purl.imsglobal.org/caliper</rdfs:isDefinedBy>
        <rdfs:label xml:lang="en">withAgents</rdfs:label>
    </owl:ObjectProperty>
    


    <!-- 
    ///////////////////////////////////////////////////////////////////////////////////////
    //
    // Data properties
    //
    ///////////////////////////////////////////////////////////////////////////////////////
     -->

    


    <!-- http://purl.imsglobal.org/caliper/academicSession -->

    <owl:DatatypeProperty rdf:about="http://purl.imsglobal.org/caliper/academicSession">
        <rdf:type rdf:resource="http://www.w3.org/2002/07/owl#FunctionalProperty"/>
        <rdfs:domain rdf:resource="http://purl.imsglobal.org/caliper/CourseOffering"/>
        <rdfs:range rdf:resource="http://www.w3.org/2001/XMLSchema#string"/>
        <rdfs:comment xml:lang="en">A human-readable identifier of the designated period in which a CourseOffering occurs.</rdfs:comment>
        <rdfs:isDefinedBy rdf:datatype="http://www.w3.org/2001/XMLSchema#string">http://purl.imsglobal.org/caliper</rdfs:isDefinedBy>
        <rdfs:label xml:lang="en">academicSession</rdfs:label>
    </owl:DatatypeProperty>
    


    <!-- http://purl.imsglobal.org/caliper/body -->

    <owl:DatatypeProperty rdf:about="http://purl.imsglobal.org/caliper/body">
        <rdf:type rdf:resource="http://www.w3.org/2002/07/owl#FunctionalProperty"/>
        <rdfs:domain rdf:resource="http://purl.imsglobal.org/caliper/Message"/>
        <rdfs:range rdf:resource="http://www.w3.org/2001/XMLSchema#string"/>
        <rdfs:comment xml:lang="en">A plain-text rendering of the body content of a Message.</rdfs:comment>
        <rdfs:isDefinedBy rdf:datatype="http://www.w3.org/2001/XMLSchema#string">http://purl.imsglobal.org/caliper</rdfs:isDefinedBy>
        <rdfs:label xml:lang="en">body</rdfs:label>
    </owl:DatatypeProperty>
    


    <!-- http://purl.imsglobal.org/caliper/bookmarkNotes -->

    <owl:DatatypeProperty rdf:about="http://purl.imsglobal.org/caliper/bookmarkNotes">
        <rdf:type rdf:resource="http://www.w3.org/2002/07/owl#FunctionalProperty"/>
        <rdfs:domain rdf:resource="http://purl.imsglobal.org/caliper/BookmarkAnnotation"/>
        <rdfs:range rdf:resource="http://www.w3.org/2001/XMLSchema#string"/>
        <rdfs:comment xml:lang="en">A plain text rendering of the note associated with a BookmarkAnnotation.</rdfs:comment>
        <rdfs:isDefinedBy rdf:datatype="http://www.w3.org/2001/XMLSchema#string">http://purl.imsglobal.org/caliper</rdfs:isDefinedBy>
        <rdfs:label xml:lang="en">bookmarkNotes</rdfs:label>
    </owl:DatatypeProperty>
    


    <!-- http://purl.imsglobal.org/caliper/category -->

    <owl:DatatypeProperty rdf:about="http://purl.imsglobal.org/caliper/category">
        <rdf:type rdf:resource="http://www.w3.org/2002/07/owl#FunctionalProperty"/>
        <rdfs:domain rdf:resource="http://purl.imsglobal.org/caliper/CourseSection"/>
        <rdfs:range rdf:resource="http://www.w3.org/2001/XMLSchema#string"/>
        <rdfs:comment xml:lang="en">A plain-text descriptor that characterizes the purpose of the CourseSection such as &quot;lecture&quot;, &quot;lab&quot; or &quot;seminar&quot;.</rdfs:comment>
        <rdfs:isDefinedBy rdf:datatype="http://www.w3.org/2001/XMLSchema#string">http://purl.imsglobal.org/caliper</rdfs:isDefinedBy>
        <rdfs:label xml:lang="en">category</rdfs:label>
    </owl:DatatypeProperty>
    


    <!-- http://purl.imsglobal.org/caliper/comment -->

    <owl:DatatypeProperty rdf:about="http://purl.imsglobal.org/caliper/comment">
        <rdf:type rdf:resource="http://www.w3.org/2002/07/owl#FunctionalProperty"/>
        <rdfs:domain rdf:resource="http://purl.imsglobal.org/caliper/Result"/>
        <rdfs:range rdf:resource="http://www.w3.org/2001/XMLSchema#string"/>
        <rdfs:comment xml:lang="en">Plain text feedback provided by the scorer of a Result.</rdfs:comment>
        <rdfs:isDefinedBy rdf:datatype="http://www.w3.org/2001/XMLSchema#string">http://purl.imsglobal.org/caliper</rdfs:isDefinedBy>
        <rdfs:label xml:lang="en">comment</rdfs:label>
    </owl:DatatypeProperty>
    


    <!-- http://purl.imsglobal.org/caliper/count -->

    <owl:DatatypeProperty rdf:about="http://purl.imsglobal.org/caliper/count">
        <rdf:type rdf:resource="http://www.w3.org/2002/07/owl#FunctionalProperty"/>
        <rdfs:domain rdf:resource="http://purl.imsglobal.org/caliper/Attempt"/>
        <rdfs:range rdf:resource="http://www.w3.org/2001/XMLSchema#nonNegativeInteger"/>
        <rdfs:comment xml:lang="en">The total number of attempts inclusive of the current Attempt that have been registered by the learner against the assigned resource.</rdfs:comment>
        <rdfs:isDefinedBy rdf:datatype="http://www.w3.org/2001/XMLSchema#string">http://purl.imsglobal.org/caliper</rdfs:isDefinedBy>
        <rdfs:label xml:lang="en">count</rdfs:label>
    </owl:DatatypeProperty>
    


    <!-- http://purl.imsglobal.org/caliper/courseNumber -->

    <owl:DatatypeProperty rdf:about="http://purl.imsglobal.org/caliper/courseNumber">
        <rdf:type rdf:resource="http://www.w3.org/2002/07/owl#FunctionalProperty"/>
        <rdfs:domain rdf:resource="http://purl.imsglobal.org/caliper/CourseOffering"/>
        <rdfs:range rdf:resource="http://www.w3.org/2001/XMLSchema#string"/>
        <rdfs:comment xml:lang="en">A human-readable identifier of the CourseOffering or CourseSection.</rdfs:comment>
        <rdfs:isDefinedBy rdf:datatype="http://www.w3.org/2001/XMLSchema#string">http://purl.imsglobal.org/caliper</rdfs:isDefinedBy>
        <rdfs:label xml:lang="en">courseNumber</rdfs:label>
    </owl:DatatypeProperty>
    


    <!-- http://purl.imsglobal.org/caliper/currentTime -->

    <owl:DatatypeProperty rdf:about="http://purl.imsglobal.org/caliper/currentTime">
        <rdf:type rdf:resource="http://www.w3.org/2002/07/owl#FunctionalProperty"/>
        <rdfs:domain rdf:resource="http://purl.imsglobal.org/caliper/MediaLocation"/>
        <rdfs:range rdf:resource="http://www.w3.org/2001/XMLSchema#duration"/>
        <rdfs:comment xml:lang="en">A time interval or duration that represents the current playback position measured from the beginning of a MediaObject.</rdfs:comment>
        <rdfs:isDefinedBy rdf:datatype="http://www.w3.org/2001/XMLSchema#string">http://purl.imsglobal.org/caliper</rdfs:isDefinedBy>
        <rdfs:label xml:lang="en">currentTime</rdfs:label>
    </owl:DatatypeProperty>
    


    <!-- http://purl.imsglobal.org/caliper/curveFactor -->

    <owl:DatatypeProperty rdf:about="http://purl.imsglobal.org/caliper/curveFactor">
        <rdf:type rdf:resource="http://www.w3.org/2002/07/owl#FunctionalProperty"/>
        <rdfs:domain rdf:resource="http://purl.imsglobal.org/caliper/Result"/>
        <rdfs:range rdf:resource="http://www.w3.org/2001/XMLSchema#decimal"/>
        <rdfs:comment xml:lang="en">A scale factor to be used in adjusting the totalScore.</rdfs:comment>
        <rdfs:isDefinedBy rdf:datatype="http://www.w3.org/2001/XMLSchema#string">http://purl.imsglobal.org/caliper</rdfs:isDefinedBy>
        <rdfs:label xml:lang="en">curveFactor</rdfs:label>
        <owl:deprecated rdf:datatype="http://www.w3.org/2001/XMLSchema#boolean">true</owl:deprecated>
    </owl:DatatypeProperty>
    


    <!-- http://purl.imsglobal.org/caliper/curvedTotalScore -->

    <owl:DatatypeProperty rdf:about="http://purl.imsglobal.org/caliper/curvedTotalScore">
        <rdf:type rdf:resource="http://www.w3.org/2002/07/owl#FunctionalProperty"/>
        <rdfs:domain rdf:resource="http://purl.imsglobal.org/caliper/Result"/>
        <rdfs:range rdf:resource="http://www.w3.org/2001/XMLSchema#decimal"/>
        <rdfs:comment xml:lang="en">The total score earned by the learner after applying a curveFactor to a method for computing a scaled score; e.g., adjusting the score equal to the sum of 100 - curvedFactor(100 - totalScore).</rdfs:comment>
        <rdfs:isDefinedBy rdf:datatype="http://www.w3.org/2001/XMLSchema#string">http://purl.imsglobal.org/caliper</rdfs:isDefinedBy>
        <rdfs:label xml:lang="en">curvedTotalScore</rdfs:label>
        <owl:deprecated rdf:datatype="http://www.w3.org/2001/XMLSchema#boolean">true</owl:deprecated>
    </owl:DatatypeProperty>
    


    <!-- http://purl.imsglobal.org/caliper/dataVersion -->

    <owl:DatatypeProperty rdf:about="http://purl.imsglobal.org/caliper/dataVersion">
        <rdf:type rdf:resource="http://www.w3.org/2002/07/owl#FunctionalProperty"/>
        <rdfs:domain rdf:resource="http://purl.imsglobal.org/caliper/Envelope"/>
        <rdfs:range rdf:resource="http://www.w3.org/2001/XMLSchema#string"/>
        <rdfs:comment xml:lang="en">Envelope data payload Caliper version.</rdfs:comment>
        <rdfs:isDefinedBy rdf:datatype="http://www.w3.org/2001/XMLSchema#string">http://purl.imsglobal.org/caliper</rdfs:isDefinedBy>
        <rdfs:label xml:lang="en">dataVersion</rdfs:label>
    </owl:DatatypeProperty>
    


    <!-- http://purl.imsglobal.org/caliper/dateCreated -->

    <owl:DatatypeProperty rdf:about="http://purl.imsglobal.org/caliper/dateCreated">
        <rdf:type rdf:resource="http://www.w3.org/2002/07/owl#FunctionalProperty"/>
        <rdfs:domain rdf:resource="http://purl.imsglobal.org/caliper/Entity"/>
        <rdfs:range rdf:resource="http://www.w3.org/2001/XMLSchema#dateTime"/>
        <owl:propertyDisjointWith rdf:resource="http://purl.imsglobal.org/caliper/dateModified"/>
        <rdfs:comment xml:lang="en">A date and time value expressed with millisecond precision that describes when an Entity was created.</rdfs:comment>
        <rdfs:isDefinedBy rdf:datatype="http://www.w3.org/2001/XMLSchema#string">http://purl.imsglobal.org/caliper</rdfs:isDefinedBy>
        <rdfs:label xml:lang="en">dateCreated</rdfs:label>
    </owl:DatatypeProperty>
    


    <!-- http://purl.imsglobal.org/caliper/dateModified -->

    <owl:DatatypeProperty rdf:about="http://purl.imsglobal.org/caliper/dateModified">
        <rdf:type rdf:resource="http://www.w3.org/2002/07/owl#FunctionalProperty"/>
        <rdfs:domain rdf:resource="http://purl.imsglobal.org/caliper/Entity"/>
        <rdfs:range rdf:resource="http://www.w3.org/2001/XMLSchema#dateTime"/>
        <rdfs:comment xml:lang="en">A date and time value expressed with millisecond precision that describes when an Entity was last changed or modified.</rdfs:comment>
        <rdfs:isDefinedBy rdf:datatype="http://www.w3.org/2001/XMLSchema#string">http://purl.imsglobal.org/caliper</rdfs:isDefinedBy>
        <rdfs:label xml:lang="en">dateModified</rdfs:label>
    </owl:DatatypeProperty>
    


    <!-- http://purl.imsglobal.org/caliper/datePublished -->

    <owl:DatatypeProperty rdf:about="http://purl.imsglobal.org/caliper/datePublished">
        <rdf:type rdf:resource="http://www.w3.org/2002/07/owl#FunctionalProperty"/>
        <rdfs:domain rdf:resource="http://purl.imsglobal.org/caliper/DigitalResource"/>
        <rdfs:range rdf:resource="http://www.w3.org/2001/XMLSchema#dateTime"/>
        <rdfs:comment xml:lang="en">A date and time value expressed with millisecond precision that provides the publication date of a resource.</rdfs:comment>
        <rdfs:isDefinedBy rdf:datatype="http://www.w3.org/2001/XMLSchema#string">http://purl.imsglobal.org/caliper</rdfs:isDefinedBy>
        <rdfs:label xml:lang="en">datePublished</rdfs:label>
    </owl:DatatypeProperty>
    


    <!-- http://purl.imsglobal.org/caliper/dateToActivate -->

    <owl:DatatypeProperty rdf:about="http://purl.imsglobal.org/caliper/dateToActivate">
        <rdf:type rdf:resource="http://www.w3.org/2002/07/owl#FunctionalProperty"/>
        <rdfs:domain rdf:resource="http://purl.imsglobal.org/caliper/DigitalResource"/>
        <rdfs:range rdf:resource="http://www.w3.org/2001/XMLSchema#dateTime"/>
        <rdfs:comment xml:lang="en">A date and time value expressed with millisecond precision that describes when a resource was activated.</rdfs:comment>
        <rdfs:isDefinedBy rdf:datatype="http://www.w3.org/2001/XMLSchema#string">http://purl.imsglobal.org/caliper</rdfs:isDefinedBy>
        <rdfs:label xml:lang="en">dateToActivate</rdfs:label>
    </owl:DatatypeProperty>
    


    <!-- http://purl.imsglobal.org/caliper/dateToShow -->

    <owl:DatatypeProperty rdf:about="http://purl.imsglobal.org/caliper/dateToShow">
        <rdf:type rdf:resource="http://www.w3.org/2002/07/owl#FunctionalProperty"/>
        <rdfs:domain rdf:resource="http://purl.imsglobal.org/caliper/DigitalResource"/>
        <rdfs:range rdf:resource="http://www.w3.org/2001/XMLSchema#dateTime"/>
        <rdfs:comment xml:lang="en">A date and time value expressed with millisecond precision that describes when a resource should be shown or made available.</rdfs:comment>
        <rdfs:isDefinedBy rdf:datatype="http://www.w3.org/2001/XMLSchema#string">http://purl.imsglobal.org/caliper</rdfs:isDefinedBy>
        <rdfs:label xml:lang="en">dateToShow</rdfs:label>
    </owl:DatatypeProperty>
    


    <!-- http://purl.imsglobal.org/caliper/dateToStartOn -->

    <owl:DatatypeProperty rdf:about="http://purl.imsglobal.org/caliper/dateToStartOn">
        <rdf:type rdf:resource="http://www.w3.org/2002/07/owl#FunctionalProperty"/>
        <rdfs:domain rdf:resource="http://purl.imsglobal.org/caliper/DigitalResource"/>
        <rdfs:range rdf:resource="http://www.w3.org/2001/XMLSchema#dateTime"/>
        <rdfs:comment xml:lang="en">A date and time value expressed with millisecond precision that describes when the resource can be started.</rdfs:comment>
        <rdfs:isDefinedBy rdf:datatype="http://www.w3.org/2001/XMLSchema#string">http://purl.imsglobal.org/caliper</rdfs:isDefinedBy>
        <rdfs:label xml:lang="en">dateToStartOn</rdfs:label>
    </owl:DatatypeProperty>
    


    <!-- http://purl.imsglobal.org/caliper/dateToSubmit -->

    <owl:DatatypeProperty rdf:about="http://purl.imsglobal.org/caliper/dateToSubmit">
        <rdf:type rdf:resource="http://www.w3.org/2002/07/owl#FunctionalProperty"/>
        <rdfs:domain rdf:resource="http://purl.imsglobal.org/caliper/DigitalResource"/>
        <rdfs:range rdf:resource="http://www.w3.org/2001/XMLSchema#dateTime"/>
        <rdfs:comment xml:lang="en">A date and time value expressed with millisecond precision that describes when the resource is to be submitted for evaluation.</rdfs:comment>
        <rdfs:isDefinedBy rdf:datatype="http://www.w3.org/2001/XMLSchema#string">http://purl.imsglobal.org/caliper</rdfs:isDefinedBy>
        <rdfs:label xml:lang="en">dateToSubmit</rdfs:label>
    </owl:DatatypeProperty>
    


    <!-- http://purl.imsglobal.org/caliper/description -->

    <owl:DatatypeProperty rdf:about="http://purl.imsglobal.org/caliper/description">
        <rdf:type rdf:resource="http://www.w3.org/2002/07/owl#FunctionalProperty"/>
        <rdfs:domain rdf:resource="http://purl.imsglobal.org/caliper/Entity"/>
        <rdfs:range rdf:resource="http://www.w3.org/2001/XMLSchema#string"/>
        <rdfs:comment xml:lang="en">A brief, plain-text representation of the resource.</rdfs:comment>
        <rdfs:isDefinedBy rdf:datatype="http://www.w3.org/2001/XMLSchema#string">http://purl.imsglobal.org/caliper</rdfs:isDefinedBy>
        <rdfs:label xml:lang="en">description</rdfs:label>
    </owl:DatatypeProperty>
    


    <!-- http://purl.imsglobal.org/caliper/duration -->

    <owl:DatatypeProperty rdf:about="http://purl.imsglobal.org/caliper/duration">
        <rdf:type rdf:resource="http://www.w3.org/2002/07/owl#FunctionalProperty"/>
        <rdfs:domain>
            <owl:Class>
                <owl:unionOf rdf:parseType="Collection">
                    <rdf:Description rdf:about="http://purl.imsglobal.org/caliper/Attempt"/>
                    <rdf:Description rdf:about="http://purl.imsglobal.org/caliper/MediaObject"/>
                    <rdf:Description rdf:about="http://purl.imsglobal.org/caliper/Response"/>
                    <rdf:Description rdf:about="http://purl.imsglobal.org/caliper/Session"/>
                </owl:unionOf>
            </owl:Class>
        </rdfs:domain>
        <rdfs:range rdf:resource="http://www.w3.org/2001/XMLSchema#duration"/>
        <rdfs:comment xml:lang="en">A time interval that represents the total time required to complete an activity.</rdfs:comment>
        <rdfs:isDefinedBy rdf:datatype="http://www.w3.org/2001/XMLSchema#string">http://purl.imsglobal.org/caliper</rdfs:isDefinedBy>
        <rdfs:label xml:lang="en">duration</rdfs:label>
    </owl:DatatypeProperty>
    


    <!-- http://purl.imsglobal.org/caliper/end -->

    <owl:DatatypeProperty rdf:about="http://purl.imsglobal.org/caliper/end">
        <rdf:type rdf:resource="http://www.w3.org/2002/07/owl#FunctionalProperty"/>
        <rdfs:domain rdf:resource="http://purl.imsglobal.org/caliper/TextPositionSelector"/>
        <rdfs:range rdf:resource="http://www.w3.org/2001/XMLSchema#nonNegativeInteger"/>
        <owl:propertyDisjointWith rdf:resource="http://purl.imsglobal.org/caliper/start"/>
        <rdfs:comment xml:lang="en">The end position of a segment of text. The first character in the full text is position 0. The character that represents the end position is NOT included within the selected segment.</rdfs:comment>
        <rdfs:isDefinedBy rdf:datatype="http://www.w3.org/2001/XMLSchema#string">http://purl.imsglobal.org/caliper</rdfs:isDefinedBy>
        <rdfs:label xml:lang="en">end</rdfs:label>
    </owl:DatatypeProperty>
    


    <!-- http://purl.imsglobal.org/caliper/endedAtTime -->

    <owl:DatatypeProperty rdf:about="http://purl.imsglobal.org/caliper/endedAtTime">
        <rdf:type rdf:resource="http://www.w3.org/2002/07/owl#FunctionalProperty"/>
        <rdfs:domain>
            <owl:Class>
                <owl:unionOf rdf:parseType="Collection">
                    <rdf:Description rdf:about="http://purl.imsglobal.org/caliper/AggregateMeasure"/>
                    <rdf:Description rdf:about="http://purl.imsglobal.org/caliper/Attempt"/>
                    <rdf:Description rdf:about="http://purl.imsglobal.org/caliper/Response"/>
                    <rdf:Description rdf:about="http://purl.imsglobal.org/caliper/Session"/>
                </owl:unionOf>
            </owl:Class>
        </rdfs:domain>
        <rdfs:range rdf:resource="http://www.w3.org/2001/XMLSchema#dateTime"/>
        <owl:propertyDisjointWith rdf:resource="http://purl.imsglobal.org/caliper/startedAtTime"/>
        <rdfs:comment xml:lang="en">A date and time value expressed with millisecond precision that describes when the activity was completed or terminated.</rdfs:comment>
        <rdfs:isDefinedBy rdf:datatype="http://www.w3.org/2001/XMLSchema#string">http://purl.imsglobal.org/caliper</rdfs:isDefinedBy>
        <rdfs:label xml:lang="en">endedAtTime</rdfs:label>
    </owl:DatatypeProperty>
    


    <!-- http://purl.imsglobal.org/caliper/eventTime -->

    <owl:DatatypeProperty rdf:about="http://purl.imsglobal.org/caliper/eventTime">
        <rdf:type rdf:resource="http://www.w3.org/2002/07/owl#FunctionalProperty"/>
        <rdfs:domain rdf:resource="http://purl.imsglobal.org/caliper/Event"/>
        <rdfs:range rdf:resource="http://www.w3.org/2001/XMLSchema#dateTime"/>
        <rdfs:comment xml:lang="en">A date and time value expressed with millisecond precision that indicates when an Event occurred.</rdfs:comment>
        <rdfs:isDefinedBy rdf:datatype="http://www.w3.org/2001/XMLSchema#string">http://purl.imsglobal.org/caliper</rdfs:isDefinedBy>
        <rdfs:label xml:lang="en">eventTime</rdfs:label>
    </owl:DatatypeProperty>
    


    <!-- http://purl.imsglobal.org/caliper/extraCreditScore -->

    <owl:DatatypeProperty rdf:about="http://purl.imsglobal.org/caliper/extraCreditScore">
        <rdf:type rdf:resource="http://www.w3.org/2002/07/owl#FunctionalProperty"/>
        <rdfs:domain rdf:resource="http://purl.imsglobal.org/caliper/Result"/>
        <rdfs:range rdf:resource="http://www.w3.org/2001/XMLSchema#decimal"/>
        <rdfs:comment xml:lang="en">The number of extra credit points earned by the learner.</rdfs:comment>
        <rdfs:isDefinedBy rdf:datatype="http://www.w3.org/2001/XMLSchema#string">http://purl.imsglobal.org/caliper</rdfs:isDefinedBy>
        <rdfs:label xml:lang="en">extraCreditScore</rdfs:label>
        <owl:deprecated rdf:datatype="http://www.w3.org/2001/XMLSchema#boolean">true</owl:deprecated>
    </owl:DatatypeProperty>
    


    <!-- http://purl.imsglobal.org/caliper/id -->

    <owl:DatatypeProperty rdf:about="http://purl.imsglobal.org/caliper/id">
        <rdf:type rdf:resource="http://www.w3.org/2002/07/owl#FunctionalProperty"/>
        <rdfs:domain>
            <owl:Class>
                <owl:unionOf rdf:parseType="Collection">
                    <rdf:Description rdf:about="http://purl.imsglobal.org/caliper/Entity"/>
                    <rdf:Description rdf:about="http://purl.imsglobal.org/caliper/Event"/>
                </owl:unionOf>
            </owl:Class>
        </rdfs:domain>
        <rdfs:range rdf:resource="http://www.w3.org/2001/XMLSchema#string"/>
        <rdfs:comment xml:lang="en">The Event or Entity identifier.  For an Event, the id MUST be a UUID expressed as a URN using the form urn:uuid:&lt;UUID&gt; per RFC 4122.  For Entities a valid IRI MUST be specified. The IRI MUST be unique and persistent. The IRI SHOULD also be dereferenceable, i.e., capable of returning a representation of the resource.  An Entity MAY be provisioned with a URI employing the URN scheme in cases where a Linked Data friendly HTTP URI is either unavailable or inappropriate.</rdfs:comment>
        <rdfs:isDefinedBy rdf:datatype="http://www.w3.org/2001/XMLSchema#string">http://purl.imsglobal.org/caliper</rdfs:isDefinedBy>
        <rdfs:label xml:lang="en">id</rdfs:label>
    </owl:DatatypeProperty>
    


    <!-- http://purl.imsglobal.org/caliper/index -->

    <owl:DatatypeProperty rdf:about="http://purl.imsglobal.org/caliper/index">
        <rdf:type rdf:resource="http://www.w3.org/2002/07/owl#FunctionalProperty"/>
        <rdfs:domain rdf:resource="http://purl.imsglobal.org/caliper/Frame"/>
        <rdfs:range rdf:resource="http://www.w3.org/2001/XMLSchema#long"/>
        <rdfs:comment xml:lang="en">A non-negative integer that represents the position of the Frame.</rdfs:comment>
        <rdfs:isDefinedBy rdf:datatype="http://www.w3.org/2001/XMLSchema#string">http://purl.imsglobal.org/caliper</rdfs:isDefinedBy>
        <rdfs:label xml:lang="en">index</rdfs:label>
    </owl:DatatypeProperty>
    


    <!-- http://purl.imsglobal.org/caliper/isTimeDependent -->

    <owl:DatatypeProperty rdf:about="http://purl.imsglobal.org/caliper/isTimeDependent">
        <rdf:type rdf:resource="http://www.w3.org/2002/07/owl#FunctionalProperty"/>
        <rdfs:domain rdf:resource="http://purl.imsglobal.org/caliper/AssessmentItem"/>
        <rdfs:range rdf:resource="http://www.w3.org/2001/XMLSchema#boolean"/>
        <rdfs:comment xml:lang="en">A boolean value indicating whether or not interacting with the item is time dependent.</rdfs:comment>
        <rdfs:isDefinedBy rdf:datatype="http://www.w3.org/2001/XMLSchema#string">http://purl.imsglobal.org/caliper</rdfs:isDefinedBy>
        <rdfs:label xml:lang="en">isTimeDependent</rdfs:label>
    </owl:DatatypeProperty>
    


    <!-- http://purl.imsglobal.org/caliper/keywords -->

    <owl:DatatypeProperty rdf:about="http://purl.imsglobal.org/caliper/keywords">
        <rdfs:domain rdf:resource="http://purl.imsglobal.org/caliper/DigitalResource"/>
        <rdfs:range rdf:resource="http://www.w3.org/2001/XMLSchema#string"/>
        <rdfs:comment xml:lang="en">An ordered collection of one or more string values that represent tags or labels used to identify the resource.</rdfs:comment>
        <rdfs:isDefinedBy rdf:datatype="http://www.w3.org/2001/XMLSchema#string">http://purl.imsglobal.org/caliper</rdfs:isDefinedBy>
        <rdfs:label xml:lang="en">keywords</rdfs:label>
    </owl:DatatypeProperty>
    


    <!-- http://purl.imsglobal.org/caliper/maxAttempts -->

    <owl:DatatypeProperty rdf:about="http://purl.imsglobal.org/caliper/maxAttempts">
        <rdf:type rdf:resource="http://www.w3.org/2002/07/owl#FunctionalProperty"/>
        <rdfs:domain rdf:resource="http://purl.imsglobal.org/caliper/DigitalResource"/>
        <rdfs:range rdf:resource="http://www.w3.org/2001/XMLSchema#nonNegativeInteger"/>
        <rdfs:comment xml:lang="en">A non-negative integer indicating the number of permitted attempts.</rdfs:comment>
        <rdfs:isDefinedBy rdf:datatype="http://www.w3.org/2001/XMLSchema#string">http://purl.imsglobal.org/caliper</rdfs:isDefinedBy>
        <rdfs:label xml:lang="en">maxAttempts</rdfs:label>
    </owl:DatatypeProperty>
    


    <!-- http://purl.imsglobal.org/caliper/maxLabel -->

    <owl:DatatypeProperty rdf:about="http://purl.imsglobal.org/caliper/maxLabel">
        <rdf:type rdf:resource="http://www.w3.org/2002/07/owl#FunctionalProperty"/>
        <rdfs:domain rdf:resource="http://purl.imsglobal.org/caliper/NumericScale"/>
        <rdfs:range rdf:resource="http://www.w3.org/2001/XMLSchema#string"/>
        <owl:propertyDisjointWith rdf:resource="http://purl.imsglobal.org/caliper/minLabel"/>
        <rdfs:comment xml:lang="en">The label for the maximum value.</rdfs:comment>
        <rdfs:isDefinedBy rdf:datatype="http://www.w3.org/2001/XMLSchema#string">https://purl.imsglobal.org/caliper</rdfs:isDefinedBy>
        <rdfs:label xml:lang="en">maxLabel</rdfs:label>
    </owl:DatatypeProperty>
    


    <!-- http://purl.imsglobal.org/caliper/maxMetricValue -->

    <owl:DatatypeProperty rdf:about="http://purl.imsglobal.org/caliper/maxMetricValue">
        <rdfs:domain rdf:resource="http://purl.imsglobal.org/caliper/AggregateMeasure"/>
        <rdfs:range rdf:resource="http://www.w3.org/2001/XMLSchema#decimal"/>
        <rdfs:comment xml:lang="en">An integer value representing the total possible curricular progress the actor can make in the context of the application.</rdfs:comment>
        <rdfs:isDefinedBy rdf:datatype="http://www.w3.org/2001/XMLSchema#string">http://purl.imsglobal.org/caliper</rdfs:isDefinedBy>
        <rdfs:label xml:lang="en">maxMetricValue</rdfs:label>
    </owl:DatatypeProperty>
    


    <!-- http://purl.imsglobal.org/caliper/maxResultScore -->

    <owl:DatatypeProperty rdf:about="http://purl.imsglobal.org/caliper/maxResultScore">
        <rdf:type rdf:resource="http://www.w3.org/2002/07/owl#FunctionalProperty"/>
        <rdfs:domain rdf:resource="http://purl.imsglobal.org/caliper/Result"/>
        <rdfs:range rdf:resource="http://www.w3.org/2001/XMLSchema#decimal"/>
        <rdfs:comment xml:lang="en">The maximum score permitted for a Result.</rdfs:comment>
        <rdfs:isDefinedBy rdf:datatype="http://www.w3.org/2001/XMLSchema#string">http://purl.imsglobal.org/caliper</rdfs:isDefinedBy>
        <rdfs:label xml:lang="en">maxResultScore</rdfs:label>
    </owl:DatatypeProperty>
    


    <!-- http://purl.imsglobal.org/caliper/maxScore -->

    <owl:DatatypeProperty rdf:about="http://purl.imsglobal.org/caliper/maxScore">
        <rdf:type rdf:resource="http://www.w3.org/2002/07/owl#FunctionalProperty"/>
        <rdfs:domain>
            <owl:Class>
                <owl:unionOf rdf:parseType="Collection">
                    <rdf:Description rdf:about="http://purl.imsglobal.org/caliper/DigitalResource"/>
                    <rdf:Description rdf:about="http://purl.imsglobal.org/caliper/Score"/>
                </owl:unionOf>
            </owl:Class>
        </rdfs:domain>
        <rdfs:range rdf:resource="http://www.w3.org/2001/XMLSchema#decimal"/>
        <rdfs:comment xml:lang="en">A non-negative integer indicating the maximum score permitted.</rdfs:comment>
        <rdfs:isDefinedBy rdf:datatype="http://www.w3.org/2001/XMLSchema#string">http://purl.imsglobal.org/caliper</rdfs:isDefinedBy>
        <rdfs:label xml:lang="en">maxScore</rdfs:label>
    </owl:DatatypeProperty>
    


    <!-- http://purl.imsglobal.org/caliper/maxSelections -->

    <owl:DatatypeProperty rdf:about="http://purl.imsglobal.org/caliper/maxSelections">
        <rdf:type rdf:resource="http://www.w3.org/2002/07/owl#FunctionalProperty"/>
        <rdfs:domain rdf:resource="http://purl.imsglobal.org/caliper/MultiSelectScale"/>
        <rdfs:range rdf:resource="http://www.w3.org/2001/XMLSchema#integer"/>
        <owl:propertyDisjointWith rdf:resource="http://purl.imsglobal.org/caliper/minSelections"/>
        <rdfs:comment xml:lang="en">Indicates the maximum number of selections that can be chosen.</rdfs:comment>
        <rdfs:isDefinedBy rdf:datatype="http://www.w3.org/2001/XMLSchema#string">https://purl.imsglobal.org/caliper</rdfs:isDefinedBy>
        <rdfs:label xml:lang="en">maxSelections</rdfs:label>
    </owl:DatatypeProperty>
    


    <!-- http://purl.imsglobal.org/caliper/maxSubmits -->

    <owl:DatatypeProperty rdf:about="http://purl.imsglobal.org/caliper/maxSubmits">
        <rdf:type rdf:resource="http://www.w3.org/2002/07/owl#FunctionalProperty"/>
        <rdfs:domain rdf:resource="http://purl.imsglobal.org/caliper/DigitalResource"/>
        <rdfs:range rdf:resource="http://www.w3.org/2001/XMLSchema#nonNegativeInteger"/>
        <rdfs:comment xml:lang="en">A non-negative integer indicating the number of permitted submissions.</rdfs:comment>
        <rdfs:isDefinedBy rdf:datatype="http://www.w3.org/2001/XMLSchema#string">http://purl.imsglobal.org/caliper</rdfs:isDefinedBy>
        <rdfs:label xml:lang="en">maxSubmits</rdfs:label>
    </owl:DatatypeProperty>
    


    <!-- http://purl.imsglobal.org/caliper/maxValue -->

    <owl:DatatypeProperty rdf:about="http://purl.imsglobal.org/caliper/maxValue">
        <rdf:type rdf:resource="http://www.w3.org/2002/07/owl#FunctionalProperty"/>
        <rdfs:domain rdf:resource="http://purl.imsglobal.org/caliper/NumericScale"/>
        <rdfs:range rdf:resource="http://www.w3.org/2001/XMLSchema#decimal"/>
        <owl:propertyDisjointWith rdf:resource="http://purl.imsglobal.org/caliper/minValue"/>
        <rdfs:comment xml:lang="en">A decimal value used to determine the maximum value of the  NumericScale.</rdfs:comment>
        <rdfs:isDefinedBy rdf:datatype="http://www.w3.org/2001/XMLSchema#string">https://purl.imsglobal.org/caliper</rdfs:isDefinedBy>
        <rdfs:label xml:lang="en">maxValue</rdfs:label>
    </owl:DatatypeProperty>
    


    <!-- http://purl.imsglobal.org/caliper/mediaType -->

    <owl:DatatypeProperty rdf:about="http://purl.imsglobal.org/caliper/mediaType">
        <rdf:type rdf:resource="http://www.w3.org/2002/07/owl#FunctionalProperty"/>
        <rdfs:domain rdf:resource="http://purl.imsglobal.org/caliper/DigitalResource"/>
        <rdfs:range rdf:resource="http://www.w3.org/2001/XMLSchema#string"/>
        <rdfs:comment xml:lang="en">A string value drawn from the list of IANA approved media types and subtypes that identifies the file format of a resource.</rdfs:comment>
        <rdfs:isDefinedBy rdf:datatype="http://www.w3.org/2001/XMLSchema#string">http://purl.imsglobal.org/caliper</rdfs:isDefinedBy>
        <rdfs:label xml:lang="en">mediaType</rdfs:label>
    </owl:DatatypeProperty>
    


    <!-- http://purl.imsglobal.org/caliper/metric -->

    <owl:DatatypeProperty rdf:about="http://purl.imsglobal.org/caliper/metric">
        <rdfs:subPropertyOf rdf:resource="http://www.w3.org/2002/07/owl#topDataProperty"/>
        <rdfs:domain rdf:resource="http://purl.imsglobal.org/caliper/AggregateMeasure"/>
        <rdfs:comment xml:lang="en">The standard of measurement associated with the progress value.</rdfs:comment>
        <rdfs:isDefinedBy rdf:datatype="http://www.w3.org/2001/XMLSchema#string">http://purl.imsglobal.org/caliper</rdfs:isDefinedBy>
        <rdfs:label xml:lang="en">metric</rdfs:label>
    </owl:DatatypeProperty>
    


    <!-- http://purl.imsglobal.org/caliper/metricValue -->

    <owl:DatatypeProperty rdf:about="http://purl.imsglobal.org/caliper/metricValue">
        <rdf:type rdf:resource="http://www.w3.org/2002/07/owl#FunctionalProperty"/>
        <rdfs:domain rdf:resource="http://purl.imsglobal.org/caliper/AggregateMeasure"/>
        <rdfs:range rdf:resource="http://www.w3.org/2001/XMLSchema#decimal"/>
        <rdfs:comment xml:lang="en">An integer value representing the total curricular progress the actor has made in the context of the application.</rdfs:comment>
        <rdfs:isDefinedBy rdf:datatype="http://www.w3.org/2001/XMLSchema#string">http://purl.imsglobal.org/caliper</rdfs:isDefinedBy>
        <rdfs:label xml:lang="en">metricValue</rdfs:label>
    </owl:DatatypeProperty>
    


    <!-- http://purl.imsglobal.org/caliper/minLabel -->

    <owl:DatatypeProperty rdf:about="http://purl.imsglobal.org/caliper/minLabel">
        <rdf:type rdf:resource="http://www.w3.org/2002/07/owl#FunctionalProperty"/>
        <rdfs:domain rdf:resource="http://purl.imsglobal.org/caliper/NumericScale"/>
        <rdfs:range rdf:resource="http://www.w3.org/2001/XMLSchema#string"/>
        <rdfs:comment xml:lang="en">The label for the minimum value.</rdfs:comment>
        <rdfs:isDefinedBy rdf:datatype="http://www.w3.org/2001/XMLSchema#string">https://purl.imsglobal.org/caliper</rdfs:isDefinedBy>
        <rdfs:label xml:lang="en">minLabel</rdfs:label>
    </owl:DatatypeProperty>
    


    <!-- http://purl.imsglobal.org/caliper/minSelections -->

    <owl:DatatypeProperty rdf:about="http://purl.imsglobal.org/caliper/minSelections">
        <rdf:type rdf:resource="http://www.w3.org/2002/07/owl#FunctionalProperty"/>
        <rdfs:domain rdf:resource="http://purl.imsglobal.org/caliper/MultiSelectScale"/>
        <rdfs:range rdf:resource="http://www.w3.org/2001/XMLSchema#integer"/>
        <rdfs:comment xml:lang="en">Indicates the minimum number of selections that can be chosen.</rdfs:comment>
        <rdfs:isDefinedBy rdf:datatype="http://www.w3.org/2001/XMLSchema#string">https://purl.imsglobal.org/caliper</rdfs:isDefinedBy>
        <rdfs:label xml:lang="en">minSelections</rdfs:label>
    </owl:DatatypeProperty>
    


    <!-- http://purl.imsglobal.org/caliper/minValue -->

    <owl:DatatypeProperty rdf:about="http://purl.imsglobal.org/caliper/minValue">
        <rdf:type rdf:resource="http://www.w3.org/2002/07/owl#FunctionalProperty"/>
        <rdfs:domain rdf:resource="http://purl.imsglobal.org/caliper/NumericScale"/>
        <rdfs:range rdf:resource="http://www.w3.org/2001/XMLSchema#decimal"/>
        <rdfs:comment xml:lang="en">A decimal value used to determine the minimum value of the  NumericScale.</rdfs:comment>
        <rdfs:isDefinedBy rdf:datatype="http://www.w3.org/2001/XMLSchema#string">https://purl.imsglobal.org/caliper</rdfs:isDefinedBy>
        <rdfs:label xml:lang="en">minValue</rdfs:label>
    </owl:DatatypeProperty>
    


    <!-- http://purl.imsglobal.org/caliper/muted -->

    <owl:DatatypeProperty rdf:about="http://purl.imsglobal.org/caliper/muted">
        <rdf:type rdf:resource="http://www.w3.org/2002/07/owl#FunctionalProperty"/>
        <rdfs:domain rdf:resource="http://purl.imsglobal.org/caliper/AudioObject"/>
        <rdfs:range rdf:resource="http://www.w3.org/2001/XMLSchema#boolean"/>
        <rdfs:comment xml:lang="en">An optional boolean value indicating whether or not the MediaObject has been muted .</rdfs:comment>
        <rdfs:isDefinedBy rdf:datatype="http://www.w3.org/2001/XMLSchema#string">http://purl.imsglobal.org/caliper</rdfs:isDefinedBy>
        <rdfs:label xml:lang="en">muted</rdfs:label>
    </owl:DatatypeProperty>
    


    <!-- http://purl.imsglobal.org/caliper/name -->

    <owl:DatatypeProperty rdf:about="http://purl.imsglobal.org/caliper/name">
        <rdf:type rdf:resource="http://www.w3.org/2002/07/owl#FunctionalProperty"/>
        <rdfs:domain rdf:resource="http://purl.imsglobal.org/caliper/Entity"/>
        <rdfs:range rdf:resource="http://www.w3.org/2001/XMLSchema#string"/>
        <rdfs:comment xml:lang="en">A string value comprising a word or phrase by which the resource is known.</rdfs:comment>
        <rdfs:isDefinedBy rdf:datatype="http://www.w3.org/2001/XMLSchema#string">http://purl.imsglobal.org/caliper</rdfs:isDefinedBy>
        <rdfs:label xml:lang="en">name</rdfs:label>
    </owl:DatatypeProperty>
    


    <!-- http://purl.imsglobal.org/caliper/normalScore -->

    <owl:DatatypeProperty rdf:about="http://purl.imsglobal.org/caliper/normalScore">
        <rdf:type rdf:resource="http://www.w3.org/2002/07/owl#FunctionalProperty"/>
        <rdfs:domain rdf:resource="http://purl.imsglobal.org/caliper/Result"/>
        <rdfs:range rdf:resource="http://www.w3.org/2001/XMLSchema#decimal"/>
        <rdfs:comment xml:lang="en">The score earned by the learner before adding the extraCreditScore, subtracting the penaltyScore or applying the curveFactor, if any.</rdfs:comment>
        <rdfs:isDefinedBy rdf:datatype="http://www.w3.org/2001/XMLSchema#string">http://purl.imsglobal.org/caliper</rdfs:isDefinedBy>
        <rdfs:label xml:lang="en">normalScore</rdfs:label>
        <owl:deprecated rdf:datatype="http://www.w3.org/2001/XMLSchema#boolean">true</owl:deprecated>
    </owl:DatatypeProperty>
    


    <!-- http://purl.imsglobal.org/caliper/objectType -->

    <owl:DatatypeProperty rdf:about="http://purl.imsglobal.org/caliper/objectType">
        <rdf:type rdf:resource="http://www.w3.org/2002/07/owl#FunctionalProperty"/>
        <rdfs:domain rdf:resource="http://purl.imsglobal.org/caliper/DigitalResource"/>
        <rdfs:comment xml:lang="en">A string value that designates the resource type.</rdfs:comment>
        <rdfs:isDefinedBy rdf:datatype="http://www.w3.org/2001/XMLSchema#string">http://purl.imsglobal.org/caliper</rdfs:isDefinedBy>
        <rdfs:label xml:lang="en">objectType</rdfs:label>
        <owl:deprecated rdf:datatype="http://www.w3.org/2001/XMLSchema#boolean">true</owl:deprecated>
    </owl:DatatypeProperty>
    


    <!-- http://purl.imsglobal.org/caliper/orderedSelection -->

    <owl:DatatypeProperty rdf:about="http://purl.imsglobal.org/caliper/orderedSelection">
        <rdf:type rdf:resource="http://www.w3.org/2002/07/owl#FunctionalProperty"/>
        <rdfs:domain rdf:resource="http://purl.imsglobal.org/caliper/MultiSelectScale"/>
        <rdfs:range rdf:resource="http://www.w3.org/2001/XMLSchema#boolean"/>
        <rdfs:comment xml:lang="en">Indicates whether the order of the selected items is important.</rdfs:comment>
        <rdfs:isDefinedBy rdf:datatype="http://www.w3.org/2001/XMLSchema#string">https://purl.imsglobal.org/caliper</rdfs:isDefinedBy>
        <rdfs:label xml:lang="en">isOrderedSelection</rdfs:label>
    </owl:DatatypeProperty>
    


    <!-- http://purl.imsglobal.org/caliper/penaltyScore -->

    <owl:DatatypeProperty rdf:about="http://purl.imsglobal.org/caliper/penaltyScore">
        <rdf:type rdf:resource="http://www.w3.org/2002/07/owl#FunctionalProperty"/>
        <rdfs:domain rdf:resource="http://purl.imsglobal.org/caliper/Result"/>
        <rdfs:range rdf:resource="http://www.w3.org/2001/XMLSchema#decimal"/>
        <rdfs:comment xml:lang="en">The number of points deducted from the normalScore due to an infraction such as submitting an Attempt after the due date.</rdfs:comment>
        <rdfs:isDefinedBy rdf:datatype="http://www.w3.org/2001/XMLSchema#string">http://purl.imsglobal.org/caliper</rdfs:isDefinedBy>
        <rdfs:label xml:lang="en">penaltyScore</rdfs:label>
        <owl:deprecated rdf:datatype="http://www.w3.org/2001/XMLSchema#boolean">true</owl:deprecated>
    </owl:DatatypeProperty>
    


    <!-- http://purl.imsglobal.org/caliper/points -->

    <owl:DatatypeProperty rdf:about="http://purl.imsglobal.org/caliper/points">
        <rdf:type rdf:resource="http://www.w3.org/2002/07/owl#FunctionalProperty"/>
        <rdfs:domain>
            <owl:Class>
                <owl:unionOf rdf:parseType="Collection">
                    <rdf:Description rdf:about="http://purl.imsglobal.org/caliper/LikertScale"/>
                    <rdf:Description rdf:about="http://purl.imsglobal.org/caliper/MultiSelectScale"/>
                </owl:unionOf>
            </owl:Class>
        </rdfs:domain>
        <rdfs:range rdf:resource="http://www.w3.org/2001/XMLSchema#integer"/>
        <rdfs:comment xml:lang="en">A integer value used to determine the amount of points on the LikertScale.</rdfs:comment>
        <rdfs:isDefinedBy rdf:datatype="http://www.w3.org/2001/XMLSchema#string">https://purl.imsglobal.org/caliper</rdfs:isDefinedBy>
        <rdfs:label xml:lang="en">scalePoints</rdfs:label>
    </owl:DatatypeProperty>
    


    <!-- http://purl.imsglobal.org/caliper/question -->

    <owl:DatatypeProperty rdf:about="http://purl.imsglobal.org/caliper/question">
        <rdf:type rdf:resource="http://www.w3.org/2002/07/owl#FunctionalProperty"/>
        <rdfs:domain rdf:resource="http://purl.imsglobal.org/caliper/Scale"/>
        <rdfs:range rdf:resource="http://www.w3.org/2001/XMLSchema#string"/>
        <rdfs:comment xml:lang="en">A string value comprising the question posed to be scaled.</rdfs:comment>
        <rdfs:isDefinedBy xml:lang="en">https://purl.imsglobal.org/caliper</rdfs:isDefinedBy>
        <rdfs:label xml:lang="en">question</rdfs:label>
    </owl:DatatypeProperty>
    


    <!-- http://purl.imsglobal.org/caliper/resultScore -->

    <owl:DatatypeProperty rdf:about="http://purl.imsglobal.org/caliper/resultScore">
        <rdf:type rdf:resource="http://www.w3.org/2002/07/owl#FunctionalProperty"/>
        <rdfs:domain rdf:resource="http://purl.imsglobal.org/caliper/Result"/>
        <rdfs:range rdf:resource="http://www.w3.org/2001/XMLSchema#decimal"/>
        <rdfs:comment xml:lang="en">The result score awarded to the learner.  A result score can be updated.</rdfs:comment>
        <rdfs:isDefinedBy rdf:datatype="http://www.w3.org/2001/XMLSchema#string">http://purl.imsglobal.org/caliper</rdfs:isDefinedBy>
        <rdfs:label xml:lang="en">resultScore</rdfs:label>
    </owl:DatatypeProperty>
    


    <!-- http://purl.imsglobal.org/caliper/scoreGiven -->

    <owl:DatatypeProperty rdf:about="http://purl.imsglobal.org/caliper/scoreGiven">
        <rdf:type rdf:resource="http://www.w3.org/2002/07/owl#FunctionalProperty"/>
        <rdfs:domain rdf:resource="http://purl.imsglobal.org/caliper/Score"/>
        <rdfs:range rdf:resource="http://www.w3.org/2001/XMLSchema#decimal"/>
        <rdfs:comment xml:lang="en">The score value.</rdfs:comment>
        <rdfs:isDefinedBy rdf:datatype="http://www.w3.org/2001/XMLSchema#string">http://purl.imsglobal.org/caliper</rdfs:isDefinedBy>
        <rdfs:label xml:lang="en">scoreGiven</rdfs:label>
    </owl:DatatypeProperty>
    


    <!-- http://purl.imsglobal.org/caliper/searchResultsItemCount -->

    <owl:DatatypeProperty rdf:about="http://purl.imsglobal.org/caliper/searchResultsItemCount">
        <rdf:type rdf:resource="http://www.w3.org/2002/07/owl#FunctionalProperty"/>
        <rdfs:domain rdf:resource="http://purl.imsglobal.org/caliper/SearchResponse"/>
        <rdfs:range rdf:resource="http://www.w3.org/2001/XMLSchema#nonNegativeInteger"/>
        <rdfs:comment xml:lang="en">A total count of searchResults returned. If the Query submitted returned no results the count equal to zero (0).</rdfs:comment>
        <rdfs:isDefinedBy rdf:datatype="http://www.w3.org/2001/XMLSchema#string">http://purl.imsglobal.org/caliper</rdfs:isDefinedBy>
        <rdfs:label xml:lang="en">searchResultsItemCount</rdfs:label>
    </owl:DatatypeProperty>
    


    <!-- http://purl.imsglobal.org/caliper/searchTerms -->

    <owl:DatatypeProperty rdf:about="http://purl.imsglobal.org/caliper/searchTerms">
        <rdf:type rdf:resource="http://www.w3.org/2002/07/owl#FunctionalProperty"/>
        <rdfs:domain rdf:resource="http://purl.imsglobal.org/caliper/Query"/>
        <rdfs:range rdf:resource="http://www.w3.org/2001/XMLSchema#string"/>
        <rdfs:comment xml:lang="en">The search terms employed by the creator of a Query.</rdfs:comment>
        <rdfs:isDefinedBy rdf:datatype="http://www.w3.org/2001/XMLSchema#string">http://purl.imsglobal.org/caliper</rdfs:isDefinedBy>
        <rdfs:label xml:lang="en">searchTerms</rdfs:label>
    </owl:DatatypeProperty>
    


    <!-- http://purl.imsglobal.org/caliper/selectionText -->

    <owl:DatatypeProperty rdf:about="http://purl.imsglobal.org/caliper/selectionText">
        <rdf:type rdf:resource="http://www.w3.org/2002/07/owl#FunctionalProperty"/>
        <rdfs:domain rdf:resource="http://purl.imsglobal.org/caliper/HighlightAnnotation"/>
        <rdfs:range rdf:resource="http://www.w3.org/2001/XMLSchema#string"/>
        <rdfs:comment xml:lang="en">A string value representing a plain-text rendering of the selected segment of the annotated resource.</rdfs:comment>
        <rdfs:isDefinedBy rdf:datatype="http://www.w3.org/2001/XMLSchema#string">http://purl.imsglobal.org/caliper</rdfs:isDefinedBy>
        <rdfs:label xml:lang="en">selectionText</rdfs:label>
    </owl:DatatypeProperty>
    


    <!-- http://purl.imsglobal.org/caliper/sendTime -->

    <owl:DatatypeProperty rdf:about="http://purl.imsglobal.org/caliper/sendTime">
        <rdf:type rdf:resource="http://www.w3.org/2002/07/owl#FunctionalProperty"/>
        <rdfs:domain rdf:resource="http://purl.imsglobal.org/caliper/Envelope"/>
        <rdfs:range rdf:resource="http://www.w3.org/2001/XMLSchema#dateTime"/>
        <rdfs:comment xml:lang="en">Envelope send time.</rdfs:comment>
        <rdfs:isDefinedBy rdf:datatype="http://www.w3.org/2001/XMLSchema#string">http://purl.imsglobal.org/caliper</rdfs:isDefinedBy>
        <rdfs:label xml:lang="en">sendTime</rdfs:label>
    </owl:DatatypeProperty>
    


    <!-- http://purl.imsglobal.org/caliper/sensor -->

    <owl:DatatypeProperty rdf:about="http://purl.imsglobal.org/caliper/sensor">
        <rdf:type rdf:resource="http://www.w3.org/2002/07/owl#FunctionalProperty"/>
        <rdfs:domain rdf:resource="http://purl.imsglobal.org/caliper/Envelope"/>
        <rdfs:range rdf:resource="http://www.w3.org/2001/XMLSchema#string"/>
        <rdfs:comment xml:lang="en">Sensor identifier.</rdfs:comment>
        <rdfs:isDefinedBy rdf:datatype="http://www.w3.org/2001/XMLSchema#string">http://purl.imsglobal.org/caliper</rdfs:isDefinedBy>
        <rdfs:label xml:lang="en">sensor</rdfs:label>
    </owl:DatatypeProperty>
    


    <!-- http://purl.imsglobal.org/caliper/start -->

    <owl:DatatypeProperty rdf:about="http://purl.imsglobal.org/caliper/start">
        <rdf:type rdf:resource="http://www.w3.org/2002/07/owl#FunctionalProperty"/>
        <rdfs:domain rdf:resource="http://purl.imsglobal.org/caliper/TextPositionSelector"/>
        <rdfs:range rdf:resource="http://www.w3.org/2001/XMLSchema#nonNegativeInteger"/>
        <rdfs:comment xml:lang="en">The starting position of a segment of text. The first character in the full text is position 0. The character that represents the start position is included within the selected segment.</rdfs:comment>
        <rdfs:isDefinedBy rdf:datatype="http://www.w3.org/2001/XMLSchema#string">http://purl.imsglobal.org/caliper</rdfs:isDefinedBy>
        <rdfs:label xml:lang="en">start</rdfs:label>
    </owl:DatatypeProperty>
    


    <!-- http://purl.imsglobal.org/caliper/startedAtTime -->

    <owl:DatatypeProperty rdf:about="http://purl.imsglobal.org/caliper/startedAtTime">
        <rdf:type rdf:resource="http://www.w3.org/2002/07/owl#FunctionalProperty"/>
        <rdfs:domain>
            <owl:Class>
                <owl:unionOf rdf:parseType="Collection">
                    <rdf:Description rdf:about="http://purl.imsglobal.org/caliper/AggregateMeasure"/>
                    <rdf:Description rdf:about="http://purl.imsglobal.org/caliper/Attempt"/>
                    <rdf:Description rdf:about="http://purl.imsglobal.org/caliper/Response"/>
                    <rdf:Description rdf:about="http://purl.imsglobal.org/caliper/Session"/>
                </owl:unionOf>
            </owl:Class>
        </rdfs:domain>
        <rdfs:range rdf:resource="http://www.w3.org/2001/XMLSchema#dateTime"/>
        <rdfs:comment xml:lang="en">A date and time value expressed with millisecond precision that describes when the activity commenced.</rdfs:comment>
        <rdfs:isDefinedBy rdf:datatype="http://www.w3.org/2001/XMLSchema#string">http://purl.imsglobal.org/caliper</rdfs:isDefinedBy>
        <rdfs:label xml:lang="en">startedAtTime</rdfs:label>
    </owl:DatatypeProperty>
    


    <!-- http://purl.imsglobal.org/caliper/step -->

    <owl:DatatypeProperty rdf:about="http://purl.imsglobal.org/caliper/step">
        <rdf:type rdf:resource="http://www.w3.org/2002/07/owl#FunctionalProperty"/>
        <rdfs:domain rdf:resource="http://purl.imsglobal.org/caliper/NumericScale"/>
        <rdfs:range rdf:resource="http://www.w3.org/2001/XMLSchema#decimal"/>
        <rdfs:comment xml:lang="en">Indicates the decimal step used for determining the options between the minimum and maximum values.</rdfs:comment>
        <rdfs:isDefinedBy rdf:datatype="http://www.w3.org/2001/XMLSchema#string">https://purl.imsglobal.org/caliper</rdfs:isDefinedBy>
        <rdfs:label xml:lang="en">step</rdfs:label>
    </owl:DatatypeProperty>
    


    <!-- http://purl.imsglobal.org/caliper/storageName -->

    <owl:DatatypeProperty rdf:about="http://purl.imsglobal.org/caliper/storageName">
        <rdf:type rdf:resource="http://www.w3.org/2002/07/owl#FunctionalProperty"/>
        <rdfs:domain rdf:resource="http://purl.imsglobal.org/caliper/DigitalResource"/>
        <rdfs:range rdf:resource="http://www.w3.org/2001/XMLSchema#string"/>
        <rdfs:comment xml:lang="en">The name of resource when stored in a file system.</rdfs:comment>
        <rdfs:isDefinedBy rdf:datatype="http://www.w3.org/2001/XMLSchema#string">http://purl.imsglobal.org/caliper</rdfs:isDefinedBy>
        <rdfs:label xml:lang="en">storageName</rdfs:label>
    </owl:DatatypeProperty>
    


    <!-- http://purl.imsglobal.org/caliper/tags -->

    <owl:DatatypeProperty rdf:about="http://purl.imsglobal.org/caliper/tags">
        <rdf:type rdf:resource="http://www.w3.org/2002/07/owl#FunctionalProperty"/>
        <rdfs:domain rdf:resource="http://purl.imsglobal.org/caliper/TagAnnotation"/>
        <rdfs:range rdf:resource="http://www.w3.org/2001/XMLSchema#string"/>
        <rdfs:comment xml:lang="en">An ordered collection of one or more string values that represent labels or tags associated with the annotated DigitalResource.</rdfs:comment>
        <rdfs:isDefinedBy rdf:datatype="http://www.w3.org/2001/XMLSchema#string">http://purl.imsglobal.org/caliper</rdfs:isDefinedBy>
        <rdfs:label xml:lang="en">tags</rdfs:label>
    </owl:DatatypeProperty>
    


    <!-- http://purl.imsglobal.org/caliper/totalScore -->

    <owl:DatatypeProperty rdf:about="http://purl.imsglobal.org/caliper/totalScore">
        <rdf:type rdf:resource="http://www.w3.org/2002/07/owl#FunctionalProperty"/>
        <rdfs:domain rdf:resource="http://purl.imsglobal.org/caliper/Result"/>
        <rdfs:range rdf:resource="http://www.w3.org/2001/XMLSchema#decimal"/>
        <rdfs:comment xml:lang="en">A score earned by the learner equal to the sum of normalScore + extraCreditScore - penaltyScore. This value does not take into account the effects of curving.</rdfs:comment>
        <rdfs:isDefinedBy rdf:datatype="http://www.w3.org/2001/XMLSchema#string">http://purl.imsglobal.org/caliper</rdfs:isDefinedBy>
        <rdfs:label xml:lang="en">totalScore</rdfs:label>
        <owl:deprecated rdf:datatype="http://www.w3.org/2001/XMLSchema#boolean">true</owl:deprecated>
    </owl:DatatypeProperty>
    


    <!-- http://purl.imsglobal.org/caliper/type -->

    <owl:DatatypeProperty rdf:about="http://purl.imsglobal.org/caliper/type">
        <rdf:type rdf:resource="http://www.w3.org/2002/07/owl#FunctionalProperty"/>
        <rdfs:domain>
            <owl:Class>
                <owl:unionOf rdf:parseType="Collection">
                    <rdf:Description rdf:about="http://purl.imsglobal.org/caliper/Entity"/>
                    <rdf:Description rdf:about="http://purl.imsglobal.org/caliper/Event"/>
                </owl:unionOf>
            </owl:Class>
        </rdfs:domain>
        <rdfs:range rdf:resource="http://www.w3.org/2001/XMLSchema#string"/>
        <rdfs:comment xml:lang="en">A string value corresponding to the Class name or label of an Event or Entity.</rdfs:comment>
        <rdfs:isDefinedBy rdf:datatype="http://www.w3.org/2001/XMLSchema#string">http://purl.imsglobal.org/caliper</rdfs:isDefinedBy>
        <rdfs:label xml:lang="en">type</rdfs:label>
    </owl:DatatypeProperty>
    


    <!-- http://purl.imsglobal.org/caliper/value -->

    <owl:DatatypeProperty rdf:about="http://purl.imsglobal.org/caliper/value">
        <rdf:type rdf:resource="http://www.w3.org/2002/07/owl#FunctionalProperty"/>
        <rdfs:domain>
            <owl:Class>
                <owl:unionOf rdf:parseType="Collection">
                    <rdf:Description rdf:about="http://purl.imsglobal.org/caliper/MultipleChoiceResponse"/>
                    <rdf:Description rdf:about="http://purl.imsglobal.org/caliper/TrueFalseResponse"/>
                </owl:unionOf>
            </owl:Class>
        </rdfs:domain>
        <rdfs:range rdf:resource="http://www.w3.org/2001/XMLSchema#string"/>
        <rdfs:comment xml:lang="en">A string value that represents the options selected.</rdfs:comment>
        <rdfs:isDefinedBy rdf:datatype="http://www.w3.org/2001/XMLSchema#string">http://purl.imsglobal.org/caliper</rdfs:isDefinedBy>
        <rdfs:label xml:lang="en">value</rdfs:label>
    </owl:DatatypeProperty>
    


    <!-- http://purl.imsglobal.org/caliper/values -->

    <owl:DatatypeProperty rdf:about="http://purl.imsglobal.org/caliper/values">
        <rdfs:domain>
            <owl:Class>
                <owl:unionOf rdf:parseType="Collection">
                    <rdf:Description rdf:about="http://purl.imsglobal.org/caliper/FillinBlankResponse"/>
                    <rdf:Description rdf:about="http://purl.imsglobal.org/caliper/MultipleResponseResponse"/>
                    <rdf:Description rdf:about="http://purl.imsglobal.org/caliper/SelectTextResponse"/>
                </owl:unionOf>
            </owl:Class>
        </rdfs:domain>
        <rdfs:range rdf:resource="http://www.w3.org/2001/XMLSchema#string"/>
        <rdfs:comment xml:lang="en">An ordered collection of one or more selected options.</rdfs:comment>
        <rdfs:isDefinedBy rdf:datatype="http://www.w3.org/2001/XMLSchema#string">http://purl.imsglobal.org/caliper</rdfs:isDefinedBy>
        <rdfs:label xml:lang="en">values</rdfs:label>
    </owl:DatatypeProperty>
    


    <!-- http://purl.imsglobal.org/caliper/version -->

    <owl:DatatypeProperty rdf:about="http://purl.imsglobal.org/caliper/version">
        <rdf:type rdf:resource="http://www.w3.org/2002/07/owl#FunctionalProperty"/>
        <rdfs:domain>
            <owl:Class>
                <owl:unionOf rdf:parseType="Collection">
                    <rdf:Description rdf:about="http://purl.imsglobal.org/caliper/DigitalResource"/>
                    <rdf:Description rdf:about="http://purl.imsglobal.org/caliper/SoftwareApplication"/>
                </owl:unionOf>
            </owl:Class>
        </rdfs:domain>
        <rdfs:range rdf:resource="http://www.w3.org/2001/XMLSchema#string"/>
        <rdfs:comment xml:lang="en">A string value that designates the current form or version of the resource.</rdfs:comment>
        <rdfs:isDefinedBy rdf:datatype="http://www.w3.org/2001/XMLSchema#string">http://purl.imsglobal.org/caliper</rdfs:isDefinedBy>
        <rdfs:label xml:lang="en">version</rdfs:label>
    </owl:DatatypeProperty>
    


    <!-- http://purl.imsglobal.org/caliper/volumeLevel -->

    <owl:DatatypeProperty rdf:about="http://purl.imsglobal.org/caliper/volumeLevel">
        <rdf:type rdf:resource="http://www.w3.org/2002/07/owl#FunctionalProperty"/>
        <rdfs:domain rdf:resource="http://purl.imsglobal.org/caliper/AudioObject"/>
        <rdfs:range rdf:resource="http://www.w3.org/2001/XMLSchema#string"/>
        <rdfs:comment xml:lang="en">The current volume level.</rdfs:comment>
        <rdfs:isDefinedBy rdf:datatype="http://www.w3.org/2001/XMLSchema#string">http://purl.imsglobal.org/caliper</rdfs:isDefinedBy>
        <rdfs:label xml:lang="en">volumeLevel</rdfs:label>
    </owl:DatatypeProperty>
    


    <!-- http://purl.imsglobal.org/caliper/volumeMax -->

    <owl:DatatypeProperty rdf:about="http://purl.imsglobal.org/caliper/volumeMax">
        <rdf:type rdf:resource="http://www.w3.org/2002/07/owl#FunctionalProperty"/>
        <rdfs:domain rdf:resource="http://purl.imsglobal.org/caliper/AudioObject"/>
        <rdfs:range rdf:resource="http://www.w3.org/2001/XMLSchema#string"/>
        <owl:propertyDisjointWith rdf:resource="http://purl.imsglobal.org/caliper/volumeMin"/>
        <rdfs:comment xml:lang="en">A string value indicating the maximum volume level permitted.</rdfs:comment>
        <rdfs:isDefinedBy rdf:datatype="http://www.w3.org/2001/XMLSchema#string">http://purl.imsglobal.org/caliper</rdfs:isDefinedBy>
        <rdfs:label xml:lang="en">volumeMax</rdfs:label>
    </owl:DatatypeProperty>
    


    <!-- http://purl.imsglobal.org/caliper/volumeMin -->

    <owl:DatatypeProperty rdf:about="http://purl.imsglobal.org/caliper/volumeMin">
        <rdf:type rdf:resource="http://www.w3.org/2002/07/owl#FunctionalProperty"/>
        <rdfs:domain rdf:resource="http://purl.imsglobal.org/caliper/AudioObject"/>
        <rdfs:range rdf:resource="http://www.w3.org/2001/XMLSchema#string"/>
        <rdfs:comment xml:lang="en">A string value indicating the minimum volume level permitted.</rdfs:comment>
        <rdfs:isDefinedBy rdf:datatype="http://www.w3.org/2001/XMLSchema#string">http://purl.imsglobal.org/caliper</rdfs:isDefinedBy>
        <rdfs:label xml:lang="en">volumeMin</rdfs:label>
    </owl:DatatypeProperty>
    


    <!-- 
    ///////////////////////////////////////////////////////////////////////////////////////
    //
    // Classes
    //
    ///////////////////////////////////////////////////////////////////////////////////////
     -->

    


    <!-- http://purl.imsglobal.org/caliper/Action -->

    <owl:Class rdf:about="http://purl.imsglobal.org/caliper/Action">
        <rdfs:comment xml:lang="en">Caliper includes a vocabulary of actions for describing learning interactions. Each action is based on the past-tense form of an English (en-US) verb. An action can also indicate a change in a particular characteristic of the object (e.g., resolution, size, speed, volume).  Each action is also linked to a brief definition (&quot;gloss&quot;) derived in whole or in part from Princeton University&apos;s WordNet® project in order to eliminate ambiguity and aid natural language processing.</rdfs:comment>
        <rdfs:isDefinedBy rdf:datatype="http://www.w3.org/2001/XMLSchema#string">http://purl.imsglobal.org/caliper</rdfs:isDefinedBy>
        <rdfs:label xml:lang="en">Action</rdfs:label>
    </owl:Class>
    


    <!-- http://purl.imsglobal.org/caliper/Agent -->

    <owl:Class rdf:about="http://purl.imsglobal.org/caliper/Agent">
        <rdfs:subClassOf rdf:resource="http://purl.imsglobal.org/caliper/Entity"/>
        <rdfs:comment xml:lang="en">A Caliper Agent is a generic type that represents an Entity that can initiate or perform an action.  Utilize Agent only if no suitable subtype exists to represent the actor being described.</rdfs:comment>
        <rdfs:isDefinedBy rdf:datatype="http://www.w3.org/2001/XMLSchema#string">http://purl.imsglobal.org/caliper</rdfs:isDefinedBy>
        <rdfs:label xml:lang="en">Agent</rdfs:label>
    </owl:Class>
    


    <!-- http://purl.imsglobal.org/caliper/AggregateMeasure -->

    <owl:Class rdf:about="http://purl.imsglobal.org/caliper/AggregateMeasure">
        <rdfs:subClassOf rdf:resource="http://purl.imsglobal.org/caliper/Entity"/>
        <rdfs:comment xml:lang="en">A Caliper AggregateMeasure represents an aggregated measure of a learner&apos;s use of a learning tool. For example, an AggregateMeasure may represent the total time on task a learner has spent on a learning tool over a period of time.</rdfs:comment>
        <rdfs:isDefinedBy rdf:datatype="http://www.w3.org/2001/XMLSchema#string">http://purl.imsglobal.org/caliper</rdfs:isDefinedBy>
        <rdfs:label xml:lang="en">AggregateMeasure</rdfs:label>
    </owl:Class>
    


    <!-- http://purl.imsglobal.org/caliper/AggregateMeasureCollection -->

    <owl:Class rdf:about="http://purl.imsglobal.org/caliper/AggregateMeasureCollection">
        <rdfs:subClassOf rdf:resource="http://purl.imsglobal.org/caliper/Collection"/>
        <rdfs:subClassOf>
            <owl:Class>
                <owl:intersectionOf rdf:parseType="Collection">
                    <owl:Restriction>
                        <owl:onProperty rdf:resource="http://purl.imsglobal.org/caliper/items"/>
                        <owl:someValuesFrom rdf:resource="http://purl.imsglobal.org/caliper/Entity"/>
                    </owl:Restriction>
                    <owl:Restriction>
                        <owl:onProperty rdf:resource="http://purl.imsglobal.org/caliper/items"/>
                        <owl:allValuesFrom rdf:resource="http://purl.imsglobal.org/caliper/AggregateMeasure"/>
                    </owl:Restriction>
                </owl:intersectionOf>
            </owl:Class>
        </rdfs:subClassOf>
        <rdfs:comment xml:lang="en">A Caliper AggregateMeasureCollection represents an unordered collection of AggregateMeasure entities.</rdfs:comment>
        <rdfs:isDefinedBy rdf:datatype="http://www.w3.org/2001/XMLSchema#string">http://purl.imsglobal.org/caliper</rdfs:isDefinedBy>
        <rdfs:label xml:lang="en">AggregateMeasureCollection</rdfs:label>
    </owl:Class>
    


    <!-- http://purl.imsglobal.org/caliper/Annotation -->

    <owl:Class rdf:about="http://purl.imsglobal.org/caliper/Annotation">
        <rdfs:subClassOf rdf:resource="http://purl.imsglobal.org/caliper/Entity"/>
        <rdfs:subClassOf>
            <owl:Class>
                <owl:intersectionOf rdf:parseType="Collection">
                    <owl:Restriction>
                        <owl:onProperty rdf:resource="http://purl.imsglobal.org/caliper/annotated"/>
                        <owl:someValuesFrom rdf:resource="http://purl.imsglobal.org/caliper/Entity"/>
                    </owl:Restriction>
                    <owl:Restriction>
                        <owl:onProperty rdf:resource="http://purl.imsglobal.org/caliper/annotated"/>
                        <owl:allValuesFrom rdf:resource="http://purl.imsglobal.org/caliper/DigitalResource"/>
                    </owl:Restriction>
                </owl:intersectionOf>
            </owl:Class>
        </rdfs:subClassOf>
        <rdfs:subClassOf>
            <owl:Class>
                <owl:intersectionOf rdf:parseType="Collection">
                    <owl:Restriction>
                        <owl:onProperty rdf:resource="http://purl.imsglobal.org/caliper/annotator"/>
                        <owl:someValuesFrom rdf:resource="http://purl.imsglobal.org/caliper/Agent"/>
                    </owl:Restriction>
                    <owl:Restriction>
                        <owl:onProperty rdf:resource="http://purl.imsglobal.org/caliper/annotator"/>
                        <owl:allValuesFrom rdf:resource="http://purl.imsglobal.org/caliper/Person"/>
                    </owl:Restriction>
                </owl:intersectionOf>
            </owl:Class>
        </rdfs:subClassOf>
        <rdfs:comment xml:lang="en">A Caliper Annotation is a generic type that represents a comment, explanation, highlight, mark, note, question or tag linked to a DigitalResource.</rdfs:comment>
        <rdfs:isDefinedBy rdf:datatype="http://www.w3.org/2001/XMLSchema#string">http://purl.imsglobal.org/caliper</rdfs:isDefinedBy>
        <rdfs:label xml:lang="en">Annotation</rdfs:label>
    </owl:Class>
    


    <!-- http://purl.imsglobal.org/caliper/AnnotationEvent -->

    <owl:Class rdf:about="http://purl.imsglobal.org/caliper/AnnotationEvent">
        <rdfs:subClassOf rdf:resource="http://purl.imsglobal.org/caliper/Event"/>
        <rdfs:subClassOf>
            <owl:Class>
                <owl:intersectionOf rdf:parseType="Collection">
                    <owl:Restriction>
                        <owl:onProperty rdf:resource="http://purl.imsglobal.org/caliper/action"/>
                        <owl:someValuesFrom rdf:resource="http://purl.imsglobal.org/caliper/Action"/>
                    </owl:Restriction>
                    <owl:Restriction>
                        <owl:onProperty rdf:resource="http://purl.imsglobal.org/caliper/action"/>
                        <owl:someValuesFrom>
                            <owl:Class>
                                <owl:oneOf rdf:parseType="Collection">
                                    <rdf:Description rdf:about="http://purl.imsglobal.org/caliper/actions/Bookmarked"/>
                                    <rdf:Description rdf:about="http://purl.imsglobal.org/caliper/actions/Highlighted"/>
                                    <rdf:Description rdf:about="http://purl.imsglobal.org/caliper/actions/Shared"/>
                                    <rdf:Description rdf:about="http://purl.imsglobal.org/caliper/actions/Tagged"/>
                                </owl:oneOf>
                            </owl:Class>
                        </owl:someValuesFrom>
                    </owl:Restriction>
                </owl:intersectionOf>
            </owl:Class>
        </rdfs:subClassOf>
        <rdfs:subClassOf>
            <owl:Class>
                <owl:intersectionOf rdf:parseType="Collection">
                    <owl:Restriction>
                        <owl:onProperty rdf:resource="http://purl.imsglobal.org/caliper/actor"/>
                        <owl:someValuesFrom rdf:resource="http://purl.imsglobal.org/caliper/Agent"/>
                    </owl:Restriction>
                    <owl:Restriction>
                        <owl:onProperty rdf:resource="http://purl.imsglobal.org/caliper/actor"/>
                        <owl:allValuesFrom rdf:resource="http://purl.imsglobal.org/caliper/Person"/>
                    </owl:Restriction>
                </owl:intersectionOf>
            </owl:Class>
        </rdfs:subClassOf>
        <rdfs:subClassOf>
            <owl:Class>
                <owl:intersectionOf rdf:parseType="Collection">
                    <owl:Restriction>
                        <owl:onProperty rdf:resource="http://purl.imsglobal.org/caliper/object"/>
                        <owl:someValuesFrom rdf:resource="http://purl.imsglobal.org/caliper/Entity"/>
                    </owl:Restriction>
                    <owl:Restriction>
                        <owl:onProperty rdf:resource="http://purl.imsglobal.org/caliper/object"/>
                        <owl:allValuesFrom rdf:resource="http://purl.imsglobal.org/caliper/DigitalResource"/>
                    </owl:Restriction>
                </owl:intersectionOf>
            </owl:Class>
        </rdfs:subClassOf>
        <rdfs:subClassOf>
            <owl:Restriction>
                <owl:onProperty rdf:resource="http://purl.imsglobal.org/caliper/generated"/>
                <owl:someValuesFrom rdf:resource="http://purl.imsglobal.org/caliper/Annotation"/>
            </owl:Restriction>
        </rdfs:subClassOf>
        <rdfs:subClassOf>
            <owl:Restriction>
                <owl:onProperty rdf:resource="http://purl.imsglobal.org/caliper/target"/>
                <owl:someValuesFrom rdf:resource="http://purl.imsglobal.org/caliper/Frame"/>
            </owl:Restriction>
        </rdfs:subClassOf>
        <rdfs:comment xml:lang="en">A Caliper AnnotationEvent models the annotating of digital content. The resulting Annotation is also described and is subtyped for greater type specificity.</rdfs:comment>
        <rdfs:isDefinedBy rdf:datatype="http://www.w3.org/2001/XMLSchema#string">http://purl.imsglobal.org/caliper</rdfs:isDefinedBy>
        <rdfs:label xml:lang="en">AnnotationEvent</rdfs:label>
    </owl:Class>
    


    <!-- http://purl.imsglobal.org/caliper/Assessment -->

    <owl:Class rdf:about="http://purl.imsglobal.org/caliper/Assessment">
        <rdfs:subClassOf>
            <owl:Class>
                <owl:intersectionOf rdf:parseType="Collection">
                    <rdf:Description rdf:about="http://purl.imsglobal.org/caliper/AssignableDigitalResource"/>
                    <rdf:Description rdf:about="http://purl.imsglobal.org/caliper/DigitalResourceCollection"/>
                </owl:intersectionOf>
            </owl:Class>
        </rdfs:subClassOf>
        <rdfs:subClassOf>
            <owl:Class>
                <owl:intersectionOf rdf:parseType="Collection">
                    <owl:Restriction>
                        <owl:onProperty rdf:resource="http://purl.imsglobal.org/caliper/items"/>
                        <owl:someValuesFrom rdf:resource="http://purl.imsglobal.org/caliper/AssignableDigitalResource"/>
                    </owl:Restriction>
                    <owl:Restriction>
                        <owl:onProperty rdf:resource="http://purl.imsglobal.org/caliper/items"/>
                        <owl:allValuesFrom rdf:resource="http://purl.imsglobal.org/caliper/AssessmentItem"/>
                    </owl:Restriction>
                </owl:intersectionOf>
            </owl:Class>
        </rdfs:subClassOf>
        <rdfs:comment xml:lang="en">A Caliper Assessment represents an assessment instrument such as a test or quiz.</rdfs:comment>
        <rdfs:isDefinedBy rdf:datatype="http://www.w3.org/2001/XMLSchema#string">http://purl.imsglobal.org/caliper</rdfs:isDefinedBy>
        <rdfs:label xml:lang="en">Assessment</rdfs:label>
    </owl:Class>
    


    <!-- http://purl.imsglobal.org/caliper/AssessmentEvent -->

    <owl:Class rdf:about="http://purl.imsglobal.org/caliper/AssessmentEvent">
        <rdfs:subClassOf rdf:resource="http://purl.imsglobal.org/caliper/Event"/>
        <rdfs:subClassOf>
            <owl:Class>
                <owl:intersectionOf rdf:parseType="Collection">
                    <owl:Restriction>
                        <owl:onProperty rdf:resource="http://purl.imsglobal.org/caliper/action"/>
                        <owl:someValuesFrom rdf:resource="http://purl.imsglobal.org/caliper/Action"/>
                    </owl:Restriction>
                    <owl:Restriction>
                        <owl:onProperty rdf:resource="http://purl.imsglobal.org/caliper/action"/>
                        <owl:someValuesFrom>
                            <owl:Class>
                                <owl:oneOf rdf:parseType="Collection">
                                    <rdf:Description rdf:about="http://purl.imsglobal.org/caliper/actions/Paused"/>
                                    <rdf:Description rdf:about="http://purl.imsglobal.org/caliper/actions/Reset"/>
                                    <rdf:Description rdf:about="http://purl.imsglobal.org/caliper/actions/Restarted"/>
                                    <rdf:Description rdf:about="http://purl.imsglobal.org/caliper/actions/Resumed"/>
                                    <rdf:Description rdf:about="http://purl.imsglobal.org/caliper/actions/Started"/>
                                    <rdf:Description rdf:about="http://purl.imsglobal.org/caliper/actions/Submitted"/>
                                </owl:oneOf>
                            </owl:Class>
                        </owl:someValuesFrom>
                    </owl:Restriction>
                </owl:intersectionOf>
            </owl:Class>
        </rdfs:subClassOf>
        <rdfs:subClassOf>
            <owl:Class>
                <owl:intersectionOf rdf:parseType="Collection">
                    <owl:Restriction>
                        <owl:onProperty rdf:resource="http://purl.imsglobal.org/caliper/actor"/>
                        <owl:someValuesFrom rdf:resource="http://purl.imsglobal.org/caliper/Agent"/>
                    </owl:Restriction>
                    <owl:Restriction>
                        <owl:onProperty rdf:resource="http://purl.imsglobal.org/caliper/actor"/>
                        <owl:allValuesFrom rdf:resource="http://purl.imsglobal.org/caliper/Person"/>
                    </owl:Restriction>
                </owl:intersectionOf>
            </owl:Class>
        </rdfs:subClassOf>
        <rdfs:subClassOf>
            <owl:Class>
                <owl:intersectionOf rdf:parseType="Collection">
                    <owl:Restriction>
                        <owl:onProperty rdf:resource="http://purl.imsglobal.org/caliper/object"/>
                        <owl:someValuesFrom rdf:resource="http://purl.imsglobal.org/caliper/AssignableDigitalResource"/>
                    </owl:Restriction>
                    <owl:Restriction>
                        <owl:onProperty rdf:resource="http://purl.imsglobal.org/caliper/object"/>
                        <owl:allValuesFrom rdf:resource="http://purl.imsglobal.org/caliper/Assessment"/>
                    </owl:Restriction>
                </owl:intersectionOf>
            </owl:Class>
        </rdfs:subClassOf>
        <rdfs:subClassOf>
            <owl:Restriction>
                <owl:onProperty rdf:resource="http://purl.imsglobal.org/caliper/generated"/>
                <owl:someValuesFrom rdf:resource="http://purl.imsglobal.org/caliper/Attempt"/>
            </owl:Restriction>
        </rdfs:subClassOf>
        <rdfs:comment xml:lang="en">A Caliper AssessmentEvent models learner interactions with assessments instruments such as online tests or quizzes.</rdfs:comment>
        <rdfs:isDefinedBy rdf:datatype="http://www.w3.org/2001/XMLSchema#string">http://purl.imsglobal.org/caliper</rdfs:isDefinedBy>
        <rdfs:label xml:lang="en">AssessmentEvent</rdfs:label>
    </owl:Class>
    


    <!-- http://purl.imsglobal.org/caliper/AssessmentItem -->

    <owl:Class rdf:about="http://purl.imsglobal.org/caliper/AssessmentItem">
        <rdfs:subClassOf rdf:resource="http://purl.imsglobal.org/caliper/AssignableDigitalResource"/>
        <rdfs:subClassOf>
            <owl:Class>
                <owl:intersectionOf rdf:parseType="Collection">
                    <owl:Restriction>
                        <owl:onProperty rdf:resource="http://purl.imsglobal.org/caliper/isPartOf"/>
                        <owl:someValuesFrom rdf:resource="http://purl.imsglobal.org/caliper/AssignableDigitalResource"/>
                    </owl:Restriction>
                    <owl:Restriction>
                        <owl:onProperty rdf:resource="http://purl.imsglobal.org/caliper/isPartOf"/>
                        <owl:allValuesFrom rdf:resource="http://purl.imsglobal.org/caliper/Assessment"/>
                    </owl:Restriction>
                </owl:intersectionOf>
            </owl:Class>
        </rdfs:subClassOf>
        <rdfs:comment xml:lang="en">A Caliper AssessmentItem represents a single test question.</rdfs:comment>
        <rdfs:isDefinedBy rdf:datatype="http://www.w3.org/2001/XMLSchema#string">http://purl.imsglobal.org/caliper</rdfs:isDefinedBy>
        <rdfs:label xml:lang="en">AssessmentItem</rdfs:label>
    </owl:Class>
    


    <!-- http://purl.imsglobal.org/caliper/AssessmentItemEvent -->

    <owl:Class rdf:about="http://purl.imsglobal.org/caliper/AssessmentItemEvent">
        <rdfs:subClassOf rdf:resource="http://purl.imsglobal.org/caliper/Event"/>
        <rdfs:subClassOf>
            <owl:Class>
                <owl:intersectionOf rdf:parseType="Collection">
                    <owl:Restriction>
                        <owl:onProperty rdf:resource="http://purl.imsglobal.org/caliper/action"/>
                        <owl:someValuesFrom rdf:resource="http://purl.imsglobal.org/caliper/Action"/>
                    </owl:Restriction>
                    <owl:Restriction>
                        <owl:onProperty rdf:resource="http://purl.imsglobal.org/caliper/action"/>
                        <owl:someValuesFrom>
                            <owl:Class>
                                <owl:oneOf rdf:parseType="Collection">
                                    <rdf:Description rdf:about="http://purl.imsglobal.org/caliper/actions/Completed"/>
                                    <rdf:Description rdf:about="http://purl.imsglobal.org/caliper/actions/Skipped"/>
                                    <rdf:Description rdf:about="http://purl.imsglobal.org/caliper/actions/Started"/>
                                </owl:oneOf>
                            </owl:Class>
                        </owl:someValuesFrom>
                    </owl:Restriction>
                </owl:intersectionOf>
            </owl:Class>
        </rdfs:subClassOf>
        <rdfs:subClassOf>
            <owl:Class>
                <owl:intersectionOf rdf:parseType="Collection">
                    <owl:Restriction>
                        <owl:onProperty rdf:resource="http://purl.imsglobal.org/caliper/actor"/>
                        <owl:someValuesFrom rdf:resource="http://purl.imsglobal.org/caliper/Agent"/>
                    </owl:Restriction>
                    <owl:Restriction>
                        <owl:onProperty rdf:resource="http://purl.imsglobal.org/caliper/actor"/>
                        <owl:allValuesFrom rdf:resource="http://purl.imsglobal.org/caliper/Person"/>
                    </owl:Restriction>
                </owl:intersectionOf>
            </owl:Class>
        </rdfs:subClassOf>
        <rdfs:subClassOf>
            <owl:Class>
                <owl:intersectionOf rdf:parseType="Collection">
                    <owl:Restriction>
                        <owl:onProperty rdf:resource="http://purl.imsglobal.org/caliper/object"/>
                        <owl:someValuesFrom rdf:resource="http://purl.imsglobal.org/caliper/AssignableDigitalResource"/>
                    </owl:Restriction>
                    <owl:Restriction>
                        <owl:onProperty rdf:resource="http://purl.imsglobal.org/caliper/object"/>
                        <owl:allValuesFrom rdf:resource="http://purl.imsglobal.org/caliper/AssessmentItem"/>
                    </owl:Restriction>
                </owl:intersectionOf>
            </owl:Class>
        </rdfs:subClassOf>
        <rdfs:subClassOf>
            <owl:Class>
                <owl:intersectionOf rdf:parseType="Collection">
                    <owl:Restriction>
                        <owl:onProperty rdf:resource="http://purl.imsglobal.org/caliper/referrer"/>
                        <owl:someValuesFrom rdf:resource="http://purl.imsglobal.org/caliper/AssignableDigitalResource"/>
                    </owl:Restriction>
                    <owl:Restriction>
                        <owl:onProperty rdf:resource="http://purl.imsglobal.org/caliper/referrer"/>
                        <owl:allValuesFrom rdf:resource="http://purl.imsglobal.org/caliper/AssessmentItem"/>
                    </owl:Restriction>
                </owl:intersectionOf>
            </owl:Class>
        </rdfs:subClassOf>
        <rdfs:subClassOf>
            <owl:Restriction>
                <owl:onProperty rdf:resource="http://purl.imsglobal.org/caliper/generated"/>
                <owl:someValuesFrom rdf:resource="http://purl.imsglobal.org/caliper/Response"/>
            </owl:Restriction>
        </rdfs:subClassOf>
        <rdfs:comment xml:lang="en">A Caliper AssessmentItemEvent models a learner&apos;s interaction with an individual AssessmentItem.</rdfs:comment>
        <rdfs:isDefinedBy rdf:datatype="http://www.w3.org/2001/XMLSchema#string">http://purl.imsglobal.org/caliper</rdfs:isDefinedBy>
        <rdfs:label xml:lang="en">AssessmentItemEvent</rdfs:label>
    </owl:Class>
    


    <!-- http://purl.imsglobal.org/caliper/AssignableDigitalResource -->

    <owl:Class rdf:about="http://purl.imsglobal.org/caliper/AssignableDigitalResource">
        <rdfs:subClassOf rdf:resource="http://purl.imsglobal.org/caliper/DigitalResource"/>
        <terms:isReplacedBy rdf:resource="http://purl.imsglobal.org/caliper/DigitalResource"/>
        <rdfs:comment xml:lang="en">A Caliper AssignableDigitalResource is a generic type that represents digital content associated with a graded or ungraded assignment.  Utilize AssignableDigitalResource only if no suitable subtype exists to represent the resource being described.</rdfs:comment>
        <rdfs:isDefinedBy rdf:datatype="http://www.w3.org/2001/XMLSchema#string">http://purl.imsglobal.org/caliper</rdfs:isDefinedBy>
        <rdfs:label xml:lang="en">AssignableDigitalResource</rdfs:label>
    </owl:Class>
    


    <!-- http://purl.imsglobal.org/caliper/AssignableEvent -->

    <owl:Class rdf:about="http://purl.imsglobal.org/caliper/AssignableEvent">
        <rdfs:subClassOf rdf:resource="http://purl.imsglobal.org/caliper/Event"/>
        <rdfs:subClassOf>
            <owl:Class>
                <owl:intersectionOf rdf:parseType="Collection">
                    <owl:Restriction>
                        <owl:onProperty rdf:resource="http://purl.imsglobal.org/caliper/action"/>
                        <owl:someValuesFrom rdf:resource="http://purl.imsglobal.org/caliper/Action"/>
                    </owl:Restriction>
                    <owl:Restriction>
                        <owl:onProperty rdf:resource="http://purl.imsglobal.org/caliper/action"/>
                        <owl:someValuesFrom>
                            <owl:Class>
                                <owl:oneOf rdf:parseType="Collection">
                                    <rdf:Description rdf:about="http://purl.imsglobal.org/caliper/actions/Activated"/>
                                    <rdf:Description rdf:about="http://purl.imsglobal.org/caliper/actions/Completed"/>
                                    <rdf:Description rdf:about="http://purl.imsglobal.org/caliper/actions/Deactivated"/>
                                    <rdf:Description rdf:about="http://purl.imsglobal.org/caliper/actions/Reviewed"/>
                                    <rdf:Description rdf:about="http://purl.imsglobal.org/caliper/actions/Started"/>
                                    <rdf:Description rdf:about="http://purl.imsglobal.org/caliper/actions/Submitted"/>
                                </owl:oneOf>
                            </owl:Class>
                        </owl:someValuesFrom>
                    </owl:Restriction>
                </owl:intersectionOf>
            </owl:Class>
        </rdfs:subClassOf>
        <rdfs:subClassOf>
            <owl:Class>
                <owl:intersectionOf rdf:parseType="Collection">
                    <owl:Restriction>
                        <owl:onProperty rdf:resource="http://purl.imsglobal.org/caliper/actor"/>
                        <owl:someValuesFrom rdf:resource="http://purl.imsglobal.org/caliper/Agent"/>
                    </owl:Restriction>
                    <owl:Restriction>
                        <owl:onProperty rdf:resource="http://purl.imsglobal.org/caliper/actor"/>
                        <owl:allValuesFrom rdf:resource="http://purl.imsglobal.org/caliper/Person"/>
                    </owl:Restriction>
                </owl:intersectionOf>
            </owl:Class>
        </rdfs:subClassOf>
        <rdfs:subClassOf>
            <owl:Class>
                <owl:intersectionOf rdf:parseType="Collection">
                    <owl:Restriction>
                        <owl:onProperty rdf:resource="http://purl.imsglobal.org/caliper/object"/>
                        <owl:someValuesFrom rdf:resource="http://purl.imsglobal.org/caliper/DigitalResource"/>
                    </owl:Restriction>
                    <owl:Restriction>
                        <owl:onProperty rdf:resource="http://purl.imsglobal.org/caliper/object"/>
                        <owl:allValuesFrom rdf:resource="http://purl.imsglobal.org/caliper/AssignableDigitalResource"/>
                    </owl:Restriction>
                </owl:intersectionOf>
            </owl:Class>
        </rdfs:subClassOf>
        <rdfs:subClassOf>
            <owl:Restriction>
                <owl:onProperty rdf:resource="http://purl.imsglobal.org/caliper/generated"/>
                <owl:someValuesFrom rdf:resource="http://purl.imsglobal.org/caliper/Attempt"/>
            </owl:Restriction>
        </rdfs:subClassOf>
        <rdfs:subClassOf>
            <owl:Restriction>
                <owl:onProperty rdf:resource="http://purl.imsglobal.org/caliper/target"/>
                <owl:someValuesFrom rdf:resource="http://purl.imsglobal.org/caliper/Frame"/>
            </owl:Restriction>
        </rdfs:subClassOf>
        <rdfs:comment xml:lang="en">A Caliper AssignableEvent models activities associated with the assignment of digital content assigned to a learner for completion.</rdfs:comment>
        <rdfs:isDefinedBy rdf:datatype="http://www.w3.org/2001/XMLSchema#string">http://purl.imsglobal.org/caliper</rdfs:isDefinedBy>
        <rdfs:label xml:lang="en">AssignableEvent</rdfs:label>
    </owl:Class>
    


    <!-- http://purl.imsglobal.org/caliper/Attempt -->

    <owl:Class rdf:about="http://purl.imsglobal.org/caliper/Attempt">
        <rdfs:subClassOf rdf:resource="http://purl.imsglobal.org/caliper/Entity"/>
        <rdfs:subClassOf>
            <owl:Class>
                <owl:intersectionOf rdf:parseType="Collection">
                    <owl:Restriction>
                        <owl:onProperty rdf:resource="http://purl.imsglobal.org/caliper/assignable"/>
                        <owl:someValuesFrom rdf:resource="http://purl.imsglobal.org/caliper/Entity"/>
                    </owl:Restriction>
                    <owl:Restriction>
                        <owl:onProperty rdf:resource="http://purl.imsglobal.org/caliper/assignable"/>
                        <owl:allValuesFrom rdf:resource="http://purl.imsglobal.org/caliper/DigitalResource"/>
                    </owl:Restriction>
                </owl:intersectionOf>
            </owl:Class>
        </rdfs:subClassOf>
        <rdfs:subClassOf>
            <owl:Class>
                <owl:intersectionOf rdf:parseType="Collection">
                    <owl:Restriction>
                        <owl:onProperty rdf:resource="http://purl.imsglobal.org/caliper/assignee"/>
                        <owl:someValuesFrom rdf:resource="http://purl.imsglobal.org/caliper/Agent"/>
                    </owl:Restriction>
                    <owl:Restriction>
                        <owl:onProperty rdf:resource="http://purl.imsglobal.org/caliper/assignee"/>
                        <owl:allValuesFrom rdf:resource="http://purl.imsglobal.org/caliper/Person"/>
                    </owl:Restriction>
                </owl:intersectionOf>
            </owl:Class>
        </rdfs:subClassOf>
        <rdfs:subClassOf>
            <owl:Restriction>
                <owl:onProperty rdf:resource="http://purl.imsglobal.org/caliper/isPartOf"/>
                <owl:someValuesFrom rdf:resource="http://purl.imsglobal.org/caliper/Attempt"/>
            </owl:Restriction>
        </rdfs:subClassOf>
        <rdfs:comment xml:lang="en">A Caliper Attempt provides a count of the number of times an actor has interacted with an AssignableDigitalResource along with start time, end time and duration information. An Attempt is generated as the result of an action such as starting an Assessment.</rdfs:comment>
        <rdfs:isDefinedBy rdf:datatype="http://www.w3.org/2001/XMLSchema#string">http://purl.imsglobal.org/caliper</rdfs:isDefinedBy>
        <rdfs:label xml:lang="en">Attempt</rdfs:label>
    </owl:Class>
    


    <!-- http://purl.imsglobal.org/caliper/AudioObject -->

    <owl:Class rdf:about="http://purl.imsglobal.org/caliper/AudioObject">
        <rdfs:subClassOf rdf:resource="http://purl.imsglobal.org/caliper/MediaObject"/>
        <rdfs:comment xml:lang="en">A Caliper AudioObject represents an audio or sound file.</rdfs:comment>
        <rdfs:isDefinedBy rdf:datatype="http://www.w3.org/2001/XMLSchema#string">http://purl.imsglobal.org/caliper</rdfs:isDefinedBy>
        <rdfs:label xml:lang="en">AudioObject</rdfs:label>
    </owl:Class>
    


    <!-- http://purl.imsglobal.org/caliper/BookmarkAnnotation -->

    <owl:Class rdf:about="http://purl.imsglobal.org/caliper/BookmarkAnnotation">
        <rdfs:subClassOf rdf:resource="http://purl.imsglobal.org/caliper/Annotation"/>
        <rdfs:comment xml:lang="en">A Caliper BookmarkAnnotation represents the act of marking a DigitalResource at a particular location.</rdfs:comment>
        <rdfs:isDefinedBy rdf:datatype="http://www.w3.org/2001/XMLSchema#string">http://purl.imsglobal.org/caliper</rdfs:isDefinedBy>
        <rdfs:label xml:lang="en">BookmarkAnnotation</rdfs:label>
    </owl:Class>
    


    <!-- http://purl.imsglobal.org/caliper/Chapter -->

    <owl:Class rdf:about="http://purl.imsglobal.org/caliper/Chapter">
        <rdfs:subClassOf rdf:resource="http://purl.imsglobal.org/caliper/DigitalResource"/>
        <rdfs:comment xml:lang="en">A Caliper Chapter represents a major sub-division of a piece of digital content.</rdfs:comment>
        <rdfs:isDefinedBy rdf:datatype="http://www.w3.org/2001/XMLSchema#string">http://purl.imsglobal.org/caliper</rdfs:isDefinedBy>
        <rdfs:label xml:lang="en">Chapter</rdfs:label>
    </owl:Class>
    


    <!-- http://purl.imsglobal.org/caliper/Collection -->

    <owl:Class rdf:about="http://purl.imsglobal.org/caliper/Collection">
        <rdfs:subClassOf rdf:resource="http://purl.imsglobal.org/caliper/Entity"/>
        <rdfs:comment xml:lang="en">A Caliper Collection represents an unordered collection of entities.</rdfs:comment>
        <rdfs:isDefinedBy rdf:datatype="http://www.w3.org/2001/XMLSchema#string">http://purl.imsglobal.org/caliper</rdfs:isDefinedBy>
        <rdfs:label xml:lang="en">Collection</rdfs:label>
    </owl:Class>
    


    <!-- http://purl.imsglobal.org/caliper/Comment -->

    <owl:Class rdf:about="http://purl.imsglobal.org/caliper/Comment">
        <rdfs:subClassOf rdf:resource="http://purl.imsglobal.org/caliper/Entity"/>
        <rdfs:subClassOf>
            <owl:Class>
                <owl:intersectionOf rdf:parseType="Collection">
                    <owl:Restriction>
                        <owl:onProperty rdf:resource="http://purl.imsglobal.org/caliper/commenter"/>
                        <owl:someValuesFrom rdf:resource="http://purl.imsglobal.org/caliper/Agent"/>
                    </owl:Restriction>
                    <owl:Restriction>
                        <owl:onProperty rdf:resource="http://purl.imsglobal.org/caliper/commenter"/>
                        <owl:allValuesFrom rdf:resource="http://purl.imsglobal.org/caliper/Person"/>
                    </owl:Restriction>
                </owl:intersectionOf>
            </owl:Class>
        </rdfs:subClassOf>
        <rdfs:subClassOf>
            <owl:Restriction>
                <owl:onProperty rdf:resource="http://purl.imsglobal.org/caliper/commentedOn"/>
                <owl:someValuesFrom rdf:resource="http://purl.imsglobal.org/caliper/Entity"/>
            </owl:Restriction>
        </rdfs:subClassOf>
        <rdfs:comment xml:lang="en">A Caliper Comment models a person&apos;s qualitative reactions to a Entity.</rdfs:comment>
        <rdfs:isDefinedBy rdf:datatype="http://www.w3.org/2001/XMLSchema#string">https://purl.imsglobal.org/caliper</rdfs:isDefinedBy>
        <rdfs:label xml:lang="en">Comment</rdfs:label>
    </owl:Class>
    


    <!-- http://purl.imsglobal.org/caliper/CourseOffering -->

    <owl:Class rdf:about="http://purl.imsglobal.org/caliper/CourseOffering">
        <rdfs:subClassOf rdf:resource="http://purl.imsglobal.org/caliper/Organization"/>
        <owl:disjointWith rdf:resource="http://purl.imsglobal.org/caliper/Group"/>
        <rdfs:comment xml:lang="en">A Caliper CourseOffering represents the occurrence of a course or a type during a specified time period.</rdfs:comment>
        <rdfs:isDefinedBy rdf:datatype="http://www.w3.org/2001/XMLSchema#string">http://purl.imsglobal.org/caliper</rdfs:isDefinedBy>
        <rdfs:label xml:lang="en">CourseOffering</rdfs:label>
    </owl:Class>
    


    <!-- http://purl.imsglobal.org/caliper/CourseSection -->

    <owl:Class rdf:about="http://purl.imsglobal.org/caliper/CourseSection">
        <rdfs:subClassOf rdf:resource="http://purl.imsglobal.org/caliper/CourseOffering"/>
        <rdfs:comment xml:lang="en">A Caliper CourseSection represents a specific instance of a CourseOffering occurring during a specific semester, term or period.</rdfs:comment>
        <rdfs:isDefinedBy rdf:datatype="http://www.w3.org/2001/XMLSchema#string">http://purl.imsglobal.org/caliper</rdfs:isDefinedBy>
        <rdfs:label xml:lang="en">CourseSection</rdfs:label>
    </owl:Class>
    


    <!-- http://purl.imsglobal.org/caliper/DigitalResource -->

    <owl:Class rdf:about="http://purl.imsglobal.org/caliper/DigitalResource">
        <rdfs:subClassOf rdf:resource="http://purl.imsglobal.org/caliper/Entity"/>
        <rdfs:comment xml:lang="en">A Caliper DigitalResource is a generic type that represents digital content.  Utilize DigitalResource only if no suitable subtype exists to represent the resource being described.</rdfs:comment>
        <rdfs:isDefinedBy rdf:datatype="http://www.w3.org/2001/XMLSchema#string">http://purl.imsglobal.org/caliper</rdfs:isDefinedBy>
        <rdfs:label xml:lang="en">DigitalResource</rdfs:label>
    </owl:Class>
    


    <!-- http://purl.imsglobal.org/caliper/DigitalResourceCollection -->

    <owl:Class rdf:about="http://purl.imsglobal.org/caliper/DigitalResourceCollection">
        <rdfs:subClassOf rdf:resource="http://purl.imsglobal.org/caliper/Collection"/>
        <rdfs:subClassOf rdf:resource="http://purl.imsglobal.org/caliper/DigitalResource"/>
        <rdfs:subClassOf>
            <owl:Class>
                <owl:intersectionOf rdf:parseType="Collection">
                    <owl:Restriction>
                        <owl:onProperty rdf:resource="http://purl.imsglobal.org/caliper/items"/>
                        <owl:someValuesFrom rdf:resource="http://purl.imsglobal.org/caliper/Entity"/>
                    </owl:Restriction>
                    <owl:Restriction>
                        <owl:onProperty rdf:resource="http://purl.imsglobal.org/caliper/items"/>
                        <owl:allValuesFrom rdf:resource="http://purl.imsglobal.org/caliper/DigitalResource"/>
                    </owl:Restriction>
                </owl:intersectionOf>
            </owl:Class>
        </rdfs:subClassOf>
        <rdfs:comment xml:lang="en">A Caliper DigitalResourceCollection represents an ordered collection of DigitalResource entities.</rdfs:comment>
        <rdfs:isDefinedBy rdf:datatype="http://www.w3.org/2001/XMLSchema#string">http://purl.imsglobal.org/caliper</rdfs:isDefinedBy>
        <rdfs:label xml:lang="en">DigitalResourceCollection</rdfs:label>
    </owl:Class>
    


    <!-- http://purl.imsglobal.org/caliper/Document -->

    <owl:Class rdf:about="http://purl.imsglobal.org/caliper/Document">
        <rdfs:subClassOf rdf:resource="http://purl.imsglobal.org/caliper/DigitalResource"/>
        <rdfs:comment xml:lang="en">A Caliper Document represents paginated textual content.</rdfs:comment>
        <rdfs:isDefinedBy rdf:datatype="http://www.w3.org/2001/XMLSchema#string">http://purl.imsglobal.org/caliper</rdfs:isDefinedBy>
        <rdfs:label xml:lang="en">Document</rdfs:label>
    </owl:Class>
    


    <!-- http://purl.imsglobal.org/caliper/Entity -->

    <owl:Class rdf:about="http://purl.imsglobal.org/caliper/Entity">
        <rdfs:comment xml:lang="en">A Caliper Entity is a generic type that represents objects or things that participate in learning-related activities. Entity is subtyped for enhanced type specificity in order to better describe people, groups, digital content, courses, assignments, assessments, forums, messages, software applications and other entities that constitute the &quot;stuff&quot; of a Caliper Event.  Utilize Entity only if no suitable subtype exists to represent the thing being described.</rdfs:comment>
        <rdfs:isDefinedBy rdf:datatype="http://www.w3.org/2001/XMLSchema#string">http://purl.imsglobal.org/caliper</rdfs:isDefinedBy>
        <rdfs:label xml:lang="en">Entity</rdfs:label>
    </owl:Class>
    


    <!-- http://purl.imsglobal.org/caliper/Envelope -->

    <owl:Class rdf:about="http://purl.imsglobal.org/caliper/Envelope">
        <rdfs:comment xml:lang="en">A Caliper Envelope is a container that is used to transmit one or more Caliper Events and/or Caliper Entity describes.</rdfs:comment>
        <rdfs:isDefinedBy rdf:datatype="http://www.w3.org/2001/XMLSchema#string">http://purl.imsglobal.org/caliper</rdfs:isDefinedBy>
        <rdfs:label xml:lang="en">Envelope</rdfs:label>
    </owl:Class>
    


    <!-- http://purl.imsglobal.org/caliper/Event -->

    <owl:Class rdf:about="http://purl.imsglobal.org/caliper/Event">
        <rdfs:comment xml:lang="en">A Caliper Event is a generic type that describes a relationship established between an actor and an object, formed as a result of a purposeful action undertaken by the actor in connection to the object at a particular moment in time.</rdfs:comment>
        <rdfs:isDefinedBy rdf:datatype="http://www.w3.org/2001/XMLSchema#string">http://purl.imsglobal.org/caliper</rdfs:isDefinedBy>
        <rdfs:label xml:lang="en">Event</rdfs:label>
    </owl:Class>
    


    <!-- http://purl.imsglobal.org/caliper/FeedbackEvent -->

    <owl:Class rdf:about="http://purl.imsglobal.org/caliper/FeedbackEvent">
        <rdfs:subClassOf rdf:resource="http://purl.imsglobal.org/caliper/Event"/>
        <rdfs:subClassOf>
            <owl:Class>
                <owl:intersectionOf rdf:parseType="Collection">
                    <owl:Restriction>
                        <owl:onProperty rdf:resource="http://purl.imsglobal.org/caliper/action"/>
                        <owl:someValuesFrom rdf:resource="http://purl.imsglobal.org/caliper/Action"/>
                    </owl:Restriction>
                    <owl:Restriction>
                        <owl:onProperty rdf:resource="http://purl.imsglobal.org/caliper/action"/>
                        <owl:someValuesFrom>
                            <owl:Class>
                                <owl:oneOf rdf:parseType="Collection">
                                    <rdf:Description rdf:about="http://purl.imsglobal.org/caliper/actions/Commented"/>
                                    <rdf:Description rdf:about="http://purl.imsglobal.org/caliper/actions/Ranked"/>
                                </owl:oneOf>
                            </owl:Class>
                        </owl:someValuesFrom>
                    </owl:Restriction>
                </owl:intersectionOf>
            </owl:Class>
        </rdfs:subClassOf>
        <rdfs:subClassOf>
            <owl:Class>
                <owl:intersectionOf rdf:parseType="Collection">
                    <owl:Restriction>
                        <owl:onProperty rdf:resource="http://purl.imsglobal.org/caliper/actor"/>
                        <owl:someValuesFrom rdf:resource="http://purl.imsglobal.org/caliper/Agent"/>
                    </owl:Restriction>
                    <owl:Restriction>
                        <owl:onProperty rdf:resource="http://purl.imsglobal.org/caliper/actor"/>
                        <owl:allValuesFrom rdf:resource="http://purl.imsglobal.org/caliper/Person"/>
                    </owl:Restriction>
                </owl:intersectionOf>
            </owl:Class>
        </rdfs:subClassOf>
        <rdfs:subClassOf>
            <owl:Class>
                <owl:intersectionOf rdf:parseType="Collection">
                    <owl:Restriction>
                        <owl:onProperty rdf:resource="http://purl.imsglobal.org/caliper/generated"/>
                        <owl:someValuesFrom rdf:resource="http://purl.imsglobal.org/caliper/Entity"/>
                    </owl:Restriction>
                    <owl:Restriction>
                        <owl:onProperty rdf:resource="http://purl.imsglobal.org/caliper/generated"/>
                        <owl:allValuesFrom>
                            <owl:Class>
                                <owl:unionOf rdf:parseType="Collection">
                                    <rdf:Description rdf:about="http://purl.imsglobal.org/caliper/Comment"/>
                                    <rdf:Description rdf:about="http://purl.imsglobal.org/caliper/Rating"/>
                                </owl:unionOf>
                            </owl:Class>
                        </owl:allValuesFrom>
                    </owl:Restriction>
                </owl:intersectionOf>
            </owl:Class>
        </rdfs:subClassOf>
        <rdfs:subClassOf>
            <owl:Class>
                <owl:intersectionOf rdf:parseType="Collection">
                    <owl:Restriction>
                        <owl:onProperty rdf:resource="http://purl.imsglobal.org/caliper/target"/>
                        <owl:someValuesFrom rdf:resource="http://purl.imsglobal.org/caliper/DigitalResource"/>
                    </owl:Restriction>
                    <owl:Restriction>
                        <owl:onProperty rdf:resource="http://purl.imsglobal.org/caliper/target"/>
                        <owl:allValuesFrom rdf:resource="http://purl.imsglobal.org/caliper/Frame"/>
                    </owl:Restriction>
                </owl:intersectionOf>
            </owl:Class>
        </rdfs:subClassOf>
        <rdfs:subClassOf>
            <owl:Restriction>
                <owl:onProperty rdf:resource="http://purl.imsglobal.org/caliper/object"/>
                <owl:someValuesFrom rdf:resource="http://purl.imsglobal.org/caliper/Entity"/>
            </owl:Restriction>
        </rdfs:subClassOf>
        <rdfs:comment xml:lang="en">A Caliper FeedbackEvent models a Person providing informal feedback on an Entity, typically a DigitalResource or another Person.</rdfs:comment>
        <rdfs:isDefinedBy rdf:datatype="http://www.w3.org/2001/XMLSchema#string">http://purl.imsglobal.org/caliper</rdfs:isDefinedBy>
        <rdfs:label xml:lang="en">FeedbackEvent</rdfs:label>
    </owl:Class>
    


    <!-- http://purl.imsglobal.org/caliper/FillinBlankResponse -->

    <owl:Class rdf:about="http://purl.imsglobal.org/caliper/FillinBlankResponse">
        <rdfs:subClassOf rdf:resource="http://purl.imsglobal.org/caliper/Response"/>
        <rdfs:comment xml:lang="en">A Caliper FillinBlankResponse represents a type of Response in which a respondent is asked to provide one or more words, expressions or short phrases that correctly completes a statement.</rdfs:comment>
        <rdfs:isDefinedBy rdf:datatype="http://www.w3.org/2001/XMLSchema#string">http://purl.imsglobal.org/caliper</rdfs:isDefinedBy>
        <rdfs:label xml:lang="en">FillinBlankResponse</rdfs:label>
    </owl:Class>
    


    <!-- http://purl.imsglobal.org/caliper/Forum -->

    <owl:Class rdf:about="http://purl.imsglobal.org/caliper/Forum">
        <rdfs:subClassOf rdf:resource="http://purl.imsglobal.org/caliper/DigitalResourceCollection"/>
        <rdfs:subClassOf>
            <owl:Class>
                <owl:intersectionOf rdf:parseType="Collection">
                    <owl:Restriction>
                        <owl:onProperty rdf:resource="http://purl.imsglobal.org/caliper/items"/>
                        <owl:someValuesFrom rdf:resource="http://purl.imsglobal.org/caliper/Entity"/>
                    </owl:Restriction>
                    <owl:Restriction>
                        <owl:onProperty rdf:resource="http://purl.imsglobal.org/caliper/items"/>
                        <owl:allValuesFrom rdf:resource="http://purl.imsglobal.org/caliper/Thread"/>
                    </owl:Restriction>
                </owl:intersectionOf>
            </owl:Class>
        </rdfs:subClassOf>
        <owl:disjointWith rdf:resource="http://purl.imsglobal.org/caliper/Thread"/>
        <rdfs:comment xml:lang="en">A Caliper Forum represents a channel or virtual space in which group discussions take place.  A Forum typically comprises one or more threaded conversations to which members can subscribe, post messages and reply to other messages.</rdfs:comment>
        <rdfs:isDefinedBy rdf:datatype="http://www.w3.org/2001/XMLSchema#string">http://purl.imsglobal.org/caliper</rdfs:isDefinedBy>
        <rdfs:label xml:lang="en">Forum</rdfs:label>
    </owl:Class>
    


    <!-- http://purl.imsglobal.org/caliper/ForumEvent -->

    <owl:Class rdf:about="http://purl.imsglobal.org/caliper/ForumEvent">
        <rdfs:subClassOf rdf:resource="http://purl.imsglobal.org/caliper/Event"/>
        <rdfs:subClassOf>
            <owl:Class>
                <owl:intersectionOf rdf:parseType="Collection">
                    <owl:Restriction>
                        <owl:onProperty rdf:resource="http://purl.imsglobal.org/caliper/action"/>
                        <owl:someValuesFrom rdf:resource="http://purl.imsglobal.org/caliper/Action"/>
                    </owl:Restriction>
                    <owl:Restriction>
                        <owl:onProperty rdf:resource="http://purl.imsglobal.org/caliper/action"/>
                        <owl:someValuesFrom>
                            <owl:Class>
                                <owl:oneOf rdf:parseType="Collection">
                                    <rdf:Description rdf:about="http://purl.imsglobal.org/caliper/actions/Subscribed"/>
                                    <rdf:Description rdf:about="http://purl.imsglobal.org/caliper/actions/Unsubscribed"/>
                                </owl:oneOf>
                            </owl:Class>
                        </owl:someValuesFrom>
                    </owl:Restriction>
                </owl:intersectionOf>
            </owl:Class>
        </rdfs:subClassOf>
        <rdfs:subClassOf>
            <owl:Class>
                <owl:intersectionOf rdf:parseType="Collection">
                    <owl:Restriction>
                        <owl:onProperty rdf:resource="http://purl.imsglobal.org/caliper/actor"/>
                        <owl:someValuesFrom rdf:resource="http://purl.imsglobal.org/caliper/Agent"/>
                    </owl:Restriction>
                    <owl:Restriction>
                        <owl:onProperty rdf:resource="http://purl.imsglobal.org/caliper/actor"/>
                        <owl:allValuesFrom rdf:resource="http://purl.imsglobal.org/caliper/Person"/>
                    </owl:Restriction>
                </owl:intersectionOf>
            </owl:Class>
        </rdfs:subClassOf>
        <rdfs:subClassOf>
            <owl:Class>
                <owl:intersectionOf rdf:parseType="Collection">
                    <owl:Restriction>
                        <owl:onProperty rdf:resource="http://purl.imsglobal.org/caliper/object"/>
                        <owl:someValuesFrom rdf:resource="http://purl.imsglobal.org/caliper/DigitalResource"/>
                    </owl:Restriction>
                    <owl:Restriction>
                        <owl:onProperty rdf:resource="http://purl.imsglobal.org/caliper/object"/>
                        <owl:allValuesFrom rdf:resource="http://purl.imsglobal.org/caliper/Forum"/>
                    </owl:Restriction>
                </owl:intersectionOf>
            </owl:Class>
        </rdfs:subClassOf>
        <rdfs:comment xml:lang="en">A Caliper ForumEvent models learners and others participating in online forum communities. Forums typically encompass one or more threads or topics to which members can subscribe, post messages and reply to other messages if a threaded discussion is permitted.</rdfs:comment>
        <rdfs:isDefinedBy rdf:datatype="http://www.w3.org/2001/XMLSchema#string">http://purl.imsglobal.org/caliper</rdfs:isDefinedBy>
        <rdfs:label xml:lang="en">ForumEvent</rdfs:label>
    </owl:Class>
    


    <!-- http://purl.imsglobal.org/caliper/Frame -->

    <owl:Class rdf:about="http://purl.imsglobal.org/caliper/Frame">
        <rdfs:subClassOf rdf:resource="http://purl.imsglobal.org/caliper/DigitalResource"/>
        <rdfs:comment xml:lang="en">A Caliper Frame represents a part, portion or segment of a DigitalResource.</rdfs:comment>
        <rdfs:isDefinedBy rdf:datatype="http://www.w3.org/2001/XMLSchema#string">http://purl.imsglobal.org/caliper</rdfs:isDefinedBy>
        <rdfs:label xml:lang="en">Frame</rdfs:label>
    </owl:Class>
    


    <!-- http://purl.imsglobal.org/caliper/GradeEvent -->

    <owl:Class rdf:about="http://purl.imsglobal.org/caliper/GradeEvent">
        <rdfs:subClassOf rdf:resource="http://purl.imsglobal.org/caliper/Event"/>
        <rdfs:subClassOf>
            <owl:Class>
                <owl:intersectionOf rdf:parseType="Collection">
                    <owl:Restriction>
                        <owl:onProperty rdf:resource="http://purl.imsglobal.org/caliper/action"/>
                        <owl:someValuesFrom rdf:resource="http://purl.imsglobal.org/caliper/Action"/>
                    </owl:Restriction>
                    <owl:Restriction>
                        <owl:onProperty rdf:resource="http://purl.imsglobal.org/caliper/action"/>
                        <owl:hasValue rdf:resource="http://purl.imsglobal.org/caliper/actions/Graded"/>
                    </owl:Restriction>
                </owl:intersectionOf>
            </owl:Class>
        </rdfs:subClassOf>
        <rdfs:subClassOf>
            <owl:Class>
                <owl:intersectionOf rdf:parseType="Collection">
                    <owl:Restriction>
                        <owl:onProperty rdf:resource="http://purl.imsglobal.org/caliper/actor"/>
                        <owl:someValuesFrom rdf:resource="http://purl.imsglobal.org/caliper/Agent"/>
                    </owl:Restriction>
                    <owl:Restriction>
                        <owl:onProperty rdf:resource="http://purl.imsglobal.org/caliper/actor"/>
                        <owl:allValuesFrom>
                            <owl:Class>
                                <owl:unionOf rdf:parseType="Collection">
                                    <rdf:Description rdf:about="http://purl.imsglobal.org/caliper/Person"/>
                                    <rdf:Description rdf:about="http://purl.imsglobal.org/caliper/SoftwareApplication"/>
                                </owl:unionOf>
                            </owl:Class>
                        </owl:allValuesFrom>
                    </owl:Restriction>
                </owl:intersectionOf>
            </owl:Class>
        </rdfs:subClassOf>
        <rdfs:subClassOf>
            <owl:Class>
                <owl:intersectionOf rdf:parseType="Collection">
                    <owl:Restriction>
                        <owl:onProperty rdf:resource="http://purl.imsglobal.org/caliper/object"/>
                        <owl:someValuesFrom rdf:resource="http://purl.imsglobal.org/caliper/Entity"/>
                    </owl:Restriction>
                    <owl:Restriction>
                        <owl:onProperty rdf:resource="http://purl.imsglobal.org/caliper/object"/>
                        <owl:allValuesFrom rdf:resource="http://purl.imsglobal.org/caliper/Attempt"/>
                    </owl:Restriction>
                </owl:intersectionOf>
            </owl:Class>
        </rdfs:subClassOf>
        <rdfs:subClassOf>
            <owl:Restriction>
                <owl:onProperty rdf:resource="http://purl.imsglobal.org/caliper/generated"/>
                <owl:someValuesFrom rdf:resource="http://purl.imsglobal.org/caliper/Score"/>
            </owl:Restriction>
        </rdfs:subClassOf>
        <rdfs:comment xml:lang="en">A Caliper GradeEvent models grading activities performed by an Agent, typically a Person or a SoftwareApplication.</rdfs:comment>
        <rdfs:isDefinedBy rdf:datatype="http://www.w3.org/2001/XMLSchema#string">http://purl.imsglobal.org/caliper</rdfs:isDefinedBy>
        <rdfs:label xml:lang="en">GradeEvent</rdfs:label>
    </owl:Class>
    


    <!-- http://purl.imsglobal.org/caliper/Group -->

    <owl:Class rdf:about="http://purl.imsglobal.org/caliper/Group">
        <rdfs:subClassOf rdf:resource="http://purl.imsglobal.org/caliper/Organization"/>
        <rdfs:comment xml:lang="en">A Caliper Group represents an ad-hoc, informal or short-lived collection of people organized for some common educational or social purpose.  A Group can act as an Agent. It can be linked both to a parent Organization and to its members.</rdfs:comment>
        <rdfs:isDefinedBy rdf:datatype="http://www.w3.org/2001/XMLSchema#string">http://purl.imsglobal.org/caliper</rdfs:isDefinedBy>
        <rdfs:label xml:lang="en">Group</rdfs:label>
    </owl:Class>
    


    <!-- http://purl.imsglobal.org/caliper/HighlightAnnotation -->

    <owl:Class rdf:about="http://purl.imsglobal.org/caliper/HighlightAnnotation">
        <rdfs:subClassOf rdf:resource="http://purl.imsglobal.org/caliper/Annotation"/>
        <rdfs:comment xml:lang="en">A Caliper HighlightAnnotation represents the act of marking a particular segment of a DigitalResource between two known coordinates.</rdfs:comment>
        <rdfs:isDefinedBy rdf:datatype="http://www.w3.org/2001/XMLSchema#string">http://purl.imsglobal.org/caliper</rdfs:isDefinedBy>
        <rdfs:label xml:lang="en">HighlightAnnotation</rdfs:label>
    </owl:Class>
    


    <!-- http://purl.imsglobal.org/caliper/ImageObject -->

    <owl:Class rdf:about="http://purl.imsglobal.org/caliper/ImageObject">
        <rdfs:subClassOf rdf:resource="http://purl.imsglobal.org/caliper/MediaObject"/>
        <rdfs:comment xml:lang="en">A Caliper ImageObject represents an image file.</rdfs:comment>
        <rdfs:isDefinedBy rdf:datatype="http://www.w3.org/2001/XMLSchema#string">http://purl.imsglobal.org/caliper</rdfs:isDefinedBy>
        <rdfs:label xml:lang="en">ImageObject</rdfs:label>
    </owl:Class>
    


    <!-- http://purl.imsglobal.org/caliper/LearningObjective -->

    <owl:Class rdf:about="http://purl.imsglobal.org/caliper/LearningObjective">
        <rdfs:subClassOf rdf:resource="http://purl.imsglobal.org/caliper/Entity"/>
        <rdfs:comment xml:lang="en">A Caliper LearningObjective represents a brief statement of what a learner should know or be able to perform after completing a unit of instruction or a period of learning.</rdfs:comment>
        <rdfs:isDefinedBy rdf:datatype="http://www.w3.org/2001/XMLSchema#string">http://purl.imsglobal.org/caliper</rdfs:isDefinedBy>
        <rdfs:label xml:lang="en">LearningObjective</rdfs:label>
    </owl:Class>
    


    <!-- http://purl.imsglobal.org/caliper/LikertScale -->

    <owl:Class rdf:about="http://purl.imsglobal.org/caliper/LikertScale">
        <rdfs:subClassOf rdf:resource="http://purl.imsglobal.org/caliper/Scale"/>
        <rdfs:comment xml:lang="en">A Caliper LikertScale models a Likert scale employed for scaling responses.</rdfs:comment>
        <rdfs:isDefinedBy rdf:datatype="http://www.w3.org/2001/XMLSchema#string">https://purl.imsglobal.org/caliper</rdfs:isDefinedBy>
        <rdfs:label xml:lang="en">LikertScale</rdfs:label>
    </owl:Class>
    


    <!-- http://purl.imsglobal.org/caliper/Link -->

    <owl:Class rdf:about="http://purl.imsglobal.org/caliper/Link">
        <rdfs:subClassOf rdf:resource="http://purl.imsglobal.org/caliper/Entity"/>
        <rdfs:comment xml:lang="en">The Link entity represents a URL that might be a UI workflow or service endpoint (transient or otherwise), and not necessarily a proper Digital Resource (such as a WebPage or LtiLink.</rdfs:comment>
        <rdfs:isDefinedBy rdf:datatype="http://www.w3.org/2001/XMLSchema#string">http://purl.imsglobal.org/caliper</rdfs:isDefinedBy>
        <rdfs:label xml:lang="en">Link</rdfs:label>
    </owl:Class>
    


    <!-- http://purl.imsglobal.org/caliper/LtiLink -->

    <owl:Class rdf:about="http://purl.imsglobal.org/caliper/LtiLink">
        <rdfs:subClassOf rdf:resource="http://purl.imsglobal.org/caliper/DigitalResource"/>
        <rdfs:comment xml:lang="en">The LtiLink entity represents a digital resource that must be retrieved from an external tool application via an LTI request message. It is, effectively, a Digital Resource that must use LTI for access.</rdfs:comment>
        <rdfs:isDefinedBy rdf:datatype="http://www.w3.org/2001/XMLSchema#string">http://purl.imsglobal.org/caliper</rdfs:isDefinedBy>
        <rdfs:label xml:lang="en">LtiLink</rdfs:label>
    </owl:Class>
    


    <!-- http://purl.imsglobal.org/caliper/LtiMessageType -->

    <owl:Class rdf:about="http://purl.imsglobal.org/caliper/LtiMessageType">
        <rdfs:comment xml:lang="en">The LTI specification defines a number of message types that are exchanged between platforms and tools.  Each LTI message type describes or asserts a set of required and optional sender claims that are communicated to a receiver at particular moments in the workflow.</rdfs:comment>
        <rdfs:isDefinedBy rdf:datatype="http://www.w3.org/2001/XMLSchema#string">http://purl.imsglobal.org/caliper</rdfs:isDefinedBy>
        <rdfs:label xml:lang="en">LtiMessageType</rdfs:label>
    </owl:Class>
    


    <!-- http://purl.imsglobal.org/caliper/LtiSession -->

    <owl:Class rdf:about="http://purl.imsglobal.org/caliper/LtiSession">
        <rdfs:subClassOf rdf:resource="http://purl.imsglobal.org/caliper/Session"/>
        <rdfs:comment xml:lang="en">A Caliper LtiSession represents an LTI Tool Consumer user session.</rdfs:comment>
        <rdfs:label xml:lang="en">LtiSession</rdfs:label>
    </owl:Class>
    


    <!-- http://purl.imsglobal.org/caliper/MediaEvent -->

    <owl:Class rdf:about="http://purl.imsglobal.org/caliper/MediaEvent">
        <rdfs:subClassOf rdf:resource="http://purl.imsglobal.org/caliper/Event"/>
        <rdfs:subClassOf>
            <owl:Class>
                <owl:intersectionOf rdf:parseType="Collection">
                    <owl:Restriction>
                        <owl:onProperty rdf:resource="http://purl.imsglobal.org/caliper/action"/>
                        <owl:someValuesFrom rdf:resource="http://purl.imsglobal.org/caliper/Action"/>
                    </owl:Restriction>
                    <owl:Restriction>
                        <owl:onProperty rdf:resource="http://purl.imsglobal.org/caliper/action"/>
                        <owl:someValuesFrom>
                            <owl:Class>
                                <owl:oneOf rdf:parseType="Collection">
                                    <rdf:Description rdf:about="http://purl.imsglobal.org/caliper/actions/ChangedResolution"/>
                                    <rdf:Description rdf:about="http://purl.imsglobal.org/caliper/actions/ChangedSize"/>
                                    <rdf:Description rdf:about="http://purl.imsglobal.org/caliper/actions/ChangedSpeed"/>
                                    <rdf:Description rdf:about="http://purl.imsglobal.org/caliper/actions/ChangedVolume"/>
                                    <rdf:Description rdf:about="http://purl.imsglobal.org/caliper/actions/ClosedPopout"/>
                                    <rdf:Description rdf:about="http://purl.imsglobal.org/caliper/actions/DisabledClosedCaptioning"/>
                                    <rdf:Description rdf:about="http://purl.imsglobal.org/caliper/actions/EnabledClosedCaptioning"/>
                                    <rdf:Description rdf:about="http://purl.imsglobal.org/caliper/actions/Ended"/>
                                    <rdf:Description rdf:about="http://purl.imsglobal.org/caliper/actions/EnteredFullScreen"/>
                                    <rdf:Description rdf:about="http://purl.imsglobal.org/caliper/actions/ExitedFullScreen"/>
                                    <rdf:Description rdf:about="http://purl.imsglobal.org/caliper/actions/ForwardedTo"/>
                                    <rdf:Description rdf:about="http://purl.imsglobal.org/caliper/actions/JumpedTo"/>
                                    <rdf:Description rdf:about="http://purl.imsglobal.org/caliper/actions/Muted"/>
                                    <rdf:Description rdf:about="http://purl.imsglobal.org/caliper/actions/OpenedPopout"/>
                                    <rdf:Description rdf:about="http://purl.imsglobal.org/caliper/actions/Paused"/>
                                    <rdf:Description rdf:about="http://purl.imsglobal.org/caliper/actions/Restarted"/>
                                    <rdf:Description rdf:about="http://purl.imsglobal.org/caliper/actions/Resumed"/>
                                    <rdf:Description rdf:about="http://purl.imsglobal.org/caliper/actions/Started"/>
                                    <rdf:Description rdf:about="http://purl.imsglobal.org/caliper/actions/Unmuted"/>
                                </owl:oneOf>
                            </owl:Class>
                        </owl:someValuesFrom>
                    </owl:Restriction>
                </owl:intersectionOf>
            </owl:Class>
        </rdfs:subClassOf>
        <rdfs:subClassOf>
            <owl:Class>
                <owl:intersectionOf rdf:parseType="Collection">
                    <owl:Restriction>
                        <owl:onProperty rdf:resource="http://purl.imsglobal.org/caliper/actor"/>
                        <owl:someValuesFrom rdf:resource="http://purl.imsglobal.org/caliper/Agent"/>
                    </owl:Restriction>
                    <owl:Restriction>
                        <owl:onProperty rdf:resource="http://purl.imsglobal.org/caliper/actor"/>
                        <owl:allValuesFrom rdf:resource="http://purl.imsglobal.org/caliper/Person"/>
                    </owl:Restriction>
                </owl:intersectionOf>
            </owl:Class>
        </rdfs:subClassOf>
        <rdfs:subClassOf>
            <owl:Class>
                <owl:intersectionOf rdf:parseType="Collection">
                    <owl:Restriction>
                        <owl:onProperty rdf:resource="http://purl.imsglobal.org/caliper/object"/>
                        <owl:someValuesFrom rdf:resource="http://purl.imsglobal.org/caliper/DigitalResource"/>
                    </owl:Restriction>
                    <owl:Restriction>
                        <owl:onProperty rdf:resource="http://purl.imsglobal.org/caliper/object"/>
                        <owl:allValuesFrom rdf:resource="http://purl.imsglobal.org/caliper/MediaObject"/>
                    </owl:Restriction>
                </owl:intersectionOf>
            </owl:Class>
        </rdfs:subClassOf>
        <rdfs:subClassOf>
            <owl:Restriction>
                <owl:onProperty rdf:resource="http://purl.imsglobal.org/caliper/target"/>
                <owl:someValuesFrom rdf:resource="http://purl.imsglobal.org/caliper/MediaLocation"/>
            </owl:Restriction>
        </rdfs:subClassOf>
        <rdfs:comment xml:lang="en">A Caliper MediaEvent models interactions between learners and rich content such as audio, images and video.</rdfs:comment>
        <rdfs:isDefinedBy rdf:datatype="http://www.w3.org/2001/XMLSchema#string">http://purl.imsglobal.org/caliper</rdfs:isDefinedBy>
        <rdfs:label xml:lang="en">MediaEvent</rdfs:label>
    </owl:Class>
    


    <!-- http://purl.imsglobal.org/caliper/MediaLocation -->

    <owl:Class rdf:about="http://purl.imsglobal.org/caliper/MediaLocation">
        <rdfs:subClassOf rdf:resource="http://purl.imsglobal.org/caliper/DigitalResource"/>
        <rdfs:comment xml:lang="en">A Caliper MediaLocation provides the current playback position in a MediaObject such as an AudioObject or VideoObject.</rdfs:comment>
        <rdfs:isDefinedBy rdf:datatype="http://www.w3.org/2001/XMLSchema#string">http://purl.imsglobal.org/caliper</rdfs:isDefinedBy>
        <rdfs:label xml:lang="en">MediaLocation</rdfs:label>
    </owl:Class>
    


    <!-- http://purl.imsglobal.org/caliper/MediaObject -->

    <owl:Class rdf:about="http://purl.imsglobal.org/caliper/MediaObject">
        <rdfs:subClassOf rdf:resource="http://purl.imsglobal.org/caliper/DigitalResource"/>
        <rdfs:comment xml:lang="en">A Caliper MediaObject represents a generic piece of media content.  Utilize MediaObject only if no suitable subtype exists to represent the resource being described.</rdfs:comment>
        <rdfs:isDefinedBy rdf:datatype="http://www.w3.org/2001/XMLSchema#string">http://purl.imsglobal.org/caliper</rdfs:isDefinedBy>
        <rdfs:label xml:lang="en">MediaObject</rdfs:label>
    </owl:Class>
    


    <!-- http://purl.imsglobal.org/caliper/Membership -->

    <owl:Class rdf:about="http://purl.imsglobal.org/caliper/Membership">
        <rdfs:subClassOf rdf:resource="http://purl.imsglobal.org/caliper/Entity"/>
        <rdfs:subClassOf>
            <owl:Class>
                <owl:intersectionOf rdf:parseType="Collection">
                    <owl:Restriction>
                        <owl:onProperty rdf:resource="http://purl.imsglobal.org/caliper/member"/>
                        <owl:someValuesFrom rdf:resource="http://purl.imsglobal.org/caliper/Agent"/>
                    </owl:Restriction>
                    <owl:Restriction>
                        <owl:onProperty rdf:resource="http://purl.imsglobal.org/caliper/member"/>
                        <owl:allValuesFrom rdf:resource="http://purl.imsglobal.org/caliper/Person"/>
                    </owl:Restriction>
                </owl:intersectionOf>
            </owl:Class>
        </rdfs:subClassOf>
        <rdfs:subClassOf>
            <owl:Class>
                <owl:intersectionOf rdf:parseType="Collection">
                    <owl:Restriction>
                        <owl:onProperty rdf:resource="http://purl.imsglobal.org/caliper/organization"/>
                        <owl:someValuesFrom rdf:resource="http://purl.imsglobal.org/caliper/Agent"/>
                    </owl:Restriction>
                    <owl:Restriction>
                        <owl:onProperty rdf:resource="http://purl.imsglobal.org/caliper/organization"/>
                        <owl:allValuesFrom rdf:resource="http://purl.imsglobal.org/caliper/Organization"/>
                    </owl:Restriction>
                </owl:intersectionOf>
            </owl:Class>
        </rdfs:subClassOf>
        <rdfs:comment xml:lang="en">A Caliper Membership describes the relationship between an Organization and a Person (i.e., a member) in terms of the roles assigned and current status.</rdfs:comment>
        <rdfs:isDefinedBy rdf:datatype="http://www.w3.org/2001/XMLSchema#string">http://purl.imsglobal.org/caliper</rdfs:isDefinedBy>
        <rdfs:label xml:lang="en">Membership</rdfs:label>
    </owl:Class>
    


    <!-- http://purl.imsglobal.org/caliper/Message -->

    <owl:Class rdf:about="http://purl.imsglobal.org/caliper/Message">
        <rdfs:subClassOf rdf:resource="http://purl.imsglobal.org/caliper/DigitalResource"/>
        <rdfs:subClassOf>
            <owl:Class>
                <owl:intersectionOf rdf:parseType="Collection">
                    <owl:Restriction>
                        <owl:onProperty rdf:resource="http://purl.imsglobal.org/caliper/isPartOf"/>
                        <owl:someValuesFrom rdf:resource="http://purl.imsglobal.org/caliper/Entity"/>
                    </owl:Restriction>
                    <owl:Restriction>
                        <owl:onProperty rdf:resource="http://purl.imsglobal.org/caliper/isPartOf"/>
                        <owl:allValuesFrom rdf:resource="http://purl.imsglobal.org/caliper/Thread"/>
                    </owl:Restriction>
                </owl:intersectionOf>
            </owl:Class>
        </rdfs:subClassOf>
        <rdfs:comment xml:lang="en">A Caliper Message is a digital form of written communication sent to a recipient. A series of messages may constitute a Thread if they share a common subject and are connected by a reply or by date relationships.</rdfs:comment>
        <rdfs:isDefinedBy rdf:datatype="http://www.w3.org/2001/XMLSchema#string">http://purl.imsglobal.org/caliper</rdfs:isDefinedBy>
        <rdfs:label xml:lang="en">Message</rdfs:label>
    </owl:Class>
    


    <!-- http://purl.imsglobal.org/caliper/MessageEvent -->

    <owl:Class rdf:about="http://purl.imsglobal.org/caliper/MessageEvent">
        <rdfs:subClassOf rdf:resource="http://purl.imsglobal.org/caliper/Event"/>
        <rdfs:subClassOf>
            <owl:Class>
                <owl:intersectionOf rdf:parseType="Collection">
                    <owl:Restriction>
                        <owl:onProperty rdf:resource="http://purl.imsglobal.org/caliper/action"/>
                        <owl:someValuesFrom rdf:resource="http://purl.imsglobal.org/caliper/Action"/>
                    </owl:Restriction>
                    <owl:Restriction>
                        <owl:onProperty rdf:resource="http://purl.imsglobal.org/caliper/action"/>
                        <owl:someValuesFrom>
                            <owl:Class>
                                <owl:oneOf rdf:parseType="Collection">
                                    <rdf:Description rdf:about="http://purl.imsglobal.org/caliper/actions/MarkedAsRead"/>
                                    <rdf:Description rdf:about="http://purl.imsglobal.org/caliper/actions/MarkedAsUnread"/>
                                    <rdf:Description rdf:about="http://purl.imsglobal.org/caliper/actions/Posted"/>
                                </owl:oneOf>
                            </owl:Class>
                        </owl:someValuesFrom>
                    </owl:Restriction>
                </owl:intersectionOf>
            </owl:Class>
        </rdfs:subClassOf>
        <rdfs:subClassOf>
            <owl:Class>
                <owl:intersectionOf rdf:parseType="Collection">
                    <owl:Restriction>
                        <owl:onProperty rdf:resource="http://purl.imsglobal.org/caliper/actor"/>
                        <owl:someValuesFrom rdf:resource="http://purl.imsglobal.org/caliper/Agent"/>
                    </owl:Restriction>
                    <owl:Restriction>
                        <owl:onProperty rdf:resource="http://purl.imsglobal.org/caliper/actor"/>
                        <owl:allValuesFrom rdf:resource="http://purl.imsglobal.org/caliper/Person"/>
                    </owl:Restriction>
                </owl:intersectionOf>
            </owl:Class>
        </rdfs:subClassOf>
        <rdfs:subClassOf>
            <owl:Class>
                <owl:intersectionOf rdf:parseType="Collection">
                    <owl:Restriction>
                        <owl:onProperty rdf:resource="http://purl.imsglobal.org/caliper/object"/>
                        <owl:someValuesFrom rdf:resource="http://purl.imsglobal.org/caliper/DigitalResource"/>
                    </owl:Restriction>
                    <owl:Restriction>
                        <owl:onProperty rdf:resource="http://purl.imsglobal.org/caliper/object"/>
                        <owl:allValuesFrom rdf:resource="http://purl.imsglobal.org/caliper/Message"/>
                    </owl:Restriction>
                </owl:intersectionOf>
            </owl:Class>
        </rdfs:subClassOf>
        <rdfs:comment xml:lang="en">A Caliper MessageEvent describes a Person posting a Message or marking a post as either read or unread.</rdfs:comment>
        <rdfs:isDefinedBy rdf:datatype="http://www.w3.org/2001/XMLSchema#string">http://purl.imsglobal.org/caliper</rdfs:isDefinedBy>
        <rdfs:label xml:lang="en">MessageEvent</rdfs:label>
    </owl:Class>
    


    <!-- http://purl.imsglobal.org/caliper/Metric -->

    <owl:Class rdf:about="http://purl.imsglobal.org/caliper/Metric">
        <rdfs:comment xml:lang="en">The AggregateMeasure entity includes a required metric property for denoting the metric related to the ToolUseEvent.</rdfs:comment>
        <rdfs:isDefinedBy rdf:datatype="http://www.w3.org/2001/XMLSchema#string">http://purl.imsglobal.org/caliper</rdfs:isDefinedBy>
        <rdfs:label xml:lang="en">Metric</rdfs:label>
    </owl:Class>
    


    <!-- http://purl.imsglobal.org/caliper/MultiSelectScale -->

    <owl:Class rdf:about="http://purl.imsglobal.org/caliper/MultiSelectScale">
        <rdfs:subClassOf rdf:resource="http://purl.imsglobal.org/caliper/Scale"/>
        <rdfs:comment xml:lang="en">A Caliper MultiselectScale models a scale used to capture one or more rating options.</rdfs:comment>
        <rdfs:isDefinedBy rdf:datatype="http://www.w3.org/2001/XMLSchema#string">https://purl.imsglobal.org/caliper</rdfs:isDefinedBy>
        <rdfs:label xml:lang="en">MultiSelectScale</rdfs:label>
    </owl:Class>
    


    <!-- http://purl.imsglobal.org/caliper/MultipleChoiceResponse -->

    <owl:Class rdf:about="http://purl.imsglobal.org/caliper/MultipleChoiceResponse">
        <rdfs:subClassOf rdf:resource="http://purl.imsglobal.org/caliper/Response"/>
        <rdfs:comment xml:lang="en">A Caliper MultipleChoiceResponse represents a type of Response in which a respondent is asked to provide the best possible answer from a list of choices.</rdfs:comment>
        <rdfs:isDefinedBy rdf:datatype="http://www.w3.org/2001/XMLSchema#string">http://purl.imsglobal.org/caliper</rdfs:isDefinedBy>
        <rdfs:label xml:lang="en">MultipleChoiceResponse</rdfs:label>
    </owl:Class>
    


    <!-- http://purl.imsglobal.org/caliper/MultipleResponseResponse -->

    <owl:Class rdf:about="http://purl.imsglobal.org/caliper/MultipleResponseResponse">
        <rdfs:subClassOf rdf:resource="http://purl.imsglobal.org/caliper/Response"/>
        <rdfs:comment xml:lang="en">A Caliper MultipleResponseResponse represents a form of response in which a respondent is asked to select more than one correct answer from a list of choices.</rdfs:comment>
        <rdfs:isDefinedBy rdf:datatype="http://www.w3.org/2001/XMLSchema#string">http://purl.imsglobal.org/caliper</rdfs:isDefinedBy>
        <rdfs:label xml:lang="en">MultipleResponseResponse</rdfs:label>
    </owl:Class>
    


    <!-- http://purl.imsglobal.org/caliper/NavigationEvent -->

    <owl:Class rdf:about="http://purl.imsglobal.org/caliper/NavigationEvent">
        <rdfs:subClassOf rdf:resource="http://purl.imsglobal.org/caliper/Event"/>
        <rdfs:subClassOf>
            <owl:Class>
                <owl:intersectionOf rdf:parseType="Collection">
                    <owl:Restriction>
                        <owl:onProperty rdf:resource="http://purl.imsglobal.org/caliper/action"/>
                        <owl:someValuesFrom rdf:resource="http://purl.imsglobal.org/caliper/Action"/>
                    </owl:Restriction>
                    <owl:Restriction>
                        <owl:onProperty rdf:resource="http://purl.imsglobal.org/caliper/action"/>
                        <owl:hasValue rdf:resource="http://purl.imsglobal.org/caliper/actions/NavigatedTo"/>
                    </owl:Restriction>
                </owl:intersectionOf>
            </owl:Class>
        </rdfs:subClassOf>
        <rdfs:subClassOf>
            <owl:Class>
                <owl:intersectionOf rdf:parseType="Collection">
                    <owl:Restriction>
                        <owl:onProperty rdf:resource="http://purl.imsglobal.org/caliper/actor"/>
                        <owl:someValuesFrom rdf:resource="http://purl.imsglobal.org/caliper/Agent"/>
                    </owl:Restriction>
                    <owl:Restriction>
                        <owl:onProperty rdf:resource="http://purl.imsglobal.org/caliper/actor"/>
                        <owl:allValuesFrom rdf:resource="http://purl.imsglobal.org/caliper/Person"/>
                    </owl:Restriction>
                </owl:intersectionOf>
            </owl:Class>
        </rdfs:subClassOf>
        <rdfs:subClassOf>
            <owl:Class>
                <owl:intersectionOf rdf:parseType="Collection">
                    <owl:Restriction>
                        <owl:onProperty rdf:resource="http://purl.imsglobal.org/caliper/object"/>
                        <owl:someValuesFrom rdf:resource="http://purl.imsglobal.org/caliper/Entity"/>
                    </owl:Restriction>
                    <owl:Restriction>
                        <owl:onProperty rdf:resource="http://purl.imsglobal.org/caliper/object"/>
                        <owl:allValuesFrom>
                            <owl:Class>
                                <owl:unionOf rdf:parseType="Collection">
                                    <rdf:Description rdf:about="http://purl.imsglobal.org/caliper/DigitalResource"/>
                                    <rdf:Description rdf:about="http://purl.imsglobal.org/caliper/SoftwareApplication"/>
                                </owl:unionOf>
                            </owl:Class>
                        </owl:allValuesFrom>
                    </owl:Restriction>
                </owl:intersectionOf>
            </owl:Class>
        </rdfs:subClassOf>
        <rdfs:subClassOf>
            <owl:Class>
                <owl:intersectionOf rdf:parseType="Collection">
                    <owl:Restriction>
                        <owl:onProperty rdf:resource="http://purl.imsglobal.org/caliper/referrer"/>
                        <owl:someValuesFrom rdf:resource="http://purl.imsglobal.org/caliper/Entity"/>
                    </owl:Restriction>
                    <owl:Restriction>
                        <owl:onProperty rdf:resource="http://purl.imsglobal.org/caliper/referrer"/>
                        <owl:allValuesFrom>
                            <owl:Class>
                                <owl:unionOf rdf:parseType="Collection">
                                    <rdf:Description rdf:about="http://purl.imsglobal.org/caliper/DigitalResource"/>
                                    <rdf:Description rdf:about="http://purl.imsglobal.org/caliper/SoftwareApplication"/>
                                </owl:unionOf>
                            </owl:Class>
                        </owl:allValuesFrom>
                    </owl:Restriction>
                </owl:intersectionOf>
            </owl:Class>
        </rdfs:subClassOf>
        <rdfs:subClassOf>
            <owl:Restriction>
                <owl:onProperty rdf:resource="http://purl.imsglobal.org/caliper/target"/>
                <owl:someValuesFrom rdf:resource="http://purl.imsglobal.org/caliper/Frame"/>
            </owl:Restriction>
        </rdfs:subClassOf>
        <rdfs:comment xml:lang="en">A Caliper NavigationEvent models an actor traversing a network of digital resources.</rdfs:comment>
        <rdfs:isDefinedBy rdf:datatype="http://www.w3.org/2001/XMLSchema#string">http://purl.imsglobal.org/caliper</rdfs:isDefinedBy>
        <rdfs:label xml:lang="en">NavigationEvent</rdfs:label>
    </owl:Class>
    


    <!-- http://purl.imsglobal.org/caliper/NumericScale -->

    <owl:Class rdf:about="http://purl.imsglobal.org/caliper/NumericScale">
        <rdfs:subClassOf rdf:resource="http://purl.imsglobal.org/caliper/Scale"/>
        <rdfs:comment xml:lang="en">A Caliper NumericScale models a numeric scale used to capture some rating.</rdfs:comment>
        <rdfs:isDefinedBy rdf:datatype="http://www.w3.org/2001/XMLSchema#string">https://purl.imsglobal.org/caliper</rdfs:isDefinedBy>
        <rdfs:label xml:lang="en">NumericScale</rdfs:label>
    </owl:Class>
    


    <!-- http://purl.imsglobal.org/caliper/Organization -->

    <owl:Class rdf:about="http://purl.imsglobal.org/caliper/Organization">
        <rdfs:subClassOf rdf:resource="http://purl.imsglobal.org/caliper/Agent"/>
        <rdfs:comment xml:lang="en">A Caliper Organization represents a formal collection of people organized for some common educational, social or administrative purpose. An Organization can act as an Agent. It can be linked both to a parent Organization and to its members.</rdfs:comment>
        <rdfs:isDefinedBy rdf:datatype="http://www.w3.org/2001/XMLSchema#string">http://purl.imsglobal.org/caliper</rdfs:isDefinedBy>
        <rdfs:label xml:lang="en">Organization</rdfs:label>
    </owl:Class>
    


    <!-- http://purl.imsglobal.org/caliper/OutcomeEvent -->

    <owl:Class rdf:about="http://purl.imsglobal.org/caliper/OutcomeEvent">
        <rdfs:subClassOf rdf:resource="http://purl.imsglobal.org/caliper/Event"/>
        <rdfs:subClassOf>
            <owl:Class>
                <owl:intersectionOf rdf:parseType="Collection">
                    <owl:Restriction>
                        <owl:onProperty rdf:resource="http://purl.imsglobal.org/caliper/action"/>
                        <owl:someValuesFrom rdf:resource="http://purl.imsglobal.org/caliper/Action"/>
                    </owl:Restriction>
                    <owl:Restriction>
                        <owl:onProperty rdf:resource="http://purl.imsglobal.org/caliper/action"/>
                        <owl:hasValue rdf:resource="http://purl.imsglobal.org/caliper/actions/Graded"/>
                    </owl:Restriction>
                </owl:intersectionOf>
            </owl:Class>
        </rdfs:subClassOf>
        <rdfs:subClassOf>
            <owl:Class>
                <owl:intersectionOf rdf:parseType="Collection">
                    <owl:Restriction>
                        <owl:onProperty rdf:resource="http://purl.imsglobal.org/caliper/actor"/>
                        <owl:someValuesFrom rdf:resource="http://purl.imsglobal.org/caliper/Agent"/>
                    </owl:Restriction>
                    <owl:Restriction>
                        <owl:onProperty rdf:resource="http://purl.imsglobal.org/caliper/actor"/>
                        <owl:allValuesFrom>
                            <owl:Class>
                                <owl:unionOf rdf:parseType="Collection">
                                    <rdf:Description rdf:about="http://purl.imsglobal.org/caliper/Person"/>
                                    <rdf:Description rdf:about="http://purl.imsglobal.org/caliper/SoftwareApplication"/>
                                </owl:unionOf>
                            </owl:Class>
                        </owl:allValuesFrom>
                    </owl:Restriction>
                </owl:intersectionOf>
            </owl:Class>
        </rdfs:subClassOf>
        <rdfs:subClassOf>
            <owl:Class>
                <owl:intersectionOf rdf:parseType="Collection">
                    <owl:Restriction>
                        <owl:onProperty rdf:resource="http://purl.imsglobal.org/caliper/generated"/>
                        <owl:someValuesFrom rdf:resource="http://purl.imsglobal.org/caliper/Entity"/>
                    </owl:Restriction>
                    <owl:Restriction>
                        <owl:onProperty rdf:resource="http://purl.imsglobal.org/caliper/generated"/>
                        <owl:allValuesFrom rdf:resource="http://purl.imsglobal.org/caliper/Result"/>
                    </owl:Restriction>
                </owl:intersectionOf>
            </owl:Class>
        </rdfs:subClassOf>
        <rdfs:subClassOf>
            <owl:Class>
                <owl:intersectionOf rdf:parseType="Collection">
                    <owl:Restriction>
                        <owl:onProperty rdf:resource="http://purl.imsglobal.org/caliper/object"/>
                        <owl:someValuesFrom rdf:resource="http://purl.imsglobal.org/caliper/Entity"/>
                    </owl:Restriction>
                    <owl:Restriction>
                        <owl:onProperty rdf:resource="http://purl.imsglobal.org/caliper/object"/>
                        <owl:allValuesFrom rdf:resource="http://purl.imsglobal.org/caliper/Attempt"/>
                    </owl:Restriction>
                </owl:intersectionOf>
            </owl:Class>
        </rdfs:subClassOf>
        <terms:isReplacedBy rdf:resource="http://purl.imsglobal.org/caliper/GradeEvent"/>
        <rdfs:comment xml:lang="en">A Caliper OutcomeEvent models grading activities performed by an Agent, typically a Person or a SoftwareApplication.  OutcomeEvent is DEPRECATED and will be removed in a future version of the specification. Use GradeEvent instead.</rdfs:comment>
        <rdfs:isDefinedBy rdf:datatype="http://www.w3.org/2001/XMLSchema#string">http://purl.imsglobal.org/caliper</rdfs:isDefinedBy>
        <rdfs:label xml:lang="en">OutcomeEvent</rdfs:label>
        <owl:deprecated rdf:datatype="http://www.w3.org/2001/XMLSchema#boolean">true</owl:deprecated>
    </owl:Class>
    


    <!-- http://purl.imsglobal.org/caliper/Page -->

    <owl:Class rdf:about="http://purl.imsglobal.org/caliper/Page">
        <rdfs:subClassOf rdf:resource="http://purl.imsglobal.org/caliper/DigitalResource"/>
        <rdfs:comment xml:lang="en">A Caliper Page represents an item of paginated content.</rdfs:comment>
        <rdfs:isDefinedBy rdf:datatype="http://www.w3.org/2001/XMLSchema#string">http://purl.imsglobal.org/caliper</rdfs:isDefinedBy>
        <rdfs:label xml:lang="en">Page</rdfs:label>
    </owl:Class>
    


    <!-- http://purl.imsglobal.org/caliper/Person -->

    <owl:Class rdf:about="http://purl.imsglobal.org/caliper/Person">
        <rdfs:subClassOf rdf:resource="http://purl.imsglobal.org/caliper/Agent"/>
        <rdfs:comment xml:lang="en">A Caliper Person represents a human being, alive or deceased, real or imaginary.</rdfs:comment>
        <rdfs:isDefinedBy rdf:datatype="http://www.w3.org/2001/XMLSchema#string">http://purl.imsglobal.org/caliper</rdfs:isDefinedBy>
        <rdfs:label xml:lang="en">Person</rdfs:label>
    </owl:Class>
    


    <!-- http://purl.imsglobal.org/caliper/Query -->

    <owl:Class rdf:about="http://purl.imsglobal.org/caliper/Query">
        <rdfs:subClassOf rdf:resource="http://purl.imsglobal.org/caliper/Entity"/>
        <rdfs:comment xml:lang="en">A Caliper Query models search criteria created by an actor that targets a searchable resource.</rdfs:comment>
        <rdfs:isDefinedBy rdf:datatype="http://www.w3.org/2001/XMLSchema#string">http://purl.imsglobal.org/caliper</rdfs:isDefinedBy>
        <rdfs:label xml:lang="en">Query</rdfs:label>
    </owl:Class>
    


    <!-- http://purl.imsglobal.org/caliper/Rating -->

    <owl:Class rdf:about="http://purl.imsglobal.org/caliper/Rating">
        <rdfs:subClassOf rdf:resource="http://purl.imsglobal.org/caliper/Entity"/>
        <rdfs:subClassOf>
            <owl:Class>
                <owl:intersectionOf rdf:parseType="Collection">
                    <owl:Restriction>
                        <owl:onProperty rdf:resource="http://purl.imsglobal.org/caliper/rater"/>
                        <owl:someValuesFrom rdf:resource="http://purl.imsglobal.org/caliper/Agent"/>
                    </owl:Restriction>
                    <owl:Restriction>
                        <owl:onProperty rdf:resource="http://purl.imsglobal.org/caliper/rater"/>
                        <owl:allValuesFrom rdf:resource="http://purl.imsglobal.org/caliper/Person"/>
                    </owl:Restriction>
                </owl:intersectionOf>
            </owl:Class>
        </rdfs:subClassOf>
        <rdfs:subClassOf>
            <owl:Restriction>
                <owl:onProperty rdf:resource="http://purl.imsglobal.org/caliper/rated"/>
                <owl:someValuesFrom rdf:resource="http://purl.imsglobal.org/caliper/Entity"/>
            </owl:Restriction>
        </rdfs:subClassOf>
        <rdfs:comment xml:lang="en">A Caliper Rating models quantitative reactions to an Entity.</rdfs:comment>
        <rdfs:isDefinedBy rdf:datatype="http://www.w3.org/2001/XMLSchema#string">https://purl.imsglobal.org/caliper</rdfs:isDefinedBy>
        <rdfs:label xml:lang="en">Rating</rdfs:label>
    </owl:Class>
    


    <!-- http://purl.imsglobal.org/caliper/Reading -->

    <owl:Class rdf:about="http://purl.imsglobal.org/caliper/Reading">
        <rdfs:subClassOf rdf:resource="http://purl.imsglobal.org/caliper/DigitalResource"/>
        <terms:isReplacedBy rdf:resource="http://purl.imsglobal.org/caliper/Document"/>
        <rdfs:comment xml:lang="en">A Caliper Reading represents paginated content. Reading is a DEPRECATED entity superseded by Document that will be removed in a future version of the specification. It SHOULD NOT be referenced.</rdfs:comment>
        <rdfs:isDefinedBy rdf:datatype="http://www.w3.org/2001/XMLSchema#string">http://purl.imsglobal.org/caliper</rdfs:isDefinedBy>
        <rdfs:label xml:lang="en">Reading</rdfs:label>
        <owl:deprecated rdf:datatype="http://www.w3.org/2001/XMLSchema#boolean">true</owl:deprecated>
    </owl:Class>
    


    <!-- http://purl.imsglobal.org/caliper/ReadingEvent -->

    <owl:Class rdf:about="http://purl.imsglobal.org/caliper/ReadingEvent">
        <rdfs:subClassOf rdf:resource="http://purl.imsglobal.org/caliper/Event"/>
        <rdfs:subClassOf>
            <owl:Class>
                <owl:intersectionOf rdf:parseType="Collection">
                    <owl:Restriction>
                        <owl:onProperty rdf:resource="http://purl.imsglobal.org/caliper/action"/>
                        <owl:someValuesFrom rdf:resource="http://purl.imsglobal.org/caliper/Action"/>
                    </owl:Restriction>
                    <owl:Restriction>
                        <owl:onProperty rdf:resource="http://purl.imsglobal.org/caliper/action"/>
                        <owl:someValuesFrom>
                            <owl:Class>
                                <owl:oneOf rdf:parseType="Collection">
                                    <rdf:Description rdf:about="http://purl.imsglobal.org/caliper/actions/NavigatedTo"/>
                                    <rdf:Description rdf:about="http://purl.imsglobal.org/caliper/actions/Searched"/>
                                    <rdf:Description rdf:about="http://purl.imsglobal.org/caliper/actions/Viewed"/>
                                </owl:oneOf>
                            </owl:Class>
                        </owl:someValuesFrom>
                    </owl:Restriction>
                </owl:intersectionOf>
            </owl:Class>
        </rdfs:subClassOf>
        <rdfs:subClassOf>
            <owl:Class>
                <owl:intersectionOf rdf:parseType="Collection">
                    <owl:Restriction>
                        <owl:onProperty rdf:resource="http://purl.imsglobal.org/caliper/actor"/>
                        <owl:someValuesFrom rdf:resource="http://purl.imsglobal.org/caliper/Agent"/>
                    </owl:Restriction>
                    <owl:Restriction>
                        <owl:onProperty rdf:resource="http://purl.imsglobal.org/caliper/actor"/>
                        <owl:allValuesFrom rdf:resource="http://purl.imsglobal.org/caliper/Person"/>
                    </owl:Restriction>
                </owl:intersectionOf>
            </owl:Class>
        </rdfs:subClassOf>
        <rdfs:subClassOf>
            <owl:Class>
                <owl:intersectionOf rdf:parseType="Collection">
                    <owl:Restriction>
                        <owl:onProperty rdf:resource="http://purl.imsglobal.org/caliper/object"/>
                        <owl:someValuesFrom rdf:resource="http://purl.imsglobal.org/caliper/Entity"/>
                    </owl:Restriction>
                    <owl:Restriction>
                        <owl:onProperty rdf:resource="http://purl.imsglobal.org/caliper/object"/>
                        <owl:allValuesFrom rdf:resource="http://purl.imsglobal.org/caliper/DigitalResource"/>
                    </owl:Restriction>
                </owl:intersectionOf>
            </owl:Class>
        </rdfs:subClassOf>
        <rdfs:subClassOf>
            <owl:Restriction>
                <owl:onProperty rdf:resource="http://purl.imsglobal.org/caliper/target"/>
                <owl:someValuesFrom rdf:resource="http://purl.imsglobal.org/caliper/Frame"/>
            </owl:Restriction>
        </rdfs:subClassOf>
        <rdfs:comment xml:lang="en">A Caliper ReadingEvent models an actor reading textural content.  ReadingEvent is DEPRECATED and will be removed in a future version of the specification.  It SHOULD NOT be referenced.</rdfs:comment>
        <rdfs:isDefinedBy rdf:datatype="http://www.w3.org/2001/XMLSchema#string">http://purl.imsglobal.org/caliper</rdfs:isDefinedBy>
        <rdfs:label xml:lang="en">ReadingEvent</rdfs:label>
        <owl:deprecated rdf:datatype="http://www.w3.org/2001/XMLSchema#boolean">true</owl:deprecated>
    </owl:Class>
    


    <!-- http://purl.imsglobal.org/caliper/ResourceManagementEvent -->

    <owl:Class rdf:about="http://purl.imsglobal.org/caliper/ResourceManagementEvent">
        <rdfs:subClassOf rdf:resource="http://purl.imsglobal.org/caliper/Event"/>
        <rdfs:subClassOf>
            <owl:Class>
                <owl:intersectionOf rdf:parseType="Collection">
                    <owl:Restriction>
                        <owl:onProperty rdf:resource="http://purl.imsglobal.org/caliper/action"/>
                        <owl:someValuesFrom rdf:resource="http://purl.imsglobal.org/caliper/Action"/>
                    </owl:Restriction>
                    <owl:Restriction>
                        <owl:onProperty rdf:resource="http://purl.imsglobal.org/caliper/action"/>
                        <owl:someValuesFrom>
                            <owl:Class>
                                <owl:oneOf rdf:parseType="Collection">
                                    <rdf:Description rdf:about="http://purl.imsglobal.org/actions/Archived"/>
                                    <rdf:Description rdf:about="http://purl.imsglobal.org/actions/Copied"/>
                                    <rdf:Description rdf:about="http://purl.imsglobal.org/actions/Published"/>
                                    <rdf:Description rdf:about="http://purl.imsglobal.org/actions/Restored"/>
                                    <rdf:Description rdf:about="http://purl.imsglobal.org/actions/Unpublished"/>
                                    <rdf:Description rdf:about="http://purl.imsglobal.org/caliper/actions/Created"/>
                                    <rdf:Description rdf:about="http://purl.imsglobal.org/caliper/actions/Deleted"/>
                                    <rdf:Description rdf:about="http://purl.imsglobal.org/caliper/actions/Described"/>
                                    <rdf:Description rdf:about="http://purl.imsglobal.org/caliper/actions/Modified"/>
                                    <rdf:Description rdf:about="http://purl.imsglobal.org/caliper/actions/Retrieved"/>
                                </owl:oneOf>
                            </owl:Class>
                        </owl:someValuesFrom>
                    </owl:Restriction>
                </owl:intersectionOf>
            </owl:Class>
        </rdfs:subClassOf>
        <rdfs:subClassOf>
            <owl:Class>
                <owl:intersectionOf rdf:parseType="Collection">
                    <owl:Restriction>
                        <owl:onProperty rdf:resource="http://purl.imsglobal.org/caliper/actor"/>
                        <owl:someValuesFrom rdf:resource="http://purl.imsglobal.org/caliper/Agent"/>
                    </owl:Restriction>
                    <owl:Restriction>
                        <owl:onProperty rdf:resource="http://purl.imsglobal.org/caliper/actor"/>
                        <owl:allValuesFrom rdf:resource="http://purl.imsglobal.org/caliper/Person"/>
                    </owl:Restriction>
                </owl:intersectionOf>
            </owl:Class>
        </rdfs:subClassOf>
        <rdfs:subClassOf>
            <owl:Class>
                <owl:intersectionOf rdf:parseType="Collection">
                    <owl:Restriction>
                        <owl:onProperty rdf:resource="http://purl.imsglobal.org/caliper/object"/>
                        <owl:someValuesFrom rdf:resource="http://purl.imsglobal.org/caliper/Entity"/>
                    </owl:Restriction>
                    <owl:Restriction>
                        <owl:onProperty rdf:resource="http://purl.imsglobal.org/caliper/object"/>
                        <owl:allValuesFrom rdf:resource="http://purl.imsglobal.org/caliper/DigitalResource"/>
                    </owl:Restriction>
                </owl:intersectionOf>
            </owl:Class>
        </rdfs:subClassOf>
        <rdfs:subClassOf>
            <owl:Restriction>
                <owl:onProperty rdf:resource="http://purl.imsglobal.org/caliper/generated"/>
                <owl:someValuesFrom rdf:resource="http://purl.imsglobal.org/caliper/Entity"/>
            </owl:Restriction>
        </rdfs:subClassOf>
        <rdfs:comment xml:lang="en">A Caliper ResourceManagementEvent models a Person managing an Entity.</rdfs:comment>
        <rdfs:isDefinedBy rdf:datatype="http://www.w3.org/2001/XMLSchema#string">http://purl.imsglobal.org/caliper</rdfs:isDefinedBy>
        <rdfs:label xml:lang="en">ResourceManagementEvent</rdfs:label>
    </owl:Class>
    


    <!-- http://purl.imsglobal.org/caliper/Response -->

    <owl:Class rdf:about="http://purl.imsglobal.org/caliper/Response">
        <rdfs:subClassOf rdf:resource="http://purl.imsglobal.org/caliper/Entity"/>
        <rdfs:comment xml:lang="en">A Caliper Response is a generic type that represents the selected option generated by a Person interacting with an AssessmentItem.  Utilize Response only if no suitable subtype exists to represent the response being described.</rdfs:comment>
        <rdfs:isDefinedBy rdf:datatype="http://www.w3.org/2001/XMLSchema#string">http://purl.imsglobal.org/caliper</rdfs:isDefinedBy>
        <rdfs:label xml:lang="en">Response</rdfs:label>
    </owl:Class>
    


    <!-- http://purl.imsglobal.org/caliper/Result -->

    <owl:Class rdf:about="http://purl.imsglobal.org/caliper/Result">
        <rdfs:subClassOf rdf:resource="http://purl.imsglobal.org/caliper/Entity"/>
        <rdfs:comment xml:lang="en">A Caliper Result represents a grade applied to an assignment submission.</rdfs:comment>
        <rdfs:isDefinedBy rdf:datatype="http://www.w3.org/2001/XMLSchema#string">http://purl.imsglobal.org/caliper</rdfs:isDefinedBy>
        <rdfs:label xml:lang="en">Result</rdfs:label>
    </owl:Class>
    


    <!-- http://purl.imsglobal.org/caliper/Role -->

    <owl:Class rdf:about="http://purl.imsglobal.org/caliper/Role">
        <rdfs:comment xml:lang="en">A member can have multiple roles in a Membership.  These different roles would be reflected in separate instances of the Role.</rdfs:comment>
        <rdfs:isDefinedBy rdf:datatype="http://www.w3.org/2001/XMLSchema#string">http://www.imsglobal.org/lis/</rdfs:isDefinedBy>
        <rdfs:label xml:lang="en">Role</rdfs:label>
    </owl:Class>
    


    <!-- http://purl.imsglobal.org/caliper/Scale -->

    <owl:Class rdf:about="http://purl.imsglobal.org/caliper/Scale">
        <rdfs:subClassOf rdf:resource="http://purl.imsglobal.org/caliper/Entity"/>
        <rdfs:comment xml:lang="en">A Caliper Scale models a scale employed in order to capture some rating.</rdfs:comment>
        <rdfs:isDefinedBy xml:lang="en">https://purl.imsglobal.org/caliper</rdfs:isDefinedBy>
        <rdfs:label xml:lang="en">Scale</rdfs:label>
    </owl:Class>
    


    <!-- http://purl.imsglobal.org/caliper/Score -->

    <owl:Class rdf:about="http://purl.imsglobal.org/caliper/Score">
        <rdfs:subClassOf rdf:resource="http://purl.imsglobal.org/caliper/Entity"/>
        <rdfs:comment xml:lang="en">A Caliper Score represents a grade.  The Score value is considered immutable.</rdfs:comment>
        <rdfs:isDefinedBy rdf:datatype="http://www.w3.org/2001/XMLSchema#string">http://purl.imsglobal.org/caliper</rdfs:isDefinedBy>
        <rdfs:label xml:lang="en">Score</rdfs:label>
    </owl:Class>
    


    <!-- http://purl.imsglobal.org/caliper/SearchEvent -->

    <owl:Class rdf:about="http://purl.imsglobal.org/caliper/SearchEvent">
        <rdfs:subClassOf rdf:resource="http://purl.imsglobal.org/caliper/Event"/>
        <rdfs:subClassOf>
            <owl:Class>
                <owl:intersectionOf rdf:parseType="Collection">
                    <owl:Restriction>
                        <owl:onProperty rdf:resource="http://purl.imsglobal.org/caliper/action"/>
                        <owl:someValuesFrom rdf:resource="http://purl.imsglobal.org/caliper/Action"/>
                    </owl:Restriction>
                    <owl:Restriction>
                        <owl:onProperty rdf:resource="http://purl.imsglobal.org/caliper/action"/>
                        <owl:hasValue rdf:resource="http://purl.imsglobal.org/caliper/actions/Searched"/>
                    </owl:Restriction>
                </owl:intersectionOf>
            </owl:Class>
        </rdfs:subClassOf>
        <rdfs:subClassOf>
            <owl:Class>
                <owl:intersectionOf rdf:parseType="Collection">
                    <owl:Restriction>
                        <owl:onProperty rdf:resource="http://purl.imsglobal.org/caliper/actor"/>
                        <owl:someValuesFrom rdf:resource="http://purl.imsglobal.org/caliper/Agent"/>
                    </owl:Restriction>
                    <owl:Restriction>
                        <owl:onProperty rdf:resource="http://purl.imsglobal.org/caliper/actor"/>
                        <owl:allValuesFrom rdf:resource="http://purl.imsglobal.org/caliper/Person"/>
                    </owl:Restriction>
                </owl:intersectionOf>
            </owl:Class>
        </rdfs:subClassOf>
        <rdfs:subClassOf>
            <owl:Restriction>
                <owl:onProperty rdf:resource="http://purl.imsglobal.org/caliper/generated"/>
                <owl:someValuesFrom rdf:resource="http://purl.imsglobal.org/caliper/SearchResponse"/>
            </owl:Restriction>
        </rdfs:subClassOf>
        <rdfs:comment xml:lang="en">A Caliper SearchEvent models a Person querying a resource for information, typically a DigitalResource or SoftwareApplication. A SearchResponse may be referenced using the generated property.</rdfs:comment>
        <rdfs:isDefinedBy rdf:datatype="http://www.w3.org/2001/XMLSchema#string">http://purl.imsglobal.org/caliper</rdfs:isDefinedBy>
        <rdfs:label xml:lang="en">SearchEvent</rdfs:label>
    </owl:Class>
    


    <!-- http://purl.imsglobal.org/caliper/SearchResponse -->

    <owl:Class rdf:about="http://purl.imsglobal.org/caliper/SearchResponse">
        <rdfs:subClassOf rdf:resource="http://purl.imsglobal.org/caliper/Entity"/>
        <rdfs:comment xml:lang="en">A Caliper SearchResponse models a search engine response to an actor querying a searchable resource.</rdfs:comment>
        <rdfs:isDefinedBy xml:lang="en">http://purl.imsglobal.org/caliper</rdfs:isDefinedBy>
        <rdfs:label xml:lang="en">SearchResponse</rdfs:label>
    </owl:Class>
    


    <!-- http://purl.imsglobal.org/caliper/SelectTextResponse -->

    <owl:Class rdf:about="http://purl.imsglobal.org/caliper/SelectTextResponse">
        <rdfs:subClassOf rdf:resource="http://purl.imsglobal.org/caliper/Response"/>
        <rdfs:comment xml:lang="en">A Caliper SelectTextResponse represents a type of Response that identifies text or a mapping from a presented paragraph or list.</rdfs:comment>
        <rdfs:isDefinedBy rdf:datatype="http://www.w3.org/2001/XMLSchema#string">http://purl.imsglobal.org/caliper</rdfs:isDefinedBy>
        <rdfs:label xml:lang="en">SelectTextResponse</rdfs:label>
    </owl:Class>
    


    <!-- http://purl.imsglobal.org/caliper/Selector -->

    <owl:Class rdf:about="http://purl.imsglobal.org/caliper/Selector">
        <rdfs:comment xml:lang="en">A Caliper Selector is a generic class that describes a fragment or segment of a resource.  Utilize Selector only if no suitable subtype exists to represent the selection being described.</rdfs:comment>
        <rdfs:isDefinedBy rdf:datatype="http://www.w3.org/2001/XMLSchema#string">http://purl.imsglobal.org/caliper</rdfs:isDefinedBy>
        <rdfs:label xml:lang="en">Selector</rdfs:label>
    </owl:Class>
    


    <!-- http://purl.imsglobal.org/caliper/Session -->

    <owl:Class rdf:about="http://purl.imsglobal.org/caliper/Session">
        <rdfs:subClassOf rdf:resource="http://purl.imsglobal.org/caliper/Entity"/>
        <rdfs:subClassOf>
            <owl:Class>
                <owl:intersectionOf rdf:parseType="Collection">
                    <owl:Restriction>
                        <owl:onProperty rdf:resource="http://purl.imsglobal.org/caliper/user"/>
                        <owl:someValuesFrom rdf:resource="http://purl.imsglobal.org/caliper/Agent"/>
                    </owl:Restriction>
                    <owl:Restriction>
                        <owl:onProperty rdf:resource="http://purl.imsglobal.org/caliper/user"/>
                        <owl:allValuesFrom rdf:resource="http://purl.imsglobal.org/caliper/Person"/>
                    </owl:Restriction>
                </owl:intersectionOf>
            </owl:Class>
        </rdfs:subClassOf>
        <rdfs:comment xml:lang="en">A Caliper Session represents a web application user session.</rdfs:comment>
        <rdfs:isDefinedBy rdf:datatype="http://www.w3.org/2001/XMLSchema#string">http://purl.imsglobal.org/caliper</rdfs:isDefinedBy>
        <rdfs:label xml:lang="en">Session</rdfs:label>
    </owl:Class>
    


    <!-- http://purl.imsglobal.org/caliper/SessionEvent -->

    <owl:Class rdf:about="http://purl.imsglobal.org/caliper/SessionEvent">
        <rdfs:subClassOf rdf:resource="http://purl.imsglobal.org/caliper/Event"/>
        <rdfs:subClassOf>
            <owl:Class>
                <owl:intersectionOf rdf:parseType="Collection">
                    <owl:Restriction>
                        <owl:onProperty rdf:resource="http://purl.imsglobal.org/caliper/action"/>
                        <owl:someValuesFrom rdf:resource="http://purl.imsglobal.org/caliper/Action"/>
                    </owl:Restriction>
                    <owl:Restriction>
                        <owl:onProperty rdf:resource="http://purl.imsglobal.org/caliper/action"/>
                        <owl:someValuesFrom>
                            <owl:Class>
                                <owl:oneOf rdf:parseType="Collection">
                                    <rdf:Description rdf:about="http://purl.imsglobal.org/caliper/actions/LoggedIn"/>
                                    <rdf:Description rdf:about="http://purl.imsglobal.org/caliper/actions/LoggedOut"/>
                                    <rdf:Description rdf:about="http://purl.imsglobal.org/caliper/actions/TimedOut"/>
                                </owl:oneOf>
                            </owl:Class>
                        </owl:someValuesFrom>
                    </owl:Restriction>
                </owl:intersectionOf>
            </owl:Class>
        </rdfs:subClassOf>
        <rdfs:subClassOf>
            <owl:Class>
                <owl:intersectionOf rdf:parseType="Collection">
                    <owl:Restriction>
                        <owl:onProperty rdf:resource="http://purl.imsglobal.org/caliper/actor"/>
                        <owl:someValuesFrom rdf:resource="http://purl.imsglobal.org/caliper/Agent"/>
                    </owl:Restriction>
                    <owl:Restriction>
                        <owl:onProperty rdf:resource="http://purl.imsglobal.org/caliper/actor"/>
                        <owl:allValuesFrom>
                            <owl:Class>
                                <owl:unionOf rdf:parseType="Collection">
                                    <rdf:Description rdf:about="http://purl.imsglobal.org/caliper/Person"/>
                                    <rdf:Description rdf:about="http://purl.imsglobal.org/caliper/SoftwareApplication"/>
                                </owl:unionOf>
                            </owl:Class>
                        </owl:allValuesFrom>
                    </owl:Restriction>
                </owl:intersectionOf>
            </owl:Class>
        </rdfs:subClassOf>
        <rdfs:subClassOf>
            <owl:Class>
                <owl:intersectionOf rdf:parseType="Collection">
                    <owl:Restriction>
                        <owl:onProperty rdf:resource="http://purl.imsglobal.org/caliper/object"/>
                        <owl:someValuesFrom rdf:resource="http://purl.imsglobal.org/caliper/Entity"/>
                    </owl:Restriction>
                    <owl:Restriction>
                        <owl:onProperty rdf:resource="http://purl.imsglobal.org/caliper/object"/>
                        <owl:allValuesFrom>
                            <owl:Class>
                                <owl:unionOf rdf:parseType="Collection">
                                    <rdf:Description rdf:about="http://purl.imsglobal.org/caliper/Session"/>
                                    <rdf:Description rdf:about="http://purl.imsglobal.org/caliper/SoftwareApplication"/>
                                </owl:unionOf>
                            </owl:Class>
                        </owl:allValuesFrom>
                    </owl:Restriction>
                </owl:intersectionOf>
            </owl:Class>
        </rdfs:subClassOf>
        <rdfs:subClassOf>
            <owl:Class>
                <owl:intersectionOf rdf:parseType="Collection">
                    <owl:Restriction>
                        <owl:onProperty rdf:resource="http://purl.imsglobal.org/caliper/referrer"/>
                        <owl:someValuesFrom rdf:resource="http://purl.imsglobal.org/caliper/Entity"/>
                    </owl:Restriction>
                    <owl:Restriction>
                        <owl:onProperty rdf:resource="http://purl.imsglobal.org/caliper/referrer"/>
                        <owl:allValuesFrom>
                            <owl:Class>
                                <owl:unionOf rdf:parseType="Collection">
                                    <rdf:Description rdf:about="http://purl.imsglobal.org/caliper/DigitalResource"/>
                                    <rdf:Description rdf:about="http://purl.imsglobal.org/caliper/SoftwareApplication"/>
                                </owl:unionOf>
                            </owl:Class>
                        </owl:allValuesFrom>
                    </owl:Restriction>
                </owl:intersectionOf>
            </owl:Class>
        </rdfs:subClassOf>
        <rdfs:subClassOf>
            <owl:Restriction>
                <owl:onProperty rdf:resource="http://purl.imsglobal.org/caliper/target"/>
                <owl:someValuesFrom rdf:resource="http://purl.imsglobal.org/caliper/DigitalResource"/>
            </owl:Restriction>
        </rdfs:subClassOf>
        <rdfs:comment xml:lang="en">A Caliper SessionEvent models the creation and subsequent termination of a user session established by a Person interacting with a SoftwareApplication.</rdfs:comment>
        <rdfs:isDefinedBy rdf:datatype="http://www.w3.org/2001/XMLSchema#string">http://purl.imsglobal.org/caliper</rdfs:isDefinedBy>
        <rdfs:label xml:lang="en">SessionEvent</rdfs:label>
    </owl:Class>
    


    <!-- http://purl.imsglobal.org/caliper/SharedAnnotation -->

    <owl:Class rdf:about="http://purl.imsglobal.org/caliper/SharedAnnotation">
        <rdfs:subClassOf rdf:resource="http://purl.imsglobal.org/caliper/Annotation"/>
        <rdfs:comment xml:lang="en">A Caliper SharedAnnotation represents the act of sharing a reference to a DigitalResource with other agents.</rdfs:comment>
        <rdfs:isDefinedBy rdf:datatype="http://www.w3.org/2001/XMLSchema#string">http://purl.imsglobal.org/caliper</rdfs:isDefinedBy>
        <rdfs:label xml:lang="en">SharedAnnotation</rdfs:label>
    </owl:Class>
    


    <!-- http://purl.imsglobal.org/caliper/SoftwareApplication -->

    <owl:Class rdf:about="http://purl.imsglobal.org/caliper/SoftwareApplication">
        <rdfs:subClassOf rdf:resource="http://purl.imsglobal.org/caliper/Agent"/>
        <rdfs:comment xml:lang="en">A Caliper SoftwareApplication represents a computer program, application, module, platform or system.</rdfs:comment>
        <rdfs:isDefinedBy rdf:datatype="http://www.w3.org/2001/XMLSchema#string">http://purl.imsglobal.org/caliper</rdfs:isDefinedBy>
        <rdfs:label xml:lang="en">SoftwareApplication</rdfs:label>
    </owl:Class>
    


    <!-- http://purl.imsglobal.org/caliper/Status -->

    <owl:Class rdf:about="http://purl.imsglobal.org/caliper/Status">
        <rdfs:comment xml:lang="en">Indicates if a member is active or inactive in the collection. This allows the source system to specifically tell the target system that a member is now active or inactive.  Another view is that the absence of a Membership object when membership data is passed implies inactivity and the existence of an object implies active membership.  This will logically work for a ‘snap-shot’ interface where all members are passed every time objects are sent from one system to another but it will not support an interface where individual Membership objects are passed.</rdfs:comment>
        <rdfs:isDefinedBy rdf:datatype="http://www.w3.org/2001/XMLSchema#string">http://www.imsglobal.org/lis/</rdfs:isDefinedBy>
        <rdfs:label xml:lang="en">Status</rdfs:label>
    </owl:Class>
    


    <!-- http://purl.imsglobal.org/caliper/TagAnnotation -->

    <owl:Class rdf:about="http://purl.imsglobal.org/caliper/TagAnnotation">
        <rdfs:subClassOf rdf:resource="http://purl.imsglobal.org/caliper/Annotation"/>
        <rdfs:comment xml:lang="en">A Caliper TagAnnotation represents the act of tagging a DigitalResource with tags or labels.</rdfs:comment>
        <rdfs:isDefinedBy rdf:datatype="http://www.w3.org/2001/XMLSchema#string">http://purl.imsglobal.org/caliper</rdfs:isDefinedBy>
        <rdfs:label xml:lang="en">TagAnnotation</rdfs:label>
    </owl:Class>
    


    <!-- http://purl.imsglobal.org/caliper/TextPositionSelector -->

    <owl:Class rdf:about="http://purl.imsglobal.org/caliper/TextPositionSelector">
        <rdfs:subClassOf rdf:resource="http://purl.imsglobal.org/caliper/Selector"/>
        <rdfs:comment xml:lang="en">A Caliper TextPositionSelector represents a fragment or selection of textual content, the starting and ending positions of which are determined by the distance in characters from the initial character (position 0) of the enclosing full text.</rdfs:comment>
        <rdfs:isDefinedBy rdf:datatype="http://www.w3.org/2001/XMLSchema#string">http://purl.imsglobal.org/caliper</rdfs:isDefinedBy>
        <rdfs:label xml:lang="en">TextPositionSelector</rdfs:label>
    </owl:Class>
    


    <!-- http://purl.imsglobal.org/caliper/Thread -->

    <owl:Class rdf:about="http://purl.imsglobal.org/caliper/Thread">
        <rdfs:subClassOf rdf:resource="http://purl.imsglobal.org/caliper/DigitalResourceCollection"/>
        <rdfs:subClassOf>
            <owl:Class>
                <owl:intersectionOf rdf:parseType="Collection">
                    <owl:Restriction>
                        <owl:onProperty rdf:resource="http://purl.imsglobal.org/caliper/isPartOf"/>
                        <owl:someValuesFrom rdf:resource="http://purl.imsglobal.org/caliper/Entity"/>
                    </owl:Restriction>
                    <owl:Restriction>
                        <owl:onProperty rdf:resource="http://purl.imsglobal.org/caliper/isPartOf"/>
                        <owl:allValuesFrom rdf:resource="http://purl.imsglobal.org/caliper/Forum"/>
                    </owl:Restriction>
                </owl:intersectionOf>
            </owl:Class>
        </rdfs:subClassOf>
        <rdfs:subClassOf>
            <owl:Class>
                <owl:intersectionOf rdf:parseType="Collection">
                    <owl:Restriction>
                        <owl:onProperty rdf:resource="http://purl.imsglobal.org/caliper/items"/>
                        <owl:someValuesFrom rdf:resource="http://purl.imsglobal.org/caliper/Entity"/>
                    </owl:Restriction>
                    <owl:Restriction>
                        <owl:onProperty rdf:resource="http://purl.imsglobal.org/caliper/items"/>
                        <owl:allValuesFrom rdf:resource="http://purl.imsglobal.org/caliper/Message"/>
                    </owl:Restriction>
                </owl:intersectionOf>
            </owl:Class>
        </rdfs:subClassOf>
        <rdfs:comment xml:lang="en">A Caliper Thread represents a series of one or more messages that share a common subject and are connected by a reply or by date relationships.</rdfs:comment>
        <rdfs:isDefinedBy rdf:datatype="http://www.w3.org/2001/XMLSchema#string">http://purl.imsglobal.org/caliper</rdfs:isDefinedBy>
        <rdfs:label xml:lang="en">Thread</rdfs:label>
    </owl:Class>
    


    <!-- http://purl.imsglobal.org/caliper/ThreadEvent -->

    <owl:Class rdf:about="http://purl.imsglobal.org/caliper/ThreadEvent">
        <rdfs:subClassOf rdf:resource="http://purl.imsglobal.org/caliper/Event"/>
        <rdfs:subClassOf>
            <owl:Class>
                <owl:intersectionOf rdf:parseType="Collection">
                    <owl:Restriction>
                        <owl:onProperty rdf:resource="http://purl.imsglobal.org/caliper/action"/>
                        <owl:someValuesFrom rdf:resource="http://purl.imsglobal.org/caliper/Action"/>
                    </owl:Restriction>
                    <owl:Restriction>
                        <owl:onProperty rdf:resource="http://purl.imsglobal.org/caliper/action"/>
                        <owl:someValuesFrom>
                            <owl:Class>
                                <owl:oneOf rdf:parseType="Collection">
                                    <rdf:Description rdf:about="http://purl.imsglobal.org/caliper/actions/MarkedAsRead"/>
                                    <rdf:Description rdf:about="http://purl.imsglobal.org/caliper/actions/MarkedAsUnread"/>
                                </owl:oneOf>
                            </owl:Class>
                        </owl:someValuesFrom>
                    </owl:Restriction>
                </owl:intersectionOf>
            </owl:Class>
        </rdfs:subClassOf>
        <rdfs:subClassOf>
            <owl:Class>
                <owl:intersectionOf rdf:parseType="Collection">
                    <owl:Restriction>
                        <owl:onProperty rdf:resource="http://purl.imsglobal.org/caliper/actor"/>
                        <owl:someValuesFrom rdf:resource="http://purl.imsglobal.org/caliper/Agent"/>
                    </owl:Restriction>
                    <owl:Restriction>
                        <owl:onProperty rdf:resource="http://purl.imsglobal.org/caliper/actor"/>
                        <owl:allValuesFrom rdf:resource="http://purl.imsglobal.org/caliper/Person"/>
                    </owl:Restriction>
                </owl:intersectionOf>
            </owl:Class>
        </rdfs:subClassOf>
        <rdfs:subClassOf>
            <owl:Class>
                <owl:intersectionOf rdf:parseType="Collection">
                    <owl:Restriction>
                        <owl:onProperty rdf:resource="http://purl.imsglobal.org/caliper/object"/>
                        <owl:someValuesFrom rdf:resource="http://purl.imsglobal.org/caliper/DigitalResource"/>
                    </owl:Restriction>
                    <owl:Restriction>
                        <owl:onProperty rdf:resource="http://purl.imsglobal.org/caliper/object"/>
                        <owl:allValuesFrom rdf:resource="http://purl.imsglobal.org/caliper/Thread"/>
                    </owl:Restriction>
                </owl:intersectionOf>
            </owl:Class>
        </rdfs:subClassOf>
        <rdfs:comment xml:lang="en">A Caliper ThreadEvent models an actor interacting with a Forum thread or topic.</rdfs:comment>
        <rdfs:isDefinedBy rdf:datatype="http://www.w3.org/2001/XMLSchema#string">http://purl.imsglobal.org/caliper</rdfs:isDefinedBy>
        <rdfs:label xml:lang="en">ThreadEvent</rdfs:label>
    </owl:Class>
    


    <!-- http://purl.imsglobal.org/caliper/ToolLaunchEvent -->

    <owl:Class rdf:about="http://purl.imsglobal.org/caliper/ToolLaunchEvent">
        <rdfs:subClassOf rdf:resource="http://purl.imsglobal.org/caliper/Event"/>
        <rdfs:subClassOf>
            <owl:Class>
                <owl:intersectionOf rdf:parseType="Collection">
                    <owl:Restriction>
                        <owl:onProperty rdf:resource="http://purl.imsglobal.org/caliper/action"/>
                        <owl:someValuesFrom rdf:resource="http://purl.imsglobal.org/caliper/Action"/>
                    </owl:Restriction>
                    <owl:Restriction>
                        <owl:onProperty rdf:resource="http://purl.imsglobal.org/caliper/action"/>
                        <owl:someValuesFrom>
                            <owl:Class>
                                <owl:oneOf rdf:parseType="Collection">
                                    <rdf:Description rdf:about="http://purl.imsglobal.org/actions/Launched"/>
                                    <rdf:Description rdf:about="http://purl.imsglobal.org/actions/Returned"/>
                                </owl:oneOf>
                            </owl:Class>
                        </owl:someValuesFrom>
                    </owl:Restriction>
                </owl:intersectionOf>
            </owl:Class>
        </rdfs:subClassOf>
        <rdfs:subClassOf>
            <owl:Class>
                <owl:intersectionOf rdf:parseType="Collection">
                    <owl:Restriction>
                        <owl:onProperty rdf:resource="http://purl.imsglobal.org/caliper/actor"/>
                        <owl:someValuesFrom rdf:resource="http://purl.imsglobal.org/caliper/Agent"/>
                    </owl:Restriction>
                    <owl:Restriction>
                        <owl:onProperty rdf:resource="http://purl.imsglobal.org/caliper/actor"/>
                        <owl:allValuesFrom rdf:resource="http://purl.imsglobal.org/caliper/Person"/>
                    </owl:Restriction>
                </owl:intersectionOf>
            </owl:Class>
        </rdfs:subClassOf>
        <rdfs:subClassOf>
            <owl:Class>
                <owl:intersectionOf rdf:parseType="Collection">
                    <owl:Restriction>
                        <owl:onProperty rdf:resource="http://purl.imsglobal.org/caliper/object"/>
                        <owl:someValuesFrom rdf:resource="http://purl.imsglobal.org/caliper/Agent"/>
                    </owl:Restriction>
                    <owl:Restriction>
                        <owl:onProperty rdf:resource="http://purl.imsglobal.org/caliper/object"/>
                        <owl:allValuesFrom rdf:resource="http://purl.imsglobal.org/caliper/SoftwareApplication"/>
                    </owl:Restriction>
                </owl:intersectionOf>
            </owl:Class>
        </rdfs:subClassOf>
        <rdfs:subClassOf>
            <owl:Class>
                <owl:intersectionOf rdf:parseType="Collection">
                    <owl:Restriction>
                        <owl:onProperty rdf:resource="http://purl.imsglobal.org/caliper/target"/>
                        <owl:someValuesFrom rdf:resource="http://purl.imsglobal.org/caliper/Entity"/>
                    </owl:Restriction>
                    <owl:Restriction>
                        <owl:onProperty rdf:resource="http://purl.imsglobal.org/caliper/target"/>
                        <owl:allValuesFrom>
                            <owl:Class>
                                <owl:unionOf rdf:parseType="Collection">
                                    <rdf:Description rdf:about="http://purl.imsglobal.org/caliper/Link"/>
                                    <rdf:Description rdf:about="http://purl.imsglobal.org/caliper/LtiLink"/>
                                </owl:unionOf>
                            </owl:Class>
                        </owl:allValuesFrom>
                    </owl:Restriction>
                </owl:intersectionOf>
            </owl:Class>
        </rdfs:subClassOf>
        <rdfs:subClassOf>
            <owl:Restriction>
                <owl:onProperty rdf:resource="http://purl.imsglobal.org/caliper/generated"/>
                <owl:someValuesFrom rdf:resource="http://purl.imsglobal.org/caliper/DigitalResource"/>
            </owl:Restriction>
        </rdfs:subClassOf>
        <rdfs:subClassOf>
            <owl:Restriction>
                <owl:onProperty rdf:resource="http://purl.imsglobal.org/caliper/federatedSession"/>
                <owl:allValuesFrom rdf:resource="http://purl.imsglobal.org/caliper/LtiSession"/>
            </owl:Restriction>
        </rdfs:subClassOf>
        <rdfs:comment xml:lang="en">The ToolLaunchEvent models an interaction between a Person and a SoftwareApplication), at a given time and in a given context at a given time and in a given context.</rdfs:comment>
        <rdfs:isDefinedBy xml:lang="en">http://purl.imsglobal.org/caliper</rdfs:isDefinedBy>
        <rdfs:label xml:lang="en">ToolLaunchEvent</rdfs:label>
    </owl:Class>
    


    <!-- http://purl.imsglobal.org/caliper/ToolUseEvent -->

    <owl:Class rdf:about="http://purl.imsglobal.org/caliper/ToolUseEvent">
        <rdfs:subClassOf rdf:resource="http://purl.imsglobal.org/caliper/Event"/>
        <rdfs:subClassOf>
            <owl:Class>
                <owl:intersectionOf rdf:parseType="Collection">
                    <owl:Restriction>
                        <owl:onProperty rdf:resource="http://purl.imsglobal.org/caliper/action"/>
                        <owl:someValuesFrom rdf:resource="http://purl.imsglobal.org/caliper/Action"/>
                    </owl:Restriction>
                    <owl:Restriction>
                        <owl:onProperty rdf:resource="http://purl.imsglobal.org/caliper/action"/>
                        <owl:hasValue rdf:resource="http://purl.imsglobal.org/caliper/actions/Used"/>
                    </owl:Restriction>
                </owl:intersectionOf>
            </owl:Class>
        </rdfs:subClassOf>
        <rdfs:subClassOf>
            <owl:Class>
                <owl:intersectionOf rdf:parseType="Collection">
                    <owl:Restriction>
                        <owl:onProperty rdf:resource="http://purl.imsglobal.org/caliper/actor"/>
                        <owl:someValuesFrom rdf:resource="http://purl.imsglobal.org/caliper/Agent"/>
                    </owl:Restriction>
                    <owl:Restriction>
                        <owl:onProperty rdf:resource="http://purl.imsglobal.org/caliper/actor"/>
                        <owl:allValuesFrom rdf:resource="http://purl.imsglobal.org/caliper/Person"/>
                    </owl:Restriction>
                </owl:intersectionOf>
            </owl:Class>
        </rdfs:subClassOf>
        <rdfs:subClassOf>
            <owl:Class>
                <owl:intersectionOf rdf:parseType="Collection">
                    <owl:Restriction>
                        <owl:onProperty rdf:resource="http://purl.imsglobal.org/caliper/object"/>
                        <owl:someValuesFrom rdf:resource="http://purl.imsglobal.org/caliper/Agent"/>
                    </owl:Restriction>
                    <owl:Restriction>
                        <owl:onProperty rdf:resource="http://purl.imsglobal.org/caliper/object"/>
                        <owl:allValuesFrom rdf:resource="http://purl.imsglobal.org/caliper/SoftwareApplication"/>
                    </owl:Restriction>
                </owl:intersectionOf>
            </owl:Class>
        </rdfs:subClassOf>
        <rdfs:subClassOf>
            <owl:Restriction>
                <owl:onProperty rdf:resource="http://purl.imsglobal.org/caliper/target"/>
                <owl:someValuesFrom rdf:resource="http://purl.imsglobal.org/caliper/SoftwareApplication"/>
            </owl:Restriction>
        </rdfs:subClassOf>
        <rdfs:comment xml:lang="en">A Caliper ToolUseEvent models a Person using a learning tool in a way that the tool&apos;s creators have determined is an indication of a learning interaction.</rdfs:comment>
        <rdfs:isDefinedBy rdf:datatype="http://www.w3.org/2001/XMLSchema#string">http://purl.imsglobal.org/caliper</rdfs:isDefinedBy>
        <rdfs:label xml:lang="en">ToolUseEvent</rdfs:label>
    </owl:Class>
    


    <!-- http://purl.imsglobal.org/caliper/TrueFalseResponse -->

    <owl:Class rdf:about="http://purl.imsglobal.org/caliper/TrueFalseResponse">
        <rdfs:subClassOf rdf:resource="http://purl.imsglobal.org/caliper/Response"/>
        <rdfs:comment xml:lang="en">A Caliper TrueFalseResponse represents a type of Response to an AssessmentItem in which only two possible options are provided (e.g., true/false, yes/no).</rdfs:comment>
        <rdfs:isDefinedBy rdf:datatype="http://www.w3.org/2001/XMLSchema#string">http://purl.imsglobal.org/caliper</rdfs:isDefinedBy>
        <rdfs:label xml:lang="en">TrueFalseResponse</rdfs:label>
    </owl:Class>
    


    <!-- http://purl.imsglobal.org/caliper/VideoObject -->

    <owl:Class rdf:about="http://purl.imsglobal.org/caliper/VideoObject">
        <rdfs:subClassOf rdf:resource="http://purl.imsglobal.org/caliper/MediaObject"/>
        <rdfs:comment xml:lang="en">A Caliper VideoObject represents a visual recording stored in digital form.</rdfs:comment>
        <rdfs:isDefinedBy rdf:datatype="http://www.w3.org/2001/XMLSchema#string">http://purl.imsglobal.org/caliper</rdfs:isDefinedBy>
        <rdfs:label xml:lang="en">VideoObject</rdfs:label>
    </owl:Class>
    


    <!-- http://purl.imsglobal.org/caliper/ViewEvent -->

    <owl:Class rdf:about="http://purl.imsglobal.org/caliper/ViewEvent">
        <rdfs:subClassOf rdf:resource="http://purl.imsglobal.org/caliper/Event"/>
        <rdfs:subClassOf>
            <owl:Class>
                <owl:intersectionOf rdf:parseType="Collection">
                    <owl:Restriction>
                        <owl:onProperty rdf:resource="http://purl.imsglobal.org/caliper/action"/>
                        <owl:someValuesFrom rdf:resource="http://purl.imsglobal.org/caliper/Action"/>
                    </owl:Restriction>
                    <owl:Restriction>
                        <owl:onProperty rdf:resource="http://purl.imsglobal.org/caliper/action"/>
                        <owl:hasValue rdf:resource="http://purl.imsglobal.org/caliper/actions/Viewed"/>
                    </owl:Restriction>
                </owl:intersectionOf>
            </owl:Class>
        </rdfs:subClassOf>
        <rdfs:subClassOf>
            <owl:Class>
                <owl:intersectionOf rdf:parseType="Collection">
                    <owl:Restriction>
                        <owl:onProperty rdf:resource="http://purl.imsglobal.org/caliper/actor"/>
                        <owl:someValuesFrom rdf:resource="http://purl.imsglobal.org/caliper/Agent"/>
                    </owl:Restriction>
                    <owl:Restriction>
                        <owl:onProperty rdf:resource="http://purl.imsglobal.org/caliper/actor"/>
                        <owl:allValuesFrom rdf:resource="http://purl.imsglobal.org/caliper/Person"/>
                    </owl:Restriction>
                </owl:intersectionOf>
            </owl:Class>
        </rdfs:subClassOf>
        <rdfs:subClassOf>
            <owl:Class>
                <owl:intersectionOf rdf:parseType="Collection">
                    <owl:Restriction>
                        <owl:onProperty rdf:resource="http://purl.imsglobal.org/caliper/object"/>
                        <owl:someValuesFrom rdf:resource="http://purl.imsglobal.org/caliper/Entity"/>
                    </owl:Restriction>
                    <owl:Restriction>
                        <owl:onProperty rdf:resource="http://purl.imsglobal.org/caliper/object"/>
                        <owl:allValuesFrom rdf:resource="http://purl.imsglobal.org/caliper/DigitalResource"/>
                    </owl:Restriction>
                </owl:intersectionOf>
            </owl:Class>
        </rdfs:subClassOf>
        <rdfs:subClassOf>
            <owl:Restriction>
                <owl:onProperty rdf:resource="http://purl.imsglobal.org/caliper/target"/>
                <owl:someValuesFrom rdf:resource="http://purl.imsglobal.org/caliper/Frame"/>
            </owl:Restriction>
        </rdfs:subClassOf>
        <rdfs:comment xml:lang="en">A Caliper ViewEvent describes an actor&apos;s examination of digital content whenever the activity emphasizes thoughtful observation or study as opposed to the mere retrieval of a resource.</rdfs:comment>
        <rdfs:isDefinedBy rdf:datatype="http://www.w3.org/2001/XMLSchema#string">http://purl.imsglobal.org/caliper</rdfs:isDefinedBy>
        <rdfs:label xml:lang="en">ViewEvent</rdfs:label>
    </owl:Class>
    


    <!-- http://purl.imsglobal.org/caliper/WebPage -->

    <owl:Class rdf:about="http://purl.imsglobal.org/caliper/WebPage">
        <rdfs:subClassOf rdf:resource="http://purl.imsglobal.org/caliper/DigitalResource"/>
        <rdfs:comment xml:lang="en">A Caliper WebPage represents a document containing markup that is suitable for display in a web browser.</rdfs:comment>
        <rdfs:isDefinedBy rdf:datatype="http://www.w3.org/2001/XMLSchema#string">http://purl.imsglobal.org/caliper</rdfs:isDefinedBy>
        <rdfs:label xml:lang="en">WebPage</rdfs:label>
    </owl:Class>
    


    <!-- http://purl.imsglobal.org/caliper/epubChapter -->

    <owl:Class rdf:about="http://purl.imsglobal.org/caliper/epubChapter">
        <rdfs:subClassOf rdf:resource="http://purl.imsglobal.org/caliper/DigitalResource"/>
        <terms:isReplacedBy rdf:resource="http://purl.imsglobal.org/caliper/Chapter"/>
        <rdfs:comment xml:lang="en">A Caliper EpubChapter represents a major structural division of a piece of writing. EpubChapter is a DEPRECATED entity that will be removed in a future version of the specification. It SHOULD NOT be referenced.</rdfs:comment>
        <rdfs:isDefinedBy rdf:datatype="http://www.w3.org/2001/XMLSchema#string">http://purl.imsglobal.org/caliper</rdfs:isDefinedBy>
        <rdfs:label xml:lang="en">EpubChapter</rdfs:label>
        <owl:deprecated rdf:datatype="http://www.w3.org/2001/XMLSchema#boolean">true</owl:deprecated>
    </owl:Class>
    


    <!-- http://purl.imsglobal.org/caliper/epubPart -->

    <owl:Class rdf:about="http://purl.imsglobal.org/caliper/epubPart">
        <rdfs:subClassOf rdf:resource="http://purl.imsglobal.org/caliper/DigitalResource"/>
        <rdfs:comment xml:lang="en">A Caliper EpubPart represents a major structural division of a piece of writing, typically encapsulating a set of related chapters. EpubPart is a DEPRECATED entity that will be removed in a future version of the specification. It SHOULD NOT be referenced.</rdfs:comment>
        <rdfs:isDefinedBy rdf:datatype="http://www.w3.org/2001/XMLSchema#string">http://purl.imsglobal.org/caliper</rdfs:isDefinedBy>
        <rdfs:label xml:lang="en">EpubPart</rdfs:label>
        <owl:deprecated rdf:datatype="http://www.w3.org/2001/XMLSchema#boolean">true</owl:deprecated>
    </owl:Class>
    


    <!-- http://purl.imsglobal.org/caliper/epubSubChapter -->

    <owl:Class rdf:about="http://purl.imsglobal.org/caliper/epubSubChapter">
        <rdfs:subClassOf rdf:resource="http://purl.imsglobal.org/caliper/DigitalResource"/>
        <rdfs:subClassOf>
            <owl:Class>
                <owl:intersectionOf rdf:parseType="Collection">
                    <owl:Restriction>
                        <owl:onProperty rdf:resource="http://purl.imsglobal.org/caliper/isPartOf"/>
                        <owl:someValuesFrom rdf:resource="http://purl.imsglobal.org/caliper/Entity"/>
                    </owl:Restriction>
                    <owl:Restriction>
                        <owl:onProperty rdf:resource="http://purl.imsglobal.org/caliper/isPartOf"/>
                        <owl:allValuesFrom rdf:resource="http://purl.imsglobal.org/caliper/epubChapter"/>
                    </owl:Restriction>
                </owl:intersectionOf>
            </owl:Class>
        </rdfs:subClassOf>
        <rdfs:comment rdf:datatype="http://www.w3.org/2001/XMLSchema#string">A Caliper EpubSubChapter represents a major sub-division of an EpubChapter. EpubSubChapter is a DEPRECATED entity that will be removed in a future version of the specification. It SHOULD NOT be referenced.</rdfs:comment>
        <rdfs:isDefinedBy rdf:datatype="http://www.w3.org/2001/XMLSchema#string">http://purl.imsglobal.org/caliper</rdfs:isDefinedBy>
        <rdfs:label xml:lang="en">EpubSubChapter</rdfs:label>
        <owl:deprecated rdf:datatype="http://www.w3.org/2001/XMLSchema#boolean">true</owl:deprecated>
    </owl:Class>
    


    <!-- http://purl.imsglobal.org/caliper/epubVolume -->

    <owl:Class rdf:about="http://purl.imsglobal.org/caliper/epubVolume">
        <rdfs:subClassOf rdf:resource="http://purl.imsglobal.org/caliper/DigitalResource"/>
        <terms:isReplacedBy rdf:resource="http://purl.imsglobal.org/caliper/Document"/>
        <rdfs:comment xml:lang="en">A Caliper EpubVolume represents a component of a collection. EpubVolume inherits all the properties and requirements defined for DigitalResource, its supertype. EpubVolume is a DEPRECATED entity that will be removed in a future version of the specification. It SHOULD NOT be referenced.</rdfs:comment>
        <rdfs:isDefinedBy rdf:datatype="http://www.w3.org/2001/XMLSchema#string">http://purl.imsglobal.org/caliper</rdfs:isDefinedBy>
        <rdfs:label xml:lang="en">EpubVolume</rdfs:label>
        <owl:deprecated rdf:datatype="http://www.w3.org/2001/XMLSchema#boolean">true</owl:deprecated>
    </owl:Class>
    


    <!-- http://purl.imsglobal.org/vocab/lis/v2/membership#Administrator -->

    <owl:Class rdf:about="http://purl.imsglobal.org/vocab/lis/v2/membership#Administrator">
        <rdfs:subClassOf rdf:resource="http://purl.imsglobal.org/caliper/Role"/>
        <rdfs:comment xml:lang="en">The role of a formal administrator in the Membership.</rdfs:comment>
        <rdfs:isDefinedBy rdf:datatype="http://www.w3.org/2001/XMLSchema#string">http://www.imsglobal.org/lis/</rdfs:isDefinedBy>
        <rdfs:label xml:lang="en">Administrator</rdfs:label>
    </owl:Class>
    


    <!-- http://purl.imsglobal.org/vocab/lis/v2/membership#ContentDeveloper -->

    <owl:Class rdf:about="http://purl.imsglobal.org/vocab/lis/v2/membership#ContentDeveloper">
        <rdfs:subClassOf rdf:resource="http://purl.imsglobal.org/caliper/Role"/>
        <rdfs:comment xml:lang="en">The role of an author of content for learning material presented through the Membership.</rdfs:comment>
        <rdfs:isDefinedBy rdf:datatype="http://www.w3.org/2001/XMLSchema#string">http://www.imsglobal.org/lis/</rdfs:isDefinedBy>
        <rdfs:label xml:lang="en">ContentDeveloper</rdfs:label>
    </owl:Class>
    


    <!-- http://purl.imsglobal.org/vocab/lis/v2/membership#Instructor -->

    <owl:Class rdf:about="http://purl.imsglobal.org/vocab/lis/v2/membership#Instructor">
        <rdfs:subClassOf rdf:resource="http://purl.imsglobal.org/caliper/Role"/>
        <rdfs:comment xml:lang="en">The role of teaching instructor for learning material presented through the Membership.</rdfs:comment>
        <rdfs:isDefinedBy rdf:datatype="http://www.w3.org/2001/XMLSchema#string">http://www.imsglobal.org/lis/</rdfs:isDefinedBy>
        <rdfs:label xml:lang="en">Instructor</rdfs:label>
    </owl:Class>
    


    <!-- http://purl.imsglobal.org/vocab/lis/v2/membership#Learner -->

    <owl:Class rdf:about="http://purl.imsglobal.org/vocab/lis/v2/membership#Learner">
        <rdfs:subClassOf rdf:resource="http://purl.imsglobal.org/caliper/Role"/>
        <rdfs:comment xml:lang="en">The role of someone undergoing some form of formal learning.</rdfs:comment>
        <rdfs:isDefinedBy rdf:datatype="http://www.w3.org/2001/XMLSchema#string">http://www.imsglobal.org/lis/</rdfs:isDefinedBy>
        <rdfs:label xml:lang="en">Learner</rdfs:label>
    </owl:Class>
    


    <!-- http://purl.imsglobal.org/vocab/lis/v2/membership#Manager -->

    <owl:Class rdf:about="http://purl.imsglobal.org/vocab/lis/v2/membership#Manager">
        <rdfs:subClassOf rdf:resource="http://purl.imsglobal.org/caliper/Role"/>
        <rdfs:comment xml:lang="en">The role of manager of the Group for which the Membership is being defined.</rdfs:comment>
        <rdfs:isDefinedBy rdf:datatype="http://www.w3.org/2001/XMLSchema#string">http://www.imsglobal.org/lis/</rdfs:isDefinedBy>
        <rdfs:label xml:lang="en">Manager</rdfs:label>
    </owl:Class>
    


    <!-- http://purl.imsglobal.org/vocab/lis/v2/membership#Member -->

    <owl:Class rdf:about="http://purl.imsglobal.org/vocab/lis/v2/membership#Member">
        <rdfs:subClassOf rdf:resource="http://purl.imsglobal.org/caliper/Role"/>
        <rdfs:comment xml:lang="en">The role of a member of the associated Membership.</rdfs:comment>
        <rdfs:isDefinedBy rdf:datatype="http://www.w3.org/2001/XMLSchema#string">http://www.imsglobal.org/lis/</rdfs:isDefinedBy>
        <rdfs:label xml:lang="en">Member</rdfs:label>
    </owl:Class>
    


    <!-- http://purl.imsglobal.org/vocab/lis/v2/membership#Mentor -->

    <owl:Class rdf:about="http://purl.imsglobal.org/vocab/lis/v2/membership#Mentor">
        <rdfs:subClassOf rdf:resource="http://purl.imsglobal.org/caliper/Role"/>
        <rdfs:comment xml:lang="en">The role of a personal mentor of other individuals in the Membership.</rdfs:comment>
        <rdfs:isDefinedBy rdf:datatype="http://www.w3.org/2001/XMLSchema#string">http://www.imsglobal.org/lis/</rdfs:isDefinedBy>
        <rdfs:label xml:lang="en">Mentor</rdfs:label>
    </owl:Class>
    


    <!-- http://purl.imsglobal.org/vocab/lis/v2/membership#Officer -->

    <owl:Class rdf:about="http://purl.imsglobal.org/vocab/lis/v2/membership#Officer">
        <rdfs:subClassOf rdf:resource="http://purl.imsglobal.org/caliper/Role"/>
        <rdfs:comment xml:lang="en">The role of an officer of organization e.g., Chair, Secretary, etc. in the Membership.</rdfs:comment>
        <rdfs:isDefinedBy rdf:datatype="http://www.w3.org/2001/XMLSchema#string">http://www.imsglobal.org/lis/</rdfs:isDefinedBy>
        <rdfs:label xml:lang="en">Officer</rdfs:label>
    </owl:Class>
    


    <!-- http://purl.imsglobal.org/vocab/lis/v2/membership#TeachingAssistant -->

    <owl:Class rdf:about="http://purl.imsglobal.org/vocab/lis/v2/membership#TeachingAssistant">
        <rdfs:subClassOf rdf:resource="http://purl.imsglobal.org/caliper/Role"/>
        <rdfs:comment xml:lang="en">The role of teaching assistant to an Instructor in the Membership.</rdfs:comment>
        <rdfs:isDefinedBy rdf:datatype="http://www.w3.org/2001/XMLSchema#string">http://www.imsglobal.org/lis/</rdfs:isDefinedBy>
        <rdfs:label xml:lang="en">TeachingAssistant</rdfs:label>
    </owl:Class>
    


    <!-- 
    ///////////////////////////////////////////////////////////////////////////////////////
    //
    // Individuals
    //
    ///////////////////////////////////////////////////////////////////////////////////////
     -->

    


    <!-- http://purl.imsglobal.org/actions/Archived -->

    <owl:NamedIndividual rdf:about="http://purl.imsglobal.org/actions/Archived">
        <rdf:type rdf:resource="http://purl.imsglobal.org/caliper/Action"/>
        <rdfs:comment xml:lang="en">Put into an archive. The Archived action signals that a resource has been put into long-term storage. Inverse of Restored.</rdfs:comment>
        <rdfs:isDefinedBy rdf:datatype="http://www.w3.org/2001/XMLSchema#string">http://wordnet-rdf.princeton.edu/wn31/201387292-v</rdfs:isDefinedBy>
        <rdfs:label xml:lang="en">Archived</rdfs:label>
    </owl:NamedIndividual>
    


    <!-- http://purl.imsglobal.org/actions/Copied -->

    <owl:NamedIndividual rdf:about="http://purl.imsglobal.org/actions/Copied">
        <rdfs:comment xml:lang="en">Make a replica of.</rdfs:comment>
        <rdfs:isDefinedBy rdf:datatype="http://www.w3.org/2001/XMLSchema#string">http://wordnet-rdf.princeton.edu/wn31/201697776-v</rdfs:isDefinedBy>
        <rdfs:label xml:lang="en">Copied</rdfs:label>
    </owl:NamedIndividual>
    


    <!-- http://purl.imsglobal.org/actions/Launched -->

    <owl:NamedIndividual rdf:about="http://purl.imsglobal.org/actions/Launched">
        <rdf:type rdf:resource="http://purl.imsglobal.org/caliper/Action"/>
        <rdfs:comment xml:lang="en">Get going; give impetus to.</rdfs:comment>
        <rdfs:isDefinedBy rdf:datatype="http://www.w3.org/2001/XMLSchema#string">href=&quot;http://wordnet-rdf.princeton.edu/wn31/01515196-v</rdfs:isDefinedBy>
        <rdfs:label xml:lang="en">Launched</rdfs:label>
    </owl:NamedIndividual>
    


    <!-- http://purl.imsglobal.org/actions/Published -->

    <owl:NamedIndividual rdf:about="http://purl.imsglobal.org/actions/Published">
        <rdfs:comment xml:lang="en">Prepare and issue for public distribution or sale. Inverse of Unpublished.</rdfs:comment>
        <rdfs:isDefinedBy rdf:datatype="http://www.w3.org/2001/XMLSchema#string">http://wordnet-rdf.princeton.edu/wn31/200969657-v</rdfs:isDefinedBy>
        <rdfs:label xml:lang="en">Published</rdfs:label>
    </owl:NamedIndividual>
    


    <!-- http://purl.imsglobal.org/actions/Restored -->

    <owl:NamedIndividual rdf:about="http://purl.imsglobal.org/actions/Restored">
        <rdfs:comment xml:lang="en">Return to its original or usable and functioning condition. Inverse of Archived.</rdfs:comment>
        <rdfs:isDefinedBy rdf:datatype="http://www.w3.org/2001/XMLSchema#string">http://wordnet-rdf.princeton.edu/wn31/202558146-v</rdfs:isDefinedBy>
        <rdfs:label xml:lang="en">Restored</rdfs:label>
    </owl:NamedIndividual>
    


    <!-- http://purl.imsglobal.org/actions/Returned -->

    <owl:NamedIndividual rdf:about="http://purl.imsglobal.org/actions/Returned">
        <rdf:type rdf:resource="http://purl.imsglobal.org/caliper/Action"/>
        <rdfs:comment xml:lang="en">Go or come back to place, condition, or activity where one has been before.</rdfs:comment>
        <rdfs:isDefinedBy rdf:datatype="http://www.w3.org/2001/XMLSchema#string">http://wordnet-rdf.princeton.edu/wn31/01515196-v</rdfs:isDefinedBy>
        <rdfs:label xml:lang="en">Returned</rdfs:label>
    </owl:NamedIndividual>
    


    <!-- http://purl.imsglobal.org/actions/Unpublished -->

    <owl:NamedIndividual rdf:about="http://purl.imsglobal.org/actions/Unpublished">
        <rdfs:comment xml:lang="en">Remove from public distribution or sale. Inverse of Published.</rdfs:comment>
        <rdfs:isDefinedBy rdf:datatype="http://www.w3.org/2001/XMLSchema#string">http://wordnet-rdf.princeton.edu/wn31/200969657-v</rdfs:isDefinedBy>
        <rdfs:label xml:lang="en">Unpublished</rdfs:label>
    </owl:NamedIndividual>
    


    <!-- http://purl.imsglobal.org/caliper/actions/Abandoned -->

    <owl:NamedIndividual rdf:about="http://purl.imsglobal.org/caliper/actions/Abandoned">
        <rdf:type rdf:resource="http://purl.imsglobal.org/caliper/Action"/>
        <rdfs:comment xml:lang="en">Forsake, leave behind.</rdfs:comment>
        <rdfs:isDefinedBy rdf:datatype="http://www.w3.org/2001/XMLSchema#string">http://wordnet-rdf.princeton.edu/wn31/202232813-v</rdfs:isDefinedBy>
        <rdfs:label xml:lang="en">Abandoned</rdfs:label>
    </owl:NamedIndividual>
    


    <!-- http://purl.imsglobal.org/caliper/actions/Activated -->

    <owl:NamedIndividual rdf:about="http://purl.imsglobal.org/caliper/actions/Activated">
        <rdf:type rdf:resource="http://purl.imsglobal.org/caliper/Action"/>
        <rdfs:comment xml:lang="en">Make active or more active. Inverse of Deactivated.</rdfs:comment>
        <rdfs:isDefinedBy rdf:datatype="http://www.w3.org/2001/XMLSchema#string">http://wordnet-rdf.princeton.edu/wn31/200191014-v</rdfs:isDefinedBy>
        <rdfs:label xml:lang="en">Activated</rdfs:label>
    </owl:NamedIndividual>
    


    <!-- http://purl.imsglobal.org/caliper/actions/Added -->

    <owl:NamedIndividual rdf:about="http://purl.imsglobal.org/caliper/actions/Added">
        <rdf:type rdf:resource="http://purl.imsglobal.org/caliper/Action"/>
        <rdfs:comment xml:lang="en">Make an addition (to); join or combine or unite with others; increase the quality, quantity, size or scope of. Inverse of Removed.</rdfs:comment>
        <rdfs:isDefinedBy rdf:datatype="http://www.w3.org/2001/XMLSchema#string">http://wordnet-rdf.princeton.edu/wn31/200182551-v</rdfs:isDefinedBy>
        <rdfs:label xml:lang="en">Added</rdfs:label>
    </owl:NamedIndividual>
    


    <!-- http://purl.imsglobal.org/caliper/actions/Attached -->

    <owl:NamedIndividual rdf:about="http://purl.imsglobal.org/caliper/actions/Attached">
        <rdf:type rdf:resource="http://purl.imsglobal.org/caliper/Action"/>
        <rdfs:comment xml:lang="en">Cause to be attached.</rdfs:comment>
        <rdfs:isDefinedBy rdf:datatype="http://www.w3.org/2001/XMLSchema#string">http://wordnet-rdf.princeton.edu/wn31/201299048-v</rdfs:isDefinedBy>
        <rdfs:label xml:lang="en">Attached</rdfs:label>
    </owl:NamedIndividual>
    


    <!-- http://purl.imsglobal.org/caliper/actions/Bookmarked -->

    <owl:NamedIndividual rdf:about="http://purl.imsglobal.org/caliper/actions/Bookmarked">
        <rdf:type rdf:resource="http://purl.imsglobal.org/caliper/Action"/>
        <rdfs:comment xml:lang="en">A marker that specifies a location of interest in a DigitalResource that is recorded for later retrieval.</rdfs:comment>
        <rdfs:isDefinedBy rdf:datatype="http://www.w3.org/2001/XMLSchema#string">http://purl.imsglobal.org/caliper</rdfs:isDefinedBy>
        <rdfs:label xml:lang="en">Bookmarked</rdfs:label>
        <rdfs:seeAlso rdf:datatype="http://www.w3.org/2001/XMLSchema#string">http://wordnet-rdf.princeton.edu/wn31/102874508-n</rdfs:seeAlso>
    </owl:NamedIndividual>
    


    <!-- http://purl.imsglobal.org/caliper/actions/ChangedResolution -->

    <owl:NamedIndividual rdf:about="http://purl.imsglobal.org/caliper/actions/ChangedResolution">
        <rdf:type rdf:resource="http://purl.imsglobal.org/caliper/Action"/>
        <rdfs:comment xml:lang="en">Cause to change; make different; cause a transformation of the number of pixels per square inch on a computer-generated display.</rdfs:comment>
        <rdfs:isDefinedBy rdf:datatype="http://www.w3.org/2001/XMLSchema#string">http://wordnet-rdf.princeton.edu/wn31/200126072-v</rdfs:isDefinedBy>
        <rdfs:label xml:lang="en">ChangedResolution</rdfs:label>
        <rdfs:seeAlso rdf:datatype="http://www.w3.org/2001/XMLSchema#string">http://wordnet-rdf.princeton.edu/wn31/111526370-n</rdfs:seeAlso>
    </owl:NamedIndividual>
    


    <!-- http://purl.imsglobal.org/caliper/actions/ChangedSize -->

    <owl:NamedIndividual rdf:about="http://purl.imsglobal.org/caliper/actions/ChangedSize">
        <rdf:type rdf:resource="http://purl.imsglobal.org/caliper/Action"/>
        <rdfs:comment xml:lang="en">Cause to change; make different; cause a transformation of the physical magnitude of something.</rdfs:comment>
        <rdfs:isDefinedBy rdf:datatype="http://www.w3.org/2001/XMLSchema#string">http://wordnet-rdf.princeton.edu/wn31/200126072-v</rdfs:isDefinedBy>
        <rdfs:label xml:lang="en">ChangedSize</rdfs:label>
        <rdfs:seeAlso rdf:datatype="http://www.w3.org/2001/XMLSchema#string">http://wordnet-rdf.princeton.edu/wn31/105106204-n</rdfs:seeAlso>
    </owl:NamedIndividual>
    


    <!-- http://purl.imsglobal.org/caliper/actions/ChangedSpeed -->

    <owl:NamedIndividual rdf:about="http://purl.imsglobal.org/caliper/actions/ChangedSpeed">
        <rdf:type rdf:resource="http://purl.imsglobal.org/caliper/Action"/>
        <rdfs:comment xml:lang="en">Cause to change; make different; cause a transformation of the rate at which something happens.</rdfs:comment>
        <rdfs:isDefinedBy rdf:datatype="http://www.w3.org/2001/XMLSchema#string">http://wordnet-rdf.princeton.edu/wn31/200126072-v</rdfs:isDefinedBy>
        <rdfs:label xml:lang="en">ChangedSpeed</rdfs:label>
        <rdfs:seeAlso rdf:datatype="http://www.w3.org/2001/XMLSchema#string">http://wordnet-rdf.princeton.edu/wn31/105065291-n</rdfs:seeAlso>
    </owl:NamedIndividual>
    


    <!-- http://purl.imsglobal.org/caliper/actions/ChangedVolume -->

    <owl:NamedIndividual rdf:about="http://purl.imsglobal.org/caliper/actions/ChangedVolume">
        <rdf:type rdf:resource="http://purl.imsglobal.org/caliper/Action"/>
        <rdfs:comment xml:lang="en">Cause to change; make different; cause a transformation of the magnitude of sound (usually in a specified direction).</rdfs:comment>
        <rdfs:isDefinedBy rdf:datatype="http://www.w3.org/2001/XMLSchema#string">http://wordnet-rdf.princeton.edu/wn31/200126072-v</rdfs:isDefinedBy>
        <rdfs:label xml:lang="en">ChangedVolume</rdfs:label>
        <rdfs:seeAlso rdf:datatype="http://www.w3.org/2001/XMLSchema#string">http://wordnet-rdf.princeton.edu/wn31/104997456-n</rdfs:seeAlso>
    </owl:NamedIndividual>
    


    <!-- http://purl.imsglobal.org/caliper/actions/Classified -->

    <owl:NamedIndividual rdf:about="http://purl.imsglobal.org/caliper/actions/Classified">
        <rdf:type rdf:resource="http://purl.imsglobal.org/caliper/Action"/>
        <rdfs:comment xml:lang="en">Assign to a class or kind.</rdfs:comment>
        <rdfs:isDefinedBy rdf:datatype="http://www.w3.org/2001/XMLSchema#string">http://wordnet-rdf.princeton.edu/wn31/200741667-v</rdfs:isDefinedBy>
        <rdfs:label xml:lang="en">Classified</rdfs:label>
    </owl:NamedIndividual>
    


    <!-- http://purl.imsglobal.org/caliper/actions/ClosedPopout -->

    <owl:NamedIndividual rdf:about="http://purl.imsglobal.org/caliper/actions/ClosedPopout">
        <rdf:type rdf:resource="http://purl.imsglobal.org/caliper/Action"/>
        <rdfs:comment xml:lang="en">Close or shut a video popout. Inverse of OpenedPopout.</rdfs:comment>
        <rdfs:isDefinedBy rdf:datatype="http://www.w3.org/2001/XMLSchema#string">http://wordnet-rdf.princeton.edu/wn31/201349660-v</rdfs:isDefinedBy>
        <rdfs:label xml:lang="en">ClosedPopout</rdfs:label>
    </owl:NamedIndividual>
    


    <!-- http://purl.imsglobal.org/caliper/actions/Commented -->

    <owl:NamedIndividual rdf:about="http://purl.imsglobal.org/caliper/actions/Commented">
        <rdf:type rdf:resource="http://purl.imsglobal.org/caliper/Action"/>
        <rdfs:comment xml:lang="en">Make or write a comment on. The Commented action signals that qualitative feedback in the form of a Comment has been provided.</rdfs:comment>
        <rdfs:isDefinedBy rdf:datatype="http://www.w3.org/2001/XMLSchema#string">http://wordnet-rdf.princeton.edu/wn31/201060446-v</rdfs:isDefinedBy>
        <rdfs:label xml:lang="en">Commented</rdfs:label>
    </owl:NamedIndividual>
    


    <!-- http://purl.imsglobal.org/caliper/actions/Completed -->

    <owl:NamedIndividual rdf:about="http://purl.imsglobal.org/caliper/actions/Completed">
        <rdf:type rdf:resource="http://purl.imsglobal.org/caliper/Action"/>
        <rdfs:comment xml:lang="en">Come or bring to a finish or an end.</rdfs:comment>
        <rdfs:isDefinedBy rdf:datatype="http://www.w3.org/2001/XMLSchema#string">http://wordnet-rdf.princeton.edu/wn31/200485097-v</rdfs:isDefinedBy>
        <rdfs:label xml:lang="en">Completed</rdfs:label>
    </owl:NamedIndividual>
    


    <!-- http://purl.imsglobal.org/caliper/actions/Copied -->

    <owl:NamedIndividual rdf:about="http://purl.imsglobal.org/caliper/actions/Copied">
        <rdf:type rdf:resource="http://purl.imsglobal.org/caliper/Action"/>
        <rdfs:comment xml:lang="en">Make a replica of. The Copied action signals that a resource has been duplicated.</rdfs:comment>
        <rdfs:isDefinedBy rdf:datatype="http://www.w3.org/2001/XMLSchema#string">http://wordnet-rdf.princeton.edu/wn31/201697776-v</rdfs:isDefinedBy>
        <rdfs:label xml:lang="en">Copied</rdfs:label>
    </owl:NamedIndividual>
    


    <!-- http://purl.imsglobal.org/caliper/actions/Created -->

    <owl:NamedIndividual rdf:about="http://purl.imsglobal.org/caliper/actions/Created">
        <rdf:type rdf:resource="http://purl.imsglobal.org/caliper/Action"/>
        <rdfs:comment xml:lang="en">Make or cause to be or to become. The Created action signals that a resource has been brought into existence. Inverse of Deleted.</rdfs:comment>
        <rdfs:isDefinedBy rdf:datatype="http://www.w3.org/2001/XMLSchema#string">http://wordnet-rdf.princeton.edu/wn31/201620211-v</rdfs:isDefinedBy>
        <rdfs:label xml:lang="en">Created</rdfs:label>
    </owl:NamedIndividual>
    


    <!-- http://purl.imsglobal.org/caliper/actions/Deactivated -->

    <owl:NamedIndividual rdf:about="http://purl.imsglobal.org/caliper/actions/Deactivated">
        <rdf:type rdf:resource="http://purl.imsglobal.org/caliper/Action"/>
        <rdfs:comment xml:lang="en">Make inactive. Inverse of Activated.</rdfs:comment>
        <rdfs:isDefinedBy rdf:datatype="http://www.w3.org/2001/XMLSchema#string">http://wordnet-rdf.princeton.edu/wn31/200191849-v</rdfs:isDefinedBy>
        <rdfs:label xml:lang="en">Deactivated</rdfs:label>
    </owl:NamedIndividual>
    


    <!-- http://purl.imsglobal.org/caliper/actions/Deleted -->

    <owl:NamedIndividual rdf:about="http://purl.imsglobal.org/caliper/actions/Deleted">
        <rdf:type rdf:resource="http://purl.imsglobal.org/caliper/Action"/>
        <rdfs:comment xml:lang="en">Wipe out digitally. The Deleted action signals that a resource has been removed permanently from a system. Inverse of Created.</rdfs:comment>
        <rdfs:isDefinedBy rdf:datatype="http://www.w3.org/2001/XMLSchema#string">http://wordnet-rdf.princeton.edu/wn31/201001860-v</rdfs:isDefinedBy>
        <rdfs:label xml:lang="en">Deleted</rdfs:label>
    </owl:NamedIndividual>
    


    <!-- http://purl.imsglobal.org/caliper/actions/Described -->

    <owl:NamedIndividual rdf:about="http://purl.imsglobal.org/caliper/actions/Described">
        <rdf:type rdf:resource="http://purl.imsglobal.org/caliper/Action"/>
        <rdfs:comment xml:lang="en">Give a description of. The Described action signals that a description of a resource has been provided.</rdfs:comment>
        <rdfs:isDefinedBy rdf:datatype="http://www.w3.org/2001/XMLSchema#string">http://wordnet-rdf.princeton.edu/wn31/200989103-v</rdfs:isDefinedBy>
        <rdfs:label xml:lang="en">Described</rdfs:label>
    </owl:NamedIndividual>
    


    <!-- http://purl.imsglobal.org/caliper/actions/DisabledClosedCaptioning -->

    <owl:NamedIndividual rdf:about="http://purl.imsglobal.org/caliper/actions/DisabledClosedCaptioning">
        <rdf:type rdf:resource="http://purl.imsglobal.org/caliper/Action"/>
        <rdfs:comment xml:lang="en">Render unable to perform the visual display of a plain text transcription of audio output. Inverse of EnabledClosedCaptioning.</rdfs:comment>
        <rdfs:isDefinedBy rdf:datatype="http://www.w3.org/2001/XMLSchema#string">http://purl.imsglobal.org/caliper</rdfs:isDefinedBy>
        <rdfs:label xml:lang="en">DisabledClosedCaptioning</rdfs:label>
        <rdfs:seeAlso rdf:datatype="http://www.w3.org/2001/XMLSchema#string">http://wordnet-rdf.princeton.edu/wn31/200513267-v</rdfs:seeAlso>
    </owl:NamedIndividual>
    


    <!-- http://purl.imsglobal.org/caliper/actions/Disliked -->

    <owl:NamedIndividual rdf:about="http://purl.imsglobal.org/caliper/actions/Disliked">
        <rdf:type rdf:resource="http://purl.imsglobal.org/caliper/Action"/>
        <rdfs:comment xml:lang="en">Have or feel a dislike or distaste for. Inverse of Liked.</rdfs:comment>
        <rdfs:isDefinedBy rdf:datatype="http://www.w3.org/2001/XMLSchema#string">http://wordnet-rdf.princeton.edu/wn31/201780648-v</rdfs:isDefinedBy>
        <rdfs:label xml:lang="en">Disliked</rdfs:label>
    </owl:NamedIndividual>
    


    <!-- http://purl.imsglobal.org/caliper/actions/Downloaded -->

    <owl:NamedIndividual rdf:about="http://purl.imsglobal.org/caliper/actions/Downloaded">
        <rdf:type rdf:resource="http://purl.imsglobal.org/caliper/Action"/>
        <rdfs:comment xml:lang="en">Transfer a file or program from a central computer to a smaller computer or to a computer at a remote location. The Downloaded action signals that a copy of the resource has been transferred from a central or primary system to a remote or secondary system. Inverse of Uploaded.</rdfs:comment>
        <rdfs:isDefinedBy rdf:datatype="http://www.w3.org/2001/XMLSchema#string">http://wordnet-rdf.princeton.edu/wn31/02233704-v</rdfs:isDefinedBy>
        <rdfs:label xml:lang="en">Downloaded</rdfs:label>
    </owl:NamedIndividual>
    


    <!-- http://purl.imsglobal.org/caliper/actions/EnabledClosedCaptioning -->

    <owl:NamedIndividual rdf:about="http://purl.imsglobal.org/caliper/actions/EnabledClosedCaptioning">
        <rdf:type rdf:resource="http://purl.imsglobal.org/caliper/Action"/>
        <rdfs:comment xml:lang="en">Render capable or able the visual display of a plain text transcription of audio output. Inverse of DisabledClosedCaptioning.</rdfs:comment>
        <rdfs:isDefinedBy rdf:datatype="http://www.w3.org/2001/XMLSchema#string">http://purl.imsglobal.org/caliper</rdfs:isDefinedBy>
        <rdfs:label xml:lang="en">EnabledClosedCaptioning</rdfs:label>
        <rdfs:seeAlso rdf:datatype="http://www.w3.org/2001/XMLSchema#string">http://wordnet-rdf.princeton.edu/wn31/200513958-v</rdfs:seeAlso>
    </owl:NamedIndividual>
    


    <!-- http://purl.imsglobal.org/caliper/actions/Ended -->

    <owl:NamedIndividual rdf:about="http://purl.imsglobal.org/caliper/actions/Ended">
        <rdf:type rdf:resource="http://purl.imsglobal.org/caliper/Action"/>
        <rdfs:comment xml:lang="en">Bring to an end or halt. Inverse of Started.</rdfs:comment>
        <rdfs:isDefinedBy rdf:datatype="http://www.w3.org/2001/XMLSchema#string">http://wordnet-rdf.princeton.edu/wn31/200353480-v</rdfs:isDefinedBy>
        <rdfs:label xml:lang="en">Ended</rdfs:label>
    </owl:NamedIndividual>
    


    <!-- http://purl.imsglobal.org/caliper/actions/EnteredFullScreen -->

    <owl:NamedIndividual rdf:about="http://purl.imsglobal.org/caliper/actions/EnteredFullScreen">
        <rdf:type rdf:resource="http://purl.imsglobal.org/caliper/Action"/>
        <rdfs:comment xml:lang="en">To come or go into a view mode that utilizes all the available display surface of a screen. Inverse of ExitedFullScreen.</rdfs:comment>
        <rdfs:isDefinedBy rdf:datatype="http://www.w3.org/2001/XMLSchema#string">http://purl.imsglobal.org/caliper</rdfs:isDefinedBy>
        <rdfs:label xml:lang="en">EnteredFullScreen</rdfs:label>
        <rdfs:seeAlso rdf:datatype="http://www.w3.org/2001/XMLSchema#string">http://wordnet-rdf.princeton.edu/wn31/202020375-v</rdfs:seeAlso>
    </owl:NamedIndividual>
    


    <!-- http://purl.imsglobal.org/caliper/actions/ExitedFullScreen -->

    <owl:NamedIndividual rdf:about="http://purl.imsglobal.org/caliper/actions/ExitedFullScreen">
        <rdf:type rdf:resource="http://purl.imsglobal.org/caliper/Action"/>
        <rdfs:comment xml:lang="en">Move out of or depart from a view mode that utilizes all the available display surface of a screen. Inverse of EnteredFullScreen.</rdfs:comment>
        <rdfs:isDefinedBy rdf:datatype="http://www.w3.org/2001/XMLSchema#string">http://purl.imsglobal.org/caliper</rdfs:isDefinedBy>
        <rdfs:label xml:lang="en">ExitedFullScreen</rdfs:label>
        <rdfs:seeAlso rdf:datatype="http://www.w3.org/2001/XMLSchema#string">http://wordnet-rdf.princeton.edu/wn31/202019450-v</rdfs:seeAlso>
    </owl:NamedIndividual>
    


    <!-- http://purl.imsglobal.org/caliper/actions/ForwardedTo -->

    <owl:NamedIndividual rdf:about="http://purl.imsglobal.org/caliper/actions/ForwardedTo">
        <rdf:type rdf:resource="http://purl.imsglobal.org/caliper/Action"/>
        <rdfs:comment xml:lang="en">Send or ship onward.</rdfs:comment>
        <rdfs:isDefinedBy rdf:datatype="http://www.w3.org/2001/XMLSchema#string">http://wordnet-rdf.princeton.edu/wn31/201959367-v</rdfs:isDefinedBy>
        <rdfs:label xml:lang="en">ForwardedTo</rdfs:label>
    </owl:NamedIndividual>
    


    <!-- http://purl.imsglobal.org/caliper/actions/Graded -->

    <owl:NamedIndividual rdf:about="http://purl.imsglobal.org/caliper/actions/Graded">
        <rdf:type rdf:resource="http://purl.imsglobal.org/caliper/Action"/>
        <rdfs:comment xml:lang="en">Assign a grade or rank to, according to one&apos;s evaluation.</rdfs:comment>
        <rdfs:isDefinedBy rdf:datatype="http://www.w3.org/2001/XMLSchema#string">http://wordnet-rdf.princeton.edu/wn31/200659399-v</rdfs:isDefinedBy>
        <rdfs:label xml:lang="en">Graded</rdfs:label>
    </owl:NamedIndividual>
    


    <!-- http://purl.imsglobal.org/caliper/actions/Hid -->

    <owl:NamedIndividual rdf:about="http://purl.imsglobal.org/caliper/actions/Hid">
        <rdf:type rdf:resource="http://purl.imsglobal.org/caliper/Action"/>
        <rdfs:comment xml:lang="en">Prevent from being seen or discovered. Inverse of Showed.</rdfs:comment>
        <rdfs:isDefinedBy rdf:datatype="http://www.w3.org/2001/XMLSchema#string">http://wordnet-rdf.princeton.edu/wn31/202149298-v</rdfs:isDefinedBy>
        <rdfs:label xml:lang="en">Hid</rdfs:label>
    </owl:NamedIndividual>
    


    <!-- http://purl.imsglobal.org/caliper/actions/Highlighted -->

    <owl:NamedIndividual rdf:about="http://purl.imsglobal.org/caliper/actions/Highlighted">
        <rdf:type rdf:resource="http://purl.imsglobal.org/caliper/Action"/>
        <rdfs:comment xml:lang="en">Move into the foreground to make more visible or prominent.</rdfs:comment>
        <rdfs:isDefinedBy rdf:datatype="http://www.w3.org/2001/XMLSchema#string">http://wordnet-rdf.princeton.edu/wn31/200515150-v</rdfs:isDefinedBy>
        <rdfs:label xml:lang="en">Highlighted</rdfs:label>
    </owl:NamedIndividual>
    


    <!-- http://purl.imsglobal.org/caliper/actions/Identified -->

    <owl:NamedIndividual rdf:about="http://purl.imsglobal.org/caliper/actions/Identified">
        <rdf:type rdf:resource="http://purl.imsglobal.org/caliper/Action"/>
        <rdfs:comment xml:lang="en">Recognize as being; establish the identity of someone or something.</rdfs:comment>
        <rdfs:isDefinedBy rdf:datatype="http://www.w3.org/2001/XMLSchema#string">http://wordnet-rdf.princeton.edu/wn31/200620568-v</rdfs:isDefinedBy>
        <rdfs:label xml:lang="en">Identified</rdfs:label>
    </owl:NamedIndividual>
    


    <!-- http://purl.imsglobal.org/caliper/actions/JumpedTo -->

    <owl:NamedIndividual rdf:about="http://purl.imsglobal.org/caliper/actions/JumpedTo">
        <rdf:type rdf:resource="http://purl.imsglobal.org/caliper/Action"/>
        <rdfs:comment xml:lang="en">Pass abruptly from one state or topic to another.</rdfs:comment>
        <rdfs:isDefinedBy rdf:datatype="http://www.w3.org/2001/XMLSchema#string">http://wordnet-rdf.princeton.edu/wn31/200561468-v</rdfs:isDefinedBy>
        <rdfs:label xml:lang="en">JumpedTo</rdfs:label>
    </owl:NamedIndividual>
    


    <!-- http://purl.imsglobal.org/caliper/actions/Liked -->

    <owl:NamedIndividual rdf:about="http://purl.imsglobal.org/caliper/actions/Liked">
        <rdf:type rdf:resource="http://purl.imsglobal.org/caliper/Action"/>
        <rdfs:comment xml:lang="en">Be fond of. Inverse of Disliked.</rdfs:comment>
        <rdfs:isDefinedBy rdf:datatype="http://www.w3.org/2001/XMLSchema#string">http://wordnet-rdf.princeton.edu/wn31/201780873-v</rdfs:isDefinedBy>
        <rdfs:label xml:lang="en">Liked</rdfs:label>
    </owl:NamedIndividual>
    


    <!-- http://purl.imsglobal.org/caliper/actions/Linked -->

    <owl:NamedIndividual rdf:about="http://purl.imsglobal.org/caliper/actions/Linked">
        <rdf:type rdf:resource="http://purl.imsglobal.org/caliper/Action"/>
        <rdfs:comment xml:lang="en">Connect, fasten, or put together two or more pieces.</rdfs:comment>
        <rdfs:isDefinedBy rdf:datatype="http://www.w3.org/2001/XMLSchema#string">http://wordnet-rdf.princeton.edu/wn31/201357376-v</rdfs:isDefinedBy>
        <rdfs:label xml:lang="en">Linked</rdfs:label>
    </owl:NamedIndividual>
    


    <!-- http://purl.imsglobal.org/caliper/actions/LoggedIn -->

    <owl:NamedIndividual rdf:about="http://purl.imsglobal.org/caliper/actions/LoggedIn">
        <rdf:type rdf:resource="http://purl.imsglobal.org/caliper/Action"/>
        <rdfs:comment xml:lang="en">Enter a computer or software application. Inverse of LoggedOut.</rdfs:comment>
        <rdfs:isDefinedBy rdf:datatype="http://www.w3.org/2001/XMLSchema#string">http://wordnet-rdf.princeton.edu/wn31/202253955-v</rdfs:isDefinedBy>
        <rdfs:label xml:lang="en">LoggedIn</rdfs:label>
    </owl:NamedIndividual>
    


    <!-- http://purl.imsglobal.org/caliper/actions/LoggedOut -->

    <owl:NamedIndividual rdf:about="http://purl.imsglobal.org/caliper/actions/LoggedOut">
        <rdf:type rdf:resource="http://purl.imsglobal.org/caliper/Action"/>
        <rdfs:comment xml:lang="en">Exit a computer or software application. Inverse of LoggedIn.</rdfs:comment>
        <rdfs:isDefinedBy rdf:datatype="http://www.w3.org/2001/XMLSchema#string">http://wordnet-rdf.princeton.edu/wn31/202254101-v</rdfs:isDefinedBy>
        <rdfs:label xml:lang="en">LoggedOut</rdfs:label>
    </owl:NamedIndividual>
    


    <!-- http://purl.imsglobal.org/caliper/actions/MarkedAsRead -->

    <owl:NamedIndividual rdf:about="http://purl.imsglobal.org/caliper/actions/MarkedAsRead">
        <rdf:type rdf:resource="http://purl.imsglobal.org/caliper/Action"/>
        <rdfs:comment xml:lang="en">Mark: designate as if by a mark, read: interpret something that is written or printed. Inverse of MarkedAsUnread.</rdfs:comment>
        <rdfs:isDefinedBy rdf:datatype="http://www.w3.org/2001/XMLSchema#string">http://wordnet-rdf.princeton.edu/wn31/200923709-v</rdfs:isDefinedBy>
        <rdfs:label xml:lang="en">MarkedAsRead</rdfs:label>
        <rdfs:seeAlso rdf:datatype="http://www.w3.org/2001/XMLSchema#string">http://wordnet-rdf.princeton.edu/wn31/200626756-v</rdfs:seeAlso>
    </owl:NamedIndividual>
    


    <!-- http://purl.imsglobal.org/caliper/actions/MarkedAsUnread -->

    <owl:NamedIndividual rdf:about="http://purl.imsglobal.org/caliper/actions/MarkedAsUnread">
        <rdf:type rdf:resource="http://purl.imsglobal.org/caliper/Action"/>
        <rdfs:comment xml:lang="en">Remove designation as if by a mark.  Inverse of MarkedAsRead.</rdfs:comment>
        <rdfs:isDefinedBy rdf:datatype="http://www.w3.org/2001/XMLSchema#string">http://purl.imsglobal.org/caliper</rdfs:isDefinedBy>
        <rdfs:label xml:lang="en">MarkedAsUnread</rdfs:label>
        <rdfs:seeAlso rdf:datatype="http://www.w3.org/2001/XMLSchema#string">http://wordnet-rdf.princeton.edu/wn31/200923709-v</rdfs:seeAlso>
    </owl:NamedIndividual>
    


    <!-- http://purl.imsglobal.org/caliper/actions/Modified -->

    <owl:NamedIndividual rdf:about="http://purl.imsglobal.org/caliper/actions/Modified">
        <rdf:type rdf:resource="http://purl.imsglobal.org/caliper/Action"/>
        <rdfs:comment xml:lang="en">Cause to change; make different; cause a transformation. The Modified action signals that a resource has been altered or changed.</rdfs:comment>
        <rdfs:isDefinedBy rdf:datatype="http://www.w3.org/2001/XMLSchema#string">http://wordnet-rdf.princeton.edu/wn31/200126072-v</rdfs:isDefinedBy>
        <rdfs:label xml:lang="en">Modified</rdfs:label>
    </owl:NamedIndividual>
    


    <!-- http://purl.imsglobal.org/caliper/actions/Muted -->

    <owl:NamedIndividual rdf:about="http://purl.imsglobal.org/caliper/actions/Muted">
        <rdf:type rdf:resource="http://purl.imsglobal.org/caliper/Action"/>
        <rdfs:comment xml:lang="en">Deaden (a sound or noise). Inverse of Unmuted.</rdfs:comment>
        <rdfs:isDefinedBy rdf:datatype="http://www.w3.org/2001/XMLSchema#string">http://wordnet-rdf.princeton.edu/wn31/mute-v</rdfs:isDefinedBy>
        <rdfs:label xml:lang="en">Muted</rdfs:label>
    </owl:NamedIndividual>
    


    <!-- http://purl.imsglobal.org/caliper/actions/NavigatedTo -->

    <owl:NamedIndividual rdf:about="http://purl.imsglobal.org/caliper/actions/NavigatedTo">
        <rdf:type rdf:resource="http://purl.imsglobal.org/caliper/Action"/>
        <rdfs:comment xml:lang="en">Direct the course; determine the direction of travelling.</rdfs:comment>
        <rdfs:isDefinedBy rdf:datatype="http://www.w3.org/2001/XMLSchema#string">http://wordnet-rdf.princeton.edu/wn31/201935739-v</rdfs:isDefinedBy>
        <rdfs:label xml:lang="en">NavigatedTo</rdfs:label>
    </owl:NamedIndividual>
    


    <!-- http://purl.imsglobal.org/caliper/actions/OpenedPopout -->

    <owl:NamedIndividual rdf:about="http://purl.imsglobal.org/caliper/actions/OpenedPopout">
        <rdf:type rdf:resource="http://purl.imsglobal.org/caliper/Action"/>
        <rdfs:comment xml:lang="en">Start to operate or function or cause to start operating or functioning a video popout. Inverse of ClosedPopout.</rdfs:comment>
        <rdfs:isDefinedBy rdf:datatype="http://www.w3.org/2001/XMLSchema#string">http://purl.imsglobal.org/caliper</rdfs:isDefinedBy>
        <rdfs:label xml:lang="en">OpenedPopout</rdfs:label>
        <rdfs:seeAlso rdf:datatype="http://www.w3.org/2001/XMLSchema#string">http://wordnet-rdf.princeton.edu/wn31/202431018-v</rdfs:seeAlso>
    </owl:NamedIndividual>
    


    <!-- http://purl.imsglobal.org/caliper/actions/Paused -->

    <owl:NamedIndividual rdf:about="http://purl.imsglobal.org/caliper/actions/Paused">
        <rdf:type rdf:resource="http://purl.imsglobal.org/caliper/Action"/>
        <rdfs:comment xml:lang="en">Cease an action temporarily. Inverse of Resumed.</rdfs:comment>
        <rdfs:isDefinedBy rdf:datatype="http://www.w3.org/2001/XMLSchema#string">http://wordnet-rdf.princeton.edu/wn31/200781106-v</rdfs:isDefinedBy>
        <rdfs:label xml:lang="en">Paused</rdfs:label>
    </owl:NamedIndividual>
    


    <!-- http://purl.imsglobal.org/caliper/actions/Posted -->

    <owl:NamedIndividual rdf:about="http://purl.imsglobal.org/caliper/actions/Posted">
        <rdf:type rdf:resource="http://purl.imsglobal.org/caliper/Action"/>
        <rdfs:comment xml:lang="en">To cause to be directed or transmitted to another place.</rdfs:comment>
        <rdfs:isDefinedBy rdf:datatype="http://www.w3.org/2001/XMLSchema#string">http://wordnet-rdf.princeton.edu/wn31/201033289-v</rdfs:isDefinedBy>
        <rdfs:label xml:lang="en">Posted</rdfs:label>
    </owl:NamedIndividual>
    


    <!-- http://purl.imsglobal.org/caliper/actions/Printed -->

    <owl:NamedIndividual rdf:about="http://purl.imsglobal.org/caliper/actions/Printed">
        <rdf:type rdf:resource="http://purl.imsglobal.org/caliper/Action"/>
        <rdfs:comment xml:lang="en">Reproduce by printing. The Printed action signals that a mechanical process has been invoked in order to produce a printed representation of a resource.</rdfs:comment>
        <rdfs:isDefinedBy rdf:datatype="http://www.w3.org/2001/XMLSchema#string">http://wordnet-rdf.princeton.edu/wn31/01747945-v</rdfs:isDefinedBy>
        <rdfs:label xml:lang="en">Printed</rdfs:label>
    </owl:NamedIndividual>
    


    <!-- http://purl.imsglobal.org/caliper/actions/Published -->

    <owl:NamedIndividual rdf:about="http://purl.imsglobal.org/caliper/actions/Published">
        <rdf:type rdf:resource="http://purl.imsglobal.org/caliper/Action"/>
        <rdfs:comment xml:lang="en">Prepare and issue for public distribution or sale. The Published action signals that a resource is now available for public consumption. Inverse of Unpublished.</rdfs:comment>
        <rdfs:isDefinedBy rdf:datatype="http://www.w3.org/2001/XMLSchema#string">http://wordnet-rdf.princeton.edu/wn31/200969657-v</rdfs:isDefinedBy>
        <rdfs:label xml:lang="en">Published</rdfs:label>
    </owl:NamedIndividual>
    


    <!-- http://purl.imsglobal.org/caliper/actions/Questioned -->

    <owl:NamedIndividual rdf:about="http://purl.imsglobal.org/caliper/actions/Questioned">
        <rdf:type rdf:resource="http://purl.imsglobal.org/caliper/Action"/>
        <rdfs:comment xml:lang="en">Pose a question.</rdfs:comment>
        <rdfs:isDefinedBy rdf:datatype="http://www.w3.org/2001/XMLSchema#string">http://wordnet-rdf.princeton.edu/wn31/200786670-v</rdfs:isDefinedBy>
        <rdfs:label xml:lang="en">Questioned</rdfs:label>
    </owl:NamedIndividual>
    


    <!-- http://purl.imsglobal.org/caliper/actions/Ranked -->

    <owl:NamedIndividual rdf:about="http://purl.imsglobal.org/caliper/actions/Ranked">
        <rdf:type rdf:resource="http://purl.imsglobal.org/caliper/Action"/>
        <rdfs:comment xml:lang="en">Assign a rank or rating to. The Ranked action signals that quantitative feedback in the form of a Rating has been provided.</rdfs:comment>
        <rdfs:isDefinedBy rdf:datatype="http://www.w3.org/2001/XMLSchema#string">http://wordnet-rdf.princeton.edu/wn31/200659723-v</rdfs:isDefinedBy>
        <rdfs:label xml:lang="en">Ranked</rdfs:label>
    </owl:NamedIndividual>
    


    <!-- http://purl.imsglobal.org/caliper/actions/Recommended -->

    <owl:NamedIndividual rdf:about="http://purl.imsglobal.org/caliper/actions/Recommended">
        <rdf:type rdf:resource="http://purl.imsglobal.org/caliper/Action"/>
        <rdfs:comment xml:lang="en">Express a good opinion of.</rdfs:comment>
        <rdfs:isDefinedBy rdf:datatype="http://www.w3.org/2001/XMLSchema#string">http://wordnet-rdf.princeton.edu/wn31/200884469-v</rdfs:isDefinedBy>
        <rdfs:label xml:lang="en">Recommended</rdfs:label>
    </owl:NamedIndividual>
    


    <!-- http://purl.imsglobal.org/caliper/actions/Removed -->

    <owl:NamedIndividual rdf:about="http://purl.imsglobal.org/caliper/actions/Removed">
        <rdf:type rdf:resource="http://purl.imsglobal.org/caliper/Action"/>
        <rdfs:comment xml:lang="en">Remove from sight. Inverse of Added.</rdfs:comment>
        <rdfs:isDefinedBy rdf:datatype="http://www.w3.org/2001/XMLSchema#string">http://wordnet-rdf.princeton.edu/wn31/200181704-v</rdfs:isDefinedBy>
        <rdfs:label xml:lang="en">Removed</rdfs:label>
    </owl:NamedIndividual>
    


    <!-- http://purl.imsglobal.org/caliper/actions/Reset -->

    <owl:NamedIndividual rdf:about="http://purl.imsglobal.org/caliper/actions/Reset">
        <rdf:type rdf:resource="http://purl.imsglobal.org/caliper/Action"/>
        <rdfs:comment xml:lang="en">Set anew.</rdfs:comment>
        <rdfs:isDefinedBy rdf:datatype="http://www.w3.org/2001/XMLSchema#string">http://wordnet-rdf.princeton.edu/wn31/200949623-v</rdfs:isDefinedBy>
        <rdfs:label xml:lang="en">Reset</rdfs:label>
    </owl:NamedIndividual>
    


    <!-- http://purl.imsglobal.org/caliper/actions/Restarted -->

    <owl:NamedIndividual rdf:about="http://purl.imsglobal.org/caliper/actions/Restarted">
        <rdf:type rdf:resource="http://purl.imsglobal.org/caliper/Action"/>
        <rdfs:comment xml:lang="en">Take up or begin anew, as in to start something, make progress but then stop and return to the beginning in order to start again.</rdfs:comment>
        <rdfs:isDefinedBy rdf:datatype="http://www.w3.org/2001/XMLSchema#string">http://purl.imglobal.org/caliper</rdfs:isDefinedBy>
        <rdfs:label xml:lang="en">Restarted</rdfs:label>
        <rdfs:seeAlso rdf:datatype="http://www.w3.org/2001/XMLSchema#string">http://wordnet-rdf.princeton.edu/wn31/200350758-v</rdfs:seeAlso>
    </owl:NamedIndividual>
    


    <!-- http://purl.imsglobal.org/caliper/actions/Restored -->

    <owl:NamedIndividual rdf:about="http://purl.imsglobal.org/caliper/actions/Restored">
        <rdf:type rdf:resource="http://purl.imsglobal.org/caliper/Action"/>
        <rdfs:comment xml:lang="en">Return to its original or usable and functioning condition. The Restored action signals that an archived resource has been retrieved from long-term storage. Inverse of Archived.</rdfs:comment>
        <rdfs:isDefinedBy rdf:datatype="http://www.w3.org/2001/XMLSchema#string">http://wordnet-rdf.princeton.edu/wn31/202558146-v</rdfs:isDefinedBy>
        <rdfs:label xml:lang="en">Restored</rdfs:label>
    </owl:NamedIndividual>
    


    <!-- http://purl.imsglobal.org/caliper/actions/Resumed -->

    <owl:NamedIndividual rdf:about="http://purl.imsglobal.org/caliper/actions/Resumed">
        <rdf:type rdf:resource="http://purl.imsglobal.org/caliper/Action"/>
        <rdfs:comment xml:lang="en">Take up or begin anew, as in to start something, pause and then begin again at the location where the pause in action occurred. Inverse of Paused.</rdfs:comment>
        <rdfs:isDefinedBy rdf:datatype="http://www.w3.org/2001/XMLSchema#string">http://purl.imsglobal.org/caliper</rdfs:isDefinedBy>
        <rdfs:label xml:lang="en">Resumed</rdfs:label>
        <rdfs:seeAlso rdf:datatype="http://www.w3.org/2001/XMLSchema#string">http://wordnet-rdf.princeton.edu/wn31/200350758-v</rdfs:seeAlso>
    </owl:NamedIndividual>
    


    <!-- http://purl.imsglobal.org/caliper/actions/Retrieved -->

    <owl:NamedIndividual rdf:about="http://purl.imsglobal.org/caliper/actions/Retrieved">
        <rdf:type rdf:resource="http://purl.imsglobal.org/caliper/Action"/>
        <rdfs:comment xml:lang="en">Obtain or retrieve from a storage device; as of information on a computer. The Retrieved action signals that a resource has been accessed or obtained.</rdfs:comment>
        <rdfs:isDefinedBy rdf:datatype="http://www.w3.org/2001/XMLSchema#string">http://wordnet-rdf.princeton.edu/wn31/202253616-v</rdfs:isDefinedBy>
        <rdfs:label xml:lang="en">Retrieved</rdfs:label>
    </owl:NamedIndividual>
    


    <!-- http://purl.imsglobal.org/caliper/actions/Reviewed -->

    <owl:NamedIndividual rdf:about="http://purl.imsglobal.org/caliper/actions/Reviewed">
        <rdf:type rdf:resource="http://purl.imsglobal.org/caliper/Action"/>
        <rdfs:comment xml:lang="en">Appraise critically.</rdfs:comment>
        <rdfs:isDefinedBy rdf:datatype="http://www.w3.org/2001/XMLSchema#string">http://wordnet-rdf.princeton.edu/wn31/200857194-v</rdfs:isDefinedBy>
        <rdfs:label xml:lang="en">Reviewed</rdfs:label>
    </owl:NamedIndividual>
    


    <!-- http://purl.imsglobal.org/caliper/actions/Rewound -->

    <owl:NamedIndividual rdf:about="http://purl.imsglobal.org/caliper/actions/Rewound">
        <rdf:type rdf:resource="http://purl.imsglobal.org/caliper/Action"/>
        <rdfs:comment xml:lang="en">Wind up again.</rdfs:comment>
        <rdfs:isDefinedBy rdf:datatype="http://www.w3.org/2001/XMLSchema#string">http://wordnet-rdf.princeton.edu/wn31/201524927-v</rdfs:isDefinedBy>
        <rdfs:label xml:lang="en">Rewound</rdfs:label>
    </owl:NamedIndividual>
    


    <!-- http://purl.imsglobal.org/caliper/actions/Saved -->

    <owl:NamedIndividual rdf:about="http://purl.imsglobal.org/caliper/actions/Saved">
        <rdf:type rdf:resource="http://purl.imsglobal.org/caliper/Action"/>
        <rdfs:comment xml:lang="en">Record data on a computer. The Saved action signals that the current state of a resource has been stored for future use.</rdfs:comment>
        <rdfs:isDefinedBy rdf:datatype="http://www.w3.org/2001/XMLSchema#string">http://wordnet-rdf.princeton.edu/wn31/00998886-v</rdfs:isDefinedBy>
        <rdfs:label xml:lang="en">Saved</rdfs:label>
    </owl:NamedIndividual>
    


    <!-- http://purl.imsglobal.org/caliper/actions/Searched -->

    <owl:NamedIndividual rdf:about="http://purl.imsglobal.org/caliper/actions/Searched">
        <rdf:type rdf:resource="http://purl.imsglobal.org/caliper/Action"/>
        <rdfs:comment xml:lang="en">Try to locate or discover, or try to establish the existence of.</rdfs:comment>
        <rdfs:isDefinedBy rdf:datatype="http://www.w3.org/2001/XMLSchema#string">http://wordnet-rdf.princeton.edu/wn31/201318273-v</rdfs:isDefinedBy>
        <rdfs:label xml:lang="en">Searched</rdfs:label>
    </owl:NamedIndividual>
    


    <!-- http://purl.imsglobal.org/caliper/actions/Shared -->

    <owl:NamedIndividual rdf:about="http://purl.imsglobal.org/caliper/actions/Shared">
        <rdf:type rdf:resource="http://purl.imsglobal.org/caliper/Action"/>
        <rdfs:comment xml:lang="en">Communicate.</rdfs:comment>
        <rdfs:isDefinedBy rdf:datatype="http://www.w3.org/2001/XMLSchema#string">http://wordnet-rdf.princeton.edu/wn31/201065952-v</rdfs:isDefinedBy>
        <rdfs:label xml:lang="en">Shared</rdfs:label>
    </owl:NamedIndividual>
    


    <!-- http://purl.imsglobal.org/caliper/actions/Showed -->

    <owl:NamedIndividual rdf:about="http://purl.imsglobal.org/caliper/actions/Showed">
        <rdf:type rdf:resource="http://purl.imsglobal.org/caliper/Action"/>
        <rdfs:comment xml:lang="en">Make visible or noticeable. Inverse of Hid.</rdfs:comment>
        <rdfs:isDefinedBy rdf:datatype="http://www.w3.org/2001/XMLSchema#string">http://wordnet-rdf.princeton.edu/wn31/202141597-v</rdfs:isDefinedBy>
        <rdfs:label xml:lang="en">Showed</rdfs:label>
    </owl:NamedIndividual>
    


    <!-- http://purl.imsglobal.org/caliper/actions/Skipped -->

    <owl:NamedIndividual rdf:about="http://purl.imsglobal.org/caliper/actions/Skipped">
        <rdf:type rdf:resource="http://purl.imsglobal.org/caliper/Action"/>
        <rdfs:comment xml:lang="en">Bypass.</rdfs:comment>
        <rdfs:isDefinedBy rdf:datatype="http://www.w3.org/2001/XMLSchema#string">http://wordnet-rdf.princeton.edu/wn31/200618188-v</rdfs:isDefinedBy>
        <rdfs:label xml:lang="en">Skipped</rdfs:label>
    </owl:NamedIndividual>
    


    <!-- http://purl.imsglobal.org/caliper/actions/Started -->

    <owl:NamedIndividual rdf:about="http://purl.imsglobal.org/caliper/actions/Started">
        <rdf:type rdf:resource="http://purl.imsglobal.org/caliper/Action"/>
        <rdfs:comment xml:lang="en">Set in motion, cause to start. Inverse of Ended.</rdfs:comment>
        <rdfs:isDefinedBy rdf:datatype="http://www.w3.org/2001/XMLSchema#string">http://wordnet-rdf.princeton.edu/wn31/200349400-v</rdfs:isDefinedBy>
        <rdfs:label xml:lang="en">Started</rdfs:label>
    </owl:NamedIndividual>
    


    <!-- http://purl.imsglobal.org/caliper/actions/Submitted -->

    <owl:NamedIndividual rdf:about="http://purl.imsglobal.org/caliper/actions/Submitted">
        <rdf:type rdf:resource="http://purl.imsglobal.org/caliper/Action"/>
        <rdfs:comment xml:lang="en">Hand over formally.</rdfs:comment>
        <rdfs:isDefinedBy rdf:datatype="http://www.w3.org/2001/XMLSchema#string">http://wordnet-rdf.princeton.edu/wn31/202267560-v</rdfs:isDefinedBy>
        <rdfs:label xml:lang="en">Submitted</rdfs:label>
    </owl:NamedIndividual>
    


    <!-- http://purl.imsglobal.org/caliper/actions/Subscribed -->

    <owl:NamedIndividual rdf:about="http://purl.imsglobal.org/caliper/actions/Subscribed">
        <rdf:type rdf:resource="http://purl.imsglobal.org/caliper/Action"/>
        <rdfs:comment xml:lang="en">Receive or obtain regularly. Inverse of Unsubscribed.</rdfs:comment>
        <rdfs:isDefinedBy rdf:datatype="http://www.w3.org/2001/XMLSchema#string">http://wordnet-rdf.princeton.edu/wn31/202214527-v</rdfs:isDefinedBy>
        <rdfs:label xml:lang="en">Subscribed</rdfs:label>
    </owl:NamedIndividual>
    


    <!-- http://purl.imsglobal.org/caliper/actions/Tagged -->

    <owl:NamedIndividual rdf:about="http://purl.imsglobal.org/caliper/actions/Tagged">
        <rdf:type rdf:resource="http://purl.imsglobal.org/caliper/Action"/>
        <rdfs:comment xml:lang="en">Attach a tag or label to.</rdfs:comment>
        <rdfs:isDefinedBy rdf:datatype="http://www.w3.org/2001/XMLSchema#string">http://wordnet-rdf.princeton.edu/wn31/201591414-v</rdfs:isDefinedBy>
        <rdfs:label xml:lang="en">Tagged</rdfs:label>
    </owl:NamedIndividual>
    


    <!-- http://purl.imsglobal.org/caliper/actions/TimedOut -->

    <owl:NamedIndividual rdf:about="http://purl.imsglobal.org/caliper/actions/TimedOut">
        <rdf:type rdf:resource="http://purl.imsglobal.org/caliper/Action"/>
        <rdfs:comment xml:lang="en">Cancellation of a user session after a predetermined time interval has occurred without activity.</rdfs:comment>
        <rdfs:isDefinedBy rdf:datatype="http://www.w3.org/2001/XMLSchema#string">http://purl.imsglobal.org/caliper</rdfs:isDefinedBy>
        <rdfs:label xml:lang="en">TimedOut</rdfs:label>
    </owl:NamedIndividual>
    


    <!-- http://purl.imsglobal.org/caliper/actions/Unmuted -->

    <owl:NamedIndividual rdf:about="http://purl.imsglobal.org/caliper/actions/Unmuted">
        <rdf:type rdf:resource="http://purl.imsglobal.org/caliper/Action"/>
        <rdfs:comment xml:lang="en">Inverse of Muted.</rdfs:comment>
        <rdfs:isDefinedBy rdf:datatype="http://www.w3.org/2001/XMLSchema#string">http://purl.imsglobal.org/caliper</rdfs:isDefinedBy>
        <rdfs:label xml:lang="en">Unmuted</rdfs:label>
        <rdfs:seeAlso rdf:datatype="http://www.w3.org/2001/XMLSchema#string">http://wordnet-rdf.princeton.edu/wn31/mute-v</rdfs:seeAlso>
    </owl:NamedIndividual>
    


    <!-- http://purl.imsglobal.org/caliper/actions/Unpublished -->

    <owl:NamedIndividual rdf:about="http://purl.imsglobal.org/caliper/actions/Unpublished">
        <rdf:type rdf:resource="http://purl.imsglobal.org/caliper/Action"/>
        <rdfs:comment xml:lang="en">Remove from public distribution or sale. The Unpublished action signals that a published resource has been rendered unavailable for public consumption. Inverse of Published.</rdfs:comment>
        <rdfs:isDefinedBy rdf:datatype="http://www.w3.org/2001/XMLSchema#string">http://wordnet-rdf.princeton.edu/wn31/200969657-v</rdfs:isDefinedBy>
        <rdfs:label xml:lang="en">Unpublished</rdfs:label>
    </owl:NamedIndividual>
    


    <!-- http://purl.imsglobal.org/caliper/actions/Unsubscribed -->

    <owl:NamedIndividual rdf:about="http://purl.imsglobal.org/caliper/actions/Unsubscribed">
        <rdf:type rdf:resource="http://purl.imsglobal.org/caliper/Action"/>
        <rdfs:comment xml:lang="en">Inverse of Subscribed.</rdfs:comment>
        <rdfs:isDefinedBy rdf:datatype="http://www.w3.org/2001/XMLSchema#string">http://purl.imsglobal.org/caliper</rdfs:isDefinedBy>
        <rdfs:label xml:lang="en">Unsubscribed</rdfs:label>
        <rdfs:seeAlso rdf:datatype="http://www.w3.org/2001/XMLSchema#string">http://wordnet-rdf.princeton.edu/wn31/202214527-v</rdfs:seeAlso>
    </owl:NamedIndividual>
    


    <!-- http://purl.imsglobal.org/caliper/actions/Uploaded -->

    <owl:NamedIndividual rdf:about="http://purl.imsglobal.org/caliper/actions/Uploaded">
        <rdf:type rdf:resource="http://purl.imsglobal.org/caliper/Action"/>
        <rdfs:comment xml:lang="en">Transfer a file or program to a central computer from a smaller computer or a computer at a remote location. The Uploaded action signals that a copy of the resource has been transferred from a remote or secondary system to a central or primary system. Inverse of Downloaded.</rdfs:comment>
        <rdfs:isDefinedBy rdf:datatype="http://www.w3.org/2001/XMLSchema#string">http://wordnet-rdf.princeton.edu/wn31/02233898-v</rdfs:isDefinedBy>
        <rdfs:label xml:lang="en">Uploaded</rdfs:label>
    </owl:NamedIndividual>
    


    <!-- http://purl.imsglobal.org/caliper/actions/Used -->

    <owl:NamedIndividual rdf:about="http://purl.imsglobal.org/caliper/actions/Used">
        <rdf:type rdf:resource="http://purl.imsglobal.org/caliper/Action"/>
        <rdfs:comment xml:lang="en">Put into service; make work or employ for a particular purpose or for its inherent or natural purpose.</rdfs:comment>
        <rdfs:isDefinedBy rdf:datatype="http://www.w3.org/2001/XMLSchema#string">http://wordnet-rdf.princeton.edu/wn31/201161188-v</rdfs:isDefinedBy>
        <rdfs:label xml:lang="en">Used</rdfs:label>
    </owl:NamedIndividual>
    


    <!-- http://purl.imsglobal.org/caliper/actions/Viewed -->

    <owl:NamedIndividual rdf:about="http://purl.imsglobal.org/caliper/actions/Viewed">
        <rdf:type rdf:resource="http://purl.imsglobal.org/caliper/Action"/>
        <rdfs:comment xml:lang="en">Look at carefully; study mentally.</rdfs:comment>
        <rdfs:isDefinedBy rdf:datatype="http://www.w3.org/2001/XMLSchema#string">http://wordnet-rdf.princeton.edu/wn31/202134765-v</rdfs:isDefinedBy>
        <rdfs:label xml:lang="en">Viewed</rdfs:label>
    </owl:NamedIndividual>
    


    <!-- http://purl.imsglobal.org/caliper/lti/LtiDeepLinkingRequest -->

    <owl:NamedIndividual rdf:about="http://purl.imsglobal.org/caliper/lti/LtiDeepLinkingRequest">
        <rdf:type rdf:resource="http://purl.imsglobal.org/caliper/LtiMessageType"/>
        <rdfs:comment xml:lang="en">An LTI message type.</rdfs:comment>
        <rdfs:isDefinedBy rdf:datatype="http://www.w3.org/2001/XMLSchema#string">http://purl.imsglobal.org/caliper</rdfs:isDefinedBy>
        <rdfs:label xml:lang="en">LtiDeepLinkingRequest</rdfs:label>
    </owl:NamedIndividual>
    


    <!-- http://purl.imsglobal.org/caliper/lti/LtiResourceLinkRequest -->

    <owl:NamedIndividual rdf:about="http://purl.imsglobal.org/caliper/lti/LtiResourceLinkRequest">
        <rdf:type rdf:resource="http://purl.imsglobal.org/caliper/LtiMessageType"/>
        <rdfs:comment xml:lang="en">An LTI message type.</rdfs:comment>
        <rdfs:isDefinedBy rdf:datatype="http://www.w3.org/2001/XMLSchema#string">http://purl.imsglobal.org/caliper</rdfs:isDefinedBy>
        <rdfs:label xml:lang="en">LtiResourceLinkRequest</rdfs:label>
    </owl:NamedIndividual>
    


    <!-- http://purl.imsglobal.org/caliper/metrics/AssessmentsPassed -->

    <owl:NamedIndividual rdf:about="http://purl.imsglobal.org/caliper/metrics/AssessmentsPassed">
        <rdf:type rdf:resource="http://purl.imsglobal.org/caliper/Metric"/>
        <rdfs:comment xml:lang="en">Count of assessments that have been passed by the learner.</rdfs:comment>
        <rdfs:isDefinedBy rdf:datatype="http://www.w3.org/2001/XMLSchema#string">http://purl.imsglobal.org/caliper</rdfs:isDefinedBy>
        <rdfs:label xml:lang="en">AssessmentsPassed</rdfs:label>
    </owl:NamedIndividual>
    


    <!-- http://purl.imsglobal.org/caliper/metrics/AssessmentsSubmitted -->

    <owl:NamedIndividual rdf:about="http://purl.imsglobal.org/caliper/metrics/AssessmentsSubmitted">
        <rdf:type rdf:resource="http://purl.imsglobal.org/caliper/Metric"/>
        <rdfs:comment xml:lang="en">Count of assessments that have been submitted by the learner.</rdfs:comment>
        <rdfs:isDefinedBy rdf:datatype="http://www.w3.org/2001/XMLSchema#string">http://purl.imsglobal.org/caliper</rdfs:isDefinedBy>
        <rdfs:label xml:lang="en">AssessmentsSubmitted</rdfs:label>
    </owl:NamedIndividual>
    


    <!-- http://purl.imsglobal.org/caliper/metrics/MinutesOnTask -->

    <owl:NamedIndividual rdf:about="http://purl.imsglobal.org/caliper/metrics/MinutesOnTask">
        <rdf:type rdf:resource="http://purl.imsglobal.org/caliper/Metric"/>
        <rdfs:comment xml:lang="en">Active time spent by learner utilizing the tool.</rdfs:comment>
        <rdfs:isDefinedBy rdf:datatype="http://www.w3.org/2001/XMLSchema#string">http://purl.imsglobal.org/caliper</rdfs:isDefinedBy>
        <rdfs:label xml:lang="en">MinutesOnTask</rdfs:label>
    </owl:NamedIndividual>
    


    <!-- http://purl.imsglobal.org/caliper/metrics/SkillsMastered -->

    <owl:NamedIndividual rdf:about="http://purl.imsglobal.org/caliper/metrics/SkillsMastered">
        <rdf:type rdf:resource="http://purl.imsglobal.org/caliper/Metric"/>
        <rdfs:comment xml:lang="en">Count of learning skills or targets for which the learner has demonstrated understanding.</rdfs:comment>
        <rdfs:isDefinedBy rdf:datatype="http://www.w3.org/2001/XMLSchema#string">http://purl.imsglobal.org/caliper</rdfs:isDefinedBy>
        <rdfs:label xml:lang="en">SkillsMastered</rdfs:label>
    </owl:NamedIndividual>
    


    <!-- http://purl.imsglobal.org/caliper/metrics/StandardsMastered -->

    <owl:NamedIndividual rdf:about="http://purl.imsglobal.org/caliper/metrics/StandardsMastered">
        <rdf:type rdf:resource="http://purl.imsglobal.org/caliper/Metric"/>
        <rdfs:comment xml:lang="en">Count of learning standards or competencies for which the learner has demonstrated understanding.</rdfs:comment>
        <rdfs:isDefinedBy rdf:datatype="http://www.w3.org/2001/XMLSchema#string">http://purl.imsglobal.org/caliper</rdfs:isDefinedBy>
        <rdfs:label xml:lang="en">StandardsMastered</rdfs:label>
    </owl:NamedIndividual>
    


    <!-- http://purl.imsglobal.org/caliper/metrics/UnitsCompleted -->

    <owl:NamedIndividual rdf:about="http://purl.imsglobal.org/caliper/metrics/UnitsCompleted">
        <rdf:type rdf:resource="http://purl.imsglobal.org/caliper/Metric"/>
        <rdfs:comment xml:lang="en">Count of instructional units completed by the learner.</rdfs:comment>
        <rdfs:isDefinedBy rdf:datatype="http://www.w3.org/2001/XMLSchema#string">http://purl.imsglobal.org/caliper</rdfs:isDefinedBy>
        <rdfs:label xml:lang="en">UnitsCompleted</rdfs:label>
    </owl:NamedIndividual>
    


    <!-- http://purl.imsglobal.org/caliper/metrics/UnitsPassed -->

    <owl:NamedIndividual rdf:about="http://purl.imsglobal.org/caliper/metrics/UnitsPassed">
        <rdf:type rdf:resource="http://purl.imsglobal.org/caliper/Metric"/>
        <rdfs:comment xml:lang="en">Count of instructional units completed by the learner, submitted for evaluation, and scored with a passing mark.</rdfs:comment>
        <rdfs:isDefinedBy rdf:datatype="http://www.w3.org/2001/XMLSchema#string">http://purl.imsglobal.org/caliper</rdfs:isDefinedBy>
        <rdfs:label xml:lang="en">UnitsPassed</rdfs:label>
    </owl:NamedIndividual>
    


    <!-- http://purl.imsglobal.org/caliper/metrics/WordsRead -->

    <owl:NamedIndividual rdf:about="http://purl.imsglobal.org/caliper/metrics/WordsRead">
        <rdf:type rdf:resource="http://purl.imsglobal.org/caliper/Metric"/>
        <rdfs:comment xml:lang="en">Count of the number of words read by the learner.</rdfs:comment>
        <rdfs:isDefinedBy rdf:datatype="http://www.w3.org/2001/XMLSchema#string">http://purl.imsglobal.org/caliper</rdfs:isDefinedBy>
        <rdfs:label xml:lang="en">WordsRead</rdfs:label>
    </owl:NamedIndividual>
    


    <!-- http://purl.imsglobal.org/vocab/lis/v2/membership/Administrator#Administrator -->

    <owl:NamedIndividual rdf:about="http://purl.imsglobal.org/vocab/lis/v2/membership/Administrator#Administrator">
        <rdf:type rdf:resource="http://purl.imsglobal.org/vocab/lis/v2/membership#Administrator"/>
        <rdfs:comment xml:lang="en">Someone who typically works with a system and all sub-structures (LMS, SIS, etc.).</rdfs:comment>
        <rdfs:isDefinedBy rdf:datatype="http://www.w3.org/2001/XMLSchema#string">http://www.imsglobal.org/lis/</rdfs:isDefinedBy>
        <rdfs:label xml:lang="en">Administrator</rdfs:label>
    </owl:NamedIndividual>
    


    <!-- http://purl.imsglobal.org/vocab/lis/v2/membership/Administrator#Developer -->

    <owl:NamedIndividual rdf:about="http://purl.imsglobal.org/vocab/lis/v2/membership/Administrator#Developer">
        <rdf:type rdf:resource="http://purl.imsglobal.org/vocab/lis/v2/membership#Administrator"/>
        <rdfs:comment xml:lang="en">Provides programmatic development for use in a LMS, SIS, or associated tool(s).</rdfs:comment>
        <rdfs:isDefinedBy rdf:datatype="http://www.w3.org/2001/XMLSchema#string">http://www.imsglobal.org/lis/</rdfs:isDefinedBy>
        <rdfs:label xml:lang="en">Developer</rdfs:label>
    </owl:NamedIndividual>
    


    <!-- http://purl.imsglobal.org/vocab/lis/v2/membership/Administrator#ExternalDeveloper -->

    <owl:NamedIndividual rdf:about="http://purl.imsglobal.org/vocab/lis/v2/membership/Administrator#ExternalDeveloper">
        <rdf:type rdf:resource="http://purl.imsglobal.org/vocab/lis/v2/membership#Administrator"/>
        <rdfs:comment xml:lang="en">A user who is not a member of the institution but provides programmatic development for use in a LMS, SIS, or associated tool(s).</rdfs:comment>
        <rdfs:isDefinedBy rdf:datatype="http://www.w3.org/2001/XMLSchema#string">http://www.imsglobal.org/lis/</rdfs:isDefinedBy>
        <rdfs:label xml:lang="en">ExternalDeveloper</rdfs:label>
    </owl:NamedIndividual>
    


    <!-- http://purl.imsglobal.org/vocab/lis/v2/membership/Administrator#ExternalSupport -->

    <owl:NamedIndividual rdf:about="http://purl.imsglobal.org/vocab/lis/v2/membership/Administrator#ExternalSupport">
        <rdf:type rdf:resource="http://purl.imsglobal.org/vocab/lis/v2/membership#Administrator"/>
        <rdfs:comment xml:lang="en">A user who is not a member of the institution but provides support for the system; usually has fewer privileges then an administrator.</rdfs:comment>
        <rdfs:isDefinedBy rdf:datatype="http://www.w3.org/2001/XMLSchema#string">http://www.imsglobal.org/lis/</rdfs:isDefinedBy>
        <rdfs:label xml:lang="en">ExternalSupport</rdfs:label>
    </owl:NamedIndividual>
    


    <!-- http://purl.imsglobal.org/vocab/lis/v2/membership/Administrator#ExternalSystemAdministrator -->

    <owl:NamedIndividual rdf:about="http://purl.imsglobal.org/vocab/lis/v2/membership/Administrator#ExternalSystemAdministrator">
        <rdf:type rdf:resource="http://purl.imsglobal.org/vocab/lis/v2/membership#Administrator"/>
        <rdfs:comment xml:lang="en">A user who is not a member of the institution that provides support, e.g., vendor support accounts, 3rd party support accounts, etc.</rdfs:comment>
        <rdfs:isDefinedBy rdf:datatype="http://www.w3.org/2001/XMLSchema#string">http://www.imsglobal.org/lis/</rdfs:isDefinedBy>
        <rdfs:label xml:lang="en">ExternalSystemAdministrator</rdfs:label>
    </owl:NamedIndividual>
    


    <!-- http://purl.imsglobal.org/vocab/lis/v2/membership/Administrator#Support -->

    <owl:NamedIndividual rdf:about="http://purl.imsglobal.org/vocab/lis/v2/membership/Administrator#Support">
        <rdf:type rdf:resource="http://purl.imsglobal.org/vocab/lis/v2/membership#Administrator"/>
        <rdfs:comment xml:lang="en">Provides support for the system, usually has fewer privileges then an administrator.</rdfs:comment>
        <rdfs:isDefinedBy rdf:datatype="http://www.w3.org/2001/XMLSchema#string">http://www.imsglobal.org/lis/</rdfs:isDefinedBy>
        <rdfs:label xml:lang="en">Support</rdfs:label>
    </owl:NamedIndividual>
    


    <!-- http://purl.imsglobal.org/vocab/lis/v2/membership/Administrator#SystemAdministrator -->

    <owl:NamedIndividual rdf:about="http://purl.imsglobal.org/vocab/lis/v2/membership/Administrator#SystemAdministrator">
        <rdf:type rdf:resource="http://purl.imsglobal.org/vocab/lis/v2/membership#Administrator"/>
        <rdfs:comment xml:lang="en">A person who has greater privileges then an administrator.</rdfs:comment>
        <rdfs:isDefinedBy rdf:datatype="http://www.w3.org/2001/XMLSchema#string">http://www.imsglobal.org/lis/</rdfs:isDefinedBy>
        <rdfs:label xml:lang="en">SystemAdministrator</rdfs:label>
    </owl:NamedIndividual>
    


    <!-- http://purl.imsglobal.org/vocab/lis/v2/membership/ContentDeveloper#ContentDeveloper -->

    <owl:NamedIndividual rdf:about="http://purl.imsglobal.org/vocab/lis/v2/membership/ContentDeveloper#ContentDeveloper">
        <rdf:type rdf:resource="http://purl.imsglobal.org/vocab/lis/v2/membership#ContentDeveloper"/>
        <rdfs:comment xml:lang="en">Someone who usually develops materials within a specific course structure.</rdfs:comment>
        <rdfs:isDefinedBy rdf:datatype="http://www.w3.org/2001/XMLSchema#string">http://www.imsglobal.org/lis/</rdfs:isDefinedBy>
        <rdfs:label xml:lang="en">ContentDeveloper</rdfs:label>
    </owl:NamedIndividual>
    


    <!-- http://purl.imsglobal.org/vocab/lis/v2/membership/ContentDeveloper#ContentExpert -->

    <owl:NamedIndividual rdf:about="http://purl.imsglobal.org/vocab/lis/v2/membership/ContentDeveloper#ContentExpert">
        <rdf:type rdf:resource="http://purl.imsglobal.org/vocab/lis/v2/membership#ContentDeveloper"/>
        <rdfs:comment xml:lang="en">An expert that participates in the course because of their knowledge; e.g., guest speaker, artist in residence, etc.</rdfs:comment>
        <rdfs:isDefinedBy rdf:datatype="http://www.w3.org/2001/XMLSchema#string">http://www.imsglobal.org/lis/</rdfs:isDefinedBy>
        <rdfs:label xml:lang="en">ContentExpert</rdfs:label>
    </owl:NamedIndividual>
    


    <!-- http://purl.imsglobal.org/vocab/lis/v2/membership/ContentDeveloper#ExternalContentExpert -->

    <owl:NamedIndividual rdf:about="http://purl.imsglobal.org/vocab/lis/v2/membership/ContentDeveloper#ExternalContentExpert">
        <rdf:type rdf:resource="http://purl.imsglobal.org/vocab/lis/v2/membership#ContentDeveloper"/>
        <rdfs:comment xml:lang="en">An expert who is not a member of the institution butparticipates in the course because of their knowledge; e.g., guest speaker, artist in residence, etc.</rdfs:comment>
        <rdfs:isDefinedBy rdf:datatype="http://www.w3.org/2001/XMLSchema#string">http://www.imsglobal.org/lis/</rdfs:isDefinedBy>
        <rdfs:label xml:lang="en">ExternalContentExpert</rdfs:label>
    </owl:NamedIndividual>
    


    <!-- http://purl.imsglobal.org/vocab/lis/v2/membership/ContentDeveloper#Librarian -->

    <owl:NamedIndividual rdf:about="http://purl.imsglobal.org/vocab/lis/v2/membership/ContentDeveloper#Librarian">
        <rdf:type rdf:resource="http://purl.imsglobal.org/vocab/lis/v2/membership#ContentDeveloper"/>
        <rdfs:comment xml:lang="en">A librarian who provides content support.</rdfs:comment>
        <rdfs:isDefinedBy rdf:datatype="http://www.w3.org/2001/XMLSchema#string">http://www.imsglobal.org/lis/</rdfs:isDefinedBy>
        <rdfs:label xml:lang="en">Librarian</rdfs:label>
    </owl:NamedIndividual>
    


    <!-- http://purl.imsglobal.org/vocab/lis/v2/membership/Instructor#ExternalInstructor -->

    <owl:NamedIndividual rdf:about="http://purl.imsglobal.org/vocab/lis/v2/membership/Instructor#ExternalInstructor">
        <rdf:type rdf:resource="http://purl.imsglobal.org/vocab/lis/v2/membership#Instructor"/>
        <rdfs:comment xml:lang="en">An instructor who is not a member of the institution.</rdfs:comment>
        <rdfs:isDefinedBy rdf:datatype="http://www.w3.org/2001/XMLSchema#string">http://www.imsglobal.org/lis/</rdfs:isDefinedBy>
        <rdfs:label xml:lang="en">ExternalInstructor</rdfs:label>
    </owl:NamedIndividual>
    


    <!-- http://purl.imsglobal.org/vocab/lis/v2/membership/Instructor#GuestInstructor -->

    <owl:NamedIndividual rdf:about="http://purl.imsglobal.org/vocab/lis/v2/membership/Instructor#GuestInstructor">
        <rdf:type rdf:resource="http://purl.imsglobal.org/vocab/lis/v2/membership#Instructor"/>
        <rdfs:comment xml:lang="en"></rdfs:comment>
        <rdfs:comment xml:lang="en">An instructor who is teaching this course outside of their normal responsibilities</rdfs:comment>
        <rdfs:isDefinedBy rdf:datatype="http://www.w3.org/2001/XMLSchema#string">http://www.imsglobal.org/lis/</rdfs:isDefinedBy>
        <rdfs:label xml:lang="en">GuestInstructor</rdfs:label>
    </owl:NamedIndividual>
    


    <!-- http://purl.imsglobal.org/vocab/lis/v2/membership/Instructor#Instructor -->

    <owl:NamedIndividual rdf:about="http://purl.imsglobal.org/vocab/lis/v2/membership/Instructor#Instructor">
        <rdf:type rdf:resource="http://purl.imsglobal.org/vocab/lis/v2/membership#Instructor"/>
        <rdfs:comment xml:lang="en">Someone who usually teaches within a specific course structure.</rdfs:comment>
        <rdfs:isDefinedBy rdf:datatype="http://www.w3.org/2001/XMLSchema#string">http://www.imsglobal.org/lis/</rdfs:isDefinedBy>
        <rdfs:label xml:lang="en">Instructor</rdfs:label>
    </owl:NamedIndividual>
    


    <!-- http://purl.imsglobal.org/vocab/lis/v2/membership/Instructor#Lecturer -->

    <owl:NamedIndividual rdf:about="http://purl.imsglobal.org/vocab/lis/v2/membership/Instructor#Lecturer">
        <rdf:type rdf:resource="http://purl.imsglobal.org/vocab/lis/v2/membership#Instructor"/>
        <rdfs:comment xml:lang="en">An instructor that has limited permissions to modify the course.</rdfs:comment>
        <rdfs:isDefinedBy rdf:datatype="http://www.w3.org/2001/XMLSchema#string">http://www.imsglobal.org/lis/</rdfs:isDefinedBy>
        <rdfs:label xml:lang="en">Lecturer</rdfs:label>
    </owl:NamedIndividual>
    


    <!-- http://purl.imsglobal.org/vocab/lis/v2/membership/Instructor#PrimaryInstructor -->

    <owl:NamedIndividual rdf:about="http://purl.imsglobal.org/vocab/lis/v2/membership/Instructor#PrimaryInstructor">
        <rdf:type rdf:resource="http://purl.imsglobal.org/vocab/lis/v2/membership#Instructor"/>
        <rdfs:comment xml:lang="en">An instructor who is primarily responsible for the instruction.</rdfs:comment>
        <rdfs:isDefinedBy rdf:datatype="http://www.w3.org/2001/XMLSchema#string">http://www.imsglobal.org/lis/</rdfs:isDefinedBy>
        <rdfs:label xml:lang="en">PrimaryInstructor</rdfs:label>
    </owl:NamedIndividual>
    


    <!-- http://purl.imsglobal.org/vocab/lis/v2/membership/Instructor#SecondaryInstructor -->

    <owl:NamedIndividual rdf:about="http://purl.imsglobal.org/vocab/lis/v2/membership/Instructor#SecondaryInstructor">
        <rdf:type rdf:resource="http://purl.imsglobal.org/vocab/lis/v2/membership#Instructor"/>
        <rdfs:comment xml:lang="en">An instructor who has secondary responsibility for the instruction.</rdfs:comment>
        <rdfs:isDefinedBy rdf:datatype="http://www.w3.org/2001/XMLSchema#string">http://www.imsglobal.org/lis/</rdfs:isDefinedBy>
        <rdfs:label xml:lang="en">SecondaryInstructor</rdfs:label>
    </owl:NamedIndividual>
    


    <!-- http://purl.imsglobal.org/vocab/lis/v2/membership/Instructor#TeachingAssistant -->

    <owl:NamedIndividual rdf:about="http://purl.imsglobal.org/vocab/lis/v2/membership/Instructor#TeachingAssistant">
        <rdf:type rdf:resource="http://purl.imsglobal.org/vocab/lis/v2/membership#TeachingAssistant"/>
        <rdfs:comment xml:lang="en">Someone who usually has a subset of instructional responsibilities for some portion of a course structure</rdfs:comment>
        <rdfs:comment xml:lang="en">The role of a teaching assistant to an Instructor in the Membership.</rdfs:comment>
        <rdfs:isDefinedBy rdf:datatype="http://www.w3.org/2001/XMLSchema#string">http://www.imsglobal.org/lis/</rdfs:isDefinedBy>
        <rdfs:label xml:lang="en">TeachingAssistant</rdfs:label>
    </owl:NamedIndividual>
    


    <!-- http://purl.imsglobal.org/vocab/lis/v2/membership/Instructor#TeachingAssistantGroup -->

    <owl:NamedIndividual rdf:about="http://purl.imsglobal.org/vocab/lis/v2/membership/Instructor#TeachingAssistantGroup">
        <rdf:type rdf:resource="http://purl.imsglobal.org/vocab/lis/v2/membership#TeachingAssistant"/>
        <rdfs:comment xml:lang="en">A teaching assistant for a Group.</rdfs:comment>
        <rdfs:isDefinedBy rdf:datatype="http://www.w3.org/2001/XMLSchema#string">http://www.imsglobal.org/lis/</rdfs:isDefinedBy>
        <rdfs:label xml:lang="en">TeachingAssistantGroup</rdfs:label>
    </owl:NamedIndividual>
    


    <!-- http://purl.imsglobal.org/vocab/lis/v2/membership/Instructor#TeachingAssistantOffering -->

    <owl:NamedIndividual rdf:about="http://purl.imsglobal.org/vocab/lis/v2/membership/Instructor#TeachingAssistantOffering">
        <rdf:type rdf:resource="http://purl.imsglobal.org/vocab/lis/v2/membership#TeachingAssistant"/>
        <rdfs:comment xml:lang="en">A teaching assistant for a CourseOffering.</rdfs:comment>
        <rdfs:isDefinedBy rdf:datatype="http://www.w3.org/2001/XMLSchema#string">http://www.imsglobal.org/lis/</rdfs:isDefinedBy>
        <rdfs:label xml:lang="en">TeachingAssistantOffering</rdfs:label>
    </owl:NamedIndividual>
    


    <!-- http://purl.imsglobal.org/vocab/lis/v2/membership/Instructor#TeachingAssistantSection -->

    <owl:NamedIndividual rdf:about="http://purl.imsglobal.org/vocab/lis/v2/membership/Instructor#TeachingAssistantSection">
        <rdf:type rdf:resource="http://purl.imsglobal.org/vocab/lis/v2/membership#TeachingAssistant"/>
        <rdfs:comment xml:lang="en">A teaching assistant for a CourseSection.</rdfs:comment>
        <rdfs:isDefinedBy rdf:datatype="http://www.w3.org/2001/XMLSchema#string">http://www.imsglobal.org/lis/</rdfs:isDefinedBy>
        <rdfs:label xml:lang="en">TeachingAssistantSection</rdfs:label>
    </owl:NamedIndividual>
    


    <!-- http://purl.imsglobal.org/vocab/lis/v2/membership/Instructor#TeachingAssistantTemplate -->

    <owl:NamedIndividual rdf:about="http://purl.imsglobal.org/vocab/lis/v2/membership/Instructor#TeachingAssistantTemplate">
        <rdf:type rdf:resource="http://purl.imsglobal.org/vocab/lis/v2/membership#TeachingAssistant"/>
        <rdfs:comment xml:lang="en">A teaching assistant for a template.</rdfs:comment>
        <rdfs:isDefinedBy rdf:datatype="http://www.w3.org/2001/XMLSchema#string">http://www.imsglobal.org/lis/</rdfs:isDefinedBy>
        <rdfs:label xml:lang="en">TeachingAssistantTemplate</rdfs:label>
    </owl:NamedIndividual>
    


    <!-- http://purl.imsglobal.org/vocab/lis/v2/membership/Learner#ExternalLearner -->

    <owl:NamedIndividual rdf:about="http://purl.imsglobal.org/vocab/lis/v2/membership/Learner#ExternalLearner">
        <rdf:type rdf:resource="http://purl.imsglobal.org/vocab/lis/v2/membership#Learner"/>
        <rdfs:comment xml:lang="en">A learner who is not a member of the institution.</rdfs:comment>
        <rdfs:isDefinedBy rdf:datatype="http://www.w3.org/2001/XMLSchema#string">http://www.imsglobal.org/lis/</rdfs:isDefinedBy>
        <rdfs:label xml:lang="en">ExternalLearner</rdfs:label>
    </owl:NamedIndividual>
    


    <!-- http://purl.imsglobal.org/vocab/lis/v2/membership/Learner#GuestLearner -->

    <owl:NamedIndividual rdf:about="http://purl.imsglobal.org/vocab/lis/v2/membership/Learner#GuestLearner">
        <rdf:type rdf:resource="http://purl.imsglobal.org/vocab/lis/v2/membership#Learner"/>
        <rdfs:comment xml:lang="en">A learner who is not enrolled in the same process as a learner; may or may not receive credit for the course.</rdfs:comment>
        <rdfs:isDefinedBy rdf:datatype="http://www.w3.org/2001/XMLSchema#string">http://www.imsglobal.org/lis/</rdfs:isDefinedBy>
        <rdfs:label xml:lang="en">GuestLearner</rdfs:label>
    </owl:NamedIndividual>
    


    <!-- http://purl.imsglobal.org/vocab/lis/v2/membership/Learner#Learner -->

    <owl:NamedIndividual rdf:about="http://purl.imsglobal.org/vocab/lis/v2/membership/Learner#Learner">
        <rdf:type rdf:resource="http://purl.imsglobal.org/vocab/lis/v2/membership#Learner"/>
        <rdfs:comment xml:lang="en">Someone who usually learns within a specific course structure.</rdfs:comment>
        <rdfs:isDefinedBy rdf:datatype="http://www.w3.org/2001/XMLSchema#string">http://www.imsglobal.org/lis/</rdfs:isDefinedBy>
        <rdfs:label xml:lang="en">Learner</rdfs:label>
    </owl:NamedIndividual>
    


    <!-- http://purl.imsglobal.org/vocab/lis/v2/membership/Learner#NonCreditLearner -->

    <owl:NamedIndividual rdf:about="http://purl.imsglobal.org/vocab/lis/v2/membership/Learner#NonCreditLearner">
        <rdf:type rdf:resource="http://purl.imsglobal.org/vocab/lis/v2/membership#Learner"/>
        <rdfs:comment xml:lang="en">A learner who is enrolled through the same process as a learner, but is not receiving credit for the course of study.</rdfs:comment>
        <rdfs:isDefinedBy rdf:datatype="http://www.w3.org/2001/XMLSchema#string">http://www.imsglobal.org/lis/</rdfs:isDefinedBy>
        <rdfs:label xml:lang="en">NonCreditLearner</rdfs:label>
    </owl:NamedIndividual>
    


    <!-- http://purl.imsglobal.org/vocab/lis/v2/membership/Manager#AreaManager -->

    <owl:NamedIndividual rdf:about="http://purl.imsglobal.org/vocab/lis/v2/membership/Manager#AreaManager">
        <rdf:type rdf:resource="http://purl.imsglobal.org/vocab/lis/v2/membership#Manager"/>
        <rdfs:comment xml:lang="en">Someone who provides assistance, administration, and/or support to multiple course structures; e.g., Departmental Staff, Cohort Leader, etc.</rdfs:comment>
        <rdfs:isDefinedBy rdf:datatype="http://www.w3.org/2001/XMLSchema#string">http://www.imsglobal.org/lis/</rdfs:isDefinedBy>
        <rdfs:label xml:lang="en">AreaManager</rdfs:label>
    </owl:NamedIndividual>
    


    <!-- http://purl.imsglobal.org/vocab/lis/v2/membership/Manager#CourseCoordinator -->

    <owl:NamedIndividual rdf:about="http://purl.imsglobal.org/vocab/lis/v2/membership/Manager#CourseCoordinator">
        <rdf:type rdf:resource="http://purl.imsglobal.org/vocab/lis/v2/membership#Manager"/>
        <rdfs:comment xml:lang="en">Someone who provides assistance to a set of course structures that are related, a lab manager, etc.</rdfs:comment>
        <rdfs:isDefinedBy rdf:datatype="http://www.w3.org/2001/XMLSchema#string">http://www.imsglobal.org/lis/</rdfs:isDefinedBy>
        <rdfs:label xml:lang="en">CourseCoordinator</rdfs:label>
    </owl:NamedIndividual>
    


    <!-- http://purl.imsglobal.org/vocab/lis/v2/membership/Manager#ExternalObserver -->

    <owl:NamedIndividual rdf:about="http://purl.imsglobal.org/vocab/lis/v2/membership/Manager#ExternalObserver">
        <rdf:type rdf:resource="http://purl.imsglobal.org/vocab/lis/v2/membership#Manager"/>
        <rdfs:comment xml:lang="en">Person that is not a member of the institution but views multiple course structures for non-instructional purposes; e.g., peer review committee, accreditation staff, etc.</rdfs:comment>
        <rdfs:isDefinedBy rdf:datatype="http://www.w3.org/2001/XMLSchema#string">http://www.imsglobal.org/lis/</rdfs:isDefinedBy>
        <rdfs:label xml:lang="en">ExternalObserver</rdfs:label>
    </owl:NamedIndividual>
    


    <!-- http://purl.imsglobal.org/vocab/lis/v2/membership/Manager#Manager -->

    <owl:NamedIndividual rdf:about="http://purl.imsglobal.org/vocab/lis/v2/membership/Manager#Manager">
        <rdf:type rdf:resource="http://purl.imsglobal.org/vocab/lis/v2/membership#Manager"/>
        <rdfs:comment xml:lang="en">Someone who usually interacts with multiple course structures.</rdfs:comment>
        <rdfs:isDefinedBy rdf:datatype="http://www.w3.org/2001/XMLSchema#string">http://www.imsglobal.org/lis/</rdfs:isDefinedBy>
        <rdfs:label xml:lang="en">Manager</rdfs:label>
    </owl:NamedIndividual>
    


    <!-- http://purl.imsglobal.org/vocab/lis/v2/membership/Manager#Observer -->

    <owl:NamedIndividual rdf:about="http://purl.imsglobal.org/vocab/lis/v2/membership/Manager#Observer">
        <rdf:type rdf:resource="http://purl.imsglobal.org/vocab/lis/v2/membership#Manager"/>
        <rdfs:comment xml:lang="en">Views multiple course structures for non-instructional purposes; e.g., peer review committee, accreditation staff, etc.</rdfs:comment>
        <rdfs:isDefinedBy rdf:datatype="http://www.w3.org/2001/XMLSchema#string">http://www.imsglobal.org/lis/</rdfs:isDefinedBy>
        <rdfs:label xml:lang="en">Observer</rdfs:label>
    </owl:NamedIndividual>
    


    <!-- http://purl.imsglobal.org/vocab/lis/v2/membership/Member#Member -->

    <owl:NamedIndividual rdf:about="http://purl.imsglobal.org/vocab/lis/v2/membership/Member#Member">
        <rdf:type rdf:resource="http://purl.imsglobal.org/vocab/lis/v2/membership#Member"/>
        <rdfs:comment xml:lang="en">Someone who is a member of an Organization.</rdfs:comment>
        <rdfs:isDefinedBy rdf:datatype="http://www.w3.org/2001/XMLSchema#string">http://www.imsglobal.org/lis/</rdfs:isDefinedBy>
        <rdfs:label xml:lang="en">Member</rdfs:label>
    </owl:NamedIndividual>
    


    <!-- http://purl.imsglobal.org/vocab/lis/v2/membership/Mentor#Advisor -->

    <owl:NamedIndividual rdf:about="http://purl.imsglobal.org/vocab/lis/v2/membership/Mentor#Advisor">
        <rdf:type rdf:resource="http://purl.imsglobal.org/vocab/lis/v2/membership#Mentor"/>
        <rdfs:comment xml:lang="en">Advises learners.</rdfs:comment>
        <rdfs:isDefinedBy rdf:datatype="http://www.w3.org/2001/XMLSchema#string">http://www.imsglobal.org/lis/</rdfs:isDefinedBy>
        <rdfs:label xml:lang="en">Advisor</rdfs:label>
    </owl:NamedIndividual>
    


    <!-- http://purl.imsglobal.org/vocab/lis/v2/membership/Mentor#Auditor -->

    <owl:NamedIndividual rdf:about="http://purl.imsglobal.org/vocab/lis/v2/membership/Mentor#Auditor">
        <rdf:type rdf:resource="http://purl.imsglobal.org/vocab/lis/v2/membership#Mentor"/>
        <rdfs:comment xml:lang="en">Audits learner activities; e.g., staff that verifies continuing eligibility for a scholarship, etc.</rdfs:comment>
        <rdfs:isDefinedBy rdf:datatype="http://www.w3.org/2001/XMLSchema#string">http://www.imsglobal.org/lis/</rdfs:isDefinedBy>
        <rdfs:label xml:lang="en">Auditor</rdfs:label>
    </owl:NamedIndividual>
    


    <!-- http://purl.imsglobal.org/vocab/lis/v2/membership/Mentor#ExternalAdvisor -->

    <owl:NamedIndividual rdf:about="http://purl.imsglobal.org/vocab/lis/v2/membership/Mentor#ExternalAdvisor">
        <rdf:type rdf:resource="http://purl.imsglobal.org/vocab/lis/v2/membership#Mentor"/>
        <rdfs:comment xml:lang="en">A user who is not a member of the institution that advises learners.</rdfs:comment>
        <rdfs:isDefinedBy rdf:datatype="http://www.w3.org/2001/XMLSchema#string">http://www.imsglobal.org/lis/</rdfs:isDefinedBy>
        <rdfs:label xml:lang="en">ExternalAdvisor</rdfs:label>
    </owl:NamedIndividual>
    


    <!-- http://purl.imsglobal.org/vocab/lis/v2/membership/Mentor#ExternalAuditor -->

    <owl:NamedIndividual rdf:about="http://purl.imsglobal.org/vocab/lis/v2/membership/Mentor#ExternalAuditor">
        <rdf:type rdf:resource="http://purl.imsglobal.org/vocab/lis/v2/membership#Mentor"/>
        <rdfs:comment xml:lang="en">A user who is not a member of the institution that audits learner activities; e.g., staff that verifies continuing eligibility for a scholarship, etc.</rdfs:comment>
        <rdfs:isDefinedBy rdf:datatype="http://www.w3.org/2001/XMLSchema#string">http://www.imsglobal.org/lis/</rdfs:isDefinedBy>
        <rdfs:label xml:lang="en">ExternalAuditor</rdfs:label>
    </owl:NamedIndividual>
    


    <!-- http://purl.imsglobal.org/vocab/lis/v2/membership/Mentor#ExternalLearningFacilitator -->

    <owl:NamedIndividual rdf:about="http://purl.imsglobal.org/vocab/lis/v2/membership/Mentor#ExternalLearningFacilitator">
        <rdf:type rdf:resource="http://purl.imsglobal.org/vocab/lis/v2/membership#Mentor"/>
        <rdfs:comment xml:lang="en">A user who is not a member of the institution that works with individual learner to access materials; e.g., translator, assistant for persons of differing abilities, etc.</rdfs:comment>
        <rdfs:isDefinedBy rdf:datatype="http://www.w3.org/2001/XMLSchema#string">http://www.imsglobal.org/lis/</rdfs:isDefinedBy>
        <rdfs:label xml:lang="en">ExternalLearningFacilitator</rdfs:label>
    </owl:NamedIndividual>
    


    <!-- http://purl.imsglobal.org/vocab/lis/v2/membership/Mentor#ExternalMentor -->

    <owl:NamedIndividual rdf:about="http://purl.imsglobal.org/vocab/lis/v2/membership/Mentor#ExternalMentor">
        <rdf:type rdf:resource="http://purl.imsglobal.org/vocab/lis/v2/membership#Mentor"/>
        <rdfs:comment xml:lang="en">A user who is not a member of the institution that mentors learners.</rdfs:comment>
        <rdfs:comment xml:lang="en">ExternalMentor</rdfs:comment>
        <rdfs:isDefinedBy rdf:datatype="http://www.w3.org/2001/XMLSchema#string">http://www.imsglobal.org/lis/</rdfs:isDefinedBy>
    </owl:NamedIndividual>
    


    <!-- http://purl.imsglobal.org/vocab/lis/v2/membership/Mentor#ExternalReviewer -->

    <owl:NamedIndividual rdf:about="http://purl.imsglobal.org/vocab/lis/v2/membership/Mentor#ExternalReviewer">
        <rdf:type rdf:resource="http://purl.imsglobal.org/vocab/lis/v2/membership#Mentor"/>
        <rdfs:comment xml:lang="en">A user who is not a member of the institution that reviews work by learners.</rdfs:comment>
        <rdfs:isDefinedBy rdf:datatype="http://www.w3.org/2001/XMLSchema#string">http://www.imsglobal.org/lis/</rdfs:isDefinedBy>
        <rdfs:label xml:lang="en">ExternalReviewer</rdfs:label>
    </owl:NamedIndividual>
    


    <!-- http://purl.imsglobal.org/vocab/lis/v2/membership/Mentor#ExternalTutor -->

    <owl:NamedIndividual rdf:about="http://purl.imsglobal.org/vocab/lis/v2/membership/Mentor#ExternalTutor">
        <rdf:type rdf:resource="http://purl.imsglobal.org/vocab/lis/v2/membership#Mentor"/>
        <rdfs:comment xml:lang="en">A user who is not a member of the institution that works with individual learners to assist in their instruction.</rdfs:comment>
        <rdfs:isDefinedBy rdf:datatype="http://www.w3.org/2001/XMLSchema#string">http://www.imsglobal.org/lis/</rdfs:isDefinedBy>
        <rdfs:label xml:lang="en">ExternalTutor</rdfs:label>
    </owl:NamedIndividual>
    


    <!-- http://purl.imsglobal.org/vocab/lis/v2/membership/Mentor#LearningFacilitator -->

    <owl:NamedIndividual rdf:about="http://purl.imsglobal.org/vocab/lis/v2/membership/Mentor#LearningFacilitator">
        <rdf:type rdf:resource="http://purl.imsglobal.org/vocab/lis/v2/membership#Mentor"/>
        <rdfs:comment xml:lang="en">Works with individual learner to access materials; e.g., translator, assistant for persons of differing abilities, etc.</rdfs:comment>
        <rdfs:isDefinedBy rdf:datatype="http://www.w3.org/2001/XMLSchema#string">http://www.imsglobal.org/lis/</rdfs:isDefinedBy>
        <rdfs:label xml:lang="en">LearningFacilitator</rdfs:label>
    </owl:NamedIndividual>
    


    <!-- http://purl.imsglobal.org/vocab/lis/v2/membership/Mentor#Mentor -->

    <owl:NamedIndividual rdf:about="http://purl.imsglobal.org/vocab/lis/v2/membership/Mentor#Mentor">
        <rdf:type rdf:resource="http://purl.imsglobal.org/vocab/lis/v2/membership#Mentor"/>
        <rdfs:comment xml:lang="en">Someone who usually works with a specific course structure with a specific learner.</rdfs:comment>
        <rdfs:isDefinedBy rdf:datatype="http://www.w3.org/2001/XMLSchema#string">http://www.imsglobal.org/lis/</rdfs:isDefinedBy>
        <rdfs:label xml:lang="en">Mentor</rdfs:label>
    </owl:NamedIndividual>
    


    <!-- http://purl.imsglobal.org/vocab/lis/v2/membership/Mentor#Reviewer -->

    <owl:NamedIndividual rdf:about="http://purl.imsglobal.org/vocab/lis/v2/membership/Mentor#Reviewer">
        <rdf:type rdf:resource="http://purl.imsglobal.org/vocab/lis/v2/membership#Mentor"/>
        <rdfs:comment xml:lang="en">Reviews work by learners.</rdfs:comment>
        <rdfs:isDefinedBy rdf:datatype="http://www.w3.org/2001/XMLSchema#string">http://www.imsglobal.org/lis/</rdfs:isDefinedBy>
        <rdfs:label xml:lang="en">Reviewer</rdfs:label>
    </owl:NamedIndividual>
    


    <!-- http://purl.imsglobal.org/vocab/lis/v2/membership/Mentor#Tutor -->

    <owl:NamedIndividual rdf:about="http://purl.imsglobal.org/vocab/lis/v2/membership/Mentor#Tutor">
        <rdf:type rdf:resource="http://purl.imsglobal.org/vocab/lis/v2/membership#Mentor"/>
        <rdfs:comment xml:lang="en">Works with individual learners to assist in their instruction.</rdfs:comment>
        <rdfs:isDefinedBy rdf:datatype="http://www.w3.org/2001/XMLSchema#string">http://www.imsglobal.org/lis/</rdfs:isDefinedBy>
        <rdfs:label xml:lang="en">Tutor</rdfs:label>
    </owl:NamedIndividual>
    


    <!-- http://purl.imsglobal.org/vocab/lis/v2/membership/Officer#Chair -->

    <owl:NamedIndividual rdf:about="http://purl.imsglobal.org/vocab/lis/v2/membership/Officer#Chair">
        <rdf:type rdf:resource="http://purl.imsglobal.org/vocab/lis/v2/membership#Officer"/>
        <rdfs:comment xml:lang="en">Chair of the Group.</rdfs:comment>
        <rdfs:isDefinedBy rdf:datatype="http://www.w3.org/2001/XMLSchema#string">http://www.imsglobal.org/lis/</rdfs:isDefinedBy>
        <rdfs:label xml:lang="en">Chair</rdfs:label>
    </owl:NamedIndividual>
    


    <!-- http://purl.imsglobal.org/vocab/lis/v2/membership/Officer#Communications -->

    <owl:NamedIndividual rdf:about="http://purl.imsglobal.org/vocab/lis/v2/membership/Officer#Communications">
        <rdf:type rdf:resource="http://purl.imsglobal.org/vocab/lis/v2/membership#Officer"/>
        <rdfs:comment xml:lang="en">Communications officer for the Group.</rdfs:comment>
        <rdfs:isDefinedBy rdf:datatype="http://www.w3.org/2001/XMLSchema#string">http://www.imsglobal.org/lis/</rdfs:isDefinedBy>
        <rdfs:label xml:lang="en">Communications</rdfs:label>
    </owl:NamedIndividual>
    


    <!-- http://purl.imsglobal.org/vocab/lis/v2/membership/Officer#Officer -->

    <owl:NamedIndividual rdf:about="http://purl.imsglobal.org/vocab/lis/v2/membership/Officer#Officer">
        <rdf:type rdf:resource="http://purl.imsglobal.org/vocab/lis/v2/membership#Officer"/>
        <rdfs:comment xml:lang="en">The role of an officer of organization e.g., Chair, Secretary, etc. in the Membership.</rdfs:comment>
        <rdfs:isDefinedBy rdf:datatype="http://www.w3.org/2001/XMLSchema#string">http://www.imsglobal.org/lis/</rdfs:isDefinedBy>
        <rdfs:label xml:lang="en">Officer</rdfs:label>
    </owl:NamedIndividual>
    


    <!-- http://purl.imsglobal.org/vocab/lis/v2/membership/Officer#Secretary -->

    <owl:NamedIndividual rdf:about="http://purl.imsglobal.org/vocab/lis/v2/membership/Officer#Secretary">
        <rdf:type rdf:resource="http://purl.imsglobal.org/vocab/lis/v2/membership#Officer"/>
        <rdfs:comment xml:lang="en">Secretary to the Group.</rdfs:comment>
        <rdfs:isDefinedBy rdf:datatype="http://www.w3.org/2001/XMLSchema#string">http://www.imsglobal.org/lis/</rdfs:isDefinedBy>
        <rdfs:label xml:lang="en">Secretary</rdfs:label>
    </owl:NamedIndividual>
    


    <!-- http://purl.imsglobal.org/vocab/lis/v2/membership/Officer#Treasurer -->

    <owl:NamedIndividual rdf:about="http://purl.imsglobal.org/vocab/lis/v2/membership/Officer#Treasurer">
        <rdf:type rdf:resource="http://purl.imsglobal.org/vocab/lis/v2/membership#Officer"/>
        <rdfs:comment xml:lang="en">Treasurer to the Group.</rdfs:comment>
        <rdfs:isDefinedBy rdf:datatype="http://www.w3.org/2001/XMLSchema#string">http://www.imsglobal.org/lis/</rdfs:isDefinedBy>
        <rdfs:label xml:lang="en">Treasurer</rdfs:label>
    </owl:NamedIndividual>
    


    <!-- http://purl.imsglobal.org/vocab/lis/v2/membership/Officer#ViceChair -->

    <owl:NamedIndividual rdf:about="http://purl.imsglobal.org/vocab/lis/v2/membership/Officer#ViceChair">
        <rdf:type rdf:resource="http://purl.imsglobal.org/vocab/lis/v2/membership#Officer"/>
        <rdfs:comment xml:lang="en">Vice Chair to the Group.</rdfs:comment>
        <rdfs:isDefinedBy rdf:datatype="http://www.w3.org/2001/XMLSchema#string">http://www.imsglobal.org/lis/</rdfs:isDefinedBy>
        <rdfs:label xml:lang="en">ViceChair</rdfs:label>
    </owl:NamedIndividual>
    


    <!-- http://purl.imsglobal.org/vocab/lis/v2/membership/TeachingAssistant#Grader -->

    <owl:NamedIndividual rdf:about="http://purl.imsglobal.org/vocab/lis/v2/membership/TeachingAssistant#Grader">
        <rdf:type rdf:resource="http://purl.imsglobal.org/vocab/lis/v2/membership#Instructor"/>
        <rdfs:comment xml:lang="en">Primary responsibility is assignment of grades.</rdfs:comment>
        <rdfs:isDefinedBy rdf:datatype="http://www.w3.org/2001/XMLSchema#string">http://www.imsglobal.org/lis/</rdfs:isDefinedBy>
        <rdfs:label xml:lang="en">Grader</rdfs:label>
    </owl:NamedIndividual>
    


    <!-- http://purl.imsglobal.org/vocab/lis/v2/membership/TeachingAssistant#TeachingAssistantSectionAssociation -->

    <owl:NamedIndividual rdf:about="http://purl.imsglobal.org/vocab/lis/v2/membership/TeachingAssistant#TeachingAssistantSectionAssociation">
        <rdf:type rdf:resource="http://purl.imsglobal.org/vocab/lis/v2/membership#TeachingAssistant"/>
        <rdfs:comment xml:lang="en">A teaching assistant for a section association.</rdfs:comment>
        <rdfs:isDefinedBy rdf:datatype="http://www.w3.org/2001/XMLSchema#string">http://www.imsglobal.org/lis/</rdfs:isDefinedBy>
        <rdfs:label xml:lang="en">TeachingAssistantSectionAssociation</rdfs:label>
    </owl:NamedIndividual>
    


    <!-- http://purl.imsglobal.org/vocab/lis/v2/status#Active -->

    <owl:NamedIndividual rdf:about="http://purl.imsglobal.org/vocab/lis/v2/status#Active">
        <rdf:type rdf:resource="http://purl.imsglobal.org/caliper/Status"/>
        <rdfs:comment xml:lang="en">The member is active in the Membership.</rdfs:comment>
        <rdfs:isDefinedBy rdf:datatype="http://www.w3.org/2001/XMLSchema#string">http://www.imsglobal.org/lis/</rdfs:isDefinedBy>
        <rdfs:label xml:lang="en">Active</rdfs:label>
    </owl:NamedIndividual>
    


    <!-- http://purl.imsglobal.org/vocab/lis/v2/status#Inactive -->

    <owl:NamedIndividual rdf:about="http://purl.imsglobal.org/vocab/lis/v2/status#Inactive">
        <rdf:type rdf:resource="http://purl.imsglobal.org/caliper/Status"/>
        <rdfs:comment xml:lang="en">The member is inactive in the Membership.</rdfs:comment>
        <rdfs:isDefinedBy rdf:datatype="http://www.w3.org/2001/XMLSchema#string">http://www.imsglobal.org/lis/</rdfs:isDefinedBy>
        <rdfs:label xml:lang="en">Inactive</rdfs:label>
    </owl:NamedIndividual>
    


    <!-- 
    ///////////////////////////////////////////////////////////////////////////////////////
    //
    // General axioms
    //
    ///////////////////////////////////////////////////////////////////////////////////////
     -->

    <rdf:Description>
        <rdf:type rdf:resource="http://www.w3.org/2002/07/owl#AllDisjointClasses"/>
        <owl:members rdf:parseType="Collection">
            <rdf:Description rdf:about="http://purl.imsglobal.org/caliper/Action"/>
            <rdf:Description rdf:about="http://purl.imsglobal.org/caliper/Entity"/>
            <rdf:Description rdf:about="http://purl.imsglobal.org/caliper/Envelope"/>
            <rdf:Description rdf:about="http://purl.imsglobal.org/caliper/Event"/>
            <rdf:Description rdf:about="http://purl.imsglobal.org/caliper/Role"/>
            <rdf:Description rdf:about="http://purl.imsglobal.org/caliper/Selector"/>
            <rdf:Description rdf:about="http://purl.imsglobal.org/caliper/Status"/>
        </owl:members>
    </rdf:Description>
    <rdf:Description>
        <rdf:type rdf:resource="http://www.w3.org/2002/07/owl#AllDisjointClasses"/>
        <owl:members rdf:parseType="Collection">
            <rdf:Description rdf:about="http://purl.imsglobal.org/caliper/Agent"/>
            <rdf:Description rdf:about="http://purl.imsglobal.org/caliper/AggregateMeasure"/>
            <rdf:Description rdf:about="http://purl.imsglobal.org/caliper/Annotation"/>
            <rdf:Description rdf:about="http://purl.imsglobal.org/caliper/Attempt"/>
            <rdf:Description rdf:about="http://purl.imsglobal.org/caliper/Collection"/>
            <rdf:Description rdf:about="http://purl.imsglobal.org/caliper/Comment"/>
            <rdf:Description rdf:about="http://purl.imsglobal.org/caliper/LearningObjective"/>
            <rdf:Description rdf:about="http://purl.imsglobal.org/caliper/Link"/>
            <rdf:Description rdf:about="http://purl.imsglobal.org/caliper/Membership"/>
            <rdf:Description rdf:about="http://purl.imsglobal.org/caliper/Query"/>
            <rdf:Description rdf:about="http://purl.imsglobal.org/caliper/Rating"/>
            <rdf:Description rdf:about="http://purl.imsglobal.org/caliper/Response"/>
            <rdf:Description rdf:about="http://purl.imsglobal.org/caliper/Result"/>
            <rdf:Description rdf:about="http://purl.imsglobal.org/caliper/Scale"/>
            <rdf:Description rdf:about="http://purl.imsglobal.org/caliper/Score"/>
            <rdf:Description rdf:about="http://purl.imsglobal.org/caliper/SearchResponse"/>
            <rdf:Description rdf:about="http://purl.imsglobal.org/caliper/Session"/>
        </owl:members>
    </rdf:Description>
    <rdf:Description>
        <rdf:type rdf:resource="http://www.w3.org/2002/07/owl#AllDisjointClasses"/>
        <owl:members rdf:parseType="Collection">
            <rdf:Description rdf:about="http://purl.imsglobal.org/caliper/Agent"/>
            <rdf:Description rdf:about="http://purl.imsglobal.org/caliper/Annotation"/>
            <rdf:Description rdf:about="http://purl.imsglobal.org/caliper/Attempt"/>
            <rdf:Description rdf:about="http://purl.imsglobal.org/caliper/Comment"/>
            <rdf:Description rdf:about="http://purl.imsglobal.org/caliper/DigitalResource"/>
            <rdf:Description rdf:about="http://purl.imsglobal.org/caliper/LearningObjective"/>
            <rdf:Description rdf:about="http://purl.imsglobal.org/caliper/Link"/>
            <rdf:Description rdf:about="http://purl.imsglobal.org/caliper/Membership"/>
            <rdf:Description rdf:about="http://purl.imsglobal.org/caliper/Query"/>
            <rdf:Description rdf:about="http://purl.imsglobal.org/caliper/Rating"/>
            <rdf:Description rdf:about="http://purl.imsglobal.org/caliper/Response"/>
            <rdf:Description rdf:about="http://purl.imsglobal.org/caliper/Result"/>
            <rdf:Description rdf:about="http://purl.imsglobal.org/caliper/Scale"/>
            <rdf:Description rdf:about="http://purl.imsglobal.org/caliper/Score"/>
            <rdf:Description rdf:about="http://purl.imsglobal.org/caliper/SearchResponse"/>
            <rdf:Description rdf:about="http://purl.imsglobal.org/caliper/Session"/>
        </owl:members>
    </rdf:Description>
    <rdf:Description>
        <rdf:type rdf:resource="http://www.w3.org/2002/07/owl#AllDisjointClasses"/>
        <owl:members rdf:parseType="Collection">
            <rdf:Description rdf:about="http://purl.imsglobal.org/caliper/Agent"/>
            <rdf:Description rdf:about="http://purl.imsglobal.org/caliper/Annotation"/>
            <rdf:Description rdf:about="http://purl.imsglobal.org/caliper/Attempt"/>
            <rdf:Description rdf:about="http://purl.imsglobal.org/caliper/DigitalResource"/>
            <rdf:Description rdf:about="http://purl.imsglobal.org/caliper/LearningObjective"/>
            <rdf:Description rdf:about="http://purl.imsglobal.org/caliper/Link"/>
            <rdf:Description rdf:about="http://purl.imsglobal.org/caliper/Membership"/>
            <rdf:Description rdf:about="http://purl.imsglobal.org/caliper/Query"/>
            <rdf:Description rdf:about="http://purl.imsglobal.org/caliper/Response"/>
            <rdf:Description rdf:about="http://purl.imsglobal.org/caliper/Result"/>
            <rdf:Description rdf:about="http://purl.imsglobal.org/caliper/Score"/>
            <rdf:Description rdf:about="http://purl.imsglobal.org/caliper/SearchResponse"/>
            <rdf:Description rdf:about="http://purl.imsglobal.org/caliper/Session"/>
        </owl:members>
    </rdf:Description>
    <rdf:Description>
        <rdf:type rdf:resource="http://www.w3.org/2002/07/owl#AllDisjointClasses"/>
        <owl:members rdf:parseType="Collection">
            <rdf:Description rdf:about="http://purl.imsglobal.org/caliper/Agent"/>
            <rdf:Description rdf:about="http://purl.imsglobal.org/caliper/Annotation"/>
            <rdf:Description rdf:about="http://purl.imsglobal.org/caliper/Attempt"/>
            <rdf:Description rdf:about="http://purl.imsglobal.org/caliper/DigitalResource"/>
            <rdf:Description rdf:about="http://purl.imsglobal.org/caliper/LearningObjective"/>
            <rdf:Description rdf:about="http://purl.imsglobal.org/caliper/Membership"/>
            <rdf:Description rdf:about="http://purl.imsglobal.org/caliper/Query"/>
            <rdf:Description rdf:about="http://purl.imsglobal.org/caliper/Response"/>
            <rdf:Description rdf:about="http://purl.imsglobal.org/caliper/Result"/>
            <rdf:Description rdf:about="http://purl.imsglobal.org/caliper/Score"/>
            <rdf:Description rdf:about="http://purl.imsglobal.org/caliper/SearchResponse"/>
            <rdf:Description rdf:about="http://purl.imsglobal.org/caliper/Session"/>
        </owl:members>
    </rdf:Description>
    <rdf:Description>
        <rdf:type rdf:resource="http://www.w3.org/2002/07/owl#AllDisjointClasses"/>
        <owl:members rdf:parseType="Collection">
            <rdf:Description rdf:about="http://purl.imsglobal.org/caliper/AnnotationEvent"/>
            <rdf:Description rdf:about="http://purl.imsglobal.org/caliper/AssessmentEvent"/>
            <rdf:Description rdf:about="http://purl.imsglobal.org/caliper/AssessmentItemEvent"/>
            <rdf:Description rdf:about="http://purl.imsglobal.org/caliper/AssignableEvent"/>
            <rdf:Description rdf:about="http://purl.imsglobal.org/caliper/FeedbackEvent"/>
            <rdf:Description rdf:about="http://purl.imsglobal.org/caliper/ForumEvent"/>
            <rdf:Description rdf:about="http://purl.imsglobal.org/caliper/GradeEvent"/>
            <rdf:Description rdf:about="http://purl.imsglobal.org/caliper/MediaEvent"/>
            <rdf:Description rdf:about="http://purl.imsglobal.org/caliper/MessageEvent"/>
            <rdf:Description rdf:about="http://purl.imsglobal.org/caliper/NavigationEvent"/>
            <rdf:Description rdf:about="http://purl.imsglobal.org/caliper/OutcomeEvent"/>
            <rdf:Description rdf:about="http://purl.imsglobal.org/caliper/ReadingEvent"/>
            <rdf:Description rdf:about="http://purl.imsglobal.org/caliper/ResourceManagementEvent"/>
            <rdf:Description rdf:about="http://purl.imsglobal.org/caliper/SearchEvent"/>
            <rdf:Description rdf:about="http://purl.imsglobal.org/caliper/SessionEvent"/>
            <rdf:Description rdf:about="http://purl.imsglobal.org/caliper/ThreadEvent"/>
            <rdf:Description rdf:about="http://purl.imsglobal.org/caliper/ToolLaunchEvent"/>
            <rdf:Description rdf:about="http://purl.imsglobal.org/caliper/ToolUseEvent"/>
            <rdf:Description rdf:about="http://purl.imsglobal.org/caliper/ViewEvent"/>
        </owl:members>
    </rdf:Description>
    <rdf:Description>
        <rdf:type rdf:resource="http://www.w3.org/2002/07/owl#AllDisjointClasses"/>
        <owl:members rdf:parseType="Collection">
            <rdf:Description rdf:about="http://purl.imsglobal.org/caliper/AssignableDigitalResource"/>
            <rdf:Description rdf:about="http://purl.imsglobal.org/caliper/Chapter"/>
            <rdf:Description rdf:about="http://purl.imsglobal.org/caliper/Document"/>
            <rdf:Description rdf:about="http://purl.imsglobal.org/caliper/Frame"/>
            <rdf:Description rdf:about="http://purl.imsglobal.org/caliper/LtiLink"/>
            <rdf:Description rdf:about="http://purl.imsglobal.org/caliper/MediaLocation"/>
            <rdf:Description rdf:about="http://purl.imsglobal.org/caliper/MediaObject"/>
            <rdf:Description rdf:about="http://purl.imsglobal.org/caliper/Message"/>
            <rdf:Description rdf:about="http://purl.imsglobal.org/caliper/Page"/>
            <rdf:Description rdf:about="http://purl.imsglobal.org/caliper/WebPage"/>
        </owl:members>
    </rdf:Description>
    <rdf:Description>
        <rdf:type rdf:resource="http://www.w3.org/2002/07/owl#AllDisjointClasses"/>
        <owl:members rdf:parseType="Collection">
            <rdf:Description rdf:about="http://purl.imsglobal.org/caliper/AudioObject"/>
            <rdf:Description rdf:about="http://purl.imsglobal.org/caliper/ImageObject"/>
            <rdf:Description rdf:about="http://purl.imsglobal.org/caliper/VideoObject"/>
        </owl:members>
    </rdf:Description>
    <rdf:Description>
        <rdf:type rdf:resource="http://www.w3.org/2002/07/owl#AllDisjointClasses"/>
        <owl:members rdf:parseType="Collection">
            <rdf:Description rdf:about="http://purl.imsglobal.org/caliper/BookmarkAnnotation"/>
            <rdf:Description rdf:about="http://purl.imsglobal.org/caliper/HighlightAnnotation"/>
            <rdf:Description rdf:about="http://purl.imsglobal.org/caliper/SharedAnnotation"/>
            <rdf:Description rdf:about="http://purl.imsglobal.org/caliper/TagAnnotation"/>
        </owl:members>
    </rdf:Description>
    <rdf:Description>
        <rdf:type rdf:resource="http://www.w3.org/2002/07/owl#AllDisjointClasses"/>
        <owl:members rdf:parseType="Collection">
            <rdf:Description rdf:about="http://purl.imsglobal.org/caliper/FillinBlankResponse"/>
            <rdf:Description rdf:about="http://purl.imsglobal.org/caliper/MultipleChoiceResponse"/>
            <rdf:Description rdf:about="http://purl.imsglobal.org/caliper/MultipleResponseResponse"/>
            <rdf:Description rdf:about="http://purl.imsglobal.org/caliper/SelectTextResponse"/>
            <rdf:Description rdf:about="http://purl.imsglobal.org/caliper/TrueFalseResponse"/>
        </owl:members>
    </rdf:Description>
    <rdf:Description>
        <rdf:type rdf:resource="http://www.w3.org/2002/07/owl#AllDisjointClasses"/>
        <owl:members rdf:parseType="Collection">
            <rdf:Description rdf:about="http://purl.imsglobal.org/caliper/LikertScale"/>
            <rdf:Description rdf:about="http://purl.imsglobal.org/caliper/MultiSelectScale"/>
            <rdf:Description rdf:about="http://purl.imsglobal.org/caliper/NumericScale"/>
        </owl:members>
    </rdf:Description>
    <rdf:Description>
        <rdf:type rdf:resource="http://www.w3.org/2002/07/owl#AllDisjointClasses"/>
        <owl:members rdf:parseType="Collection">
            <rdf:Description rdf:about="http://purl.imsglobal.org/caliper/Organization"/>
            <rdf:Description rdf:about="http://purl.imsglobal.org/caliper/Person"/>
            <rdf:Description rdf:about="http://purl.imsglobal.org/caliper/SoftwareApplication"/>
        </owl:members>
    </rdf:Description>
    <rdf:Description>
        <rdf:type rdf:resource="http://www.w3.org/2002/07/owl#AllDisjointClasses"/>
        <owl:members rdf:parseType="Collection">
            <rdf:Description rdf:about="http://purl.imsglobal.org/vocab/lis/v2/membership#Administrator"/>
            <rdf:Description rdf:about="http://purl.imsglobal.org/vocab/lis/v2/membership#ContentDeveloper"/>
            <rdf:Description rdf:about="http://purl.imsglobal.org/vocab/lis/v2/membership#Instructor"/>
            <rdf:Description rdf:about="http://purl.imsglobal.org/vocab/lis/v2/membership#Learner"/>
            <rdf:Description rdf:about="http://purl.imsglobal.org/vocab/lis/v2/membership#Manager"/>
            <rdf:Description rdf:about="http://purl.imsglobal.org/vocab/lis/v2/membership#Member"/>
            <rdf:Description rdf:about="http://purl.imsglobal.org/vocab/lis/v2/membership#Mentor"/>
            <rdf:Description rdf:about="http://purl.imsglobal.org/vocab/lis/v2/membership#Officer"/>
        </owl:members>
    </rdf:Description>
    <rdf:Description>
        <rdf:type rdf:resource="http://www.w3.org/2002/07/owl#AllDifferent"/>
        <owl:distinctMembers rdf:parseType="Collection">
            <rdf:Description rdf:about="http://purl.imsglobal.org/actions/Archived"/>
            <rdf:Description rdf:about="http://purl.imsglobal.org/actions/Copied"/>
            <rdf:Description rdf:about="http://purl.imsglobal.org/actions/Launched"/>
            <rdf:Description rdf:about="http://purl.imsglobal.org/actions/Published"/>
            <rdf:Description rdf:about="http://purl.imsglobal.org/actions/Restored"/>
            <rdf:Description rdf:about="http://purl.imsglobal.org/actions/Returned"/>
            <rdf:Description rdf:about="http://purl.imsglobal.org/actions/Unpublished"/>
            <rdf:Description rdf:about="http://purl.imsglobal.org/caliper/actions/Abandoned"/>
            <rdf:Description rdf:about="http://purl.imsglobal.org/caliper/actions/Activated"/>
            <rdf:Description rdf:about="http://purl.imsglobal.org/caliper/actions/Added"/>
            <rdf:Description rdf:about="http://purl.imsglobal.org/caliper/actions/Attached"/>
            <rdf:Description rdf:about="http://purl.imsglobal.org/caliper/actions/Bookmarked"/>
            <rdf:Description rdf:about="http://purl.imsglobal.org/caliper/actions/ChangedResolution"/>
            <rdf:Description rdf:about="http://purl.imsglobal.org/caliper/actions/ChangedSize"/>
            <rdf:Description rdf:about="http://purl.imsglobal.org/caliper/actions/ChangedSpeed"/>
            <rdf:Description rdf:about="http://purl.imsglobal.org/caliper/actions/ChangedVolume"/>
            <rdf:Description rdf:about="http://purl.imsglobal.org/caliper/actions/Classified"/>
            <rdf:Description rdf:about="http://purl.imsglobal.org/caliper/actions/ClosedPopout"/>
            <rdf:Description rdf:about="http://purl.imsglobal.org/caliper/actions/Commented"/>
            <rdf:Description rdf:about="http://purl.imsglobal.org/caliper/actions/Completed"/>
            <rdf:Description rdf:about="http://purl.imsglobal.org/caliper/actions/Copied"/>
            <rdf:Description rdf:about="http://purl.imsglobal.org/caliper/actions/Created"/>
            <rdf:Description rdf:about="http://purl.imsglobal.org/caliper/actions/Deactivated"/>
            <rdf:Description rdf:about="http://purl.imsglobal.org/caliper/actions/Deleted"/>
            <rdf:Description rdf:about="http://purl.imsglobal.org/caliper/actions/Described"/>
            <rdf:Description rdf:about="http://purl.imsglobal.org/caliper/actions/DisabledClosedCaptioning"/>
            <rdf:Description rdf:about="http://purl.imsglobal.org/caliper/actions/Disliked"/>
            <rdf:Description rdf:about="http://purl.imsglobal.org/caliper/actions/Downloaded"/>
            <rdf:Description rdf:about="http://purl.imsglobal.org/caliper/actions/EnabledClosedCaptioning"/>
            <rdf:Description rdf:about="http://purl.imsglobal.org/caliper/actions/Ended"/>
            <rdf:Description rdf:about="http://purl.imsglobal.org/caliper/actions/EnteredFullScreen"/>
            <rdf:Description rdf:about="http://purl.imsglobal.org/caliper/actions/ExitedFullScreen"/>
            <rdf:Description rdf:about="http://purl.imsglobal.org/caliper/actions/ForwardedTo"/>
            <rdf:Description rdf:about="http://purl.imsglobal.org/caliper/actions/Graded"/>
            <rdf:Description rdf:about="http://purl.imsglobal.org/caliper/actions/Hid"/>
            <rdf:Description rdf:about="http://purl.imsglobal.org/caliper/actions/Highlighted"/>
            <rdf:Description rdf:about="http://purl.imsglobal.org/caliper/actions/Identified"/>
            <rdf:Description rdf:about="http://purl.imsglobal.org/caliper/actions/JumpedTo"/>
            <rdf:Description rdf:about="http://purl.imsglobal.org/caliper/actions/Liked"/>
            <rdf:Description rdf:about="http://purl.imsglobal.org/caliper/actions/Linked"/>
            <rdf:Description rdf:about="http://purl.imsglobal.org/caliper/actions/LoggedIn"/>
            <rdf:Description rdf:about="http://purl.imsglobal.org/caliper/actions/LoggedOut"/>
            <rdf:Description rdf:about="http://purl.imsglobal.org/caliper/actions/MarkedAsRead"/>
            <rdf:Description rdf:about="http://purl.imsglobal.org/caliper/actions/MarkedAsUnread"/>
            <rdf:Description rdf:about="http://purl.imsglobal.org/caliper/actions/Modified"/>
            <rdf:Description rdf:about="http://purl.imsglobal.org/caliper/actions/Muted"/>
            <rdf:Description rdf:about="http://purl.imsglobal.org/caliper/actions/NavigatedTo"/>
            <rdf:Description rdf:about="http://purl.imsglobal.org/caliper/actions/OpenedPopout"/>
            <rdf:Description rdf:about="http://purl.imsglobal.org/caliper/actions/Paused"/>
            <rdf:Description rdf:about="http://purl.imsglobal.org/caliper/actions/Posted"/>
            <rdf:Description rdf:about="http://purl.imsglobal.org/caliper/actions/Printed"/>
            <rdf:Description rdf:about="http://purl.imsglobal.org/caliper/actions/Published"/>
            <rdf:Description rdf:about="http://purl.imsglobal.org/caliper/actions/Questioned"/>
            <rdf:Description rdf:about="http://purl.imsglobal.org/caliper/actions/Ranked"/>
            <rdf:Description rdf:about="http://purl.imsglobal.org/caliper/actions/Recommended"/>
            <rdf:Description rdf:about="http://purl.imsglobal.org/caliper/actions/Removed"/>
            <rdf:Description rdf:about="http://purl.imsglobal.org/caliper/actions/Reset"/>
            <rdf:Description rdf:about="http://purl.imsglobal.org/caliper/actions/Restarted"/>
            <rdf:Description rdf:about="http://purl.imsglobal.org/caliper/actions/Restored"/>
            <rdf:Description rdf:about="http://purl.imsglobal.org/caliper/actions/Resumed"/>
            <rdf:Description rdf:about="http://purl.imsglobal.org/caliper/actions/Retrieved"/>
            <rdf:Description rdf:about="http://purl.imsglobal.org/caliper/actions/Reviewed"/>
            <rdf:Description rdf:about="http://purl.imsglobal.org/caliper/actions/Rewound"/>
            <rdf:Description rdf:about="http://purl.imsglobal.org/caliper/actions/Saved"/>
            <rdf:Description rdf:about="http://purl.imsglobal.org/caliper/actions/Searched"/>
            <rdf:Description rdf:about="http://purl.imsglobal.org/caliper/actions/Shared"/>
            <rdf:Description rdf:about="http://purl.imsglobal.org/caliper/actions/Showed"/>
            <rdf:Description rdf:about="http://purl.imsglobal.org/caliper/actions/Skipped"/>
            <rdf:Description rdf:about="http://purl.imsglobal.org/caliper/actions/Started"/>
            <rdf:Description rdf:about="http://purl.imsglobal.org/caliper/actions/Submitted"/>
            <rdf:Description rdf:about="http://purl.imsglobal.org/caliper/actions/Subscribed"/>
            <rdf:Description rdf:about="http://purl.imsglobal.org/caliper/actions/Tagged"/>
            <rdf:Description rdf:about="http://purl.imsglobal.org/caliper/actions/TimedOut"/>
            <rdf:Description rdf:about="http://purl.imsglobal.org/caliper/actions/Unmuted"/>
            <rdf:Description rdf:about="http://purl.imsglobal.org/caliper/actions/Unpublished"/>
            <rdf:Description rdf:about="http://purl.imsglobal.org/caliper/actions/Unsubscribed"/>
            <rdf:Description rdf:about="http://purl.imsglobal.org/caliper/actions/Uploaded"/>
            <rdf:Description rdf:about="http://purl.imsglobal.org/caliper/actions/Used"/>
            <rdf:Description rdf:about="http://purl.imsglobal.org/caliper/actions/Viewed"/>
        </owl:distinctMembers>
    </rdf:Description>
    <rdf:Description>
        <rdf:type rdf:resource="http://www.w3.org/2002/07/owl#AllDifferent"/>
        <owl:distinctMembers rdf:parseType="Collection">
            <rdf:Description rdf:about="http://purl.imsglobal.org/caliper/lti/LtiDeepLinkingRequest"/>
            <rdf:Description rdf:about="http://purl.imsglobal.org/caliper/lti/LtiResourceLinkRequest"/>
        </owl:distinctMembers>
    </rdf:Description>
    <rdf:Description>
        <rdf:type rdf:resource="http://www.w3.org/2002/07/owl#AllDifferent"/>
        <owl:distinctMembers rdf:parseType="Collection">
            <rdf:Description rdf:about="http://purl.imsglobal.org/caliper/metrics/AssessmentsPassed"/>
            <rdf:Description rdf:about="http://purl.imsglobal.org/caliper/metrics/AssessmentsSubmitted"/>
            <rdf:Description rdf:about="http://purl.imsglobal.org/caliper/metrics/MinutesOnTask"/>
            <rdf:Description rdf:about="http://purl.imsglobal.org/caliper/metrics/SkillsMastered"/>
            <rdf:Description rdf:about="http://purl.imsglobal.org/caliper/metrics/StandardsMastered"/>
            <rdf:Description rdf:about="http://purl.imsglobal.org/caliper/metrics/UnitsCompleted"/>
            <rdf:Description rdf:about="http://purl.imsglobal.org/caliper/metrics/UnitsPassed"/>
            <rdf:Description rdf:about="http://purl.imsglobal.org/caliper/metrics/WordsRead"/>
        </owl:distinctMembers>
    </rdf:Description>
</rdf:RDF>



<!-- Generated by the OWL API (version 4.5.9.2019-02-01T07:24:44Z) https://github.com/owlcs/owlapi -->

